format-version: 1.2
idspace: rdf http://www.w3.org/1999/02/22-rdf-syntax-ns# ""
idspace: rdfs http://www.w3.org/2000/01/rdf-schema# ""
idspace: owl http://www.w3.org/2002/07/owl# ""
idspace: xsd http://www.w3.org/2001/XMLSchema# ""
idspace: dc http://purl.org/dc/elements/1.1/ ""
idspace: eor http://dublincore.org/2000/03/13/eor# ""
idspace: serql http://www.openrdf.org/schema/serql# ""
idspace: obd http://www.bioontology.org/obd/obd-ontology# ""
idspace: oboInOwl http://www.bioontology.org/oboInOwl# ""
idspace: ncithesaurus http://ncicb.nci.nih.gov/xml/owl/EVS/Thesaurus.owl# ""
idspace: biopax1 http://www.biopax.org/release/biopax-level1.owl# ""
idspace: mged http://mged.sourceforge.net/ontologies/MGEDOntology.owl# ""

[Typedef]
id: rdf:first
name: first
namespace: http://www.w3.org/1999/02/22-rdf-syntax-ns#
comment: The first item in an RDF list. Also often called the head.
domain: rdf:List     ! List
property_value: rdfs:comment "The first item in an RDF list. Also often called the head." xsd:string

[Typedef]
id: rdf:object
name: object
namespace: http://www.w3.org/1999/02/22-rdf-syntax-ns#
comment: The object of an RDF statement.
domain: rdf:Statement     ! Statement
property_value: rdfs:comment "The object of an RDF statement." xsd:string

[Typedef]
id: rdf:predicate
name: predicate
namespace: http://www.w3.org/1999/02/22-rdf-syntax-ns#
comment: the predicate of an RDF statement.
domain: rdf:Statement     ! Statement
range: rdf:Property     ! Property
property_value: rdfs:comment "the predicate of an RDF statement." xsd:string

[Typedef]
id: rdf:rest
name: rest
namespace: http://www.w3.org/1999/02/22-rdf-syntax-ns#
comment: The rest of an RDF list after the first item. Also often called the tail.
domain: rdf:List     ! List
range: rdf:List     ! List
property_value: rdfs:comment "The rest of an RDF list after the first item. Also often called the tail." xsd:string

[Typedef]
id: rdf:subject
name: subject
namespace: http://www.w3.org/1999/02/22-rdf-syntax-ns#
comment: The subject of an RDF statement.
domain: rdf:Statement     ! Statement
range: rdfs:Resource     ! Resource
property_value: rdfs:comment "The subject of an RDF statement." xsd:string

[Typedef]
id: rdf:type
name: type
namespace: http://www.w3.org/1999/02/22-rdf-syntax-ns#
comment: Indicates membership of a class
domain: rdfs:Resource     ! Resource
range: rdfs:Class     ! Class
property_value: rdfs:comment "Indicates membership of a class" xsd:string

[Typedef]
id: rdf:value
name: value
namespace: http://www.w3.org/1999/02/22-rdf-syntax-ns#
comment: Identifies the principal value (usually a xsd:string) of a property when the property value is a structured resource
domain: rdfs:Resource     ! Resource
property_value: rdfs:comment "Identifies the principal value (usually a xsd:string) of a property when the property value is a structured resource" xsd:string

[Typedef]
id: rdfs:comment
name: comment
namespace: http://www.w3.org/2000/01/rdf-schema#
comment: A description of the subject resource.
comment: Use this for descriptions
domain: rdfs:Resource     ! Resource
range: rdfs:Literal     ! Literal
property_value: rdfs:comment "A description of the subject resource." xsd:string
property_value: rdfs:comment "Use this for descriptions" xsd:string

[Typedef]
id: rdfs:domain
name: domain
namespace: http://www.w3.org/2000/01/rdf-schema#
comment: A domain class for a property type
comment: A domain of the subject property.
domain: rdf:Property     ! Property
range: rdfs:Class     ! Class
property_value: rdfs:comment "A domain class for a property type" xsd:string
property_value: rdfs:comment "A domain of the subject property." xsd:string

[Typedef]
id: rdfs:isDefinedBy
name: isDefinedBy
namespace: http://www.w3.org/2000/01/rdf-schema#
comment: Indicates the namespace of a resource
comment: The defininition of the subject resource.
domain: rdfs:Resource     ! Resource
range: rdfs:Resource     ! Resource
property_value: rdfs:comment "Indicates the namespace of a resource" xsd:string
property_value: rdfs:comment "The defininition of the subject resource." xsd:string

[Typedef]
id: rdfs:label
name: label
namespace: http://www.w3.org/2000/01/rdf-schema#
comment: A human-readable name for the subject.
comment: Provides a human-readable version of a resource name.
domain: rdfs:Resource     ! Resource
range: rdfs:Literal     ! Literal
property_value: rdfs:comment "A human-readable name for the subject." xsd:string
property_value: rdfs:comment "Provides a human-readable version of a resource name." xsd:string

[Typedef]
id: rdfs:member
name: member
namespace: http://www.w3.org/2000/01/rdf-schema#
comment: A member of the subject resource.
comment: a member of a container
domain: rdfs:Container     ! Container
domain: rdfs:Resource     ! Resource
range: rdfs:Resource     ! Resource
property_value: rdfs:comment "A member of the subject resource." xsd:string
property_value: rdfs:comment "a member of a container" xsd:string

[Typedef]
id: rdfs:range
name: range
namespace: http://www.w3.org/2000/01/rdf-schema#
comment: A range class for a property type
comment: A range of the subject property.
domain: rdf:Property     ! Property
range: rdfs:Class     ! Class
property_value: rdfs:comment "A range class for a property type" xsd:string
property_value: rdfs:comment "A range of the subject property." xsd:string

[Typedef]
id: rdfs:seeAlso
name: seeAlso
namespace: http://www.w3.org/2000/01/rdf-schema#
comment: A resource that provides information about the subject resource
comment: Further information about the subject resource.
domain: rdfs:Resource     ! Resource
range: rdfs:Resource     ! Resource
property_value: rdfs:comment "A resource that provides information about the subject resource" xsd:string
property_value: rdfs:comment "Further information about the subject resource." xsd:string

[Typedef]
id: rdfs:subClassOf
name: subClassOf
namespace: http://www.w3.org/2000/01/rdf-schema#
comment: Indicates membership of a class
comment: The subject is a subclass of a class.
domain: rdfs:Class     ! Class
range: rdfs:Class     ! Class
property_value: rdfs:comment "Indicates membership of a class" xsd:string
property_value: rdfs:comment "The subject is a subclass of a class." xsd:string

[Typedef]
id: rdfs:subPropertyOf
name: subPropertyOf
namespace: http://www.w3.org/2000/01/rdf-schema#
comment: Indicates specialization of properties
comment: The subject is a subproperty of a property.
domain: rdf:Property     ! Property
range: rdf:Property     ! Property
property_value: rdfs:comment "Indicates specialization of properties" xsd:string
property_value: rdfs:comment "The subject is a subproperty of a property." xsd:string

[Term]
id: rdf:Alt
name: Alt
namespace: rdf:
comment: A collection of alternatives.
property_value: rdfs:comment "A collection of alternatives." xsd:string

[Term]
id: rdf:Bag
name: Bag
namespace: rdf:
comment: An unordered collection.
property_value: rdfs:comment "An unordered collection." xsd:string

[Term]
id: rdf:List
name: List
namespace: rdf:
comment: The class of RDF Lists
property_value: rdfs:comment "The class of RDF Lists" xsd:string

[Term]
id: rdf:Property
name: Property
namespace: rdf:
comment: The concept of a property.
property_value: rdfs:comment "The concept of a property." xsd:string

[Term]
id: rdf:Seq
name: Seq
namespace: rdf:
comment: An ordered collection.
property_value: rdfs:comment "An ordered collection." xsd:string

[Term]
id: rdf:Statement
name: Statement
namespace: rdf:
comment: The class of RDF statements.
property_value: rdfs:comment "The class of RDF statements." xsd:string

[Term]
id: rdfs:Class
name: Class
namespace: rdfs:
comment: The class of classes.
comment: The concept of Class
property_value: rdfs:comment "The class of classes." xsd:string
property_value: rdfs:comment "The concept of Class" xsd:string

[Term]
id: rdfs:Container
name: Container
namespace: rdfs:
comment: The class of RDF containers.
comment: This represents the set Containers.
property_value: rdfs:comment "The class of RDF containers." xsd:string
property_value: rdfs:comment "This represents the set Containers." xsd:string

[Term]
id: rdfs:ContainerMembershipProperty
name: ContainerMembershipProperty
namespace: rdfs:
comment: The class of container membership properties, rdf:_1, rdf:_2, ...,\n                    all of which are sub-properties of 'member'.
comment: The container membership properties, rdf:1, rdf:2, ..., all of which are sub-properties of 'member'.
property_value: rdfs:comment "The class of container membership properties, rdf:_1, rdf:_2, ...,\n                    all of which are sub-properties of 'member'." xsd:string
property_value: rdfs:comment "The container membership properties, rdf:1, rdf:2, ..., all of which are sub-properties of 'member'." xsd:string

[Term]
id: rdfs:Datatype
name: Datatype
namespace: rdfs:
comment: The class of RDF datatypes.
comment: The class of datatypes.
property_value: rdfs:comment "The class of RDF datatypes." xsd:string
property_value: rdfs:comment "The class of datatypes." xsd:string

[Term]
id: rdfs:Literal
name: Literal
namespace: rdfs:
comment: The class of literal values, eg. textual xsd:strings and integers.
comment: This represents the set of atomic values, eg. textual xsd:strings.
property_value: rdfs:comment "The class of literal values, eg. textual xsd:strings and integers." xsd:string
property_value: rdfs:comment "This represents the set of atomic values, eg. textual xsd:strings." xsd:string

[Term]
id: rdfs:Resource
name: Resource
namespace: rdfs:
comment: The class resource, everything.
property_value: rdfs:comment "The class resource, everything." xsd:string

[Term]
id: rdfs:XMLLiteral
name: XMLLiteral
namespace: rdfs:
comment: The class of XML literals.
property_value: rdfs:comment "The class of XML literals." xsd:string

