format-version: 1.0
version: $Revision: 1.6 $
date: 13:03:2007 14:52
saved-by: cwt6
auto-generated-by: DAG-Edit 1.419 rev 3
default-namespace: cereal_plant_growth_stage
remark: This is the first version of the cereal plant growth stage ontology.  This is created from the files temporal_gramene.ontology (ver 1.12) and temporal_gramene.definition (ver 1.13).

[Term]
id: GRO:0007000
name: in-vitro culture stage
def: "The stages describing the callus growth and differentiation in the tissue culture experiments." [GR:pj]
is_a: GRO:0007139 ! A-vegetative stage

[Term]
id: GRO:0007001
name: rice plant growth stage
def: "The gross developmental stages defined for the plant." [GR:pj]
is_a: GRO:0007040 ! rice growth stage

[Term]
id: GRO:0007002
name: maize growth stage
def: "The development and growth of maize have been translated into several scales to quantify development for scientific and management purposes. The growth stage terms and their descriptors were provided by the MaizeDB." [GR:pj, MaizeDB:lv, web:http //www.agron.missouri.edu/phenotypes.html]
is_a: GRO:0007199 ! cereal plant growth stage ontology

[Term]
id: GRO:0007003
name: 00-germination
def: "Process by which embryonic organs formed during kernel development and which have been dormant in the dry seed\, resume their growth under appropriate temperature and moisture conditions" [MaizeDB:64055]
synonym: "maize growth stage-0" []
is_a: GRO:0007002 ! maize growth stage

[Term]
id: GRO:0007004
name: rice growth stage unknown
def: "A case when it is difficult to annotate the growth stage defined in an experiment" [GR:pj]
is_a: GRO:0007001 ! rice plant growth stage

[Term]
id: GRO:0007005
name: 0.02-radicle emergence from seed
def: "The radicle and its enclosing sheath\, the coleorhiza\, break through the pericarp." [MaizeDB:67351]
synonym: "maize growth stage-0.2" []
is_a: GRO:0007003 ! 00-germination

[Term]
id: GRO:0007006
name: 0.03-coleoptile emergence from seed
def: "The coleoptile\, enclosing the plumule or embryonic shoot\, pushes through the pericarp" [MaizeDB:67352]
synonym: "maize growth stage-0.3" []
is_a: GRO:0007003 ! 00-germination

[Term]
id: GRO:0007007
name: 01-seedling
def: "Commonly refers to the growth stage between germination and tassel differentiation\, with a duration of approximately three weeks for adapted cultivars in the US Corn Belt" [MaizeDB:1863]
synonym: "maize growth stage-1" []
is_a: GRO:0007002 ! maize growth stage

[Term]
id: GRO:0007008
name: 1.01-seedling emergence
def: "Coleoptile appears above the soil surface. Nodal roots begin to develop." [MaizeDB:64057]
synonym: "maize growth stage-1.1" []
is_a: GRO:0007007 ! 01-seedling

[Term]
id: GRO:0007009
name: 1.02-one to two leaves
def: "First or second leaf collar visible." [MaizeDB:67353]
synonym: "maize growth stage-1.2" []
is_a: GRO:0007007 ! 01-seedling

[Term]
id: GRO:0007010
name: 1.03-three to four leaves
def: "3 or 4 leaf collars visible" [MaizeDB:25331]
synonym: "maize growth stage-1.3" []
is_a: GRO:0007007 ! 01-seedling

[Term]
id: GRO:0007011
name: 02-tassel initiation
def: "Apical dome of shoot meristem elongates\, followed by appearance of tassel branch primordia. Under favorable conditions in adapted hybrids in the US Corn Belt\, this may occur about  2-3 weeks after seedling emergence\, when 4-6 leaf collars are visible. Stem growing point is at or near soil surface. Tassel initiation is very sensitive to photoperiod and temperature\, maximal sensitivity to these factors occurs during a brief period with a duration\, equivalent to the emergence of two leaves\, just before tassel initiation" [MaizeDB:67306]
synonym: "4-6 leaf stage" []
synonym: "early whorl stage" []
synonym: "maize growth stage-2" []
synonym: "tassel differentiation" []
is_a: GRO:0007002 ! maize growth stage

[Term]
id: GRO:0007012
name: 03-rapid stem elongation
def: "After tassel initiation\, stem length begins to increase rapidly\, through elongation of cells formed by the intercalary meristem at the base of above-ground internodes. The rate of elongation decreases prior to anthesis\, but plant height may continue to increase until after flowering" [MaizeDB:67358]
synonym: "maize growth stage-3" []
synonym: "mid-whorl stage" []
synonym: "stem elongation" []
synonym: "telescoping" []
is_a: GRO:0007002 ! maize growth stage

[Term]
id: GRO:0007013
name: 3.01-ear initiation
def: "Elongation of apical dome of axillary meristem corresponding to top ear\, followed by appearance of spikelet primordia. Typically\, in adapted materials in the US Corn Belt\, 6-8 leaf collars are visible\, but this depends on genotype and environmental conditions." [MaizeDB:67356]
synonym: "6 leaf" []
synonym: "6-8 leaf" []
synonym: "7 leaf" []
synonym: "8 leaf" []
synonym: "V6" []
synonym: "V7" []
synonym: "V8" []
synonym: "maize growth stage-3.1" []
synonym: "mid-whorl stage" []
is_a: GRO:0007012 ! 03-rapid stem elongation

[Term]
id: GRO:0007014
name: 3.02-late whorl stage
def: "In adapted materials in the US Corn Belt\, the collars of leaves 9-11 are visible (some of the lowest leaves may already have degenerated by this stage). By 10-leaf stage\, new leaves appear every 2-3 days. Tassel development accelerates\, and rapid stem elongation continues." [MaizeDB:67357]
synonym: "1-11 leaf" []
synonym: "10-leaf" []
synonym: "11-leaf" []
synonym: "9-leaf" []
synonym: "V-11" []
synonym: "V10" []
synonym: "V9" []
synonym: "maize growth stage-3.2" []
is_a: GRO:0007012 ! 03-rapid stem elongation

[Term]
id: GRO:0007015
name: 3.03-mid-vegetative
def: "Rapid stem elongation continues. In adapted materials in the US Corn Belt\, 12-14 leaf collars are visible. Number of ovules (potential kernels) is being determined. Male meiosis begins about this time" [MaizeDB:67359]
synonym: "V12" []
synonym: "V13" []
synonym: "V14" []
synonym: "maize growth stage-3.3" []
is_a: GRO:0007012 ! 03-rapid stem elongation

[Term]
id: GRO:0007016
name: 3.04-late vegetative
def: "Late vegetative stage\, corresponding to the 15-leaf stage or later in adapted hybrids in the US Corn Belt\, which normally have a total of about 20 leaves. Depending on genotype and environmental conditions\, a corn plant may develop 10-30 leaves. Ear is developing rapidly and silk elongation begins. Female meiosis begins when silks are approx. 2 mm long and ears approx. 2 cm long. Brace roots begin growing\, a new leaf is added every 1-2 days " [MaizeDB:67360]
synonym: "V15" []
synonym: "V16" []
synonym: "V17" []
synonym: "V18" []
synonym: "V19" []
synonym: "V20" []
synonym: "maize growth stage-3.4" []
is_a: GRO:0007012 ! 03-rapid stem elongation

[Term]
id: GRO:0007017
name: 04-gametophyte development
def: "Includes both male (pollen) and female (embryo sac) gametophyte development\, which are sub stages of this stage" [MaizeDB:67385]
synonym: "gametogenesis" []
synonym: "maize growth stage-4" []
is_a: GRO:0007002 ! maize growth stage
relationship: part_of GRO:0007016 ! 3.04-late vegetative

[Term]
id: GRO:0007018
name: 4.01-pollen development
def: "Microsporogenesis\, or pollen development\, includes all stages from microsporocyte meiosis through the mature pollen grain" [MaizeDB:67383]
synonym: "maize growth stage-4.1" []
synonym: "male gametophyte development" []
synonym: "microspore development" []
synonym: "microsporogenesis" []
is_a: GRO:0007017 ! 04-gametophyte development

[Term]
id: GRO:0007019
name: 4.02-embryo sac development
def: "Includes megasporogenesis (female meiosis) and megagametogenesis (beginning with mitotic division of the meiotic products through maturation of the embryo sac)" [MaizeDB:67384]
synonym: "female gametophyte development" []
synonym: "maize growth stage-4.2" []
synonym: "megagametogenesis" []
synonym: "megaspore development" []
synonym: "megasporogenesis" []
is_a: GRO:0007017 ! 04-gametophyte development

[Term]
id: GRO:0007020
name: 05-flowering
def: "The term \"flowering\" is used here to encompass the processes of anthesis (pollen shed)\, silking (emergence of styles from husk)\, pollination\, and fertilization" [MaizeDB:13811]
synonym: "maize growth stage-5" []
is_a: GRO:0007002 ! maize growth stage

[Term]
id: GRO:0007021
name: 5.01-anthesis
def: "Anthers are extruded between glume and lemma\, pores at the anther tip break open\, and pollen is released. Pollen shed occurs first from spikelets slightly above the middle of the central axis of the tassel\, then proceeds towards tip and base\, pollen shedding from lateral branches occurs somewhat later. " [MaizeDB:67361]
synonym: "Pollen shed" []
synonym: "Pollen shedding" []
synonym: "VT" []
synonym: "maize growth stage-5.1" []
is_a: GRO:0007020 ! 05-flowering

[Term]
id: GRO:0007022
name: 5.02-silking
def: "Silks (styles) emerge from the husks at the ear tip. Normally the first silks appear slightly after anthesis begins\, but this interval can be delayed by drought or other stresses. Silks of  spikelets at the base of the ear emerge prior to those from more apical spikelets" [MaizeDB:67362]
synonym: "R1" []
synonym: "maize growth stage-5.2" []
synonym: "silk emergence" []
is_a: GRO:0007020 ! 05-flowering

[Term]
id: GRO:0007023
name: 5.03-pollination
def: "Pollen lands on a silk hair\, hydrates\, and germinates by sending out a pollen tube through the pollen pore. The pollen tube grows rapidly (0.5 cm/hr) down the length of the silk to the ovary and the embryo sac" [MaizeDB:67364]
synonym: "maize growth stage-5.3" []
is_a: GRO:0007020 ! 05-flowering

[Term]
id: GRO:0007024
name: 5.04-fertilization
def: "Fertilization occurs 16-24 hours after pollination. It consists of the simultaneous fusion of 1 sperm cell with the egg to form the diploid zygote\, and the other sperm cell with 2 polar nuclei to form the triploid primary endosperm nucleus" [GR:pj, MAizeDB:67365]
synonym: "double fecundation" []
synonym: "double fertilization" []
synonym: "fecundation" []
synonym: "maize growth stage-5.4" []
is_a: GRO:0007020 ! 05-flowering

[Term]
id: GRO:0007025
name: 06-post-flowering
def: "The period of slow kernel growth between fertilization and the beginning of linear grain-filling\, lasting roughly 10-12 days. Some workers divides this period into dilatory and exponential phases\, which approximately coincide with the endosperm's free nuclear and mitotic stages\, respectively. From about 4-10 days after pollination\, the embryo is in the proembryo stage\, a club-shaped mass of cells with little differentiation except for a basal suspensor region\, and an apical region of smaller cells\, the embryo proper" [MaizeDB:67370]
synonym: "R1" []
synonym: "lag phase" []
synonym: "maize growth stage-6" []
synonym: "proembryo" []
is_a: GRO:0007002 ! maize growth stage

[Term]
id: GRO:0007026
name: 6.01-dilatory
def: "This phase is the initial few days following fertilization\, during which time very slow dry matter accumulation occurs in the kernel. In the endosperm\, the primary endosperm nucleus divides 2-4 hours after fertilization\, followed by rapid synchronous divisions to produce a free nuclear tissue. The fertilized egg undergoes its first division about 10-12 hours after fertilization\, and by the end of this stage will have developed into the proembryo with about 12-24 cells" [MaizeDB:67371]
synonym: "free nuclear" []
synonym: "maize growth stage-6.1" []
is_a: GRO:0007025 ! 06-post-flowering

[Term]
id: GRO:0007027
name: 6.02-exponential
def: "The phase with increased metabolic activity and rapid kernel development that links the dilatory phase with the linear grain-filling period. It occurs approximately 5-12 days after pollination (dap). In the endosperm\, cell walls are laid down beginning about 5 dap\, changing the free nuclear tissue into a cellular one. The embryo continues in the proembryo stage through about 10 dap. MaizeDB includes a sub-stage." [MaizeDB:67369]
synonym: "maize growth stage-6.2" []
is_a: GRO:0007025 ! 06-post-flowering

[Term]
id: GRO:0007028
name: 6.02.1-transition stage
def: "Occurs when the ovoid\, radially symmetrical proembryo elongates to form a cone-shaped structure\, establishing the future shoot-root meristem axis\, about 10-12 days after pollination. " [MaizeDB:67451]
comment: In the endosperm\, mitotic activity in the central region declines\, and nuclear size and DNA content begin to increase  (endoreduplication)
synonym: "endoreduplication" []
synonym: "maize growth stage-6.2.1" []
is_a: GRO:0007027 ! 6.02-exponential

[Term]
id: GRO:0007029
name: 07-linear grain-filling
def: "Stage of rapid\, nearly linear increase in kernel dry matter\, that begins about 2 weeks after pollination and lasts almost until physiological maturity" [MaizeDB:64632]
synonym: "effective filling period" []
synonym: "grain filling" []
synonym: "maize growth stage-7" []
is_a: GRO:0007002 ! maize growth stage

[Term]
id: GRO:0007030
name: 7.01-blister stage
def: "This stage is initiated when significant starch accumulation begins\, approximately 12-17 days after pollination (dap). Kernels  appear white and translucent\, endosperm and its inner fluid are clear. Endoreduplication\, an increase in DNA content in endosperm cells\, which began in the transition stage\, peaks about 16-18 dap" [MaizeDB:67372]
comment: dap is days after pollination
synonym: "R2" []
synonym: "maize growth stage-7.1" []
is_a: GRO:0007029 ! 07-linear grain-filling

[Term]
id: GRO:0007031
name: 7.01.1-coleoptilar stage
def: "In the coleoptilar stage\, the embryo develops a prominent shoot apical meristem surrounded by the coleoptilar ring\, and backed by the flattened\, spade-shaped scutellum\, it occurs about 12-14 days after pollination" [MaizeDB:67376]
synonym: "embryo coleoptilar stage" []
synonym: "maize growth stage-7.1.1" []
is_a: GRO:0007030 ! 7.01-blister stage

[Term]
id: GRO:0007032
name: 7.01.2-embryo-1
def: "Embryo stage 1 is defined by the appearance of first leaf primordium from the shoot apical meristem\, it occurs about 14-18 days after pollination\, when embryo is slightly more than 1 mm long" [MaizeDB:67377]
comment: Stage 1 embryos are often used to initiate embryonic callus in tissue culture experiments
synonym: "embryo stage 1" []
synonym: "maize growth stage-7.1.2" []
is_a: GRO:0007030 ! 7.01-blister stage

[Term]
id: GRO:0007033
name: 7.02-stage
def: "Endosperm fluid has changed from clear to a milky white\, more viscous substance due to accumulating starch\, kernels are about 80% moisture\, aleurone color characteristic of the genotype appears\, occurs about 18-22 days after pollination" [MaizeDB:67373]
comment: The embryo is at stage 2\: second leaf primordium is formed\, and embryo length is approx. 2 mm
synonym: "R3" []
synonym: "embryo stage 2" []
synonym: "embryo-2" []
synonym: "maize growth stage-7.2" []
is_a: GRO:0007029 ! 07-linear grain-filling

[Term]
id: GRO:0007034
name: 7.03-early dough stage
def: "Endosperm fluid has changed to a pasty or soft dough-like consistency\, kernels have about 70% moisture\, occurs about 22-28 days after pollination. Embryo is at stage 3\: third leaf primordium forms\, radicle is recognizable within the coleorhiza\, embryo is about 3 mm long" [MaizeDB:67374]
synonym: "R4" []
synonym: "dough stage" []
synonym: "embryo stage 3" []
synonym: "embryo-3" []
synonym: "maize growth stage-7.3" []
is_a: GRO:0007029 ! 07-linear grain-filling

[Term]
id: GRO:0007035
name: 7.04-late dough stage
def: "Endosperm consistency checked by firmer dough than in the previous stage. Towards end of this stage\, in dent genotypes\, kernels begin to dent on top\, occurs about 28-35 days after pollination. Embryo is at stage 4\: fourth leaf primordium has formed\, embryo is 5-6 mm long" [MaizeDB:67379]
synonym: "embryo stage 4" []
synonym: "embryo-4" []
synonym: "maize growth stage-7.4" []
is_a: GRO:0007029 ! 07-linear grain-filling

[Term]
id: GRO:0007036
name: 08-leveling of of grain-filling
def: "Rate of dry matter accumulation in kernel diminishes as endosperm transfer cells are crushed. All or nearly all kernels are dented (in a dent genotype)\, kernels are about 50-55% moisture\, husk has begun to dry rapidly\, occurs about 35-42 days after pollination. Embryo is at stage 5\, fifth leaf  primordium has formed and lateral seminal root primordia can be observed" [MaizeDB:67382]
synonym: "R5" []
synonym: "attenuative" []
synonym: "dent stage" []
synonym: "embryo stage 5" []
synonym: "embryo-5" []
synonym: "leveling of of dry matter accumulation" []
synonym: "maize growth stage-8" []
is_a: GRO:0007002 ! maize growth stage

[Term]
id: GRO:0007037
name: 09-maturity
def: "The stage begins at physiological maturity (when the kernel has approximately 30-35% moisture) and continues through dry kernel (15% moisture or less). This stage is subdivided into the two stages listed above." [MaizeDB:11088]
synonym: "maize growth stage-9" []
synonym: "senescence" []
is_a: GRO:0007002 ! maize growth stage

[Term]
id: GRO:0007038
name: 9.01-physiological maturity
def: "Occurs when grain dry matter accumulation ceases and a black abscission layer forms at the base of the kernel\, approx. 50-65 days after pollination\, grain moisture is about 30-35%. Embryo is at stage 6\: a sixth leaf primordium may have formed\, although many genotypes form only 5 embryonic leaves\, dormancy occurs after massive hydration of embryo cells" [MaizeDB:67380]
synonym: "R6" []
synonym: "black layer" []
synonym: "embryo stage 6" []
synonym: "embryo-6" []
synonym: "maize growth stage-9.1" []
is_a: GRO:0007037 ! 09-maturity

[Term]
id: GRO:0007039
name: 9.02-dry kernel
def: "The kernel has dried to safe storage moisture\, 15% or less" [MaizeDB:67381]
synonym: "dry seed" []
synonym: "maize growth stage-9.2" []
synonym: "storage maturity" []
is_a: GRO:0007037 ! 09-maturity

[Term]
id: GRO:0007040
name: rice growth stage
def: "The growth and developmental stages defined for the rice plant." [GR:pj]
synonym: "rice growth stages" []
is_a: GRO:0007199 ! cereal plant growth stage ontology

[Term]
id: GRO:0007041
name: 4.2-panicle differentiation stage
def: "At this point\, the panicle is 1 to 2 mm in length and the branching of the panicle is visible" [web:http //www.uaex.edu/Other_Areas/publications/HTML/MP192/1_Rice_Growth_and_Development_Reproductive.asp, GR:pj]
comment: In parallel the stem elongation is continuing
synonym: "PD" []
synonym: "rice growth stage-4.2" []
relationship: part_of GRO:0007048 ! 04-stem elongation stage

[Term]
id: GRO:0007042
name: 08-dough stage
def: "One of the ripening stages when endosperm starts hardening." [GR:pj]
synonym: "rice growth stage-8" []
is_a: GRO:0007141 ! C-embryo stage

[Term]
id: GRO:0007043
name: 01-germination
def: "Occurs when the seed coat has imbibed adequate water becoming soft and elastic. The coleorhiza elongates slightly\, emerging through the seed coat and the radicle breaks through the coleorhiza and becomes anchored in the soil or growth media." [GR:pj, web:http //www.uaex.edu/Other_Areas/publications/HTML/MP192/1_Rice_Growth_and_Development_Vegetative.asp]
comment: Thus\, under dry-seeded or aerobic conditions\, the radicle emerges before the coleoptile. Under water-seeded or reduced oxygen (anaerobic) conditions\, the coleoptile may emerge before the root. The coleoptile continues to elongate and several lateral roots called seminal roots form.
synonym: "rice growth stage-1" []
is_a: GRO:0007139 ! A-vegetative stage

[Term]
id: GRO:0007044
name: 06-heading stage
def: "is the time when the panicle begins to exsert from the boot." [web:http //www.uaex.edu/Other_Areas/publications/HTML/MP192/1_Rice_Growth_and_Development_Reproductive.asp, GR:pj]
comment: Heading may take over 10 to 14 days due to variations within tillers on the same plant and between plants in the field. Agronomically\, heading date is defined as the time when 50 percent of the panicles have at least partially exserted from the boot.
synonym: "rice growth stage-6" []
is_a: GRO:0007140 ! B-reproductive stage

[Term]
id: GRO:0007045
name: 09-mature grain stage
def: "The whole grain is hard and ready for harvest. This stage is reached at approximately 15-20 percent moisture" [GR:pj, web:http //www.uaex.edu/Other_Areas/publications/HTML/MP192/1_Rice_Growth_and_Development_Ripening.asp]
synonym: "maturity stage" []
synonym: "rice growth stage-9" []
is_a: GRO:0007141 ! C-embryo stage

[Term]
id: GRO:0007046
name: 07-milk stage
def: "At this stage\, the developing starch grains in the kernel are soft\, and the interior of the kernel is filled with a white liquid resembling milk." [GR:pj, web:http //www.uaex.edu/Other_Areas/publications/HTML/MP192/1_Rice_Growth_and_Development_Ripening.asp]
synonym: "milk grain" []
synonym: "rice growth stage-7" []
is_a: GRO:0007141 ! C-embryo stage

[Term]
id: GRO:0007047
name: 02-seedling
def: "occurs when the first internode called the mesocotyl has elongated and pushed the tip of the rice coleoptile (epiblast or first sheathing leaf) through the soil surface" [GR:pj, web:http //www.uaex.edu/Other_Areas/publications/HTML/MP192/1_Rice_Growth_and_Development_Vegetative.asp]
comment: The length of the mesocotyl varies with cultivars. Some Semi-dwarf varieties may have a very short mesocotyl and generally will not emerge if covered by more than 1/2 to 3/4 inch of soil. The mesocotyl only develops in the dark and doesnt show up in water-seeded rice
synonym: "rice growth stage-2" []
is_a: GRO:0007139 ! A-vegetative stage

[Term]
id: GRO:0007048
name: 04-stem elongation stage
def: "Begins about the same time panicle initiation is occurring. It continues until full plant height is reached." [GR:pj, web:http //www.uaex.edu/Other_Areas/publications/HTML/MP192/1_Rice_Growth_and_Development_Vegetative.asp]
comment: The top five internodes may elongate. Stem internodes can be distinguished from root internodes by the green color in the stem wall. Overlaps the vegetative and reproductive stages
synonym: "internode elongation" []
synonym: "jointing stage" []
synonym: "rice growth stage-4" []
is_a: GRO:0007139 ! A-vegetative stage
relationship: part_of GRO:0007140 ! B-reproductive stage

[Term]
id: GRO:0007049
name: 03-tillering stage
def: "Usually begins at the fifth leaf stage when the first tiller is visible and emerges from the axillary bud of the second leaf on the culm. Tillering continues when the sixth leaf emerges\, the second tiller comes from the axillary bud of the third leaf." [GR:pj, web:http //www.uaex.edu/Other_Areas/publications/HTML/MP192/1_Rice_Growth_and_Development_Vegetative.asp]
comment: In direct-seeded rice fields with a normal plant population (10 to 20 plants per square foot)\, rice plants generally produce 2 to 5 panicle bearing tillers per plant compared to 10 to 30 tillers per plant in transplanted rice where more space is available between plants.
synonym: "rice growth stage-3" []
is_a: GRO:0007139 ! A-vegetative stage

[Term]
id: GRO:0007051
name: 01-germination
def: "  " [web:http //weeds.montana.edu/crop/Growth_stages_book/p22_23.htm, GR:pj]
is_a: GRO:0007156 ! wheat, barley and oat growth stage

[Term]
id: GRO:0007052
name: 1.01-dry seed
def: "  " [web:http //weeds.montana.edu/crop/Growth_stages_book/p22_23.htm, GR:pj]
comment: Zadok scale-0
is_a: GRO:0007051 ! 01-germination

[Term]
id: GRO:0007053
name: 1.02-start of imbibition
def: "  " [web:http //weeds.montana.edu/crop/Growth_stages_book/p22_23.htm, GR:pj]
comment: Zadok scale-1
is_a: GRO:0007051 ! 01-germination

[Term]
id: GRO:0007054
name: 1.03-imbibition complete
def: "When the imbibition of the seed is complete." [GR:pj, web:http //weeds.montana.edu/crop/Growth_stages_book/p22_23.htm]
comment: Zadok scale-3
is_a: GRO:0007051 ! 01-germination

[Term]
id: GRO:0007055
name: 1.04-radicle emerged from seed
def: "  " [GR:pj, web:http //weeds.montana.edu/crop/Growth_stages_book/p22_23.htm]
comment: Zadok scale-5
is_a: GRO:0007051 ! 01-germination

[Term]
id: GRO:0007056
name: 1.05-coleoptile emerged from seed
def: "  " [GR:pj, web:http //weeds.montana.edu/crop/Growth_stages_book/p22_23.htm]
comment: Zadok scale-7
is_a: GRO:0007051 ! 01-germination

[Term]
id: GRO:0007057
name: 1.06-leaf just at coleoptile tip
def: "The leaf has just emerged." [web:http //weeds.montana.edu/crop/Growth_stages_book/p22_23.htm, GR:pj]
comment: Zadok scale-9\, Haun scale-0
is_a: GRO:0007051 ! 01-germination

[Term]
id: GRO:0007058
name: 02-seedling growth
is_a: GRO:0007156 ! wheat, barley and oat growth stage

[Term]
id: GRO:0007059
name: 2.01-first leaf through coleoptile
def: "  " [GR:pj, web:http //weeds.montana.edu/crop/Growth_stages_book/p22_23.htm]
comment: Zadok scale-10\, Feekes scale-1
is_a: GRO:0007058 ! 02-seedling growth

[Term]
id: GRO:0007060
name: 2.02-first leaf unfolded
def: "  " [web:http //weeds.montana.edu/crop/Growth_stages_book/p22_23.htm, GR:pj]
comment: Zadok scale-11\, Haun scale-1.+
is_a: GRO:0007058 ! 02-seedling growth

[Term]
id: GRO:0007061
name: 2.03-two leaves unfolded
def: "  " [GR:pj, web:http //weeds.montana.edu/crop/Growth_stages_book/p22_23.htm]
comment: Zadok scale-12\, Haun scale-1.+
is_a: GRO:0007058 ! 02-seedling growth

[Term]
id: GRO:0007062
name: 2.04-three leaves unfolded
def: "  " [web:http //weeds.montana.edu/crop/Growth_stages_book/p22_23.htm, GR:pj]
comment: Zadok scale-13\, Haun scale-2.+
is_a: GRO:0007058 ! 02-seedling growth

[Term]
id: GRO:0007063
name: 2.05-four leaves unfolded
def: "  " [GR:pj, web:http //weeds.montana.edu/crop/Growth_stages_book/p22_23.htm]
comment: Zadok scale-14\, Haun scale-3.+
is_a: GRO:0007058 ! 02-seedling growth

[Term]
id: GRO:0007064
name: 2.06-five leaves unfolded
def: "  " [web:http //weeds.montana.edu/crop/Growth_stages_book/p22_23.htm, GR:pj]
comment: Zadok scale-15\, Haun scale-4.+
is_a: GRO:0007058 ! 02-seedling growth

[Term]
id: GRO:0007065
name: 2.07-six leaves unfolded
def: "  " [GR:pj, web:http //weeds.montana.edu/crop/Growth_stages_book/p22_23.htm]
comment: Zadok scale-16\, Haun scale-5.+
is_a: GRO:0007058 ! 02-seedling growth

[Term]
id: GRO:0007066
name: 2.08-seven leaves unfolded
def: "  " [web:http //weeds.montana.edu/crop/Growth_stages_book/p22_23.htm, GR:pj]
comment: Zadok scale-\,  scale-6.+
is_a: GRO:0007058 ! 02-seedling growth

[Term]
id: GRO:0007067
name: 2.09-eight leaves unfolded
def: "  " [GR:pj, web:http //weeds.montana.edu/crop/Growth_stages_book/p22_23.htm]
comment: Zadok scale-18\, Haun scale-7.+
is_a: GRO:0007058 ! 02-seedling growth

[Term]
id: GRO:0007068
name: 2.10 nine or more leaves unfolded
def: "When 9 or more leaves have unfolded or exposed." [web:http //weeds.montana.edu/crop/Growth_stages_book/p22_23.htm, GR:pj]
comment: Zadok scale-19
is_a: GRO:0007058 ! 02-seedling growth

[Term]
id: GRO:0007069
name: 03-tillering
is_a: GRO:0007156 ! wheat, barley and oat growth stage

[Term]
id: GRO:0007070
name: 3.01-main shoot only
def: "  " [GR:pj, web:http //weeds.montana.edu/crop/Growth_stages_book/p22_23.htm]
comment: Zadok scale-20
is_a: GRO:0007069 ! 03-tillering

[Term]
id: GRO:0007071
name: 3.02-main shoot and one tiller
def: "  " [web:http //weeds.montana.edu/crop/Growth_stages_book/p22_23.htm, GR:pj]
comment: Zadok scale-21\, Feekes scale-2
is_a: GRO:0007069 ! 03-tillering

[Term]
id: GRO:0007072
name: 3.03-main shoot and two tillers
def: "  " [GR:pj, web:http //weeds.montana.edu/crop/Growth_stages_book/p22_23.htm]
comment: Zadok scale-22
is_a: GRO:0007069 ! 03-tillering

[Term]
id: GRO:0007073
name: 3.04-main shoot and three tillers
def: "  " [web:http //weeds.montana.edu/crop/Growth_stages_book/p22_23.htm, GR:pj]
comment: Zadok scale-23
is_a: GRO:0007069 ! 03-tillering

[Term]
id: GRO:0007074
name: 3.05-main shoot and four tillers
def: "  " [GR:pj, web:http //weeds.montana.edu/crop/Growth_stages_book/p22_23.htm]
comment: Zadok scale-24
is_a: GRO:0007069 ! 03-tillering

[Term]
id: GRO:0007075
name: 3.06-main shoot and five tillers
def: "  " [web:http //weeds.montana.edu/crop/Growth_stages_book/p22_23.htm, GR:pj]
comment: Zadok scale-25
is_a: GRO:0007069 ! 03-tillering

[Term]
id: GRO:0007076
name: 3.07-shoot and six tillers
def: "  " [GR:pj, web:http //weeds.montana.edu/crop/Growth_stages_book/p22_23.htm]
comment: Zadok scale-26\, Feekes scale-3
is_a: GRO:0007069 ! 03-tillering

[Term]
id: GRO:0007077
name: 3.08-main shoot and seven tillers
def: "  " [web:http //weeds.montana.edu/crop/Growth_stages_book/p22_23.htm, GR:pj]
comment: Zadok scale-27
is_a: GRO:0007069 ! 03-tillering

[Term]
id: GRO:0007078
name: 3.09-main shoot and eight tillers
def: "  " [GR:pj, web:http //weeds.montana.edu/crop/Growth_stages_book/p22_23.htm]
comment: Zadok scale-28
is_a: GRO:0007069 ! 03-tillering

[Term]
id: GRO:0007079
name: 3.10-main shoot and nine or more tillers
def: "  " [web:http //weeds.montana.edu/crop/Growth_stages_book/p22_23.htm, GR:pj]
comment: Zadok scale-29
is_a: GRO:0007069 ! 03-tillering

[Term]
id: GRO:0007080
name: 04-stem elongation
is_a: GRO:0007156 ! wheat, barley and oat growth stage

[Term]
id: GRO:0007081
name: 4.01-pseudo stem erection
def: "  " [GR:pj, web:http //weeds.montana.edu/crop/Growth_stages_book/p22_23.htm]
comment: Zadok scale-30\, Feekes scale 4-5
is_a: GRO:0007080 ! 04-stem elongation

[Term]
id: GRO:0007082
name: 4.02 first node detectable
def: "  " [GR:pj, web:http //weeds.montana.edu/crop/Growth_stages_book/p22_23.htm]
comment: Zadok scale-31\, Feekes scale-6
is_a: GRO:0007080 ! 04-stem elongation

[Term]
id: GRO:0007083
name: 4.03-second node detectable
def: "  " [web:http //weeds.montana.edu/crop/Growth_stages_book/p22_23.htm, GR:pj]
comment: Zadok scale-32\, Feekes scale-7
is_a: GRO:0007080 ! 04-stem elongation

[Term]
id: GRO:0007084
name: 4.04-third node detectable
def: "  " [GR:pj, web:http //weeds.montana.edu/crop/Growth_stages_book/p22_23.htm]
comment: Zadok scale-33
is_a: GRO:0007080 ! 04-stem elongation

[Term]
id: GRO:0007085
name: 4.05-fourth node detectable
def: "  " [web:http //weeds.montana.edu/crop/Growth_stages_book/p22_23.htm, GR:pj]
comment: Zadok scale-34
is_a: GRO:0007080 ! 04-stem elongation

[Term]
id: GRO:0007086
name: 4.06-fifth node detectable
def: "  " [GR:pj, web:http //weeds.montana.edu/crop/Growth_stages_book/p22_23.htm]
comment: Zadok scale-35
is_a: GRO:0007080 ! 04-stem elongation

[Term]
id: GRO:0007087
name: 4.07-sixth node detectable
def: "  " [web:http //weeds.montana.edu/crop/Growth_stages_book/p22_23.htm, GR:pj]
comment: Zadok scale-36
is_a: GRO:0007080 ! 04-stem elongation

[Term]
id: GRO:0007088
name: 4.08-flag leaf just visible
def: "  " [GR:pj, web:http //weeds.montana.edu/crop/Growth_stages_book/p22_23.htm]
comment: Zadok scale-37\, Feekes scale-8
is_a: GRO:0007080 ! 04-stem elongation

[Term]
id: GRO:0007089
name: 4.09-flag leaf ligule/collar just visible
def: "  " [web:http //weeds.montana.edu/crop/Growth_stages_book/p22_23.htm, GR:pj]
comment: Zadok scale-39\, Feekes scale-9
is_a: GRO:0007080 ! 04-stem elongation

[Term]
id: GRO:0007090
name: 05-booting
def: "  " [GR:pj, web:http //weeds.montana.edu/crop/Growth_stages_book/p22_23.htm]
comment: Zadok scale-40
is_a: GRO:0007156 ! wheat, barley and oat growth stage

[Term]
id: GRO:0007091
name: 5.01-flag leaf sheath extending
def: "  " [web:http //weeds.montana.edu/crop/Growth_stages_book/p22_23.htm, GR:pj]
comment: Zadok scale-41\, Haun scale-8 to 9
is_a: GRO:0007090 ! 05-booting

[Term]
id: GRO:0007092
name: 5.02-boots just swollen
def: "  " [web:http //weeds.montana.edu/crop/Growth_stages_book/p22_23.htm, GR:pj]
comment: Zadok scale-45\, Feekes scale-10\, Haun scale-9.2
is_a: GRO:0007090 ! 05-booting

[Term]
id: GRO:0007093
name: 5.03-flag leaf sheath opening
def: "  " [GR:pj, web:http //weeds.montana.edu/crop/Growth_stages_book/p22_23.htm]
comment: Zadok scale-47
is_a: GRO:0007090 ! 05-booting

[Term]
id: GRO:0007094
name: 5.04-first awns visible
def: "  " [GR:pj, web:http //weeds.montana.edu/crop/Growth_stages_book/p22_23.htm]
comment: Zadok scale-49\, Haun scale-10.1
is_a: GRO:0007090 ! 05-booting

[Term]
id: GRO:0007095
name: 06-inflorescence emergence
is_a: GRO:0007156 ! wheat, barley and oat growth stage

[Term]
id: GRO:0007096
name: 6.01-first spikelet of inflorescence visible
def: "  " [GR:pj, web:http //weeds.montana.edu/crop/Growth_stages_book/p22_23.htm]
comment: Zadok scale-50\, Feekes scale-10.1\, Haun scale-10.2
is_a: GRO:0007095 ! 06-inflorescence emergence

[Term]
id: GRO:0007097
name: 6.02-1/4 of inflorescence emerged
def: "When a quarter of the inflorescence has emerged." [web:http //weeds.montana.edu/crop/Growth_stages_book/p22_23.htm, GR:pj]
comment: Zadok scale-53\, Feekes scale-10.2
is_a: GRO:0007095 ! 06-inflorescence emergence

[Term]
id: GRO:0007098
name: 6.03-1/2 of inflorescence emerged
def: "When half of the inflorescence has emerged." [GR:pj, web:http //weeds.montana.edu/crop/Growth_stages_book/p22_23.htm]
comment: Zadok scale-1\, Feekes scale-10.3\, Haun scale-10.5
is_a: GRO:0007095 ! 06-inflorescence emergence

[Term]
id: GRO:0007099
name: 6.04-3/4 of inflorescence emerged
def: "  " [GR:pj, web:http //weeds.montana.edu/crop/Growth_stages_book/p22_23.htm]
comment: Zadok scale-57\, Feekes scale-10.4\, Haun scale-10.7
is_a: GRO:0007095 ! 06-inflorescence emergence

[Term]
id: GRO:0007100
name: 6.05-emergence of inflorescence completed
def: "  " [web:http //weeds.montana.edu/crop/Growth_stages_book/p22_23.htm, GR:pj]
comment: Zadok scale-59\, Feekes scale-10.5\, Haun scale-11
is_a: GRO:0007095 ! 06-inflorescence emergence

[Term]
id: GRO:0007101
name: 07-anthesis
def: "The time of flowering or pollination." [web:http //weeds.montana.edu/crop/Growth_stages_book/p22_23.htm, GR:pj]
is_a: GRO:0007156 ! wheat, barley and oat growth stage

[Term]
id: GRO:0007102
name: 7.01-anthesis beginning
def: "When the of flowering or pollination has just begun" [web:http //weeds.montana.edu/crop/Growth_stages_book/p22_23.htm, GR:pj]
comment: Zadok scale-60\, Feekes scale-10.51\, Haun scale-11.4
synonym: "Beginning on anthesis" []
is_a: GRO:0007101 ! 07-anthesis

[Term]
id: GRO:0007103
name: 7.02-anthesis half-way
def: "When the of flowering or pollination has occurred on 50 percent of  all florets in the inflorescence" [GR:pj, web:http //weeds.montana.edu/crop/Growth_stages_book/p22_23.htm]
comment: Haun scale-11.5
is_a: GRO:0007101 ! 07-anthesis

[Term]
id: GRO:0007104
name: 7.03-anthesis completed
def: "When the flowering or pollination is complete in all florets." [web:http //www.extension.umn.edu/distribution/cropsystems/DC2547.html#systems]
comment: Zadok scale-69\, Haun scale-11.6
is_a: GRO:0007101 ! 07-anthesis

[Term]
id: GRO:0007105
name: 08-milk development
def: "  " [web:http //weeds.montana.edu/crop/Growth_stages_book/p22_23.htm, GR:pj]
comment: Zadok scale-70
is_a: GRO:0007156 ! wheat, barley and oat growth stage

[Term]
id: GRO:0007106
name: 8.01-kernel watery ripe
def: "  " [web:http //weeds.montana.edu/crop/Growth_stages_book/p22_23.htm, GR:pj]
comment: Zadok scale-71\, Feekes scale-10.54\, Haun scale-12.1
is_a: GRO:0007105 ! 08-milk development

[Term]
id: GRO:0007107
name: 8.02-early milk
def: "  " [GR:pj, web:http //weeds.montana.edu/crop/Growth_stages_book/p22_23.htm]
comment: Zadok scale-73\, Haun scale-13
is_a: GRO:0007105 ! 08-milk development

[Term]
id: GRO:0007108
name: 8.04-medium milk
def: "  " [web:http //weeds.montana.edu/crop/Growth_stages_book/p22_23.htm, GR:pj]
comment: Zadok scale-75\, Feekes scale-11.1
is_a: GRO:0007105 ! 08-milk development

[Term]
id: GRO:0007109
name: 8.03-late milk
def: "  " [GR:pj, web:http //weeds.montana.edu/crop/Growth_stages_book/p22_23.htm]
comment: Zadok scale-77
is_a: GRO:0007105 ! 08-milk development

[Term]
id: GRO:0007110
name: 09-dough development
def: "  " [web:http //www.ibiblio.org/botnet/glossary/a_vi.html, GR:pj]
comment: Zadok scale-80
is_a: GRO:0007156 ! wheat, barley and oat growth stage

[Term]
id: GRO:0007111
name: 9.01-early dough
def: "  " [GR:pj, web:http //weeds.montana.edu/crop/Growth_stages_book/p22_23.htm]
comment: Zadok scale-83\, Haun scale-14
is_a: GRO:0007110 ! 09-dough development

[Term]
id: GRO:0007112
name: 9.02-soft dough
def: "   " [GR:pj, web:http //weeds.montana.edu/crop/Growth_stages_book/p22_23.htm]
comment: Zadok scale-85\, Feekes scale-11.2
is_a: GRO:0007110 ! 09-dough development

[Term]
id: GRO:0007113
name: 9.03-hard dough
def: "  " [web:http //weeds.montana.edu/crop/Growth_stages_book/p22_23.htm, GR:pj]
comment: Zadok scale-87\, Haun scale-15
is_a: GRO:0007110 ! 09-dough development

[Term]
id: GRO:0007114
name: 10-ripening
def: "  " [GR:pj, web:http //weeds.montana.edu/crop/Growth_stages_book/p22_23.htm]
comment: Zadok scale-90
is_a: GRO:0007156 ! wheat, barley and oat growth stage

[Term]
id: GRO:0007115
name: 10.01-kernel medium hard
def: "Kernel is difficult to divide by using the thumbnail." [web:http //weeds.montana.edu/crop/Growth_stages_book/p22_23.htm, GR:pj]
comment: Zadok scale-91\, Feekes scale-11.3
is_a: GRO:0007114 ! 10-ripening

[Term]
id: GRO:0007116
name: 10.02-kernel hard
def: "Kernel can no longer be dented with thumbnail." [GR:pj, web:http //weeds.montana.edu/crop/Growth_stages_book/p22_23.htm]
comment: Zadok scale-92\, Feekes scale-11.4\, Haun scale-16
is_a: GRO:0007114 ! 10-ripening

[Term]
id: GRO:0007117
name: 10.03-kernel loosening in daytime
def: "  " [web:http //weeds.montana.edu/crop/Growth_stages_book/p22_23.htm, GR:pj]
comment: Zadok scale-93
is_a: GRO:0007114 ! 10-ripening

[Term]
id: GRO:0007118
name: 10.04-overripe, straw dead and collapsing
def: "  " [GR:pj, web:http //weeds.montana.edu/crop/Growth_stages_book/p22_23.htm]
comment: Zadok scale-94
is_a: GRO:0007114 ! 10-ripening

[Term]
id: GRO:0007119
name: 10.05-seed dormant
def: "  " [web:http //weeds.montana.edu/crop/Growth_stages_book/p22_23.htm, GR:pj]
comment: Zadok scale-95
is_a: GRO:0007114 ! 10-ripening

[Term]
id: GRO:0007120
name: 10.06-viable seed germination
def: "Viable seed giving 50 percent germination." [web:http //weeds.montana.edu/crop/Growth_stages_book/p22_23.htm, GR:pj]
comment: Zadok scale-96
is_a: GRO:0007114 ! 10-ripening

[Term]
id: GRO:0007121
name: 10.07-seed not dormant
def: "  " [GR:pj, web:http //weeds.montana.edu/crop/Growth_stages_book/p22_23.htm]
comment: Zadok scale-97
is_a: GRO:0007114 ! 10-ripening

[Term]
id: GRO:0007122
name: 10.08-secondary dormancy induced
def: "  " [web:http //weeds.montana.edu/crop/Growth_stages_book/p22_23.htm, GR:pj]
comment: Zadok scale-98
is_a: GRO:0007114 ! 10-ripening

[Term]
id: GRO:0007123
name: 10.09-secondary dormancy lost
def: "  " [GR:pj, web:http //weeds.montana.edu/crop/Growth_stages_book/p22_23.htm]
comment: Zadok scale-99
is_a: GRO:0007114 ! 10-ripening

[Term]
id: GRO:0007124
name: sorghum growth stage
def: "Sorghum Development and Key Growth Stages as described by Brent Bean and Carl Patrick\, Extension Agronomist and Entomologist at the Texas A&M\, Agricultural Research and Extension station. " [web:http //primera.tamu.edu/ir4/sor-stage.pdf, GR:pj]
comment: The growth stages defined for Sorghum were extracted from the document at http\://primera.tamu.edu/ir4/sor-stage.pdf
is_a: GRO:0007199 ! cereal plant growth stage ontology

[Term]
id: GRO:0007125
name: 01-seedling emergence
def: "Coleoptile visible at soil surface. " [web:http //primera.tamu.edu/ir4/sor-stage.pdf, GR:pj]
comment: Coleoptile is the first leaf and is shorter than the later emerging leaves and has a rounded tip
synonym: "sorghum growth stage-0" []
is_a: GRO:0007124 ! sorghum growth stage

[Term]
id: GRO:0007126
name: 02-three leaf stage
def: "Collar of 3rd leaf is visible" [GR:pj, web:http //primera.tamu.edu/ir4/sor-stage.pdf]
comment: This stage will occur approximately 10 days after emergence\, depending on soil temperature\, moisture\, planting depth\, etc.
synonym: "sorghum growth stage-1" []
is_a: GRO:0007124 ! sorghum growth stage

[Term]
id: GRO:0007127
name: 04-five leaf stage
def: "Collar of 5th leaf is visible" [GR:pj, web:http //primera.tamu.edu/ir4/sor-stage.pdf]
comment: Occurs approximately 20 days after emergence. May have lost first leaf (coleoptile) by this time.
synonym: "sorghum growth stage-3" []
is_a: GRO:0007124 ! sorghum growth stage

[Term]
id: GRO:0007128
name: 05-growing point differentiation
def: "Growing point visible above the soil surface." [web:http //primera.tamu.edu/ir4/sor-stage.pdf, GR:pj]
comment: Occurs approximately 30 to 35 days after emergence. Generally corresponds with the 7 to 8 leaf stage. May have lost 1 to 3 leaves from the bottom of the plant.
synonym: "sorghum growth stage-4" []
is_a: GRO:0007124 ! sorghum growth stage

[Term]
id: GRO:0007129
name: 06-flag leaf visible
def: "Tip of the flag leaf (last leaf) is visible in the whorl. " [GR:pj, web:http //primera.tamu.edu/ir4/sor-stage.pdf]
comment: The last 3 to 4 leaves may not be fully expanded (collars not visible).
synonym: "sorghum growth stage-5" []
is_a: GRO:0007124 ! sorghum growth stage

[Term]
id: GRO:0007130
name: 07-boot stage
def: "Leaf collars of all leaves are now visible. Sorghum head is enclosed in the flag leaf sheath" [web:http //primera.tamu.edu/ir4/sor-stage.pdf, GR:pj]
comment: Peduncle (stalk supporting the head) is beginning to elongate
synonym: "sorghum growth stage-6" []
is_a: GRO:0007124 ! sorghum growth stage

[Term]
id: GRO:0007131
name: 08-heading
def: "50% of the plants in the field have visible heads" [GR:pj, web:http //primera.tamu.edu/ir4/sor-stage.pdf]
synonym: "half-bloom" []
synonym: "sorghum growth stage-7" []
is_a: GRO:0007124 ! sorghum growth stage

[Term]
id: GRO:0007132
name: 10-dough stage
is_a: GRO:0007124 ! sorghum growth stage

[Term]
id: GRO:0007133
name: 10.01-soft dough
def: "Grain can be easily squeezed between the fingers" [GR:pj, web:http //primera.tamu.edu/ir4/sor-stage.pdf]
comment: 8 to 12 functional leaves present. One half of grain dry weight has accumulated.
synonym: "sorghum growth stage-9" []
is_a: GRO:0007132 ! 10-dough stage

[Term]
id: GRO:0007134
name: 10.02-hard dough
def: "Cannot squeeze grain between the fingers." [web:http //primera.tamu.edu/ir4/sor-stage.pdf, GR:pj]
comment: Three-fourths of grain dry weight has accumulated
synonym: "sorghum growth stage-10" []
is_a: GRO:0007132 ! 10-dough stage

[Term]
id: GRO:0007135
name: 11-physiological maturity
def: "This stage is identified by the dark spot on the tip of the kernel. Grain will contain 25 to 35% moisture." [GR:pj, web:http //primera.tamu.edu/ir4/sor-stage.pdf]
comment: Maximum total dry weight has been achieved
synonym: "black layer" []
synonym: "sorghum growth stage-11" []
is_a: GRO:0007124 ! sorghum growth stage

[Term]
id: GRO:0007136
name: rice plant part development stage
def: "The developmental stages of individual plant parts or organs in a rice plant." [GR:pj]
comment: The rice plant organ developmental stages were defined by the Oryzabase\, in Japan. ref\: http\://www.shigen.nig.ac.jp/rice/oryzabase/development/organAndStage.jsp
is_a: GRO:0007040 ! rice growth stage

[Term]
id: GRO:0007137
name: embryo development
def: "Defines all the stages of embryo development from fertilization stage to maturity stage." [Oryzabase:Embryo, GR:pj]
comment: The embryo developmental stages were defined by the Oryzabase\, in Japan. ref\:  http\://earth.lab.nig.ac.jp\:8080/IneDatabase/query?type=browse&data=embryo&item=All
is_a: GRO:0007136 ! rice plant part development stage

[Term]
id: GRO:0007138
name: leaf development
def: "Defines all the stages of leaf development from recruitment of leaf primordial cells to fully developed leaf." [Oryzabase:Embryo, GR:pj]
comment: The leaf developmental stages were defined by the Oryzabase\, in Japan. ref\:  http\://earth.lab.nig.ac.jp\:8080/IneDatabase/query?type=browse&data=leaf&item=All
is_a: GRO:0007136 ! rice plant part development stage

[Term]
id: GRO:0007139
name: A-vegetative stage
def: "growth stages from germination to panicle initiation stage." [GR:pj, web:http //www.uaex.edu/Other_Areas/publications/HTML/MP192/1_Rice_Growth_and_Development.asp#Vegetative]
comment: The later stage (lag phase) may overlap with the reproductive stage
is_a: GRO:0007001 ! rice plant growth stage

[Term]
id: GRO:0007140
name: B-reproductive stage
def: "Growth stages from panicle initiation to heading stage." [GR:pj, web:http //www.uaex.edu/Other_Areas/publications/HTML/MP192/1_Rice_Growth_and_Development_Reproductive.asp]
is_a: GRO:0007001 ! rice plant growth stage

[Term]
id: GRO:0007141
name: C-embryo stage
def: "Growth stages from fertilization\, embryo formation to ripening and maturation stage." [GR:pj, web:http //www.uaex.edu/Other_Areas/publications/HTML/MP192/1_Rice_Growth_and_Development_Ripening.asp]
comment: Light intensity is very important during this interval since 60 percent or more of the carbohydrates used in grain filling are photosynthesized during this time interval. High temperatures tend to reduce the grain filling period and may reduce grain weight. Low temperatures tend to lengthen the time required for grain fill and ripening.
synonym: "grain-filling stage" []
synonym: "ripening stage" []
is_a: GRO:0007001 ! rice plant growth stage

[Term]
id: GRO:0007142
name: 1-4 leaf stage
def: "The period from development of the first to fourth leaf stage" [GR:pj, web:http //www.uaex.edu/Other_Areas/publications/HTML/MP192/1_Rice_Growth_and_Development_Vegetative.asp]
comment: During this time\, the seminal roots further develop\, the secondary or lateral roots develop and the first four leaves appear
synonym: "pre-tillering" []
synonym: "rice growth stage-2.1" []
is_a: GRO:0007047 ! 02-seedling

[Term]
id: GRO:0007143
name: 03-four leaf stage
def: "Collar of 4th leaf is visible." [web:http //primera.tamu.edu/ir4/sor-stage.pdf, GR:pj]
comment: Occurs approximately 15 days after emergence
synonym: "sorghum growth stage-2" []
is_a: GRO:0007124 ! sorghum growth stage

[Term]
id: GRO:0007144
name: 3.1-maximum tillering
def: "tillering increases in a sigmoidal-shaped curve until the maximum tiller number is reached. At this point\, the main culm may be difficult to distinguish from the tiller." [GR:pj, web:http //www.uaex.edu/Other_Areas/publications/HTML/MP192/1_Rice_Growth_and_Development_Vegetative.asp]
comment: After maximum tillering has occurred\, no more effective tillers are produced. A portion of the late tillers will generally die due to competition effects
synonym: "rice growth stage-3.1" []
is_a: GRO:0007049 ! 03-tillering stage

[Term]
id: GRO:0007145
name: ratooning stage
def: "Producing new tillers from nodes after harvest" [GR:pj \, JCL]
comment: Excluding germination and early seedling stages\, it begins a fresh cycle producing new tillers from nodes post-harvest. It may or may not be considered as a growth stage by others. However\, Gramene is proposing it to be included as one of the new growth stage.
synonym: "rice growth stage-3A" []
is_a: GRO:0007139 ! A-vegetative stage

[Term]
id: GRO:0007146
name: vegetative lag phase
def: "Is the period from the end of active tillering to the beginning of the reproductive stage. Tiller number decreases\, height and stem diameter continue to increase but at a slower rate." [GR:pj, web:http //www.uaex.edu/Other_Areas/publications/HTML/MP192/1_Rice_Growth_and_Development_Vegetative.asp]
comment: The length of this period is a function of the maturation period of the cultivar. For very-short season cultivars with 110-day maturity\, this period may not be evident. In this situation\, maximum tillering stage and the beginning of reproductive growth may overlap. In a 150-day rice cultivar\, the lag phase period may last more than two weeks. The vegetative lag phase in midseason varieties is characterized by yellowing plants
synonym: "rice growth stage-4.3" []
is_a: GRO:0007139 ! A-vegetative stage

[Term]
id: GRO:0007147
name: 4.1-panicle initiation stage
def: "Is the time when the panicle primordia initiate the production of a panicle in the uppermost node of the culm" [GR:pj, web:http //www.uaex.edu/Other_Areas/publications/HTML/MP192/1_Rice_Growth_and_Development_Reproductive.asp]
comment: A thin green band is visible just above the top node\, and represents the very beginning of internode elongation (stem elongation stage) and is evident for only a couple of days
synonym: "PI" []
synonym: "green ring stage" []
synonym: "rice growth stage-4.1" []
relationship: part_of GRO:0007048 ! 04-stem elongation stage

[Term]
id: GRO:0007148
name: 05-booting stage
def: "This stage is characterized by a swelling of the flag leaf sheath\, caused by an increase in the size of the panicle as it grows up the leaf sheath. " [GR:pj, web:http //www.uaex.edu/Other_Areas/publications/HTML/MP192/1_Rice_Growth_and_Development_Reproductive.asp]
synonym: "rice growth stage-5" []
is_a: GRO:0007140 ! B-reproductive stage

[Term]
id: GRO:0007149
name: 5.1-early booting stage
def: "In this stage\, meiosis occurs. Panicle continues to grow." [web:http //www.uaex.edu/Other_Areas/publications/HTML/MP192/1_Rice_Growth_and_Development_Reproductive.asp, GR:pj]
synonym: "rice growth stage-5.1" []
is_a: GRO:0007148 ! 05-booting stage

[Term]
id: GRO:0007150
name: 5.2-late booting stage
def: "In this stage the flag leaf has completely extended. It occurs about 6 days prior to heading. " [GR:pj, web:http //www.uaex.edu/Other_Areas/publications/HTML/MP192/1_Rice_Growth_and_Development_Reproductive.asp]
synonym: "rice growth stage-5.2" []
is_a: GRO:0007148 ! 05-booting stage

[Term]
id: GRO:0007151
name: 6.1-flowering stage
def: "Refers to the events between the opening and closing of floret" [GR:pj, web:http //www.uaex.edu/Other_Areas/publications/HTML/MP192/1_Rice_Growth_and_Development_Reproductive.asp]
comment: The events occurring in this stage are\: (a). The tips of the lemma and palea (hulls) open. #(b) The filaments elongate.# (c). The anthers exsert from the lemma and palea. #(d). As the lemma and palea open further\, the tips of the feathery stigma become visible. #(e). The filaments elongate past the tips of lemma and palea. #(f). The spikelet closes\, leaving the anther outside. Anther dehiscence (pollen shed) usually occurs just prior to or at the time the lemma and palea open (step a).
synonym: "anthesis" []
synonym: "anthesis stage" []
synonym: "rice growth stage-6.1" []
is_a: GRO:0007044 ! 06-heading stage

[Term]
id: GRO:0007152
name: 8.1-dough stage
def: "The starch in the grain begins to become firm but is still soft" [GR:pj, web:http //www.uaex.edu/Other_Areas/publications/HTML/MP192/1_Rice_Growth_and_Development_Ripening.asp]
synonym: "early dough grain" []
synonym: "early dough stage" []
synonym: "rice growth stage-8.1" []
is_a: GRO:0007042 ! 08-dough stage

[Term]
id: GRO:0007153
name: 09-flowering
def: "Occurs when 50% of the plants in the field are in some stage of bloom" [web:http //primera.tamu.edu/ir4/sor-stage.pdf, GR:pj]
comment: Flowering occurs over a 4 to 9 day period.
synonym: "sorghum growth stage8" []
is_a: GRO:0007124 ! sorghum growth stage

[Term]
id: GRO:0007154
name: 8.2-hard dough stage
def: "The whole grain is firm during this stage and almost ready for harvest. The moisture content is still above 22 percent." [GR:pj, web:http //www.uaex.edu/Other_Areas/publications/HTML/MP192/1_Rice_Growth_and_Development_Ripening.asp]
synonym: "late dough grain" []
synonym: "late dough stage" []
synonym: "rice growth stage-8.2" []
is_a: GRO:0007042 ! 08-dough stage

[Term]
id: GRO:0007156
name: wheat, barley and oat growth stage
alt_id: GRO:0007050
alt_id: GRO:0007155
def: "The development and growth of cereals wheat\, oat and barley has been translated into several numeric scales to quantify development for scientific and management purposes. These are based on the most commonly used scales defined by Feekes\, Zadok and Haun." [GR:pj, web:http //weeds.montana.edu/crop/Growth_stages_book/p22_23.htm]
comment: The curators have extracted the growth stage information based on the document available at http\://weeds.montana.edu/crop/Growth_stages_book/p22_23.htm
synonym: "Triticeae plant growth stage" []
synonym: "barley growth stage" []
synonym: "oat growth stage" []
synonym: "wheat growth stage" []
is_a: GRO:0007199 ! cereal plant growth stage ontology

[Term]
id: GRO:0007157
name: panicle development
def: "Defines all the stages of panicle or rice inflorescence development from switching over of the stem apical meristem into rachis meristem to mature panicle formation." [Oryzabase:Embryo, GR:pj]
comment: The panicle developmental stages were defined by the Oryzabase\, in Japan. ref\: http\://earth.lab.nig.ac.jp\:8080/IneDatabase/query?type=browse&data=panicle&item=All
is_a: GRO:0007136 ! rice plant part development stage

[Term]
id: GRO:0007158
name: spikelet development
def: "Defines all the stages of spikelet development from formation of rudimentary glumes to floret development." [Oryzabase:Embryo, GR:pj]
comment: The spikelet developmental stages were defined by the Oryzabase\, in Japan. ref\: http\://earth.lab.nig.ac.jp\:8080/IneDatabase/query?type=browse&data=spikelet&item=All
is_a: GRO:0007136 ! rice plant part development stage

[Term]
id: GRO:0007159
name: stamen development
def: "Defines all the stages of stamen development from stamen primordia differentiation to end of microgametogenesis." [GR:pj, Oryzabase:Embryo]
comment: The stamen developmental stages were defined by the Oryzabase\, in Japan. ref\: http\://earth.lab.nig.ac.jp\:8080/IneDatabase/query?type=browse&data=stamen&item=All
is_a: GRO:0007136 ! rice plant part development stage

[Term]
id: GRO:0007160
name: ovule development
def: "Defines all the stages of ovule development from carpel primordium formation to megagametogenesis." [Oryzabase:Embryo, GR:pj]
comment: The ovule developmental stages were defined by the Oryzabase\, in Japan. ref\: http\://earth.lab.nig.ac.jp\:8080/IneDatabase/query?type=browse&data=ovule&item=All
is_a: GRO:0007136 ! rice plant part development stage

[Term]
id: GRO:0007161
name: leaf stage P0
def: "Recruitment of leaf founder or primordial cells occurs." [Oryzabase:Leaf, GR:pj]
comment: Marked by down regulation of Osh1 gene (GR_protein_id=77897) and expression of OsPnh gene (GR_protein_id=90881).
is_a: GRO:0007138 ! leaf development

[Term]
id: GRO:0007162
name: leaf stage P4
def: "Elongation of leaf blade occurs along with differentiation of epidermis specific bulliform cells\, silica cells\, cork cells and stomata.  " [Oryzabase:Leaf, GR:pj]
is_a: GRO:0007138 ! leaf development

[Term]
id: GRO:0007163
name: leaf stage P2
def: "Foot-like shape\, with overlapping of two leaf margins occurs along with differentiation of vascular bundle and establishment of leaf domains along the central-marginal axis." [Oryzabase:Leaf, GR:pj]
is_a: GRO:0007138 ! leaf development

[Term]
id: GRO:0007164
name: leaf stage P1
def: "Protrusion of leaf primordium and elongation of leaf margin around stem apical meristem (SAM) occurs." [Oryzabase:Leaf, GR:pj]
is_a: GRO:0007138 ! leaf development

[Term]
id: GRO:0007165
name: leaf stage P5
def: "Elongation of leaf sheath\, emergence of leaf blade from the sheath of preceding leaf and formation of lacunae occurs. The leaf blade\, sheath\, ligule and auricles are fully developed in the juvenile leaf." [Oryzabase:Leaf, GR:pj]
is_a: GRO:0007138 ! leaf development

[Term]
id: GRO:0007166
name: leaf stage P3
def: "Formation of ligule primordia and leaf blade and leaf sheath boundary occurs\, along with differentiation of sclerenchymatous cells and initiation of epidermis." [GR:pj, Oryzabase:Leaf]
is_a: GRO:0007138 ! leaf development

[Term]
id: GRO:0007167
name: leaf stage PX
def: "Completely mature adult leaf." [GR:pj, Oryzabase:Leaf]
is_a: GRO:0007138 ! leaf development

[Term]
id: GRO:0007168
name: embryo stage EM1
def: "The stage marked by the fertilization event." [Oryzabase:Embryo, GR:pj]
comment: Occurs at zero days after pollination. Number of embryo cells at this stage are one (zygote).
is_a: GRO:0007137 ! embryo development

[Term]
id: GRO:0007169
name: embryo stage EM5
def: "Marked with onset of coleoptile\, stem apical meristem (SAM) and radicle differentiation." [GR:pj, Oryzabase:Embryo]
comment: Occurs at four days after pollination.
is_a: GRO:0007137 ! embryo development

[Term]
id: GRO:0007170
name: embryo stage EM3
def: "Globular stage of the embryo." [Oryzabase:Embryo, GR:pj]
comment: Occurs at tow days after pollination.
is_a: GRO:0007137 ! embryo development

[Term]
id: GRO:0007171
name: embryo stage EM2
def: "First division of fertilized egg. Globular stage ca.25-cell stage marked with rapid cell division." [Oryzabase:Leaf, GR:pj]
comment: Occurs at one day after pollination.
is_a: GRO:0007137 ! embryo development

[Term]
id: GRO:0007172
name: embryo stage EM6
def: "Protrusion of first leaf primordium and enlargement of scutellum occurs at this stage. Marks the onset of juvenile vegetative stage." [GR:pj, Oryzabase:Embryo]
comment: Occurs at five-six days after pollination. Expression of Amy1A (GR_protein_id=77717) in scutellar epithelium appears.
is_a: GRO:0007137 ! embryo development

[Term]
id: GRO:0007173
name: embryo stage EM4
def: "It's a globular stage with oblong-shaped embryo. Marked by onset of exponential increase in size and cell number. Formation of gradient of cell size along dorsoventral direction and marked regionalization in the developing embryo." [GR:pj, Oryzabase:Embryo]
comment: Occurs at three days after pollination.
is_a: GRO:0007137 ! embryo development

[Term]
id: GRO:0007174
name: embryo stage EM7
def: "Identified by protrusion of 2nd and 3rd leaf primordia and epiblast." [GR:pj, Oryzabase:Embryo]
comment: Occurs at seven-eight days after pollination.
is_a: GRO:0007137 ! embryo development

[Term]
id: GRO:0007175
name: embryo stage EM8
def: "Enlargement of embryo parts and morphological completion." [Oryzabase:Embryo, GR:pj]
comment: Occurs at nine-ten days after pollination. Expression of maturation-related genes such as OsEM (GR_protein_id=77791)\, Rab16A\, VP1 (GR_protein_id=78075\, 89294) observed.
is_a: GRO:0007137 ! embryo development

[Term]
id: GRO:0007176
name: embryo stage EM9
def: "Embryo maturation process begins." [GR:pj, Oryzabase:Embryo, GR_ref:6590]
comment: Occurs at eleven-twenty days after pollination. Expression of maturation-related genes such as OsEM (GR_protein_id=77791)\, Rab16A\, VP1 (GR_protein_id=78075\, 89294) observed.
is_a: GRO:0007137 ! embryo development

[Term]
id: GRO:0007177
name: embryo stage EM10
def: "Embryo gains dormancy and tolerance for desiccation. Embryonic shoot\, radicle\, scutellum\, epiblast and bundle sheath are mature." [GR:pj, Oryzabase:Embryo, GR_ref:6590]
comment: Occurs at 21 and onwards of days after pollination.
is_a: GRO:0007137 ! embryo development

[Term]
id: GRO:0007178
name: ovule stage OV0
def: "Starts with carpel primordium formation." [GR:pj, Oryzabase:Ovule]
comment: Panicle length at this stage is less than 0.3 cm.
is_a: GRO:0007160 ! ovule development

[Term]
id: GRO:0007179
name: ovule stage OV4
def: "Meiotic division of the megaspore mother cell results in a linear tetrad of megaspores. The inner integument elongation also occurs." [GR_Ref:2512, Oryzabase:Ovule, GR:pj]
comment: Panicle length at this stage is about 5-7 cm.
is_a: GRO:0007160 ! ovule development

[Term]
id: GRO:0007180
name: ovule stage OV2
def: "Integument primordia are initiated on both sides of the ovule primordium. Megasporogenesis starts with the formation of archespore from one of the sub-epidermal cells in the nucellus. The archespore is distinguished by its large size. " [GR_Ref:2512, GR:pj, Oryzabase:Ovule]
comment: Panicle length at this stage is about 1-3 cm.
is_a: GRO:0007160 ! ovule development

[Term]
id: GRO:0007181
name: ovule stage OV1
def: "Ovule primordium formation and carpel elongation occurs." [GR:pj, GR_Ref:2512, Oryzabase:Ovule]
comment: Panicle length at this stage is about 0.3-1.0 cm.
is_a: GRO:0007160 ! ovule development

[Term]
id: GRO:0007182
name: ovule stage OV5
def: "The inner integument fully encloses the nucellus\, except for the area where micropyle forms. The ovule acquires an anatropous shape by rotating 60 degrees from its original position." [GR:pj, GR_Ref:2512, Oryzabase:Ovule]
comment: Panicle length at this stage is about 7-10 cm.
is_a: GRO:0007160 ! ovule development

[Term]
id: GRO:0007183
name: ovule stage OV3
def: "Integument primordia starts differentiation\, firstly into outer integument and later into the outer integument. Funiculus develops on adaxial side of the ovary. The archespore expands and differentiates into the megaspore mother cell. The megaspore mother cell is polarized with its nucleus at the micropylar end." [GR_Ref:2512, GR:pj, Oryzabase:Ovule]
comment: Panicle length at this stage is about 3-5 cm.
is_a: GRO:0007160 ! ovule development

[Term]
id: GRO:0007184
name: ovule stage OV6
def: "Micropylar megaspore degenerates and the functional megaspore enlarges. " [GR_Ref:2512, Oryzabase:Ovule, GR:pj]
comment: Panicle length at this stage is about 10-12 cm.
is_a: GRO:0007160 ! ovule development

[Term]
id: GRO:0007185
name: ovule stage OV7
def: "The developing embryosac is at the two-nucleate megagametophyte stage. Degenerate megaspores are still visible. Marks the start of megagametogenesis." [GR:pj, GR_Ref:2512, Oryzabase:Ovule]
comment: Panicle length at this stage is about 12-14 cm.
is_a: GRO:0007160 ! ovule development

[Term]
id: GRO:0007186
name: ovule stage OV10
def: "Embryosac matures. The events include\, polarization of the egg cell and synergids\, fusion of the polar nuclei and mitosis of the antipodal cells to yield as many as eight cells. A single layer of four to five nucellus cells borders the micropyle." [GR:pj, GR_Ref:2512, Oryzabase:Ovule]
comment: Panicle length at this stage is about 18-25 cm.
is_a: GRO:0007160 ! ovule development

[Term]
id: GRO:0007187
name: ovule stage OV9
def: "Formation of eight nucleate megagametophyte\, followed by migration of the nuclei and cellularization. The ovule rotates approximately 90 degrees from its original position." [GR:pj, GR_Ref:2512, Oryzabase:Ovule]
comment: Panicle length at this stage is about 6-18 cm.
is_a: GRO:0007160 ! ovule development

[Term]
id: GRO:0007188
name: ovule stage OV8
def: "Large central vacuole develops between the two nuclei of megagametophyte\, followed by mitosis of both the nuclei\, resulting in the four nucleate stage. " [GR_Ref:2512, Oryzabase:Ovule, GR:pj]
comment: Panicle length at this stage is about 14-16 cm.
is_a: GRO:0007160 ! ovule development

[Term]
id: GRO:0007189
name: panicle stage PA1
def: "Starts with conversion of stem apical meristem into inflorescence (panicle) apical meristem or rachis meristem." [GR:pj, Oryzabase:Panicle]
is_a: GRO:0007157 ! panicle development

[Term]
id: GRO:0007190
name: panicle stage PA6
def: "Formation of lateral meristems from primary rachis meristem occurs." [Oryzabase:Panicle, GR:pj]
comment: Rachis is about 0.7 mm in length.
is_a: GRO:0007157 ! panicle development

[Term]
id: GRO:0007191
name: callus initiation
def: "Beginning of the callus formation from a single protoplast or pollen cell" [GR:pj]
is_a: GRO:0007000 ! in-vitro culture stage

[Term]
id: GRO:0007192
name: callus promotion
def: "multiplication of the callus in undifferentiated form" [GR:pj]
is_a: GRO:0007000 ! in-vitro culture stage

[Term]
id: GRO:0007193
name: plantlet regeneration
def: "Differentiation of  the callus tissue in the plantlet form." [GR:pj]
synonym: "callus regeneration" []
is_a: GRO:0007000 ! in-vitro culture stage

[Term]
id: GRO:0007194
name: 0.01-imbibition
def: "Adsorption of water by colloidal materials of the seed\, leading to seed swelling and increased metabolic activity in the initial stages of germination." [MaizeDB:64054]
synonym: "maize growth stage-0.1" []
is_a: GRO:0007003 ! 00-germination

[Term]
id: GRO:0007195
name: panicle stage PA4
def: "Formation of third and subsequent bracts and 7-15 primary branch primordia occurs. Rachis meristem aborts turning the panicle into a determinate inflorescence from its indeterminate type in early stages of development." [Oryzabase:Panicle, GR:pj]
comment: Rachis is about 0.1 mm in length.
is_a: GRO:0007157 ! panicle development

[Term]
id: GRO:0007196
name: panicle stage PA2
def: "Rachis meristem enlarges and first bract formation occurs." [Oryzabase:Panicle, GR:pj]
is_a: GRO:0007157 ! panicle development

[Term]
id: GRO:0007197
name: panicle stage PA8
is_a: GRO:0007157 ! panicle development

[Term]
id: GRO:0007198
name: panicle stage PA7
def: "Formation of spikelets and florets occurs." [GR:pj, Oryzabase:Panicle]
comment: Rachis is more than 1 mm in length.
is_a: GRO:0007157 ! panicle development

[Term]
id: GRO:0007199
name: cereal plant growth stage ontology
alt_id: GRO:0080001
def: "Ontology of the growth stages in various cereal crops." [GR:pj]
synonym: "cereal plant ontology" []

[Term]
id: GRO:0007200
name: panicle stage PA5
def: "Elongation of primary branch primordia occurs." [GR:pj, Oryzabase:Panicle]
comment: Marked by down regulation of OsH1 gene in rachis meristem. Rachis is less than 0.5 mm in length.
is_a: GRO:0007157 ! panicle development

[Term]
id: GRO:0007201
name: panicle stage PA3
def: "Rachis meristem enlarges and second bract formation occurs." [GR:pj, Oryzabase:Panicle]
is_a: GRO:0007157 ! panicle development

[Term]
id: GRO:0007202
name: spikelet stage SP1
def: "Formation of two rudimentary glumes in distichous phyllotaxy occurs." [GR:pj, Oryzabase:Spikelet]
is_a: GRO:0007158 ! spikelet development

[Term]
id: GRO:0007203
name: spikelet stage SP5
def: "Formation of lodicules occurs." [Oryzabase:Spikelet, GR:pj]
is_a: GRO:0007158 ! spikelet development

[Term]
id: GRO:0007204
name: spikelet stage SP3
def: "Formation of lemma in distichous phyllotaxy occurs." [Oryzabase:Spikelet, GR:pj]
is_a: GRO:0007158 ! spikelet development

[Term]
id: GRO:0007205
name: spikelet stage SP2
def: "Formation of two empty glumes in distichous phyllotaxy occurs." [GR:pj, Oryzabase:Spikelet]
is_a: GRO:0007158 ! spikelet development

[Term]
id: GRO:0007206
name: spikelet stage SP6
def: "Formation of stamen primordia in a whorl occurs." [GR:pj, Oryzabase:Spikelet]
is_a: GRO:0007158 ! spikelet development

[Term]
id: GRO:0007207
name: spikelet stage SP4
def: "Formation of Palea in distichous phyllotaxy occurs." [GR:pj, Oryzabase:Spikelet]
is_a: GRO:0007158 ! spikelet development

[Term]
id: GRO:0007208
name: spikelet stage SP7
def: "Starts with formation of carpel primordium and establishment of rudimentary and empty glumes\, lemma\, palea\, stamen and pistil occurs." [Oryzabase:Spikelet, GR:pj]
is_a: GRO:0007158 ! spikelet development

[Term]
id: GRO:0007209
name: stamen stage ST0
def: "Stamen primordia differentiation occurs." [GR:pj, Oryzabase:Stamen]
comment: At this stage floret is less than 1 mm in length.
is_a: GRO:0007159 ! stamen development

[Term]
id: GRO:0007210
name: stamen stage ST3
def: "Primary parietal cells periclinally divide into endothecium and secondary parietal cells." [GR:pj, Oryzabase:Stamen]
comment: At this stage floret is less than 2 mm in length.
is_a: GRO:0007159 ! stamen development

[Term]
id: GRO:0007211
name: stamen stage ST1
def: "Archesporial cell differentiate at four corners of the anther hypodermal layer." [GR:pj, Oryzabase:Stamen]
comment: At this stage floret is about 1 mm in length.
is_a: GRO:0007159 ! stamen development

[Term]
id: GRO:0007212
name: stamen stage ST5
def: "This stage describes the microsporogenesis in rice plant." [GR:pj, Oryzabase:Stamen]
comment: At this stage floret is about 2-5 mm in length.
is_a: GRO:0007159 ! stamen development

[Term]
id: GRO:0007213
name: stamen stage ST4
def: "Secondary parietal cells periclinally divide into middle layer and tapetum cells. Premeiotic DNA synthesis occurs and Pollen mother cell (PMC) enters into meiosis stage." [Oryzabase:Stamen, GR:pj]
comment: At this stage floret is about 2 mm in length.
is_a: GRO:0007159 ! stamen development

[Term]
id: GRO:0007214
name: stamen stage ST2
def: "Archesporial cells divide into primary sporogenous cells and primary parietal cells." [Oryzabase:Stamen, GR:pj]
comment: At this stage floret is about 1.5 mm in length.
is_a: GRO:0007159 ! stamen development

[Term]
id: GRO:0007215
name: obsolete cereal plant growth stage terms
def: "Terms that are deleted from growth stage ontology are assigned this new parent term." [GR:pj]
is_obsolete: true

[Term]
id: GRO:0007216
name: 1.1-dry seed
def: "The physiologically mature seed that is ready to undergo the germination phase. The seed may or maynot be in the dormant state." [GR:pj ""]
is_a: GRO:0007043 ! 01-germination

[Term]
id: GRO:0007217
name: stamen stage ST5-1
def: "Pollen mother cell meiosis enters Meiosis-I leptotene stage." [Oryzabase:Stamen, GR:pj]
is_a: GRO:0007212 ! stamen stage ST5

[Term]
id: GRO:0007218
name: stamen stage ST5-2
def: "Pollen mother cell meiosis enters Meiosis-I zygotene stage." [GR:pj, Oryzabase:Stamen]
is_a: GRO:0007212 ! stamen stage ST5

[Term]
id: GRO:0007219
name: stamen stage ST5-3
def: "Pollen mother cell meiosis enters Meiosis-I pachytene stage." [Oryzabase:Stamen, GR:pj]
comment: At this stage floret is about 3-3.4 mm in length.
is_a: GRO:0007212 ! stamen stage ST5

[Term]
id: GRO:0007220
name: stamen stage ST5-4
def: "Pollen mother cell meiosis enters Meiosis-I diplotene stage." [GR:pj, Oryzabase:Stamen]
comment: At this stage floret is about 3.5 mm in length.
is_a: GRO:0007212 ! stamen stage ST5

[Term]
id: GRO:0007221
name: stamen stage ST5-5
def: "Pollen mother cell meiosis enters Meiosis-I diakinesis stage." [Oryzabase:Stamen, GR:pj]
comment: At this stage floret is about 3.8 mm in length.
is_a: GRO:0007212 ! stamen stage ST5

[Term]
id: GRO:0007222
name: stamen stage ST5-6
def: "Pollen mother cell meiosis enters Meiosis-I metaphase-I and anaphase-I stage." [GR:pj, Oryzabase:Stamen]
comment: At this stage floret is about 4.2 mm in length.
is_a: GRO:0007212 ! stamen stage ST5

[Term]
id: GRO:0007223
name: stamen stage ST5-7
def: "Pollen mother cell meiosis enters Meiosis-II stage." [Oryzabase:Stamen, GR:pj]
comment: At this stage floret is about 4.5 mm in length.
is_a: GRO:0007212 ! stamen stage ST5

[Term]
id: GRO:0007224
name: stamen stage ST5-8
def: "Tetrad formation occurs. Endothecium and middle layer cells degrade." [GR:pj, Oryzabase:Stamen]
comment: At this stage floret is about 5 mm in length.
is_a: GRO:0007212 ! stamen stage ST5

[Term]
id: GRO:0007225
name: stamen stage ST6
def: "Describes the microgametogenesis stages in rice plant." [GR:pj]
is_a: GRO:0007159 ! stamen development

[Term]
id: GRO:0007226
name: stamen stage ST6-1
def: "Uninucleate pollen formation." [GR:pj, Oryzabase:Stamen]
is_a: GRO:0007225 ! stamen stage ST6

[Term]
id: GRO:0007227
name: stamen stage ST6-3
def: "Pollen is in binucleate stage." [GR:pj, Oryzabase:Stamen]
is_a: GRO:0007225 ! stamen stage ST6

[Term]
id: GRO:0007228
name: stamen stage ST6-2
def: "Pollen undergoes mitosis-I." [Oryzabase:Stamen, GR:pj]
is_a: GRO:0007225 ! stamen stage ST6

[Term]
id: GRO:0007229
name: stamen stage ST6-4
def: "Pollen undergoes mitosis-II." [Oryzabase:Stamen, GR:pj]
is_a: GRO:0007225 ! stamen stage ST6

[Term]
id: GRO:0007230
name: stamen stage ST6-5
def: "Pollen undergoes maturation phase and so the anthers. " [GR:pj, Oryzabase:Stamen]
comment: At this stage floret is about 7 mm in length.
is_a: GRO:0007225 ! stamen stage ST6

[Term]
id: GRO:0007231
name: 1.2-imbibition stage
def: "Absorption of water by  the seed\, leading to the swelling of endosperm\, embryo and seedcoat tissues. The process increases metabolic activity in the initial stages of germination." [GR:pj]
is_a: GRO:0007043 ! 01-germination

[Term]
id: GRO:0007232
name: 1.21-early imbibition stage
def: "The process of absorption of water by  the seed\, leading to the swelling of endosperm\, embryo and seedcoat tissues has just begun. Compared to the dry state seed\, the metabolic activity may not show any significant increase at this stage." [GR:pj]
is_a: GRO:0007231 ! 1.2-imbibition stage

[Term]
id: GRO:0007233
name: 1.22-late imbibition stage
def: "Absorption of water by  the seed\, leading to the swelling of endosperm\, embryo and seedcoat tissues is complete. The increase in metabolic activity is well established." [GR:pj]
is_a: GRO:0007231 ! 1.2-imbibition stage

[Term]
id: GRO:0007234
name: 1.3-radicle emergence stage
def: "The radicle and its enclosing sheath\, the coleorhiza\, breaks through the pericarp. In some rice varieties the coleoptile emerges before the radicle." [GR:pj]
is_a: GRO:0007236 ! 1.3-radicle and coleoptile emergence stage

[Term]
id: GRO:0007235
name: 1.3-coleoptile emergence stage
def: "The coleoptile\, enclosing the plumule emerges through the pericarp. In some rice varieties the radicle emerges before the coleoptile." [GR:pj]
is_a: GRO:0007236 ! 1.3-radicle and coleoptile emergence stage

[Term]
id: GRO:0007236
name: 1.3-radicle and coleoptile emergence stage
def: "The radicle with coleorhiza and coleoptile\, enclosing the plumule\, breaks through the pericarp. In some rice varieties the coleoptile and radicle emergence may occur together or preceed either depending on the rice variety. " [GR:pj]
is_a: GRO:0007043 ! 01-germination

[Typedef]
id: part_of
name: part of

