format-version: 1.2
date: 03:06:2010 15:36
default-namespace: museum

[Term]
id: COLLECTION:0000000
name: fish_collection_abbreviation
def: "List of collection abbreviations based on Catalog of Fishes (Eschmeyer et al. 1998) with modifications from http://silurus.acnatsci.org/ACSI/museums/abbrev.html" [Phenoscape:Curator]

[Term]
id: COLLECTION:0000001
name: ABE
def: "Personal collection of T. Abe; some types are housed at the Tokyo fish market. Collection will be transferred." [COLLECTION:curator]
synonym: "Personal collection of T. Abe; some types are housed at the Tokyo fish market. Collection will be transferred." EXACT []
is_a: COLLECTION:0000000 ! fish_collection_abbreviation

[Term]
id: COLLECTION:0000002
name: ACAP
def: "Aquaculture Center, Aomori, Japan." [COLLECTION:curator]
synonym: "Aquaculture Center, Aomori, Japan." EXACT []
xref: urn\:lsid\:biocol.org\:col:35146
is_a: COLLECTION:0000000 ! fish_collection_abbreviation

[Term]
id: COLLECTION:0000003
name: AFAQ
def: "Amateur Fisheries Association of Queensland, Australia. Most specimens transferred to Queensland Museum (QM), Brisbane." [COLLECTION:curator]
synonym: "Amateur Fisheries Association of Queensland, Australia. Most specimens transferred to Queensland Museum (QM), Brisbane." EXACT []
is_a: COLLECTION:0000000 ! fish_collection_abbreviation

[Term]
id: COLLECTION:0000004
name: AFY
def: "Agustin Fernandez-Yepez collection. Personal collection; at least some of this collection is at SCN, Venezuela." [COLLECTION:curator]
synonym: "Agustin Fernandez-Yepez collection. Personal collection; at least some of this collection is at SCN, Venezuela." EXACT []
is_a: COLLECTION:0000000 ! fish_collection_abbreviation

[Term]
id: COLLECTION:0000005
name: AHF
def: "Allan Hancock Foundation, University of Southern California, California, U.S.A. Types incorporated into the LACM collection." [COLLECTION:curator]
synonym: "Allan Hancock Foundation, University of Southern California, California, U.S.A. Types incorporated into the LACM collection." EXACT []
is_a: COLLECTION:0000000 ! fish_collection_abbreviation

[Term]
id: COLLECTION:0000006
name: AIM
def: "Auckland Institute and Museum, Auckland, New Zealand." [COLLECTION:curator]
synonym: "Auckland Institute and Museum, Auckland, New Zealand." EXACT []
is_a: COLLECTION:0000000 ! fish_collection_abbreviation

[Term]
id: COLLECTION:0000007
name: ALA
def: "University of Alabama Museum of Natural History, University, Alabama, U.S.A." [COLLECTION:curator]
synonym: "University of Alabama Museum of Natural History, University, Alabama, U.S.A." EXACT []
is_a: COLLECTION:0000000 ! fish_collection_abbreviation

[Term]
id: COLLECTION:0000008
name: AMG
def: "Albany Museum, Grahamstown, South Africa." [COLLECTION:curator]
synonym: "Albany Museum, Grahamstown, South Africa." EXACT []
xref: urn\:lsid\:biocol.org\:col:35147
is_a: COLLECTION:0000000 ! fish_collection_abbreviation

[Term]
id: COLLECTION:0000009
name: AMNH
def: "American Museum of Natural History, New York, U.S.A." [COLLECTION:curator]
synonym: "American Museum of Natural History, New York, U.S.A." EXACT []
is_a: COLLECTION:0000000 ! fish_collection_abbreviation

[Term]
id: COLLECTION:0000010
name: AMS
def: "Australian Museum, Sydney, N. S. W., Australia." [COLLECTION:curator]
synonym: "Australian Museum, Sydney, N. S. W., Australia." EXACT []
is_a: COLLECTION:0000000 ! fish_collection_abbreviation

[Term]
id: COLLECTION:0000011
name: ANSP
def: "Academy of Natural Sciences, Philadelphia, Pennsylvania, U.S.A." [COLLECTION:curator]
synonym: "Academy of Natural Sciences, Philadelphia, Pennsylvania, U.S.A." EXACT []
is_a: COLLECTION:0000000 ! fish_collection_abbreviation

[Term]
id: COLLECTION:0000012
name: ARC
def: "Atlantic Reference Centre, New Brunswick, Canada." [COLLECTION:curator]
synonym: "Atlantic Reference Centre, New Brunswick, Canada." EXACT []
is_a: COLLECTION:0000000 ! fish_collection_abbreviation

[Term]
id: COLLECTION:0000013
name: ASIO
def: "Academia Sinica Institute of Oceanology, Quingdao, China." [COLLECTION:curator]
synonym: "Academia Sinica Institute of Oceanology, Quingdao, China." EXACT []
is_a: COLLECTION:0000000 ! fish_collection_abbreviation

[Term]
id: COLLECTION:0000014
name: ASIZB
def: "Academia Sinica Institute of Zoology, Beijing, China." [COLLECTION:curator]
synonym: "Academia Sinica Institute of Zoology, Beijing, China." EXACT []
xref: urn\:lsid\:biocol.org\:col:35148
is_a: COLLECTION:0000000 ! fish_collection_abbreviation

[Term]
id: COLLECTION:0000015
name: ASIZP
def: "See ASIZT." [COLLECTION:curator]
synonym: "See ASIZT." EXACT []
is_a: COLLECTION:0000000 ! fish_collection_abbreviation

[Term]
id: COLLECTION:0000016
name: ASIZT
def: "Academia Sinica Institute of Zoology, Taipei, Taiwan. Also seen as ASIZP." [COLLECTION:curator]
synonym: "Academia Sinica Institute of Zoology, Taipei, Taiwan. Also seen as ASIZP." EXACT []
is_a: COLLECTION:0000000 ! fish_collection_abbreviation

[Term]
id: COLLECTION:0000017
name: ASU
def: "Arizona State University, Tempe, Arizona, U.S.A." [COLLECTION:curator]
synonym: "Arizona State University, Tempe, Arizona, U.S.A." EXACT []
is_a: COLLECTION:0000000 ! fish_collection_abbreviation

[Term]
id: COLLECTION:0000018
name: AUM
def: "Auburn University Museum, Auburn, Alabama, U.S.A." [COLLECTION:curator]
synonym: "Auburn University Museum, Auburn, Alabama, U.S.A." EXACT []
xref: urn\:lsid\:biocol.org\:col:35149
is_a: COLLECTION:0000000 ! fish_collection_abbreviation

[Term]
id: COLLECTION:0000019
name: BAH
def: "Biologische Anstalt Helgoland Marine Station, Helgoland, Germany." [COLLECTION:curator]
synonym: "Biologische Anstalt Helgoland Marine Station, Helgoland, Germany." EXACT []
is_a: COLLECTION:0000000 ! fish_collection_abbreviation

[Term]
id: COLLECTION:0000020
name: BCFH
def: "Bureau of Commercial Fisheries, Honlulu, Hawaii. Much of collection transferred to BPBM." [COLLECTION:curator]
synonym: "Bureau of Commercial Fisheries, Honlulu, Hawaii. Much of collection transferred to BPBM." EXACT []
is_a: COLLECTION:0000000 ! fish_collection_abbreviation

[Term]
id: COLLECTION:0000021
name: BCPM
def: "British Columbia Provincial Museum, Victoria B. C., Canada. Now RBCM = Royal British Columbia Museum." [COLLECTION:curator]
synonym: "British Columbia Provincial Museum, Victoria B. C., Canada. Now RBCM = Royal British Columbia Museum." EXACT []
is_a: COLLECTION:0000000 ! fish_collection_abbreviation

[Term]
id: COLLECTION:0000022
name: BCUE
def: "Department of Biology, Ch'ongju University of Education, Korea." [COLLECTION:curator]
synonym: "Department of Biology, Ch'ongju University of Education, Korea." EXACT []
is_a: COLLECTION:0000000 ! fish_collection_abbreviation

[Term]
id: COLLECTION:0000023
name: BKNU
def: "Kunsan National University, Department of Biology, Korea." [COLLECTION:curator]
synonym: "Kunsan National University, Department of Biology, Korea." EXACT []
is_a: COLLECTION:0000000 ! fish_collection_abbreviation

[Term]
id: COLLECTION:0000024
name: BLUZ
def: "Museo de Biologia, Universidad del Zulia, Maracaibo, Zulia, Venezuela." [COLLECTION:curator]
synonym: "Museo de Biologia, Universidad del Zulia, Maracaibo, Zulia, Venezuela." EXACT []
is_a: COLLECTION:0000000 ! fish_collection_abbreviation

[Term]
id: COLLECTION:0000025
name: BMAM
def: "Beijing Natural History Museum, Beijing, China." [COLLECTION:curator]
synonym: "Beijing Natural History Museum, Beijing, China." EXACT []
is_a: COLLECTION:0000000 ! fish_collection_abbreviation

[Term]
id: COLLECTION:0000026
name: BMNH
def: "Natural History Museum, London. Formerly British Museum Natural History, London. Preferred style BMNH 1945.6.6.3-4, with periods, no colon; year cataloged. month cataloged. day cataloged. specimens." [COLLECTION:curator]
synonym: "Natural History Museum, London. Formerly British Museum Natural History, London. Preferred style BMNH 1945.6.6.3-4, with periods, no colon; year cataloged. month cataloged. day cataloged. specimens." EXACT []
xref: urn\:lsid\:biocol.org\:col:1004
is_a: COLLECTION:0000000 ! fish_collection_abbreviation

[Term]
id: COLLECTION:0000027
name: BNHM
def: "Bombay Natural History Museum, Bombay, India." [COLLECTION:curator]
synonym: "Bombay Natural History Museum, Bombay, India." EXACT []
is_a: COLLECTION:0000000 ! fish_collection_abbreviation

[Term]
id: COLLECTION:0000028
name: BOC
def: "Bingham Oceanographic Collection, now Yale Peabody Museum [YPM]." [COLLECTION:curator]
synonym: "Bingham Oceanographic Collection, now Yale Peabody Museum [YPM]." EXACT []
is_a: COLLECTION:0000000 ! fish_collection_abbreviation

[Term]
id: COLLECTION:0000029
name: BPBM
def: "Bernice P. Bishop Museum, Honolulu, Hawaii, U.S.A." [COLLECTION:curator]
synonym: "Bernice P. Bishop Museum, Honolulu, Hawaii, U.S.A." EXACT []
is_a: COLLECTION:0000000 ! fish_collection_abbreviation

[Term]
id: COLLECTION:0000030
name: BSKU
def: "Kochi University, Department of Biology, Faculty of Science, Kochi, Japan." [COLLECTION:curator]
synonym: "Kochi University, Department of Biology, Faculty of Science, Kochi, Japan." EXACT []
xref: urn\:lsid\:biocol.org\:col:35150
is_a: COLLECTION:0000000 ! fish_collection_abbreviation

[Term]
id: COLLECTION:0000031
name: BSMP
def: "Department of Agriculture, Bureau of Science, Manila, Philippines. " [COLLECTION:curator]
synonym: "Department of Agriculture, Bureau of Science, Manila, Philippines. " EXACT []
is_a: COLLECTION:0000000 ! fish_collection_abbreviation

[Term]
id: COLLECTION:0000032
name: BSNH
def: "Boston Society of Natural History. Surviving specimens now at MCZ." [COLLECTION:curator]
synonym: "Boston Society of Natural History. Surviving specimens now at MCZ." EXACT []
is_a: COLLECTION:0000000 ! fish_collection_abbreviation

[Term]
id: COLLECTION:0000033
name: BSRM
def: "Biological Station Reference Museum at Porto Novo, Annamalai University, India." [COLLECTION:curator]
synonym: "Biological Station Reference Museum at Porto Novo, Annamalai University, India." EXACT []
is_a: COLLECTION:0000000 ! fish_collection_abbreviation

[Term]
id: COLLECTION:0000034
name: BYU
def: "Brigham Young University, Monte L. Bean Life Science Museum, Provo, Utah, U.S.A." [COLLECTION:curator]
synonym: "Brigham Young University, Monte L. Bean Life Science Museum, Provo, Utah, U.S.A." EXACT []
is_a: COLLECTION:0000000 ! fish_collection_abbreviation

[Term]
id: COLLECTION:0000035
name: BZT
def: "Biological Institute Titograd, Yugoslavia." [COLLECTION:curator]
synonym: "Biological Institute Titograd, Yugoslavia." EXACT []
is_a: COLLECTION:0000000 ! fish_collection_abbreviation

[Term]
id: COLLECTION:0000036
name: CAS
def: "California Academy of Sciences, San Francisco, California, U.S.A." [COLLECTION:curator]
synonym: "California Academy of Sciences, San Francisco, California, U.S.A." EXACT []
xref: urn\:lsid\:biocol.org\:col:1003
is_a: COLLECTION:0000000 ! fish_collection_abbreviation

[Term]
id: COLLECTION:0000037
name: CAS-IU
def: "CAS(IUM)" [COLLECTION:curator]
synonym: "CAS(IUM)" EXACT []
synonym: "Indiana University. Now mostly at CAS and recataloged with CAS numbers." EXACT []
is_a: COLLECTION:0000000 ! fish_collection_abbreviation

[Term]
id: COLLECTION:0000038
name: CAS-SU
def: "See SU [now at CAS]." [COLLECTION:curator]
synonym: "See SU [now at CAS]." EXACT []
is_a: COLLECTION:0000000 ! fish_collection_abbreviation

[Term]
id: COLLECTION:0000039
name: CAUSC
def: "Universidade Federal de Santa Catarina Centro de Agrarias, Santa Catarina, Brazil." [COLLECTION:curator]
synonym: "Universidade Federal de Santa Catarina Centro de Agrarias, Santa Catarina, Brazil." EXACT []
is_a: COLLECTION:0000000 ! fish_collection_abbreviation

[Term]
id: COLLECTION:0000040
name: CBD
def: "Collezione Ittiologica Balma-Delmastro. Collection of G.A.C Balma and G. B. Delmastro [Torino, Italy]." [COLLECTION:curator]
synonym: "Collezione Ittiologica Balma-Delmastro. Collection of G.A.C Balma and G. B. Delmastro [Torino, Italy]." EXACT []
is_a: COLLECTION:0000000 ! fish_collection_abbreviation

[Term]
id: COLLECTION:0000041
name: CBF
def: "Coleccion Boliviana de Fauna, Museo Nacional de Histoire Natural, Instituto de Ecologia, Bolivia." [COLLECTION:curator]
synonym: "Coleccion Boliviana de Fauna, Museo Nacional de Histoire Natural, Instituto de Ecologia, Bolivia." EXACT []
is_a: COLLECTION:0000000 ! fish_collection_abbreviation

[Term]
id: COLLECTION:0000042
name: CBM
def: "Natural History Museum and Institute, Chiba, Japan." [COLLECTION:curator]
synonym: "Natural History Museum and Institute, Chiba, Japan." EXACT []
is_a: COLLECTION:0000000 ! fish_collection_abbreviation

[Term]
id: COLLECTION:0000043
name: CBSIZA
def: "Caspian Biological Station Institute of Zoology, Azerbijan." [COLLECTION:curator]
synonym: "Caspian Biological Station Institute of Zoology, Azerbijan." EXACT []
is_a: COLLECTION:0000000 ! fish_collection_abbreviation

[Term]
id: COLLECTION:0000044
name: CCB
def: "Central College, Bangalore, India." [COLLECTION:curator]
synonym: "Central College, Bangalore, India." EXACT []
is_a: COLLECTION:0000000 ! fish_collection_abbreviation

[Term]
id: COLLECTION:0000045
name: CCML
def: "Coleccion Ictiologica del Departamento de Ciencias Marinas de la Universidad de la Laguna, Tenerife, Canary Islands." [COLLECTION:curator]
synonym: "Coleccion Ictiologica del Departamento de Ciencias Marinas de la Universidad de la Laguna, Tenerife, Canary Islands." EXACT []
is_a: COLLECTION:0000000 ! fish_collection_abbreviation

[Term]
id: COLLECTION:0000046
name: CEMBP
def: "Centre of Excellence in Marine Biology, University of Karachi, Pakistan." [COLLECTION:curator]
synonym: "Centre of Excellence in Marine Biology, University of Karachi, Pakistan." EXACT []
is_a: COLLECTION:0000000 ! fish_collection_abbreviation

[Term]
id: COLLECTION:0000047
name: CIB
def: "Academia Sinica, Chengdu Institute of Biology, China." [COLLECTION:curator]
synonym: "Academia Sinica, Chengdu Institute of Biology, China." EXACT []
is_a: COLLECTION:0000000 ! fish_collection_abbreviation

[Term]
id: COLLECTION:0000048
name: CIMAR
def: "Universidad Catolica de Valparaiso, Centro de Investigaciones del Mar, Valparaiso, Chile." [COLLECTION:curator]
synonym: "Universidad Catolica de Valparaiso, Centro de Investigaciones del Mar, Valparaiso, Chile." EXACT []
is_a: COLLECTION:0000000 ! fish_collection_abbreviation

[Term]
id: COLLECTION:0000049
name: CIP
def: "Centro de Investigaciones Pesqueras, Cartagena, Colombia." [COLLECTION:curator]
synonym: "Centro de Investigaciones Pesqueras, Cartagena, Colombia." EXACT []
is_a: COLLECTION:0000000 ! fish_collection_abbreviation

[Term]
id: COLLECTION:0000050
name: CIZ
def: "Centro de Investigaciones Zoologicas, Chile." [COLLECTION:curator]
synonym: "Centro de Investigaciones Zoologicas, Chile." EXACT []
is_a: COLLECTION:0000000 ! fish_collection_abbreviation

[Term]
id: COLLECTION:0000051
name: CM
def: "Carnegie Museum, Pittsburgh, Pennsylvania, U.S.A. Now mostly at FMNH and CAS." [COLLECTION:curator]
synonym: "Carnegie Museum, Pittsburgh, Pennsylvania, U.S.A. Now mostly at FMNH and CAS." EXACT []
xref: urn\:lsid\:biocol.org\:col:35157
is_a: COLLECTION:0000000 ! fish_collection_abbreviation

[Term]
id: COLLECTION:0000052
name: CMC
def: "Canterbury Museum, Christchurch, New Zealand." [COLLECTION:curator]
synonym: "Canterbury Museum, Christchurch, New Zealand." EXACT []
is_a: COLLECTION:0000000 ! fish_collection_abbreviation

[Term]
id: COLLECTION:0000053
name: CMFRI
def: "See FMRI." [COLLECTION:curator]
synonym: "See FMRI." EXACT []
is_a: COLLECTION:0000000 ! fish_collection_abbreviation

[Term]
id: COLLECTION:0000054
name: CMK
def: "Personal collection of Maurice Kottelat [Switzerland]. See also ZSM/CMK." [COLLECTION:curator]
synonym: "Personal collection of Maurice Kottelat [Switzerland]. See also ZSM/CMK." EXACT []
is_a: COLLECTION:0000000 ! fish_collection_abbreviation

[Term]
id: COLLECTION:0000055
name: CMNFI
def: "CMN" [COLLECTION:curator]
synonym: "Canadian Museum of Nature, Ottawa. Same as NMC - National Museums of Canada." EXACT []
synonym: "CMN" EXACT []
xref: urn\:lsid\:biocol.org\:col:35186
is_a: COLLECTION:0000000 ! fish_collection_abbreviation

[Term]
id: COLLECTION:0000056
name: CNRO
def: "Centre National de Recherches Oceanographiques, Nossi-Be, Madagascar." [COLLECTION:curator]
synonym: "Centre National de Recherches Oceanographiques, Nossi-Be, Madagascar." EXACT []
is_a: COLLECTION:0000000 ! fish_collection_abbreviation

[Term]
id: COLLECTION:0000057
name: CNU
def: "Department of Biology, College of Natural Science, Chonbuk National University, Chonju, Korea. Also seen as CNUC." [COLLECTION:curator]
synonym: "Department of Biology, College of Natural Science, Chonbuk National University, Chonju, Korea. Also seen as CNUC." EXACT []
is_a: COLLECTION:0000000 ! fish_collection_abbreviation

[Term]
id: COLLECTION:0000058
name: CNUC
def: "Chonbuk National University, Chonju, Korea. Also seen as CUBK." [COLLECTION:curator]
synonym: "Chonbuk National University, Chonju, Korea. Also seen as CUBK." EXACT []
is_a: COLLECTION:0000000 ! fish_collection_abbreviation

[Term]
id: COLLECTION:0000059
name: CRH
def: "Centre de Recherche en Hydrobiologie, Uvira, Zaire. Also as CRHU." [COLLECTION:curator]
synonym: "Centre de Recherche en Hydrobiologie, Uvira, Zaire. Also as CRHU." EXACT []
is_a: COLLECTION:0000000 ! fish_collection_abbreviation

[Term]
id: COLLECTION:0000060
name: CRHU
def: "See CRH." [COLLECTION:curator]
synonym: "See CRH." EXACT []
is_a: COLLECTION:0000000 ! fish_collection_abbreviation

[Term]
id: COLLECTION:0000061
name: CRRHA
def: "Centre Regional de Recherches en Hydrobiologie Appliquee, Bujumbura, Burandi." [COLLECTION:curator]
synonym: "Centre Regional de Recherches en Hydrobiologie Appliquee, Bujumbura, Burandi." EXACT []
is_a: COLLECTION:0000000 ! fish_collection_abbreviation

[Term]
id: COLLECTION:0000062
name: CRS-ZSI
def: "Central Regional Station, Zoological Survey of India, Jabalpur, India." [COLLECTION:curator]
synonym: "Central Regional Station, Zoological Survey of India, Jabalpur, India." EXACT []
is_a: COLLECTION:0000000 ! fish_collection_abbreviation

[Term]
id: COLLECTION:0000063
name: CSIRO
def: "Commonwealth Science & Industrial Research Organization, Division of Marine Research, Hobart, Tasmania, Australia. Formerly at Cronulla, Australia, also includes specimens from Marine Lab. Sydney." [COLLECTION:curator]
synonym: "Commonwealth Science & Industrial Research Organization, Division of Marine Research, Hobart, Tasmania, Australia. Formerly at Cronulla, Australia, also includes specimens from Marine Lab. Sydney." EXACT []
xref: urn\:lsid\:biocol.org\:col:35151
is_a: COLLECTION:0000000 ! fish_collection_abbreviation

[Term]
id: COLLECTION:0000064
name: CSU
def: "Colorado State University, Colorado Cooperative Fishery Unit, Fort Collins, Colorado, U.S.A." [COLLECTION:curator]
synonym: "Colorado State University, Colorado Cooperative Fishery Unit, Fort Collins, Colorado, U.S.A." EXACT []
is_a: COLLECTION:0000000 ! fish_collection_abbreviation

[Term]
id: COLLECTION:0000065
name: CU
def: "Cornell University Museum of Vertebrates, Ithaca, New York, U.S.A; formerly Cornell University Vertebrate Collections." [COLLECTION:curator]
synonym: "Cornell University Museum of Vertebrates, Ithaca, New York, U.S.A; formerly Cornell University Vertebrate Collections." EXACT []
xref: urn\:lsid\:biocol.org\:col:34787
is_a: COLLECTION:0000000 ! fish_collection_abbreviation

[Term]
id: COLLECTION:0000066
name: CUB
def: "Chulalongkorn University, Bangkok, Thailand." [COLLECTION:curator]
synonym: "Chulalongkorn University, Bangkok, Thailand." EXACT []
is_a: COLLECTION:0000000 ! fish_collection_abbreviation

[Term]
id: COLLECTION:0000067
name: CUBK
def: "Department of Biology, Chonbuk National University, Korea. Also seen as CNUC and CUB but not our CUB above." [COLLECTION:curator]
synonym: "Department of Biology, Chonbuk National University, Korea. Also seen as CNUC and CUB but not our CUB above." EXACT []
is_a: COLLECTION:0000000 ! fish_collection_abbreviation

[Term]
id: COLLECTION:0000068
name: CUP
def: "Charles University, Division of Hydrobiology and Ichthyology, Prague, Czechoslovakia." [COLLECTION:curator]
synonym: "Charles University, Division of Hydrobiology and Ichthyology, Prague, Czechoslovakia." EXACT []
is_a: COLLECTION:0000000 ! fish_collection_abbreviation

[Term]
id: COLLECTION:0000069
name: DBCUCH
def: "Universidad de Chile, Departamento de Biologia Celular y Genetica, Santiago, Chile." [COLLECTION:curator]
synonym: "Universidad de Chile, Departamento de Biologia Celular y Genetica, Santiago, Chile." EXACT []
is_a: COLLECTION:0000000 ! fish_collection_abbreviation

[Term]
id: COLLECTION:0000070
name: DBFFEUCS
def: "Departamento de Biologia de la Faculdad de Filosofia y Educacion de la Universidad de Chile, Santiago, Chile." [COLLECTION:curator]
synonym: "Departamento de Biologia de la Faculdad de Filosofia y Educacion de la Universidad de Chile, Santiago, Chile." EXACT []
is_a: COLLECTION:0000000 ! fish_collection_abbreviation

[Term]
id: COLLECTION:0000071
name: DHISUB
def: "Department of Hydrobiology and Ichthyology, Sofia University, Bulgaria." [COLLECTION:curator]
synonym: "Department of Hydrobiology and Ichthyology, Sofia University, Bulgaria." EXACT []
is_a: COLLECTION:0000000 ! fish_collection_abbreviation

[Term]
id: COLLECTION:0000072
name: DHMB
def: "Department of Harbours and Marine, Brisbane, Australia. Collection transferred to Queensland Museum (QM), Brisbane, Australia." [COLLECTION:curator]
synonym: "Department of Harbours and Marine, Brisbane, Australia. Collection transferred to Queensland Museum (QM), Brisbane, Australia." EXACT []
is_a: COLLECTION:0000000 ! fish_collection_abbreviation

[Term]
id: COLLECTION:0000073
name: EBRG
def: "DISCA" [COLLECTION:curator]
synonym: "DISCA" EXACT []
synonym: "Estacion Biologica de Rancho Grande, Ministerio del Ambiente y Recursos Naturales Renovables, Venezuela." EXACT []
is_a: COLLECTION:0000000 ! fish_collection_abbreviation

[Term]
id: COLLECTION:0000074
name: DU
def: "DUCV" [COLLECTION:curator]
synonym: "DUCV" EXACT []
synonym: "Duke University Vertebrate Collection, Durham, North Carolina, U.S.A." EXACT []
xref: urn\:lsid\:biocol.org\:col:35155
is_a: COLLECTION:0000000 ! fish_collection_abbreviation

[Term]
id: COLLECTION:0000075
name: DVZUT
def: "Department of Vertebrate Zoology, University of Tong-Hop, Hanoi, Vietnam." [COLLECTION:curator]
synonym: "Department of Vertebrate Zoology, University of Tong-Hop, Hanoi, Vietnam." EXACT []
is_a: COLLECTION:0000000 ! fish_collection_abbreviation

[Term]
id: COLLECTION:0000076
name: DZSASP
def: "Departamento de Zoologia, Secretaria da Agricultura, Sao Paulo, Brazil. Formerly Museu Paulista." [COLLECTION:curator]
synonym: "Departamento de Zoologia, Secretaria da Agricultura, Sao Paulo, Brazil. Formerly Museu Paulista." EXACT []
is_a: COLLECTION:0000000 ! fish_collection_abbreviation

[Term]
id: COLLECTION:0000077
name: DZUFRGS
def: "Departamento de Zoologia da Universidade Federal do Rio Grande do Sul, Porto Alegre, Brazil." [COLLECTION:curator]
synonym: "Departamento de Zoologia da Universidade Federal do Rio Grande do Sul, Porto Alegre, Brazil." EXACT []
is_a: COLLECTION:0000000 ! fish_collection_abbreviation

[Term]
id: COLLECTION:0000078
name: DZUH
def: "Departamento de Zoologia, Universidad de Havana, Cuba." [COLLECTION:curator]
synonym: "Departamento de Zoologia, Universidad de Havana, Cuba." EXACT []
is_a: COLLECTION:0000000 ! fish_collection_abbreviation

[Term]
id: COLLECTION:0000079
name: DZVU
def: "Universidad de Uruguay, Departmento de Zoologia Vertebrados, Montevideo, Uruguay." [COLLECTION:curator]
synonym: "Universidad de Uruguay, Departmento de Zoologia Vertebrados, Montevideo, Uruguay." EXACT []
is_a: COLLECTION:0000000 ! fish_collection_abbreviation

[Term]
id: COLLECTION:0000080
name: EBMC
def: "Universidad de Chile, Estacion Biologia Marina de Montemar, Chile." [COLLECTION:curator]
synonym: "Universidad de Chile, Estacion Biologia Marina de Montemar, Chile." EXACT []
is_a: COLLECTION:0000000 ! fish_collection_abbreviation

[Term]
id: COLLECTION:0000081
name: EBMTV
def: "Estacion de Biologia Marina del Instituto Tecnologico de Veracruz, Mexico." [COLLECTION:curator]
synonym: "Estacion de Biologia Marina del Instituto Tecnologico de Veracruz, Mexico." EXACT []
is_a: COLLECTION:0000000 ! fish_collection_abbreviation

[Term]
id: COLLECTION:0000082
name: ECSFI
def: "East China Sea Fisheries Institute, Shanghai, China." [COLLECTION:curator]
synonym: "East China Sea Fisheries Institute, Shanghai, China." EXACT []
is_a: COLLECTION:0000000 ! fish_collection_abbreviation

[Term]
id: COLLECTION:0000083
name: EEBP
def: "Estacao Experimental de Biologia e Piscicultura de Pirassununga, Brazil." [COLLECTION:curator]
synonym: "Estacao Experimental de Biologia e Piscicultura de Pirassununga, Brazil." EXACT []
is_a: COLLECTION:0000000 ! fish_collection_abbreviation

[Term]
id: COLLECTION:0000084
name: ENCB
def: "Escuela Nacional Ciencias, Coleccion Herpetozoarios, Mexico." [COLLECTION:curator]
synonym: "Escuela Nacional Ciencias, Coleccion Herpetozoarios, Mexico." EXACT []
is_a: COLLECTION:0000000 ! fish_collection_abbreviation

[Term]
id: COLLECTION:0000085
name: EPN
def: "Escuela Politecnica Nacional, Quito, Ecuador." [COLLECTION:curator]
synonym: "Escuela Politecnica Nacional, Quito, Ecuador." EXACT []
is_a: COLLECTION:0000000 ! fish_collection_abbreviation

[Term]
id: COLLECTION:0000086
name: EUB
def: "Laboratory of Biology, Faculty of Science, Ehime University, Japan." [COLLECTION:curator]
synonym: "Laboratory of Biology, Faculty of Science, Ehime University, Japan." EXACT []
is_a: COLLECTION:0000000 ! fish_collection_abbreviation

[Term]
id: COLLECTION:0000087
name: FAKOU
def: "Faculty of Agriculture, Kochi Univerisity, Kochi, Japan. Specimens now in BSKU." [COLLECTION:curator]
synonym: "Faculty of Agriculture, Kochi Univerisity, Kochi, Japan. Specimens now in BSKU." EXACT []
is_a: COLLECTION:0000000 ! fish_collection_abbreviation

[Term]
id: COLLECTION:0000088
name: FAKU
def: "Kyoto University, Department of Fisheries, Faculty of Agriculture, Japan. FAKU has several catalog series, including a K, W, and A series. The collection is housed at Maizuru, Japan, not at Kyoto." [COLLECTION:curator]
synonym: "Kyoto University, Department of Fisheries, Faculty of Agriculture, Japan. FAKU has several catalog series, including a K, W, and A series. The collection is housed at Maizuru, Japan, not at Kyoto." EXACT []
is_a: COLLECTION:0000000 ! fish_collection_abbreviation

[Term]
id: COLLECTION:0000089
name: FBQ
def: "Fisheries Branch, Departement of Primary Industries, Brisbane, Australia." [COLLECTION:curator]
synonym: "Fisheries Branch, Departement of Primary Industries, Brisbane, Australia." EXACT []
is_a: COLLECTION:0000000 ! fish_collection_abbreviation

[Term]
id: COLLECTION:0000090
name: FCLR
def: "Fundacion Cientifica Los Roques, Caracas, Venezuela." [COLLECTION:curator]
synonym: "Fundacion Cientifica Los Roques, Caracas, Venezuela." EXACT []
is_a: COLLECTION:0000000 ! fish_collection_abbreviation

[Term]
id: COLLECTION:0000091
name: FCRM
def: "Fisheries College Reference Museum, Tuticorin Tamil Nadu, India." [COLLECTION:curator]
synonym: "Fisheries College Reference Museum, Tuticorin Tamil Nadu, India." EXACT []
is_a: COLLECTION:0000000 ! fish_collection_abbreviation

[Term]
id: COLLECTION:0000092
name: FDNR
def: "Florida Department of Natural Resources, St. Petersburg, Florida, U.S.A." [COLLECTION:curator]
synonym: "Florida Department of Natural Resources, St. Petersburg, Florida, U.S.A." EXACT []
is_a: COLLECTION:0000000 ! fish_collection_abbreviation

[Term]
id: COLLECTION:0000093
name: FFSUC
def: "Faculty of Forestry Sciences, Universidad de Chile, Ichthyological Collection, Santiago, Chile." [COLLECTION:curator]
synonym: "Faculty of Forestry Sciences, Universidad de Chile, Ichthyological Collection, Santiago, Chile." EXACT []
is_a: COLLECTION:0000000 ! fish_collection_abbreviation

[Term]
id: COLLECTION:0000094
name: FML
def: "Instituto Fundacion Miguel Lillo, Tucuman, Argentina (Leviton et al. 1985:806)" [COLLECTION:curator]
synonym: "Instituto Fundacion Miguel Lillo, Tucuman, Argentina (Leviton et al. 1985:806)" EXACT []
xref: urn\:lsid\:biocol.org\:col:35152
is_a: COLLECTION:0000000 ! fish_collection_abbreviation

[Term]
id: COLLECTION:0000095
name: FMNH
def: "Field Museum of Natural History, Chicago, Illinois, U.S.A." [COLLECTION:curator]
synonym: "Field Museum of Natural History, Chicago, Illinois, U.S.A." EXACT []
xref: urn\:lsid\:biocol.org\:col:35153
is_a: COLLECTION:0000000 ! fish_collection_abbreviation

[Term]
id: COLLECTION:0000096
name: FMRI
def: "Central Marine Fisheries Marine Research Institute, Mandapam Camp, India." [COLLECTION:curator]
synonym: "Central Marine Fisheries Marine Research Institute, Mandapam Camp, India." EXACT []
is_a: COLLECTION:0000000 ! fish_collection_abbreviation

[Term]
id: COLLECTION:0000097
name: FNU
def: "Nagasaki University, Faculty of Fisheries, Nakasaki, Japan." [COLLECTION:curator]
synonym: "Nagasaki University, Faculty of Fisheries, Nakasaki, Japan." EXACT []
is_a: COLLECTION:0000000 ! fish_collection_abbreviation

[Term]
id: COLLECTION:0000098
name: FOSJ
def: "Fisheries and Oceans Biological Station, St. John's, Newfoundland, Canada." [COLLECTION:curator]
synonym: "Fisheries and Oceans Biological Station, St. John's, Newfoundland, Canada." EXACT []
is_a: COLLECTION:0000000 ! fish_collection_abbreviation

[Term]
id: COLLECTION:0000099
name: FRCL
def: "Fisheries Research Centre, Likas, Kota Kinabalu, Malaysia." [COLLECTION:curator]
synonym: "Fisheries Research Centre, Likas, Kota Kinabalu, Malaysia." EXACT []
is_a: COLLECTION:0000000 ! fish_collection_abbreviation

[Term]
id: COLLECTION:0000100
name: FRIHP
def: "Fisheries Research Institute of Hunan Province, China." [COLLECTION:curator]
synonym: "Fisheries Research Institute of Hunan Province, China." EXACT []
is_a: COLLECTION:0000000 ! fish_collection_abbreviation

[Term]
id: COLLECTION:0000101
name: FRLM
def: "Faculty of Fisheries, Mie University, Fisheries Research Laboratory, Mie-ken, Japan." [COLLECTION:curator]
synonym: "Faculty of Fisheries, Mie University, Fisheries Research Laboratory, Mie-ken, Japan." EXACT []
is_a: COLLECTION:0000000 ! fish_collection_abbreviation

[Term]
id: COLLECTION:0000102
name: FRSKU
def: "Kyoto University, Fisheries Research Station, Japan. Same as FAKU." [COLLECTION:curator]
synonym: "Kyoto University, Fisheries Research Station, Japan. Same as FAKU." EXACT []
is_a: COLLECTION:0000000 ! fish_collection_abbreviation

[Term]
id: COLLECTION:0000103
name: FSFRL
def: "Far Seas Fisheries Research Laboratory, Shimizu, Japan. Most types now at FAKU." [COLLECTION:curator]
synonym: "Far Seas Fisheries Research Laboratory, Shimizu, Japan. Most types now at FAKU." EXACT []
is_a: COLLECTION:0000000 ! fish_collection_abbreviation

[Term]
id: COLLECTION:0000104
name: FSU
def: "Florida State Univeristy. Transferred to Florida State Museum, see UF-FSU." [COLLECTION:curator]
synonym: "Florida State Univeristy. Transferred to Florida State Museum, see UF-FSU." EXACT []
is_a: COLLECTION:0000000 ! fish_collection_abbreviation

[Term]
id: COLLECTION:0000105
name: FUMT
def: "University of Tokyo, Department of Fisheries, University Museum, Tokyo, Japan." [COLLECTION:curator]
synonym: "University of Tokyo, Department of Fisheries, University Museum, Tokyo, Japan." EXACT []
is_a: COLLECTION:0000000 ! fish_collection_abbreviation

[Term]
id: COLLECTION:0000106
name: GCM
def: "Government College, Department of Zoology, Lahore, Pakistan." [COLLECTION:curator]
synonym: "Government College, Department of Zoology, Lahore, Pakistan." EXACT []
is_a: COLLECTION:0000000 ! fish_collection_abbreviation

[Term]
id: COLLECTION:0000107
name: GCRL
def: "Gulf Coast Research Laboratory, Ocean Springs, Mississippi, U.S.A." [COLLECTION:curator]
synonym: "Gulf Coast Research Laboratory, Ocean Springs, Mississippi, U.S.A." EXACT []
xref: urn\:lsid\:biocol.org\:col:35154
is_a: COLLECTION:0000000 ! fish_collection_abbreviation

[Term]
id: COLLECTION:0000108
name: GMBL
def: "College of Charleston, Grice Marine Biological Laboratory, Charleston, South Carolina, U.S.A." [COLLECTION:curator]
synonym: "College of Charleston, Grice Marine Biological Laboratory, Charleston, South Carolina, U.S.A." EXACT []
is_a: COLLECTION:0000000 ! fish_collection_abbreviation

[Term]
id: COLLECTION:0000109
name: GMNGZ
def: "Glasgow Museum and Art Galleries, Natural History/Zoology, Glasgow, Scotland." [COLLECTION:curator]
synonym: "Glasgow Museum and Art Galleries, Natural History/Zoology, Glasgow, Scotland." EXACT []
is_a: COLLECTION:0000000 ! fish_collection_abbreviation

[Term]
id: COLLECTION:0000110
name: GNHNA
def: "Gallery of Natural History and Native Art, Medlow Bath, New South Wales, Australia." [COLLECTION:curator]
synonym: "Gallery of Natural History and Native Art, Medlow Bath, New South Wales, Australia." EXACT []
is_a: COLLECTION:0000000 ! fish_collection_abbreviation

[Term]
id: COLLECTION:0000111
name: GNM
def: "See NMG." [COLLECTION:curator]
synonym: "See NMG." EXACT []
is_a: COLLECTION:0000000 ! fish_collection_abbreviation

[Term]
id: COLLECTION:0000112
name: GVF
def: "George Vanderbilt Foundation. Specimens now at CAS." [COLLECTION:curator]
synonym: "George Vanderbilt Foundation. Specimens now at CAS." EXACT []
is_a: COLLECTION:0000000 ! fish_collection_abbreviation

[Term]
id: COLLECTION:0000113
name: HACW
def: "Department of Fishery, Huazhong Agriculture Collection, Wuhan, China." [COLLECTION:curator]
synonym: "Department of Fishery, Huazhong Agriculture Collection, Wuhan, China." EXACT []
is_a: COLLECTION:0000000 ! fish_collection_abbreviation

[Term]
id: COLLECTION:0000114
name: HKFRS
def: "Hong Kong Fisheries Research Station, Aberdeen, Hong Kong." [COLLECTION:curator]
synonym: "Hong Kong Fisheries Research Station, Aberdeen, Hong Kong." EXACT []
is_a: COLLECTION:0000000 ! fish_collection_abbreviation

[Term]
id: COLLECTION:0000115
name: HSU
def: "Humboldt State University, Arcata, California, U.S.A." [COLLECTION:curator]
synonym: "Humboldt State University, Arcata, California, U.S.A." EXACT []
is_a: COLLECTION:0000000 ! fish_collection_abbreviation

[Term]
id: COLLECTION:0000116
name: HUJ
def: "AJ" [COLLECTION:curator]
synonym: "AJ" EXACT []
synonym: "EY" EXACT []
synonym: "Hebrew University, Department of Zoology, Jerusalem, Israel." EXACT []
is_a: COLLECTION:0000000 ! fish_collection_abbreviation

[Term]
id: COLLECTION:0000117
name: HUMZ
def: "Hokkaido University, Laboratory of Marine Zoology, Faculty of Fisheries, Hokkaido, Japan." [COLLECTION:curator]
synonym: "Hokkaido University, Laboratory of Marine Zoology, Faculty of Fisheries, Hokkaido, Japan." EXACT []
xref: urn\:lsid\:biocol.org\:col:35156
is_a: COLLECTION:0000000 ! fish_collection_abbreviation

[Term]
id: COLLECTION:0000118
name: HZM
def: "Museum of Natural History (Hrvatski Zooloski Muzej), Zagreb, Croatia." [COLLECTION:curator]
synonym: "Museum of Natural History (Hrvatski Zooloski Muzej), Zagreb, Croatia." EXACT []
is_a: COLLECTION:0000000 ! fish_collection_abbreviation

[Term]
id: COLLECTION:0000119
name: IAA
def: "Instituto Antartico Argentino, Buenos Aires, Argentina." [COLLECTION:curator]
synonym: "Instituto Antartico Argentino, Buenos Aires, Argentina." EXACT []
is_a: COLLECTION:0000000 ! fish_collection_abbreviation

[Term]
id: COLLECTION:0000120
name: IADIZA
def: "Instituto Argentino de Investigacion de Zonas Aridas, Mendoza, Argentina (Fernandez & Vari 2002:739)" [COLLECTION:curator]
synonym: "Instituto Argentino de Investigacion de Zonas Aridas, Mendoza, Argentina (Fernandez & Vari 2002:739)" EXACT []
is_a: COLLECTION:0000000 ! fish_collection_abbreviation

[Term]
id: COLLECTION:0000121
name: IBAUNC
def: "Universidad Nacional de Cuyo, Instituto de Biologia Animal, Medoza, Argentina." [COLLECTION:curator]
synonym: "Universidad Nacional de Cuyo, Instituto de Biologia Animal, Medoza, Argentina." EXACT []
is_a: COLLECTION:0000000 ! fish_collection_abbreviation

[Term]
id: COLLECTION:0000122
name: IBH
def: "Universidad Nacional Autonoma de Mexico, Instituto de Biologia, Mexico." [COLLECTION:curator]
synonym: "Universidad Nacional Autonoma de Mexico, Instituto de Biologia, Mexico." EXACT []
is_a: COLLECTION:0000000 ! fish_collection_abbreviation

[Term]
id: COLLECTION:0000123
name: IBRP
def: "Institute for Breeding Research, Tokyo University of Agriculture, Tokyo, Japan." [COLLECTION:curator]
synonym: "Institute for Breeding Research, Tokyo University of Agriculture, Tokyo, Japan." EXACT []
xref: urn\:lsid\:biocol.org\:col:35158
is_a: COLLECTION:0000000 ! fish_collection_abbreviation

[Term]
id: COLLECTION:0000124
name: IBTS
def: "Institutul de Biologie, Tr. Savulescu, Bucharest, Romania." [COLLECTION:curator]
synonym: "Institutul de Biologie, Tr. Savulescu, Bucharest, Romania." EXACT []
is_a: COLLECTION:0000000 ! fish_collection_abbreviation

[Term]
id: COLLECTION:0000125
name: IBUNAM
def: "Universidad Nacional Autonoma de Mexico, Departmento de Zoologia, Instituto de Biologia, Mexico, DF, Mexico. Apparently the same as UNAM and IBH." [COLLECTION:curator]
synonym: "Universidad Nacional Autonoma de Mexico, Departmento de Zoologia, Instituto de Biologia, Mexico, DF, Mexico. Apparently the same as UNAM and IBH." EXACT []
xref: urn\:lsid\:biocol.org\:col:35159
is_a: COLLECTION:0000000 ! fish_collection_abbreviation

[Term]
id: COLLECTION:0000126
name: ICM
def: "Instituto de Ciencias del Mar, Barcelona, Spain." [COLLECTION:curator]
synonym: "Instituto de Ciencias del Mar, Barcelona, Spain." EXACT []
is_a: COLLECTION:0000000 ! fish_collection_abbreviation

[Term]
id: COLLECTION:0000127
name: ICNMHN
def: "Instituto de Ciencias Naturales, Museo de Historia Natural, Universidad Nacional de Colombia, Bogota, Colombia. Also seen as ICNMNH." [COLLECTION:curator]
synonym: "Instituto de Ciencias Naturales, Museo de Historia Natural, Universidad Nacional de Colombia, Bogota, Colombia. Also seen as ICNMNH." EXACT []
is_a: COLLECTION:0000000 ! fish_collection_abbreviation

[Term]
id: COLLECTION:0000128
name: IFAN
def: "Institut Fondamental d'Afrique Noire, Dakar, Senegal." [COLLECTION:curator]
synonym: "Institut Fondamental d'Afrique Noire, Dakar, Senegal." EXACT []
is_a: COLLECTION:0000000 ! fish_collection_abbreviation

[Term]
id: COLLECTION:0000129
name: IFI
def: "Imperial Fisheries Institute, Tokyo University of Fisheries. Matsubara's collection that was transferred to FAKU in 1947, although some specimens were lost, FAKU catalog numbers = Matsubara numbers." [COLLECTION:curator]
synonym: "Imperial Fisheries Institute, Tokyo University of Fisheries. Matsubara's collection that was transferred to FAKU in 1947, although some specimens were lost, FAKU catalog numbers = Matsubara numbers." EXACT []
is_a: COLLECTION:0000000 ! fish_collection_abbreviation

[Term]
id: COLLECTION:0000130
name: IHB
def: "IHASW" [COLLECTION:curator]
synonym: "IHASW" EXACT []
synonym: "Institute of Hydrobiology, Academy Sinica, Wuhan, People's Republic of China." EXACT []
synonym: "WUH" EXACT []
xref: urn\:lsid\:biocol.org\:col:35160
is_a: COLLECTION:0000000 ! fish_collection_abbreviation

[Term]
id: COLLECTION:0000131
name: IIPB
def: "Instituto de Investigaciones Pesqueras de Barcelona, Spain." [COLLECTION:curator]
synonym: "Instituto de Investigaciones Pesqueras de Barcelona, Spain." EXACT []
is_a: COLLECTION:0000000 ! fish_collection_abbreviation

[Term]
id: COLLECTION:0000132
name: ILPLA
def: "Museo de La Plata, Instituto de Limnologia, La Plata, Argentina." [COLLECTION:curator]
synonym: "Museo de La Plata, Instituto de Limnologia, La Plata, Argentina." EXACT []
is_a: COLLECTION:0000000 ! fish_collection_abbreviation

[Term]
id: COLLECTION:0000133
name: IMARPE
def: "Instituto del Mar del Perú, Lima, Peru." [COLLECTION:curator]
synonym: "Instituto del Mar del Perú, Lima, Peru." EXACT []
is_a: COLLECTION:0000000 ! fish_collection_abbreviation

[Term]
id: COLLECTION:0000134
name: INALI
def: "Instituto Limnologia, Santo Tome, Argentina." [COLLECTION:curator]
synonym: "Instituto Limnologia, Santo Tome, Argentina." EXACT []
is_a: COLLECTION:0000000 ! fish_collection_abbreviation

[Term]
id: COLLECTION:0000135
name: INHS
def: "Illinois Natural History Survey, Champaigne, Illinois, U.S.A." [COLLECTION:curator]
synonym: "Illinois Natural History Survey, Champaigne, Illinois, U.S.A." EXACT []
xref: urn\:lsid\:biocol.org\:col:35161
is_a: COLLECTION:0000000 ! fish_collection_abbreviation

[Term]
id: COLLECTION:0000136
name: INIBP
def: "Instituto Nacional de Investigaciones Biologico Pesqueras, Mexico." [COLLECTION:curator]
synonym: "Instituto Nacional de Investigaciones Biologico Pesqueras, Mexico." EXACT []
is_a: COLLECTION:0000000 ! fish_collection_abbreviation

[Term]
id: COLLECTION:0000137
name: INIP
def: "Instituto Nacional de Investigacao das Pescas, Alges, Portugal." [COLLECTION:curator]
synonym: "Instituto Nacional de Investigacao das Pescas, Alges, Portugal." EXACT []
is_a: COLLECTION:0000000 ! fish_collection_abbreviation

[Term]
id: COLLECTION:0000138
name: INPA
def: "Instituto Nacional de Pesquisas da Amazonia, Manaus, Amazonas, Brazil." [COLLECTION:curator]
synonym: "Instituto Nacional de Pesquisas da Amazonia, Manaus, Amazonas, Brazil." EXACT []
xref: /urn\:lsid\:biocol.org\:col:35162
is_a: COLLECTION:0000000 ! fish_collection_abbreviation

[Term]
id: COLLECTION:0000139
name: INVEMAR
def: "Instituto de Investigaciones Marinas de Punta de Betin, Santa Marta, Colombia." [COLLECTION:curator]
synonym: "Instituto de Investigaciones Marinas de Punta de Betin, Santa Marta, Colombia." EXACT []
is_a: COLLECTION:0000000 ! fish_collection_abbreviation

[Term]
id: COLLECTION:0000140
name: IO
def: "Instituto Oceanografico da Universidade de Sao Paulo, Brazil. Formerly Instituto Paulista de Oceanografia." [COLLECTION:curator]
synonym: "Instituto Oceanografico da Universidade de Sao Paulo, Brazil. Formerly Instituto Paulista de Oceanografia." EXACT []
is_a: COLLECTION:0000000 ! fish_collection_abbreviation

[Term]
id: COLLECTION:0000141
name: IOAN
def: "See IOM." [COLLECTION:curator]
synonym: "See IOM." EXACT []
is_a: COLLECTION:0000000 ! fish_collection_abbreviation

[Term]
id: COLLECTION:0000142
name: IOH
def: "Academia de Ciencias, Instituto de Oceanologia, Habana, Cuba." [COLLECTION:curator]
synonym: "Academia de Ciencias, Instituto de Oceanologia, Habana, Cuba." EXACT []
is_a: COLLECTION:0000000 ! fish_collection_abbreviation

[Term]
id: COLLECTION:0000143
name: IOM
def: "Institute of Oceanology, Academy of Sciences, Moscow, Russia." [COLLECTION:curator]
synonym: "Institute of Oceanology, Academy of Sciences, Moscow, Russia." EXACT []
is_a: COLLECTION:0000000 ! fish_collection_abbreviation

[Term]
id: COLLECTION:0000144
name: IOPM
def: "Izu Oceanic Park Museum, Izu, Japan." [COLLECTION:curator]
synonym: "Izu Oceanic Park Museum, Izu, Japan." EXACT []
is_a: COLLECTION:0000000 ! fish_collection_abbreviation

[Term]
id: COLLECTION:0000145
name: IORD
def: "Takai University, Institute of Oceanic Research and Development, Shimuzu, Japan." [COLLECTION:curator]
synonym: "Takai University, Institute of Oceanic Research and Development, Shimuzu, Japan." EXACT []
is_a: COLLECTION:0000000 ! fish_collection_abbreviation

[Term]
id: COLLECTION:0000146
name: IOS
def: "Institute of Oceanographic Sciences, Surrey, England." [COLLECTION:curator]
synonym: "Institute of Oceanographic Sciences, Surrey, England." EXACT []
is_a: COLLECTION:0000000 ! fish_collection_abbreviation

[Term]
id: COLLECTION:0000147
name: IPN
def: "Instituto Politecnico, Escuela Nacional de Ciencias Biologicas de Mexico, Mexico." [COLLECTION:curator]
synonym: "Instituto Politecnico, Escuela Nacional de Ciencias Biologicas de Mexico, Mexico." EXACT []
is_a: COLLECTION:0000000 ! fish_collection_abbreviation

[Term]
id: COLLECTION:0000148
name: IRSM
def: "Institut Recherche Scientifique de Madagascar." [COLLECTION:curator]
synonym: "Institut Recherche Scientifique de Madagascar." EXACT []
is_a: COLLECTION:0000000 ! fish_collection_abbreviation

[Term]
id: COLLECTION:0000149
name: IRSNB
def: "Institut Royal des Sciences Natureles de Belgique, Brussels, Belgium." [COLLECTION:curator]
synonym: "Institut Royal des Sciences Natureles de Belgique, Brussels, Belgium." EXACT []
xref: /urn\:lsid\:biocol.org\:col:35163
is_a: COLLECTION:0000000 ! fish_collection_abbreviation

[Term]
id: COLLECTION:0000150
name: ISBB
def: "Institutul de Stiinte Biologice, Bucuresti, Romania." [COLLECTION:curator]
synonym: "Institutul de Stiinte Biologice, Bucuresti, Romania." EXACT []
is_a: COLLECTION:0000000 ! fish_collection_abbreviation

[Term]
id: COLLECTION:0000151
name: ISC
def: "Iowa State College, Ames, Iowa, U.S.A." [COLLECTION:curator]
synonym: "Iowa State College, Ames, Iowa, U.S.A." EXACT []
is_a: COLLECTION:0000000 ! fish_collection_abbreviation

[Term]
id: COLLECTION:0000152
name: ISER
def: "Institutul Speologie Emil G. Racovita, Bucurest, Romania." [COLLECTION:curator]
synonym: "Institutul Speologie Emil G. Racovita, Bucurest, Romania." EXACT []
is_a: COLLECTION:0000000 ! fish_collection_abbreviation

[Term]
id: COLLECTION:0000153
name: ISH
def: "Universite Hamburg, Institut fur Seefischerei, Hamburg, Germany. Citation of catalog numbers perferred by ISH is to use a complete year, i.e. ISF 130/71 becomes 130-1971." [COLLECTION:curator]
synonym: "Universite Hamburg, Institut fur Seefischerei, Hamburg, Germany. Citation of catalog numbers perferred by ISH is to use a complete year, i.e. ISF 130/71 becomes 130-1971." EXACT []
is_a: COLLECTION:0000000 ! fish_collection_abbreviation

[Term]
id: COLLECTION:0000154
name: ISTPM
def: "Institut Scientifique et Technique des Peches Maritimes, Nantes, France." [COLLECTION:curator]
synonym: "Institut Scientifique et Technique des Peches Maritimes, Nantes, France." EXACT []
is_a: COLLECTION:0000000 ! fish_collection_abbreviation

[Term]
id: COLLECTION:0000155
name: ISU
def: "Indiana State University, Terre Haute, Indiana, U.S.A." [COLLECTION:curator]
synonym: "Indiana State University, Terre Haute, Indiana, U.S.A." EXACT []
is_a: COLLECTION:0000000 ! fish_collection_abbreviation

[Term]
id: COLLECTION:0000156
name: IU
def: "Indiana University. Now mostly at California Academy of Sciences (CAS)." [COLLECTION:curator]
synonym: "Indiana University. Now mostly at California Academy of Sciences (CAS)." EXACT []
xref: /urn\:lsid\:biocol.org\:col:35164
is_a: COLLECTION:0000000 ! fish_collection_abbreviation

[Term]
id: COLLECTION:0000157
name: IZA
def: "Universita di l'Aguila, Instituto di Zoologia, Aquila, Italy." [COLLECTION:curator]
synonym: "Universita di l'Aguila, Instituto di Zoologia, Aquila, Italy." EXACT []
is_a: COLLECTION:0000000 ! fish_collection_abbreviation

[Term]
id: COLLECTION:0000158
name: IZAC
def: "Academia de Ciencias, Instituto de Zoologia, Habana, Cuba." [COLLECTION:curator]
synonym: "Academia de Ciencias, Instituto de Zoologia, Habana, Cuba." EXACT []
is_a: COLLECTION:0000000 ! fish_collection_abbreviation

[Term]
id: COLLECTION:0000159
name: IZPAN
def: "Zoological Institute, Polish Academy of Sciences, Warsaw, Poland." [COLLECTION:curator]
synonym: "Zoological Institute, Polish Academy of Sciences, Warsaw, Poland." EXACT []
is_a: COLLECTION:0000000 ! fish_collection_abbreviation

[Term]
id: COLLECTION:0000160
name: IZUA
def: "Universidad Austral de Chile, Instituto de Zoologia, Valdivia, Chile." [COLLECTION:curator]
synonym: "Universidad Austral de Chile, Instituto de Zoologia, Valdivia, Chile." EXACT []
xref: urn\:lsid\:biocol.org\:col:35165
is_a: COLLECTION:0000000 ! fish_collection_abbreviation

[Term]
id: COLLECTION:0000161
name: IZUCS
def: "Universita di Cagliari, Instituto de Zoologia, Sardinia, Italy." [COLLECTION:curator]
synonym: "Universita di Cagliari, Instituto de Zoologia, Sardinia, Italy." EXACT []
is_a: COLLECTION:0000000 ! fish_collection_abbreviation

[Term]
id: COLLECTION:0000162
name: JNU
def: "Department of Biology, Ji Nan University, China." [COLLECTION:curator]
synonym: "Department of Biology, Ji Nan University, China." EXACT []
is_a: COLLECTION:0000000 ! fish_collection_abbreviation

[Term]
id: COLLECTION:0000163
name: KFRS
def: "Kanudi Fisheries Research Station, Konedobu, Papua New Guinea." [COLLECTION:curator]
synonym: "Kanudi Fisheries Research Station, Konedobu, Papua New Guinea." EXACT []
xref: urn\:lsid\:biocol.org\:col:35166
is_a: COLLECTION:0000000 ! fish_collection_abbreviation

[Term]
id: COLLECTION:0000164
name: KHMM
def: "Kulturhistorisches Museum, Magdeburg, Germany." [COLLECTION:curator]
synonym: "Kulturhistorisches Museum, Magdeburg, Germany." EXACT []
is_a: COLLECTION:0000000 ! fish_collection_abbreviation

[Term]
id: COLLECTION:0000165
name: KIFB
def: "Korean Institute of Freshwater Biology, Seoul, Korea." [COLLECTION:curator]
synonym: "Korean Institute of Freshwater Biology, Seoul, Korea." EXACT []
is_a: COLLECTION:0000000 ! fish_collection_abbreviation

[Term]
id: COLLECTION:0000166
name: KIZ
def: "Kunming Institute of Zoology, Yannan, China." [COLLECTION:curator]
synonym: "Kunming Institute of Zoology, Yannan, China." EXACT []
xref: urn\:lsid\:biocol.org\:col:35167
is_a: COLLECTION:0000000 ! fish_collection_abbreviation

[Term]
id: COLLECTION:0000167
name: KMMA
def: "Koninklijk Museum voor Midden-Afrika, Tervuren. Same as MRAC." [COLLECTION:curator]
synonym: "Koninklijk Museum voor Midden-Afrika, Tervuren. Same as MRAC." EXACT []
is_a: COLLECTION:0000000 ! fish_collection_abbreviation

[Term]
id: COLLECTION:0000168
name: KSHS
def: "Kochi Senior High School, Kochi-shi, Japan. Private collection of Yamakawa; specimens have BSKU catalog numbers 50000-79999." [COLLECTION:curator]
synonym: "Kochi Senior High School, Kochi-shi, Japan. Private collection of Yamakawa; specimens have BSKU catalog numbers 50000-79999." EXACT []
is_a: COLLECTION:0000000 ! fish_collection_abbreviation

[Term]
id: COLLECTION:0000169
name: KU
def: "University of Kansas, Museum of Natural History, Lawrence, Kansas, U.S.A." [COLLECTION:curator]
synonym: "University of Kansas, Museum of Natural History, Lawrence, Kansas, U.S.A." EXACT []
xref: urn\:lsid\:biocol.org\:col:35050
is_a: COLLECTION:0000000 ! fish_collection_abbreviation

[Term]
id: COLLECTION:0000170
name: KUMF
def: "Kasetsart University Museum of Fisheries, Bangkok, Thailand." [COLLECTION:curator]
synonym: "Kasetsart University Museum of Fisheries, Bangkok, Thailand." EXACT []
xref: urn\:lsid\:biocol.org\:col:35168
is_a: COLLECTION:0000000 ! fish_collection_abbreviation

[Term]
id: COLLECTION:0000171
name: LACM
def: "Los Angeles County Museum of Natural History, Los Angeles, California, U.S.A." [COLLECTION:curator]
synonym: "Los Angeles County Museum of Natural History, Los Angeles, California, U.S.A." EXACT []
xref: urn\:lsid\:biocol.org\:col:34804
is_a: COLLECTION:0000000 ! fish_collection_abbreviation

[Term]
id: COLLECTION:0000172
name: LBN
def: "Lembaga Biologi Nasional, Bogor, Indonesia." [COLLECTION:curator]
synonym: "Lembaga Biologi Nasional, Bogor, Indonesia." EXACT []
is_a: COLLECTION:0000000 ! fish_collection_abbreviation

[Term]
id: COLLECTION:0000173
name: LFBKU
def: "Laboratory of Fishery Biology, Kyushu University, Japan." [COLLECTION:curator]
synonym: "Laboratory of Fishery Biology, Kyushu University, Japan." EXACT []
is_a: COLLECTION:0000000 ! fish_collection_abbreviation

[Term]
id: COLLECTION:0000174
name: LIAIP
def: "Laboratory of Ichthyology, Akasaka Imperial Palace, Tokyo, Japan." [COLLECTION:curator]
synonym: "Laboratory of Ichthyology, Akasaka Imperial Palace, Tokyo, Japan." EXACT []
is_a: COLLECTION:0000000 ! fish_collection_abbreviation

[Term]
id: COLLECTION:0000175
name: LICPP
def: "The Crown Prince's Palace, Laboratory of Ichthyology, Tokyo, Japan" [COLLECTION:curator]
synonym: "The Crown Prince's Palace, Laboratory of Ichthyology, Tokyo, Japan" EXACT []
is_a: COLLECTION:0000000 ! fish_collection_abbreviation

[Term]
id: COLLECTION:0000176
name: LON
def: "Lembaga Oseanologie Nasional, Djakarta [National Institute of Oceanology], Indonesia." [COLLECTION:curator]
synonym: "Lembaga Oseanologie Nasional, Djakarta [National Institute of Oceanology], Indonesia." EXACT []
is_a: COLLECTION:0000000 ! fish_collection_abbreviation

[Term]
id: COLLECTION:0000177
name: LS
def: "Linnean Society of London, Piccadilly, London, England." [COLLECTION:curator]
synonym: "Linnean Society of London, Piccadilly, London, England." EXACT []
is_a: COLLECTION:0000000 ! fish_collection_abbreviation

[Term]
id: COLLECTION:0000178
name: LSUMZ
def: "Louisiana State University, Museum of Zoology, Baton Rouge, Louisiana, U.S.A." [COLLECTION:curator]
synonym: "Louisiana State University, Museum of Zoology, Baton Rouge, Louisiana, U.S.A." EXACT []
is_a: COLLECTION:0000000 ! fish_collection_abbreviation

[Term]
id: COLLECTION:0000179
name: MAC-APU
def: "Ministerio de Agricultura y Cria, Estacion Experimental Apure, San Fernando de Apure, Venezuela." [COLLECTION:curator]
synonym: "Ministerio de Agricultura y Cria, Estacion Experimental Apure, San Fernando de Apure, Venezuela." EXACT []
is_a: COLLECTION:0000000 ! fish_collection_abbreviation

[Term]
id: COLLECTION:0000180
name: MAC-PAY
def: "Ministerio de Agricultura y Cria, Estacion Experimental Amazonas, Puerto Ayacucho, Venezuela." [COLLECTION:curator]
synonym: "Ministerio de Agricultura y Cria, Estacion Experimental Amazonas, Puerto Ayacucho, Venezuela." EXACT []
xref: urn\:lsid\:biocol.org\:col:35169
is_a: COLLECTION:0000000 ! fish_collection_abbreviation

[Term]
id: COLLECTION:0000181
name: MACLPI
def: "Ministerio de Agricultura y Cria, Seccion de Pesca Interior y Piscicultura, Venezuela." [COLLECTION:curator]
synonym: "Ministerio de Agricultura y Cria, Seccion de Pesca Interior y Piscicultura, Venezuela." EXACT []
is_a: COLLECTION:0000000 ! fish_collection_abbreviation

[Term]
id: COLLECTION:0000182
name: MACN
def: "Museo Argentino de Ciencias Naturales, Bernardino Rivadavia, Capital Federal, Argentina." [COLLECTION:curator]
synonym: "Museo Argentino de Ciencias Naturales, Bernardino Rivadavia, Capital Federal, Argentina." EXACT []
is_a: COLLECTION:0000000 ! fish_collection_abbreviation

[Term]
id: COLLECTION:0000183
name: MAMU
def: "University of Sydney, Macleay Museum, Sydney, New South Wales, Australia. Types are at AMS." [COLLECTION:curator]
synonym: "University of Sydney, Macleay Museum, Sydney, New South Wales, Australia. Types are at AMS." EXACT []
is_a: COLLECTION:0000000 ! fish_collection_abbreviation

[Term]
id: COLLECTION:0000184
name: MAPA
def: "Museu Anchieta Porto Alegra, Rio Grande do Sul, Brasil." [COLLECTION:curator]
synonym: "Museu Anchieta Porto Alegra, Rio Grande do Sul, Brasil." EXACT []
xref: urn\:lsid\:biocol.org\:col:35170
is_a: COLLECTION:0000000 ! fish_collection_abbreviation

[Term]
id: COLLECTION:0000185
name: MB
def: "Universidade de Lisboa, Museu Bocage, Lisboa, Portugal." [COLLECTION:curator]
synonym: "Universidade de Lisboa, Museu Bocage, Lisboa, Portugal." EXACT []
xref: urn\:lsid\:biocol.org\:col:35171
is_a: COLLECTION:0000000 ! fish_collection_abbreviation

[Term]
id: COLLECTION:0000186
name: MBLUZ
def: "Museo de Biologia de la Universidad del Zulia, Venezuela (Perez & Viloria 1994)" [COLLECTION:curator]
synonym: "Museo de Biologia de la Universidad del Zulia, Venezuela (Perez & Viloria 1994)" EXACT []
is_a: COLLECTION:0000000 ! fish_collection_abbreviation

[Term]
id: COLLECTION:0000187
name: MBUCV
def: "Universidad Central de Venezuela, Museo de Biologia, Caracas, Venezuela." [COLLECTION:curator]
synonym: "Universidad Central de Venezuela, Museo de Biologia, Caracas, Venezuela." EXACT []
xref: urn\:lsid\:biocol.org\:col:35172
is_a: COLLECTION:0000000 ! fish_collection_abbreviation

[Term]
id: COLLECTION:0000188
name: MCLSBB
def: "Museo Colegio La Salle Bonanova de Barcelona, Spain." [COLLECTION:curator]
synonym: "Museo Colegio La Salle Bonanova de Barcelona, Spain." EXACT []
is_a: COLLECTION:0000000 ! fish_collection_abbreviation

[Term]
id: COLLECTION:0000189
name: MCN
def: "Fundacacao Zoobotânica do Rio Grande do Sul, Museu de Ciencias Naturais, Rio Grande do Sul, Brazil." [COLLECTION:curator]
synonym: "Fundacacao Zoobotânica do Rio Grande do Sul, Museu de Ciencias Naturais, Rio Grande do Sul, Brazil." EXACT []
is_a: COLLECTION:0000000 ! fish_collection_abbreviation

[Term]
id: COLLECTION:0000190
name: MCNC
def: "Museo de Ciencias Naturales, Caracas, Venezuela." [COLLECTION:curator]
synonym: "Museo de Ciencias Naturales, Caracas, Venezuela." EXACT []
is_a: COLLECTION:0000000 ! fish_collection_abbreviation

[Term]
id: COLLECTION:0000191
name: MCNG
def: "Museo de Ciencias Naturales, Portuguesa, Venezuela." [COLLECTION:curator]
synonym: "Museo de Ciencias Naturales, Portuguesa, Venezuela." EXACT []
xref: urn\:lsid\:biocol.org\:col:35173
is_a: COLLECTION:0000000 ! fish_collection_abbreviation

[Term]
id: COLLECTION:0000192
name: MCP
def: "Pontificia Universidade Catoica do Rio Grande do Sul, Museu de Ciencias, Rio Grande do Sul, Porto Alegre, Brazil." [COLLECTION:curator]
synonym: "Pontificia Universidade Catoica do Rio Grande do Sul, Museu de Ciencias, Rio Grande do Sul, Porto Alegre, Brazil." EXACT []
xref: urn\:lsid\:biocol.org\:col:35174
is_a: COLLECTION:0000000 ! fish_collection_abbreviation

[Term]
id: COLLECTION:0000193
name: MCSNC
def: "Museo Civico di Storia Naturale, Carmagnola, Italy." [COLLECTION:curator]
synonym: "Museo Civico di Storia Naturale, Carmagnola, Italy." EXACT []
is_a: COLLECTION:0000000 ! fish_collection_abbreviation

[Term]
id: COLLECTION:0000194
name: MCZ
def: "Museum of Comparative Zoology, Harvard University, Cambridge, Massachusetts." [COLLECTION:curator]
synonym: "Museum of Comparative Zoology, Harvard University, Cambridge, Massachusetts." EXACT []
xref: urn\:lsid\:biocol.org\:col:35175
is_a: COLLECTION:0000000 ! fish_collection_abbreviation

[Term]
id: COLLECTION:0000195
name: MD
def: "Museo do Dundo, Dundo, Angola." [COLLECTION:curator]
synonym: "Museo do Dundo, Dundo, Angola." EXACT []
is_a: COLLECTION:0000000 ! fish_collection_abbreviation

[Term]
id: COLLECTION:0000196
name: MDZAU
def: "Museum Deptartment of Zoology, Andhra Univ., India." [COLLECTION:curator]
synonym: "Museum Deptartment of Zoology, Andhra Univ., India." EXACT []
is_a: COLLECTION:0000000 ! fish_collection_abbreviation

[Term]
id: COLLECTION:0000197
name: MEPAN
def: "Museum of Evolution, Polish Academy of Sciences." [COLLECTION:curator]
synonym: "Museum of Evolution, Polish Academy of Sciences." EXACT []
is_a: COLLECTION:0000000 ! fish_collection_abbreviation

[Term]
id: COLLECTION:0000198
name: MEPN
def: "Museo Escuela Politecnica Nacional, Quito, Ecuador. Also as Museo de Biologia de la Escuela." [COLLECTION:curator]
synonym: "Museo Escuela Politecnica Nacional, Quito, Ecuador. Also as Museo de Biologia de la Escuela." EXACT []
xref: urn\:lsid\:biocol.org\:col:35176
is_a: COLLECTION:0000000 ! fish_collection_abbreviation

[Term]
id: COLLECTION:0000199
name: MFA
def: "Museo 'Florentino Ameghino', Santa Fe, Argentina." [COLLECTION:curator]
synonym: "Museo 'Florentino Ameghino', Santa Fe, Argentina." EXACT []
is_a: COLLECTION:0000000 ! fish_collection_abbreviation

[Term]
id: COLLECTION:0000200
name: MFLB
def: "Marine Fisheries Laboratory, Bangkok, Thailand." [COLLECTION:curator]
synonym: "Marine Fisheries Laboratory, Bangkok, Thailand." EXACT []
is_a: COLLECTION:0000000 ! fish_collection_abbreviation

[Term]
id: COLLECTION:0000201
name: MFRU
def: "Malawi Fisheries Research Unit, Lake Malawi, Africa. Also seen as MFU." [COLLECTION:curator]
synonym: "Malawi Fisheries Research Unit, Lake Malawi, Africa. Also seen as MFU." EXACT []
is_a: COLLECTION:0000000 ! fish_collection_abbreviation

[Term]
id: COLLECTION:0000202
name: MG
def: "See MGHNL." [COLLECTION:curator]
synonym: "See MGHNL." EXACT []
is_a: COLLECTION:0000000 ! fish_collection_abbreviation

[Term]
id: COLLECTION:0000203
name: MGAB
def: "Muzeul de Istorie Naturala 'Grigore Antipa', Bucharest, Romania." [COLLECTION:curator]
synonym: "Muzeul de Istorie Naturala 'Grigore Antipa', Bucharest, Romania." EXACT []
is_a: COLLECTION:0000000 ! fish_collection_abbreviation

[Term]
id: COLLECTION:0000204
name: MGHNL
def: "Musee Guimet d'Histoire Naturelle de Lyon, Lyon, France." [COLLECTION:curator]
synonym: "Musee Guimet d'Histoire Naturelle de Lyon, Lyon, France." EXACT []
is_a: COLLECTION:0000000 ! fish_collection_abbreviation

[Term]
id: COLLECTION:0000205
name: MGHSJ
def: "Matuyama Girl's High School, Matuyama City, Japan." [COLLECTION:curator]
synonym: "Matuyama Girl's High School, Matuyama City, Japan." EXACT []
is_a: COLLECTION:0000000 ! fish_collection_abbreviation

[Term]
id: COLLECTION:0000206
name: MHN-UNC
def: "Departamento de Ictiologia del Museo de Historia Natural de la Universidad Nacional de Colombia, Bogota, Colombia." [COLLECTION:curator]
synonym: "Departamento de Ictiologia del Museo de Historia Natural de la Universidad Nacional de Colombia, Bogota, Colombia." EXACT []
is_a: COLLECTION:0000000 ! fish_collection_abbreviation

[Term]
id: COLLECTION:0000207
name: MHNG
def: "Museum d'Histoire Naturelle, Geneve, Switzerland." [COLLECTION:curator]
synonym: "Museum d'Histoire Naturelle, Geneve, Switzerland." EXACT []
xref: urn\:lsid\:biocol.org\:col:34809
is_a: COLLECTION:0000000 ! fish_collection_abbreviation

[Term]
id: COLLECTION:0000208
name: MHNGA
def: "See MGAB." [COLLECTION:curator]
synonym: "See MGAB." EXACT []
is_a: COLLECTION:0000000 ! fish_collection_abbreviation

[Term]
id: COLLECTION:0000209
name: MHNI
def: "Museu Hist. Naturales Universidade Federal Minas Gerais, Brazil." [COLLECTION:curator]
synonym: "Museu Hist. Naturales Universidade Federal Minas Gerais, Brazil." EXACT []
is_a: COLLECTION:0000000 ! fish_collection_abbreviation

[Term]
id: COLLECTION:0000210
name: MHNJP
def: "Universidad Nacional Mayor de San Marcos, Museo de Historia Natural 'Javier Prado', Lima, Peru. MUSM sometimes used but not equal to MUSM below." [COLLECTION:curator]
synonym: "Universidad Nacional Mayor de San Marcos, Museo de Historia Natural 'Javier Prado', Lima, Peru. MUSM sometimes used but not equal to MUSM below." EXACT []
is_a: COLLECTION:0000000 ! fish_collection_abbreviation

[Term]
id: COLLECTION:0000211
name: MHNLR
def: "Museum d'Histoire Naturelle, La Rochelle, France." [COLLECTION:curator]
synonym: "Museum d'Histoire Naturelle, La Rochelle, France." EXACT []
is_a: COLLECTION:0000000 ! fish_collection_abbreviation

[Term]
id: COLLECTION:0000212
name: MHNLS
def: "Museo de Historia Natural de La Salle, Caracas, Venezuela." [COLLECTION:curator]
synonym: "Museo de Historia Natural de La Salle, Caracas, Venezuela." EXACT []
xref: urn\:lsid\:biocol.org\:col:35177
is_a: COLLECTION:0000000 ! fish_collection_abbreviation

[Term]
id: COLLECTION:0000213
name: MHNM
def: "Museo de Historia Natural de Montevideo, Montevideo, Uruguay." [COLLECTION:curator]
synonym: "Museo de Historia Natural de Montevideo, Montevideo, Uruguay." EXACT []
is_a: COLLECTION:0000000 ! fish_collection_abbreviation

[Term]
id: COLLECTION:0000214
name: MHV
def: "Musee de Haute Volta, Ouagadougou, Upper Volta." [COLLECTION:curator]
synonym: "Musee de Haute Volta, Ouagadougou, Upper Volta." EXACT []
is_a: COLLECTION:0000000 ! fish_collection_abbreviation

[Term]
id: COLLECTION:0000215
name: MIKU
def: "Marine Biological Institute, Kyoto University, Japan. Specimens now at FAKU." [COLLECTION:curator]
synonym: "Marine Biological Institute, Kyoto University, Japan. Specimens now at FAKU." EXACT []
is_a: COLLECTION:0000000 ! fish_collection_abbreviation

[Term]
id: COLLECTION:0000216
name: MLP
def: "Museo de La Plata, La Plata, Argentina." [COLLECTION:curator]
synonym: "Museo de La Plata, La Plata, Argentina." EXACT []
is_a: COLLECTION:0000000 ! fish_collection_abbreviation

[Term]
id: COLLECTION:0000217
name: MLS
def: "Marine Laboratory Sydney. Now at CSIRO." [COLLECTION:curator]
synonym: "Marine Laboratory Sydney. Now at CSIRO." EXACT []
is_a: COLLECTION:0000000 ! fish_collection_abbreviation

[Term]
id: COLLECTION:0000218
name: MM
def: "Museo del Mar, Bogota, Colombia." [COLLECTION:curator]
synonym: "Museo del Mar, Bogota, Colombia." EXACT []
is_a: COLLECTION:0000000 ! fish_collection_abbreviation

[Term]
id: COLLECTION:0000219
name: MMB
def: "Moravske Muzeum, Brno, Czech Republic." [COLLECTION:curator]
synonym: "Moravske Muzeum, Brno, Czech Republic." EXACT []
is_a: COLLECTION:0000000 ! fish_collection_abbreviation

[Term]
id: COLLECTION:0000220
name: MMF
def: "Museu Municipal do Funchal, Funchal, Madeira." [COLLECTION:curator]
synonym: "Museu Municipal do Funchal, Funchal, Madeira." EXACT []
is_a: COLLECTION:0000000 ! fish_collection_abbreviation

[Term]
id: COLLECTION:0000221
name: MMG
def: "Museo Marino de la Isla de Gorgona, Colombia. Also seen as MMGPe." [COLLECTION:curator]
synonym: "Museo Marino de la Isla de Gorgona, Colombia. Also seen as MMGPe." EXACT []
is_a: COLLECTION:0000000 ! fish_collection_abbreviation

[Term]
id: COLLECTION:0000222
name: MMNHS
def: "Macedonian Museum of Natural History, Skopje, former Yugoslavian Republic of Macedonia." [COLLECTION:curator]
synonym: "Macedonian Museum of Natural History, Skopje, former Yugoslavian Republic of Macedonia." EXACT []
is_a: COLLECTION:0000000 ! fish_collection_abbreviation

[Term]
id: COLLECTION:0000223
name: MMNS
def: "Mississippi Museum of Natural Science, Jackson, Mississippi, U.S.A." [COLLECTION:curator]
synonym: "Mississippi Museum of Natural Science, Jackson, Mississippi, U.S.A." EXACT []
is_a: COLLECTION:0000000 ! fish_collection_abbreviation

[Term]
id: COLLECTION:0000224
name: MMSU
def: "See ZMMU." [COLLECTION:curator]
synonym: "See ZMMU." EXACT []
is_a: COLLECTION:0000000 ! fish_collection_abbreviation

[Term]
id: COLLECTION:0000225
name: MMTT
def: "Muze-ye Melli-ye Tarikh-i Tabi'i, Tehran, Iran." [COLLECTION:curator]
synonym: "Muze-ye Melli-ye Tarikh-i Tabi'i, Tehran, Iran." EXACT []
is_a: COLLECTION:0000000 ! fish_collection_abbreviation

[Term]
id: COLLECTION:0000226
name: MMUS
def: "See MAMU." [COLLECTION:curator]
synonym: "See MAMU." EXACT []
is_a: COLLECTION:0000000 ! fish_collection_abbreviation

[Term]
id: COLLECTION:0000227
name: MNCN
def: "Museo Nacional de Ciencias Naturales, Madrid, Spain" [COLLECTION:curator]
synonym: "Museo Nacional de Ciencias Naturales, Madrid, Spain" EXACT []
is_a: COLLECTION:0000000 ! fish_collection_abbreviation

[Term]
id: COLLECTION:0000228
name: MNHN
def: "Museum National d'Histoire Naturelle, Paris. Several cataloging systems including numbers only, an A. series and B. series and later a system of year plus lot, MNHN 1899-456 [sometimes as 99-456]." [COLLECTION:curator]
synonym: "Museum National d'Histoire Naturelle, Paris. Several cataloging systems including numbers only, an A. series and B. series and later a system of year plus lot, MNHN 1899-456 [sometimes as 99-456]." EXACT []
xref: urn\:lsid\:biocol.org\:col:1005
is_a: COLLECTION:0000000 ! fish_collection_abbreviation

[Term]
id: COLLECTION:0000229
name: MNHNC
def: "Museo Nacional de Historia Natural, Santiago, Chile. Also as MNHNCH." [COLLECTION:curator]
synonym: "Museo Nacional de Historia Natural, Santiago, Chile. Also as MNHNCH." EXACT []
is_a: COLLECTION:0000000 ! fish_collection_abbreviation

[Term]
id: COLLECTION:0000230
name: MNHNCH
def: "Museo Nacional de Historia Natural de Chile, Santiago, Chile. Also seen as NMHNC." [COLLECTION:curator]
synonym: "Museo Nacional de Historia Natural de Chile, Santiago, Chile. Also seen as NMHNC." EXACT []
is_a: COLLECTION:0000000 ! fish_collection_abbreviation

[Term]
id: COLLECTION:0000231
name: MNHNM
def: "Museo Nacional de Historia Natural, Mexico City, Mexico." [COLLECTION:curator]
synonym: "Museo Nacional de Historia Natural, Mexico City, Mexico." EXACT []
is_a: COLLECTION:0000000 ! fish_collection_abbreviation

[Term]
id: COLLECTION:0000232
name: MNHNSD
def: "Museo Nacional de Historia Natural, Santo Domingo, Dominican Republic." [COLLECTION:curator]
synonym: "Museo Nacional de Historia Natural, Santo Domingo, Dominican Republic." EXACT []
is_a: COLLECTION:0000000 ! fish_collection_abbreviation

[Term]
id: COLLECTION:0000233
name: MNRJ
def: "Universidade Federal do Rio de Janeiro, Museu Nacional, Rio de Janeiro, Brazil." [COLLECTION:curator]
synonym: "Universidade Federal do Rio de Janeiro, Museu Nacional, Rio de Janeiro, Brazil." EXACT []
xref: urn\:lsid\:biocol.org\:col:35178
is_a: COLLECTION:0000000 ! fish_collection_abbreviation

[Term]
id: COLLECTION:0000234
name: MNSB
def: "Museum of Natural Sciences, Budapest, Hungary." [COLLECTION:curator]
synonym: "Museum of Natural Sciences, Budapest, Hungary." EXACT []
is_a: COLLECTION:0000000 ! fish_collection_abbreviation

[Term]
id: COLLECTION:0000235
name: MNZ
def: "Museum of New Zealand Te Papa Tongarewa, Wellington. Formerly NMNZ, continue to use NMNZ on bottle lots." [COLLECTION:curator]
synonym: "Museum of New Zealand Te Papa Tongarewa, Wellington. Formerly NMNZ, continue to use NMNZ on bottle lots." EXACT []
is_a: COLLECTION:0000000 ! fish_collection_abbreviation

[Term]
id: COLLECTION:0000236
name: MOFUNG
def: "Museu Oceanogr. Fundacao Universidade Federal do Rio Grande, Brazil." [COLLECTION:curator]
synonym: "Museu Oceanogr. Fundacao Universidade Federal do Rio Grande, Brazil." EXACT []
is_a: COLLECTION:0000000 ! fish_collection_abbreviation

[Term]
id: COLLECTION:0000237
name: MOM
def: "Musee Oceanographique Monaco, Monaco." [COLLECTION:curator]
synonym: "Musee Oceanographique Monaco, Monaco." EXACT []
is_a: COLLECTION:0000000 ! fish_collection_abbreviation

[Term]
id: COLLECTION:0000238
name: MPEG
def: "Museu Paraenese 'Emilio Goeldi', Para, Brazil." [COLLECTION:curator]
synonym: "Museu Paraenese 'Emilio Goeldi', Para, Brazil." EXACT []
is_a: COLLECTION:0000000 ! fish_collection_abbreviation

[Term]
id: COLLECTION:0000239
name: MRAC
def: "Musee Royal de l'Afrique Centrale, Tervuren, Belgium." [COLLECTION:curator]
synonym: "Musee Royal de l'Afrique Centrale, Tervuren, Belgium." EXACT []
xref: urn\:lsid\:biocol.org\:col:35179
is_a: COLLECTION:0000000 ! fish_collection_abbreviation

[Term]
id: COLLECTION:0000240
name: MRCN
def: "Museu Rio-Grandense de Ciencias Naturais, Brazil." [COLLECTION:curator]
synonym: "Museu Rio-Grandense de Ciencias Naturais, Brazil." EXACT []
is_a: COLLECTION:0000000 ! fish_collection_abbreviation

[Term]
id: COLLECTION:0000241
name: MSINR
def: "Museum Sichuan Institute of Natural Resources, China." [COLLECTION:curator]
synonym: "Museum Sichuan Institute of Natural Resources, China." EXACT []
is_a: COLLECTION:0000000 ! fish_collection_abbreviation

[Term]
id: COLLECTION:0000242
name: MSLH
def: "Chinese University of Hong Kong, Marine Sciences Laboratory, Hong Kong." [COLLECTION:curator]
synonym: "Chinese University of Hong Kong, Marine Sciences Laboratory, Hong Kong." EXACT []
is_a: COLLECTION:0000000 ! fish_collection_abbreviation

[Term]
id: COLLECTION:0000243
name: MSM
def: "Marine Science Museum, Tokai Univ., Shimizu City, Japan." [COLLECTION:curator]
synonym: "Marine Science Museum, Tokai Univ., Shimizu City, Japan." EXACT []
is_a: COLLECTION:0000000 ! fish_collection_abbreviation

[Term]
id: COLLECTION:0000244
name: MSNC
def: "Museo Civico di Storia Naturale, Carmagnola, Italy. Also seen as MCSNC." [COLLECTION:curator]
synonym: "Museo Civico di Storia Naturale, Carmagnola, Italy. Also seen as MCSNC." EXACT []
is_a: COLLECTION:0000000 ! fish_collection_abbreviation

[Term]
id: COLLECTION:0000245
name: MSNG
def: "Museo Civico di Storia Naturale di Genova 'Giacomo Doria', Genova, Italy." [COLLECTION:curator]
synonym: "Museo Civico di Storia Naturale di Genova 'Giacomo Doria', Genova, Italy." EXACT []
is_a: COLLECTION:0000000 ! fish_collection_abbreviation

[Term]
id: COLLECTION:0000246
name: MSNM
def: "Museo Civico di Storia Naturale, Milano, Italy." [COLLECTION:curator]
synonym: "Museo Civico di Storia Naturale, Milano, Italy." EXACT []
is_a: COLLECTION:0000000 ! fish_collection_abbreviation

[Term]
id: COLLECTION:0000247
name: MSNV
def: "Museo Civico di Storia Naturale, Venezia, Italy." [COLLECTION:curator]
synonym: "Museo Civico di Storia Naturale, Venezia, Italy." EXACT []
is_a: COLLECTION:0000000 ! fish_collection_abbreviation

[Term]
id: COLLECTION:0000248
name: MSNVR
def: "Museo Civico di Storia Naturale, Verona, Italy." [COLLECTION:curator]
synonym: "Museo Civico di Storia Naturale, Verona, Italy." EXACT []
is_a: COLLECTION:0000000 ! fish_collection_abbreviation

[Term]
id: COLLECTION:0000249
name: MSUM
def: "Michigan State University, University Museum, East Lansing, Michigan, U.S.A." [COLLECTION:curator]
synonym: "Michigan State University, University Museum, East Lansing, Michigan, U.S.A." EXACT []
is_a: COLLECTION:0000000 ! fish_collection_abbreviation

[Term]
id: COLLECTION:0000250
name: MT
def: "Museum Tinro, Vladyvostok, Russia -- now probably the private collection of Dolganov." [COLLECTION:curator]
synonym: "Museum Tinro, Vladyvostok, Russia -- now probably the private collection of Dolganov." EXACT []
is_a: COLLECTION:0000000 ! fish_collection_abbreviation

[Term]
id: COLLECTION:0000251
name: MTD
def: "Museum fur Tierkunde, Dresden, Germany. [Staatliches Museum fur Tierkunde]." [COLLECTION:curator]
synonym: "Museum fur Tierkunde, Dresden, Germany. [Staatliches Museum fur Tierkunde]." EXACT []
is_a: COLLECTION:0000000 ! fish_collection_abbreviation

[Term]
id: COLLECTION:0000252
name: MTKD
def: "Staatliches Museum fur Tierkunde, Dresden, Germany. See MTD." [COLLECTION:curator]
synonym: "Staatliches Museum fur Tierkunde, Dresden, Germany. See MTD." EXACT []
is_a: COLLECTION:0000000 ! fish_collection_abbreviation

[Term]
id: COLLECTION:0000253
name: MTUF
def: "University Museum, Tokyo University of Fisheries, Tokyo, Japan." [COLLECTION:curator]
synonym: "University Museum, Tokyo University of Fisheries, Tokyo, Japan." EXACT []
is_a: COLLECTION:0000000 ! fish_collection_abbreviation

[Term]
id: COLLECTION:0000254
name: MUMF
def: "Department of Life Sciences, Manipur University Museum of Fishes, Canchipur, Manipur, India." [COLLECTION:curator]
synonym: "Department of Life Sciences, Manipur University Museum of Fishes, Canchipur, Manipur, India." EXACT []
is_a: COLLECTION:0000000 ! fish_collection_abbreviation

[Term]
id: COLLECTION:0000255
name: MUSM
def: "Museo de Historia Natural de la Universidad Nacional Mayor de San Marcos, Lima, Peru." [COLLECTION:curator]
synonym: "Museo de Historia Natural de la Universidad Nacional Mayor de San Marcos, Lima, Peru." EXACT []
xref: urn\:lsid\:biocol.org\:col:35180
is_a: COLLECTION:0000000 ! fish_collection_abbreviation

[Term]
id: COLLECTION:0000256
name: MVZ
def: "University of California at Berkeley, Museum of Vertebrate Zoology, Berkeley, California, U.S.A. Most of collection now at CAS." [COLLECTION:curator]
synonym: "University of California at Berkeley, Museum of Vertebrate Zoology, Berkeley, California, U.S.A. Most of collection now at CAS." EXACT []
is_a: COLLECTION:0000000 ! fish_collection_abbreviation

[Term]
id: COLLECTION:0000257
name: MZB
def: "Museum Zoologicum Bogoriense, Bogor, Java, Indonesia." [COLLECTION:curator]
synonym: "Museum Zoologicum Bogoriense, Bogor, Java, Indonesia." EXACT []
xref: urn\:lsid\:biocol.org\:col:35181
is_a: COLLECTION:0000000 ! fish_collection_abbreviation

[Term]
id: COLLECTION:0000258
name: MZH
def: "Zoolgical Museum Helsinki, Finland." [COLLECTION:curator]
synonym: "Zoolgical Museum Helsinki, Finland." EXACT []
is_a: COLLECTION:0000000 ! fish_collection_abbreviation

[Term]
id: COLLECTION:0000259
name: MZN
def: "Musee Zoologie, Nancy, France." [COLLECTION:curator]
synonym: "Musee Zoologie, Nancy, France." EXACT []
is_a: COLLECTION:0000000 ! fish_collection_abbreviation

[Term]
id: COLLECTION:0000260
name: MZUABCS
def: "Museo de Zoologia de la Universidad Automica de Baja California Sur, Mexico." [COLLECTION:curator]
synonym: "Museo de Zoologia de la Universidad Automica de Baja California Sur, Mexico." EXACT []
xref: urn\:lsid\:biocol.org\:col:35182
is_a: COLLECTION:0000000 ! fish_collection_abbreviation

[Term]
id: COLLECTION:0000261
name: MZUF
def: "Universita di Firenze, Museo Zoologico de la Specola, Firenze, Italy." [COLLECTION:curator]
synonym: "Universita di Firenze, Museo Zoologico de la Specola, Firenze, Italy." EXACT []
is_a: COLLECTION:0000000 ! fish_collection_abbreviation

[Term]
id: COLLECTION:0000262
name: MZUS
def: "Universite de Strasbourg, Musee de Zoologie, Strasbourg, France." [COLLECTION:curator]
synonym: "Universite de Strasbourg, Musee de Zoologie, Strasbourg, France." EXACT []
is_a: COLLECTION:0000000 ! fish_collection_abbreviation

[Term]
id: COLLECTION:0000263
name: MZUSP
def: "Universidade de Sao Paulo, Museu de Zoologia, Sao Paulo, Brazil." [COLLECTION:curator]
synonym: "Universidade de Sao Paulo, Museu de Zoologia, Sao Paulo, Brazil." EXACT []
xref: urn\:lsid\:biocol.org\:col:35183
is_a: COLLECTION:0000000 ! fish_collection_abbreviation

[Term]
id: COLLECTION:0000264
name: MZUT
def: "Universita di Torino, Museo Zoologico, Torino, Italy." [COLLECTION:curator]
synonym: "Universita di Torino, Museo Zoologico, Torino, Italy." EXACT []
is_a: COLLECTION:0000000 ! fish_collection_abbreviation

[Term]
id: COLLECTION:0000265
name: MZUTH
def: "Museum of Zoology, University of Thessaloniki, Greece." [COLLECTION:curator]
synonym: "Museum of Zoology, University of Thessaloniki, Greece." EXACT []
is_a: COLLECTION:0000000 ! fish_collection_abbreviation

[Term]
id: COLLECTION:0000266
name: MZYU
def: "Museum of Zoology, Yunnan University, China." [COLLECTION:curator]
synonym: "Museum of Zoology, Yunnan University, China." EXACT []
is_a: COLLECTION:0000000 ! fish_collection_abbreviation

[Term]
id: COLLECTION:0000267
name: NARA
def: "National Aquatic Resources Agency, Colombo, Sri Lanka." [COLLECTION:curator]
synonym: "National Aquatic Resources Agency, Colombo, Sri Lanka." EXACT []
is_a: COLLECTION:0000000 ! fish_collection_abbreviation

[Term]
id: COLLECTION:0000268
name: NCIP
def: "Pusat Penelitian dan Pengembangan Oseanologi, Jakarta, Java, Indonesia." [COLLECTION:curator]
synonym: "Pusat Penelitian dan Pengembangan Oseanologi, Jakarta, Java, Indonesia." EXACT []
xref: urn\:lsid\:biocol.org\:col:35184
is_a: COLLECTION:0000000 ! fish_collection_abbreviation

[Term]
id: COLLECTION:0000269
name: NGI
def: "Nanjing Geographical Institute, Academia Sinica, Nanjing, China. Also as NIGL and NIG." [COLLECTION:curator]
synonym: "Nanjing Geographical Institute, Academia Sinica, Nanjing, China. Also as NIGL and NIG." EXACT []
is_a: COLLECTION:0000000 ! fish_collection_abbreviation

[Term]
id: COLLECTION:0000270
name: NHMG
def: "Naturhistoriska Museum Goteborg, Sweden. Also sometimes as GNM and NMG in literature." [COLLECTION:curator]
synonym: "Naturhistoriska Museum Goteborg, Sweden. Also sometimes as GNM and NMG in literature." EXACT []
is_a: COLLECTION:0000000 ! fish_collection_abbreviation

[Term]
id: COLLECTION:0000271
name: NHMR
def: "Natural History Museum, Reykjavik, Iceland." [COLLECTION:curator]
synonym: "Natural History Museum, Reykjavik, Iceland." EXACT []
is_a: COLLECTION:0000000 ! fish_collection_abbreviation

[Term]
id: COLLECTION:0000272
name: NHRM
def: "See NRM." [COLLECTION:curator]
synonym: "See NRM." EXACT []
xref: urn\:lsid\:biocol.org\:col:35011
is_a: COLLECTION:0000000 ! fish_collection_abbreviation

[Term]
id: COLLECTION:0000273
name: NIFI
def: "National Inland Fisheries Institute, Fish Taxonomy Division, Bangkok, Thailand." [COLLECTION:curator]
synonym: "National Inland Fisheries Institute, Fish Taxonomy Division, Bangkok, Thailand." EXACT []
is_a: COLLECTION:0000000 ! fish_collection_abbreviation

[Term]
id: COLLECTION:0000274
name: NIG
def: "Nanjing Geographical Institute, Academia Sinica, Nanjing, China. Also as NIGL and NGI." [COLLECTION:curator]
synonym: "Nanjing Geographical Institute, Academia Sinica, Nanjing, China. Also as NIGL and NGI." EXACT []
is_a: COLLECTION:0000000 ! fish_collection_abbreviation

[Term]
id: COLLECTION:0000275
name: NIGL
def: "Nanjing Institute of Geography and Limnology, Academia Sinica." [COLLECTION:curator]
synonym: "Nanjing Institute of Geography and Limnology, Academia Sinica." EXACT []
is_a: COLLECTION:0000000 ! fish_collection_abbreviation

[Term]
id: COLLECTION:0000276
name: NIWA
def: "National Institute of Water and Atmospheric Research, Christchurch, New Zealand." [COLLECTION:curator]
synonym: "National Institute of Water and Atmospheric Research, Christchurch, New Zealand." EXACT []
is_a: COLLECTION:0000000 ! fish_collection_abbreviation

[Term]
id: COLLECTION:0000277
name: NKMC
def: "National Kweiyang Medical College, Division of Biology, Kweichow, China." [COLLECTION:curator]
synonym: "National Kweiyang Medical College, Division of Biology, Kweichow, China." EXACT []
is_a: COLLECTION:0000000 ! fish_collection_abbreviation

[Term]
id: COLLECTION:0000278
name: NLU
def: "Northeast Lousiana University, Museum of Zoology, Monroe, Louisiana, U.S.A." [COLLECTION:curator]
synonym: "Northeast Lousiana University, Museum of Zoology, Monroe, Louisiana, U.S.A." EXACT []
xref: urn\:lsid\:biocol.org\:col:35185
is_a: COLLECTION:0000000 ! fish_collection_abbreviation

[Term]
id: COLLECTION:0000279
name: NMBA
def: "Naturhistorisches Museum Basel, Basel, Switzerland." [COLLECTION:curator]
synonym: "Naturhistorisches Museum Basel, Basel, Switzerland." EXACT []
is_a: COLLECTION:0000000 ! fish_collection_abbreviation

[Term]
id: COLLECTION:0000280
name: NMBE
def: "Naturhistorisches Museum Bern, Bern, Switzerland." [COLLECTION:curator]
synonym: "Naturhistorisches Museum Bern, Bern, Switzerland." EXACT []
is_a: COLLECTION:0000000 ! fish_collection_abbreviation

[Term]
id: COLLECTION:0000281
name: NMC
def: "National Museums of Canada, Ottawa, Canada." [COLLECTION:curator]
synonym: "National Museums of Canada, Ottawa, Canada." EXACT []
xref: urn\:lsid\:biocol.org\:col:35186
is_a: COLLECTION:0000000 ! fish_collection_abbreviation

[Term]
id: COLLECTION:0000282
name: NMFSH
def: "National Marine Fisheries Service, Honolulu, Hawaii. Also as BCFH, Bureau of Commercial Fisheries, Honolulu; much of collection at BPBM]." [COLLECTION:curator]
synonym: "National Marine Fisheries Service, Honolulu, Hawaii. Also as BCFH, Bureau of Commercial Fisheries, Honolulu; much of collection at BPBM]." EXACT []
is_a: COLLECTION:0000000 ! fish_collection_abbreviation

[Term]
id: COLLECTION:0000283
name: NMG
def: "Naturhistoriska Riksmuseet, Goteborg, Sweden. Also seen as NHMG." [COLLECTION:curator]
synonym: "Naturhistoriska Riksmuseet, Goteborg, Sweden. Also seen as NHMG." EXACT []
is_a: COLLECTION:0000000 ! fish_collection_abbreviation

[Term]
id: COLLECTION:0000284
name: NMI
def: "National Museum of Ireland, Dublin, Ireland." [COLLECTION:curator]
synonym: "National Museum of Ireland, Dublin, Ireland." EXACT []
is_a: COLLECTION:0000000 ! fish_collection_abbreviation

[Term]
id: COLLECTION:0000285
name: NMK
def: "National Museum, Nairobi, Kenya." [COLLECTION:curator]
synonym: "National Museum, Nairobi, Kenya." EXACT []
is_a: COLLECTION:0000000 ! fish_collection_abbreviation

[Term]
id: COLLECTION:0000286
name: NMMH
def: "North Manchurian Museum, Harbin, Manchuria, China." [COLLECTION:curator]
synonym: "North Manchurian Museum, Harbin, Manchuria, China." EXACT []
is_a: COLLECTION:0000000 ! fish_collection_abbreviation

[Term]
id: COLLECTION:0000287
name: NMNH
def: "National Museum of Natural History, New Delhi, India." [COLLECTION:curator]
synonym: "National Museum of Natural History, New Delhi, India." EXACT []
is_a: COLLECTION:0000000 ! fish_collection_abbreviation

[Term]
id: COLLECTION:0000288
name: NMNZ
def: "National Museum of New Zealand, Wellington, New Zealand. Since 1992: Museum of New Zealand Te Papa Tongarewa." [COLLECTION:curator]
synonym: "National Museum of New Zealand, Wellington, New Zealand. Since 1992: Museum of New Zealand Te Papa Tongarewa." EXACT []
is_a: COLLECTION:0000000 ! fish_collection_abbreviation

[Term]
id: COLLECTION:0000289
name: NMP
def: "Natal Museum, Pietermaritzburg, Natal, South Africa." [COLLECTION:curator]
synonym: "Natal Museum, Pietermaritzburg, Natal, South Africa." EXACT []
is_a: COLLECTION:0000000 ! fish_collection_abbreviation

[Term]
id: COLLECTION:0000290
name: NMS
def: "National Museum, Singapore." [COLLECTION:curator]
synonym: "National Museum, Singapore." EXACT []
is_a: COLLECTION:0000000 ! fish_collection_abbreviation

[Term]
id: COLLECTION:0000291
name: NMSL
def: "National Museum, Sir Marcus Fernando Mawatha, Colombo, Sri Lanka. Also seen as CMS." [COLLECTION:curator]
synonym: "National Museum, Sir Marcus Fernando Mawatha, Colombo, Sri Lanka. Also seen as CMS." EXACT []
is_a: COLLECTION:0000000 ! fish_collection_abbreviation

[Term]
id: COLLECTION:0000292
name: NMSZ
def: "National Museums of Scotland, Edinburgh, Scotland [after 1985, formerly Royal Scottish Museum]." [COLLECTION:curator]
synonym: "National Museums of Scotland, Edinburgh, Scotland [after 1985, formerly Royal Scottish Museum]." EXACT []
is_a: COLLECTION:0000000 ! fish_collection_abbreviation

[Term]
id: COLLECTION:0000293
name: NMV
def: "National Museum of Victoria, Melbourne, Victoria, Australia. Style is A2345 with no period after the A; also an R series and straight number system." [COLLECTION:curator]
synonym: "National Museum of Victoria, Melbourne, Victoria, Australia. Style is A2345 with no period after the A; also an R series and straight number system." EXACT []
xref: urn\:lsid\:biocol.org\:col:35187
is_a: COLLECTION:0000000 ! fish_collection_abbreviation

[Term]
id: COLLECTION:0000294
name: NMW
def: "Naturhistorisches Museum, Wien (Vienna), Austria." [COLLECTION:curator]
synonym: "Naturhistorisches Museum, Wien (Vienna), Austria." EXACT []
xref: urn\:lsid\:biocol.org\:col:35188
is_a: COLLECTION:0000000 ! fish_collection_abbreviation

[Term]
id: COLLECTION:0000295
name: NOI
def: "Nanhai Oceanographic Institute, Nanhai, China." [COLLECTION:curator]
synonym: "Nanhai Oceanographic Institute, Nanhai, China." EXACT []
is_a: COLLECTION:0000000 ! fish_collection_abbreviation

[Term]
id: COLLECTION:0000296
name: NPIB
def: "Northwest Plateau Institute of Biology, Xining, Qinghai, China." [COLLECTION:curator]
synonym: "Northwest Plateau Institute of Biology, Xining, Qinghai, China." EXACT []
is_a: COLLECTION:0000000 ! fish_collection_abbreviation

[Term]
id: COLLECTION:0000297
name: NRIBAS
def: "National Research Institute of Biology, Academia Sinica, Nanking, China." [COLLECTION:curator]
synonym: "National Research Institute of Biology, Academia Sinica, Nanking, China." EXACT []
is_a: COLLECTION:0000000 ! fish_collection_abbreviation

[Term]
id: COLLECTION:0000298
name: NRM
def: "Naturhistoriska Riksmuseet, Stockholm, Sweden." [COLLECTION:curator]
synonym: "Naturhistoriska Riksmuseet, Stockholm, Sweden." EXACT []
xref: urn\:lsid\:biocol.org\:col:35011
is_a: COLLECTION:0000000 ! fish_collection_abbreviation

[Term]
id: COLLECTION:0000299
name: NRMS
def: "See NRM." [COLLECTION:curator]
synonym: "See NRM." EXACT []
is_a: COLLECTION:0000000 ! fish_collection_abbreviation

[Term]
id: COLLECTION:0000300
name: NRS
def: "Northern Regional Station, Zoological Survey of India [also as ZSI/NRS]." [COLLECTION:curator]
synonym: "Northern Regional Station, Zoological Survey of India [also as ZSI/NRS]." EXACT []
is_a: COLLECTION:0000000 ! fish_collection_abbreviation

[Term]
id: COLLECTION:0000301
name: NSMT
def: "NSMT-P" [COLLECTION:curator]
synonym: "National Science Museum, Department of Zoology, Tokyo, Japan. Preferred style is NSMT-P 12345." EXACT []
synonym: "NSMT-P" EXACT []
xref: urn\:lsid\:biocol.org\:col:35189
is_a: COLLECTION:0000000 ! fish_collection_abbreviation

[Term]
id: COLLECTION:0000302
name: NSYU
def: "National Sun Yat-sen University, Kaohsiung, Taiwan. Also as NSYSU." [COLLECTION:curator]
synonym: "National Sun Yat-sen University, Kaohsiung, Taiwan. Also as NSYSU." EXACT []
is_a: COLLECTION:0000000 ! fish_collection_abbreviation

[Term]
id: COLLECTION:0000303
name: NTM
def: "Northern Territory Museum of Arts & Sciences, Darwin, Northern Terr., Australia" [COLLECTION:curator]
synonym: "Northern Territory Museum of Arts & Sciences, Darwin, Northern Terr., Australia" EXACT []
xref: urn\:lsid\:biocol.org\:col:35190
is_a: COLLECTION:0000000 ! fish_collection_abbreviation

[Term]
id: COLLECTION:0000304
name: NTUM
def: "National Taiwan University, Department of Zoology, Taipei, Taiwan" [COLLECTION:curator]
synonym: "National Taiwan University, Department of Zoology, Taipei, Taiwan" EXACT []
is_a: COLLECTION:0000000 ! fish_collection_abbreviation

[Term]
id: COLLECTION:0000305
name: NUSMBS
def: "Niigata University, Sado Marine Biological Station, Niigata, Japan." [COLLECTION:curator]
synonym: "Niigata University, Sado Marine Biological Station, Niigata, Japan." EXACT []
is_a: COLLECTION:0000000 ! fish_collection_abbreviation

[Term]
id: COLLECTION:0000306
name: NYSM
def: "New York State Museum, Albany, New York, U.S.A." [COLLECTION:curator]
synonym: "New York State Museum, Albany, New York, U.S.A." EXACT []
is_a: COLLECTION:0000000 ! fish_collection_abbreviation

[Term]
id: COLLECTION:0000307
name: NYZS
def: "New York Zoological Society, New York, U.S.A. Some specimens at CAS." [COLLECTION:curator]
synonym: "New York Zoological Society, New York, U.S.A. Some specimens at CAS." EXACT []
is_a: COLLECTION:0000000 ! fish_collection_abbreviation

[Term]
id: COLLECTION:0000308
name: NZOI
def: "New Zealand Oceanographic Institute, Wellington, New Zealand." [COLLECTION:curator]
synonym: "New Zealand Oceanographic Institute, Wellington, New Zealand." EXACT []
is_a: COLLECTION:0000000 ! fish_collection_abbreviation

[Term]
id: COLLECTION:0000309
name: OM
def: "Otago Museum, Dunedin, New Zealand." [COLLECTION:curator]
synonym: "Otago Museum, Dunedin, New Zealand." EXACT []
is_a: COLLECTION:0000000 ! fish_collection_abbreviation

[Term]
id: COLLECTION:0000310
name: OMNH
def: "Osaka Museum of Natural History, Osaka, Japan." [COLLECTION:curator]
synonym: "Osaka Museum of Natural History, Osaka, Japan." EXACT []
is_a: COLLECTION:0000000 ! fish_collection_abbreviation

[Term]
id: COLLECTION:0000311
name: OPM
def: "Okinawa Prefectual Museum, Naha, Okinawa, Japan." [COLLECTION:curator]
synonym: "Okinawa Prefectual Museum, Naha, Okinawa, Japan." EXACT []
is_a: COLLECTION:0000000 ! fish_collection_abbreviation

[Term]
id: COLLECTION:0000312
name: ORI
def: "Ocean Research Institute, Durban, South Africa." [COLLECTION:curator]
synonym: "Ocean Research Institute, Durban, South Africa." EXACT []
is_a: COLLECTION:0000000 ! fish_collection_abbreviation

[Term]
id: COLLECTION:0000313
name: ORIT
def: "University of Tokyo, Ocean Research Institute, Tokyo, Japan. Most types now at ZUMT." [COLLECTION:curator]
synonym: "University of Tokyo, Ocean Research Institute, Tokyo, Japan. Most types now at ZUMT." EXACT []
is_a: COLLECTION:0000000 ! fish_collection_abbreviation

[Term]
id: COLLECTION:0000314
name: ORSTOM
def: "Office de la Recherche scientifique et Technique Outre-mer. Several collections, such as at Noumea, New Caledonia; Dakar, Senegal; Trinidad, Bolivia." [COLLECTION:curator]
synonym: "Office de la Recherche scientifique et Technique Outre-mer. Several collections, such as at Noumea, New Caledonia; Dakar, Senegal; Trinidad, Bolivia." EXACT []
is_a: COLLECTION:0000000 ! fish_collection_abbreviation

[Term]
id: COLLECTION:0000315
name: OS
def: "Oregon State University, Museum of Natural History, Corvallis, Oregon, U.S.A. Also seen as OSU." [COLLECTION:curator]
synonym: "Oregon State University, Museum of Natural History, Corvallis, Oregon, U.S.A. Also seen as OSU." EXACT []
xref: urn\:lsid\:biocol.org\:col:35191
is_a: COLLECTION:0000000 ! fish_collection_abbreviation

[Term]
id: COLLECTION:0000316
name: OSM
def: "OSUM" [COLLECTION:curator]
synonym: "Ohio State University Museum, Columbus, Ohio, U.S.A." EXACT []
synonym: "OSUM" EXACT []
xref: urn\:lsid\:biocol.org\:col:35192
is_a: COLLECTION:0000000 ! fish_collection_abbreviation

[Term]
id: COLLECTION:0000317
name: OSU
def: "See OS." [COLLECTION:curator]
synonym: "See OS." EXACT []
is_a: COLLECTION:0000000 ! fish_collection_abbreviation

[Term]
id: COLLECTION:0000318
name: OSUO
def: "Oregon State University, School of Oceanography, Corvallis, Oregon, U.S.A. Most specimens transferred to OS main collection." [COLLECTION:curator]
synonym: "Oregon State University, School of Oceanography, Corvallis, Oregon, U.S.A. Most specimens transferred to OS main collection." EXACT []
is_a: COLLECTION:0000000 ! fish_collection_abbreviation

[Term]
id: COLLECTION:0000319
name: OSUS
def: "Oklahoma State University, Department of Zoology, Stillwater, Oklahoma, U.S.A." [COLLECTION:curator]
synonym: "Oklahoma State University, Department of Zoology, Stillwater, Oklahoma, U.S.A." EXACT []
is_a: COLLECTION:0000000 ! fish_collection_abbreviation

[Term]
id: COLLECTION:0000320
name: OUM
def: "Oxford University Museum, Oxford, England." [COLLECTION:curator]
synonym: "Oxford University Museum, Oxford, England." EXACT []
is_a: COLLECTION:0000000 ! fish_collection_abbreviation

[Term]
id: COLLECTION:0000321
name: PEM
def: "Port Elizabeth Museum, Port Elizabeth, South Africa." [COLLECTION:curator]
synonym: "Port Elizabeth Museum, Port Elizabeth, South Africa." EXACT []
is_a: COLLECTION:0000000 ! fish_collection_abbreviation

[Term]
id: COLLECTION:0000322
name: PMBC
def: "Phuket Marine Biological Centre, Phuket, Thailand." [COLLECTION:curator]
synonym: "Phuket Marine Biological Centre, Phuket, Thailand." EXACT []
is_a: COLLECTION:0000000 ! fish_collection_abbreviation

[Term]
id: COLLECTION:0000323
name: PNGM
def: "National Museum and Art Gallery, Port Moresby, Papua New Guinea." [COLLECTION:curator]
synonym: "National Museum and Art Gallery, Port Moresby, Papua New Guinea." EXACT []
is_a: COLLECTION:0000000 ! fish_collection_abbreviation

[Term]
id: COLLECTION:0000324
name: PNM
def: "Philippine National Museum, Manila, Luzon, Philippines." [COLLECTION:curator]
synonym: "Philippine National Museum, Manila, Luzon, Philippines." EXACT []
is_a: COLLECTION:0000000 ! fish_collection_abbreviation

[Term]
id: COLLECTION:0000325
name: PPSIO
def: "P. P. Shirshov Institute of Oceanology, Moscow, Russia. Same as IOM." [COLLECTION:curator]
synonym: "P. P. Shirshov Institute of Oceanology, Moscow, Russia. Same as IOM." EXACT []
is_a: COLLECTION:0000000 ! fish_collection_abbreviation

[Term]
id: COLLECTION:0000326
name: PSU
def: "Pennsylvania State University, University Park, Philadelphia, Pennsylvania, U.S.A." [COLLECTION:curator]
synonym: "Pennsylvania State University, University Park, Philadelphia, Pennsylvania, U.S.A." EXACT []
is_a: COLLECTION:0000000 ! fish_collection_abbreviation

[Term]
id: COLLECTION:0000327
name: PU
def: "Princeton University, Princeton, New Jersey, U.S.A." [COLLECTION:curator]
synonym: "Princeton University, Princeton, New Jersey, U.S.A." EXACT []
xref: urn\:lsid\:biocol.org\:col:35193
is_a: COLLECTION:0000000 ! fish_collection_abbreviation

[Term]
id: COLLECTION:0000328
name: QM
def: "Queensland Museum, Brisbane, Queensland, Australia. Sometimes seen as QMB." [COLLECTION:curator]
synonym: "Queensland Museum, Brisbane, Queensland, Australia. Sometimes seen as QMB." EXACT []
xref: urn\:lsid\:biocol.org\:col:35194
is_a: COLLECTION:0000000 ! fish_collection_abbreviation

[Term]
id: COLLECTION:0000329
name: QVMS
def: "Queen Victoria Museum, Salisbury, Zimbabwe." [COLLECTION:curator]
synonym: "Queen Victoria Museum, Salisbury, Zimbabwe." EXACT []
is_a: COLLECTION:0000000 ! fish_collection_abbreviation

[Term]
id: COLLECTION:0000330
name: RBCM
def: "Royal British Columbia Museum, Victoria, Canada. Formerly BCPM." [COLLECTION:curator]
synonym: "Royal British Columbia Museum, Victoria, Canada. Formerly BCPM." EXACT []
is_a: COLLECTION:0000000 ! fish_collection_abbreviation

[Term]
id: COLLECTION:0000331
name: RIFFL
def: "Research Institute of Freshwater Fisheries, Liaoning, China." [COLLECTION:curator]
synonym: "Research Institute of Freshwater Fisheries, Liaoning, China." EXACT []
is_a: COLLECTION:0000000 ! fish_collection_abbreviation

[Term]
id: COLLECTION:0000332
name: RMNH
def: "Rijksmuseum van Natuurlijke Historie, Leiden, Netherlands. Two systems initially, with overlapping numbers, dry collection preceded by a D." [COLLECTION:curator]
synonym: "Rijksmuseum van Natuurlijke Historie, Leiden, Netherlands. Two systems initially, with overlapping numbers, dry collection preceded by a D." EXACT []
xref: urn\:lsid\:biocol.org\:col:34992
is_a: COLLECTION:0000000 ! fish_collection_abbreviation

[Term]
id: COLLECTION:0000333
name: ROM
def: "Royal Ontario Museum, Toronto, Ontario, Canada." [COLLECTION:curator]
synonym: "Royal Ontario Museum, Toronto, Ontario, Canada." EXACT []
xref: urn\:lsid\:biocol.org\:col:35195
is_a: COLLECTION:0000000 ! fish_collection_abbreviation

[Term]
id: COLLECTION:0000334
name: RUSI
def: "JLBS" [COLLECTION:curator]
synonym: "JLBS" EXACT []
synonym: "South African Institute for Aquatic Biodiversity (SAIAB); formerly J. L. B. Smith Institute of Ichthyology, Grahamstown, South Africa." EXACT []
is_a: COLLECTION:0000000 ! fish_collection_abbreviation

[Term]
id: COLLECTION:0000335
name: SACON
def: "Salim Ali Centre for Ornithology and Natural History, Tamil Nadu, India." [COLLECTION:curator]
synonym: "Salim Ali Centre for Ornithology and Natural History, Tamil Nadu, India." EXACT []
is_a: COLLECTION:0000000 ! fish_collection_abbreviation

[Term]
id: COLLECTION:0000336
name: SAIAB
def: "See RUSI." [COLLECTION:curator]
synonym: "See RUSI." EXACT []
xref: urn\:lsid\:biocol.org\:col:34984
is_a: COLLECTION:0000000 ! fish_collection_abbreviation

[Term]
id: COLLECTION:0000337
name: SAM
def: "South African Museum, Cape Town, South Africa." [COLLECTION:curator]
synonym: "South African Museum, Cape Town, South Africa." EXACT []
xref: urn\:lsid\:biocol.org\:col:35196
is_a: COLLECTION:0000000 ! fish_collection_abbreviation

[Term]
id: COLLECTION:0000338
name: SAMA
def: "South Australian Museum, Adelaide, South Australia, Australia." [COLLECTION:curator]
synonym: "South Australian Museum, Adelaide, South Australia, Australia." EXACT []
xref: urn\:lsid\:biocol.org\:col:35197
is_a: COLLECTION:0000000 ! fish_collection_abbreviation

[Term]
id: COLLECTION:0000339
name: SAU
def: "Southern Arkansas University, Magnolia, Arkansas, U.S.A." [COLLECTION:curator]
synonym: "Southern Arkansas University, Magnolia, Arkansas, U.S.A." EXACT []
is_a: COLLECTION:0000000 ! fish_collection_abbreviation

[Term]
id: COLLECTION:0000340
name: SBM
def: "Sabah Museum, Sabah, East Malaysia (Ng, Martin-Smith & Ng 2000)" [COLLECTION:curator]
synonym: "Sabah Museum, Sabah, East Malaysia (Ng, Martin-Smith & Ng 2000)" EXACT []
is_a: COLLECTION:0000000 ! fish_collection_abbreviation

[Term]
id: COLLECTION:0000341
name: SCN
def: "Sociedad de Ciencias Naturales 'La Salle', Museo de Historia Natural 'La Salle', Caracas, Venezuela." [COLLECTION:curator]
synonym: "Sociedad de Ciencias Naturales 'La Salle', Museo de Historia Natural 'La Salle', Caracas, Venezuela." EXACT []
is_a: COLLECTION:0000000 ! fish_collection_abbreviation

[Term]
id: COLLECTION:0000342
name: SCSFRI
def: "South China Sea Fisheries Research Institute, Guangzhau, China." [COLLECTION:curator]
synonym: "South China Sea Fisheries Research Institute, Guangzhau, China." EXACT []
is_a: COLLECTION:0000000 ! fish_collection_abbreviation

[Term]
id: COLLECTION:0000343
name: SDSU
def: "San Diego State University, San Diego, California, U.S.A." [COLLECTION:curator]
synonym: "San Diego State University, San Diego, California, U.S.A." EXACT []
is_a: COLLECTION:0000000 ! fish_collection_abbreviation

[Term]
id: COLLECTION:0000344
name: SFC
def: "Laboratory of Fishes, Shanghai Fisheries University, China [also as Shanghai Fish. College]." [COLLECTION:curator]
synonym: "Laboratory of Fishes, Shanghai Fisheries University, China [also as Shanghai Fish. College]." EXACT []
is_a: COLLECTION:0000000 ! fish_collection_abbreviation

[Term]
id: COLLECTION:0000345
name: SFRS
def: "Sea Fisheries Research Station, Haifa, Israel." [COLLECTION:curator]
synonym: "Sea Fisheries Research Station, Haifa, Israel." EXACT []
is_a: COLLECTION:0000000 ! fish_collection_abbreviation

[Term]
id: COLLECTION:0000346
name: SIO
def: "Scripps Institution of Oceanography, La Jolla, California, U.S.A." [COLLECTION:curator]
synonym: "Scripps Institution of Oceanography, La Jolla, California, U.S.A." EXACT []
xref: urn\:lsid\:biocol.org\:col:35137
is_a: COLLECTION:0000000 ! fish_collection_abbreviation

[Term]
id: COLLECTION:0000347
name: SIUC
def: "Southern Illinois University (Carbondale), University Museum, Carbondale, Illinois, U.S.A." [COLLECTION:curator]
synonym: "Southern Illinois University (Carbondale), University Museum, Carbondale, Illinois, U.S.A." EXACT []
is_a: COLLECTION:0000000 ! fish_collection_abbreviation

[Term]
id: COLLECTION:0000348
name: SM
def: "Sarawak Museum, Kuching, Sarawak, Malaysia. Also seen as SMK." [COLLECTION:curator]
synonym: "Sarawak Museum, Kuching, Sarawak, Malaysia. Also seen as SMK." EXACT []
is_a: COLLECTION:0000000 ! fish_collection_abbreviation

[Term]
id: COLLECTION:0000349
name: SMBL
def: "Kyoto University, Seto Marine Biology Laboratory, Wakayama Prefecture, Japan. Specimens transferred to FAKU, some lost." [COLLECTION:curator]
synonym: "Kyoto University, Seto Marine Biology Laboratory, Wakayama Prefecture, Japan. Specimens transferred to FAKU, some lost." EXACT []
is_a: COLLECTION:0000000 ! fish_collection_abbreviation

[Term]
id: COLLECTION:0000350
name: SMF
def: "Naturmuseum und Forschungsinstitut Senckenberg, Frankfurt-am-Main, Germany." [COLLECTION:curator]
synonym: "Naturmuseum und Forschungsinstitut Senckenberg, Frankfurt-am-Main, Germany." EXACT []
is_a: COLLECTION:0000000 ! fish_collection_abbreviation

[Term]
id: COLLECTION:0000351
name: SMK
def: "Sarawak Museum, Kuching, Sarawak, Malaysia. See SM." [COLLECTION:curator]
synonym: "Sarawak Museum, Kuching, Sarawak, Malaysia. See SM." EXACT []
is_a: COLLECTION:0000000 ! fish_collection_abbreviation

[Term]
id: COLLECTION:0000352
name: SMNS
def: "Staatliches Museum fur Naturkunde in Stuttgart, Ludwigsburg, Germany." [COLLECTION:curator]
synonym: "Staatliches Museum fur Naturkunde in Stuttgart, Ludwigsburg, Germany." EXACT []
xref: urn\:lsid\:biocol.org\:col:35198
is_a: COLLECTION:0000000 ! fish_collection_abbreviation

[Term]
id: COLLECTION:0000353
name: SMWU
def: "Sangmyung University, Seoul, South Korea." [COLLECTION:curator]
synonym: "Sangmyung University, Seoul, South Korea." EXACT []
xref: urn\:lsid\:biocol.org\:col:35199
is_a: COLLECTION:0000000 ! fish_collection_abbreviation

[Term]
id: COLLECTION:0000354
name: SNHM
def: "Sudan Natural History Museum, Sudan." [COLLECTION:curator]
synonym: "Sudan Natural History Museum, Sudan." EXACT []
is_a: COLLECTION:0000000 ! fish_collection_abbreviation

[Term]
id: COLLECTION:0000355
name: SNMB
def: "Slovak National Museum, Bratislava, Czechoslovakia." [COLLECTION:curator]
synonym: "Slovak National Museum, Bratislava, Czechoslovakia." EXACT []
is_a: COLLECTION:0000000 ! fish_collection_abbreviation

[Term]
id: COLLECTION:0000356
name: SNMBR
def: "Staatliches Naturhistorisches Museum in Braunschweig, Germany. Also earlier seen as NMB and SNMB." [COLLECTION:curator]
synonym: "Staatliches Naturhistorisches Museum in Braunschweig, Germany. Also earlier seen as NMB and SNMB." EXACT []
is_a: COLLECTION:0000000 ! fish_collection_abbreviation

[Term]
id: COLLECTION:0000357
name: SNMNH
def: "Saudi Arabian National Museum of Natural History, Riyadh, Saudi Arabia." [COLLECTION:curator]
synonym: "Saudi Arabian National Museum of Natural History, Riyadh, Saudi Arabia." EXACT []
is_a: COLLECTION:0000000 ! fish_collection_abbreviation

[Term]
id: COLLECTION:0000358
name: SPNRI
def: "Sichuan Province, Natrual Resources Institute, China." [COLLECTION:curator]
synonym: "Sichuan Province, Natrual Resources Institute, China." EXACT []
is_a: COLLECTION:0000000 ! fish_collection_abbreviation

[Term]
id: COLLECTION:0000359
name: SRS/ZSI
def: "Southern Regional Station, Zoological Survey of India, Madras, India." [COLLECTION:curator]
synonym: "Southern Regional Station, Zoological Survey of India, Madras, India." EXACT []
is_a: COLLECTION:0000000 ! fish_collection_abbreviation

[Term]
id: COLLECTION:0000360
name: SSCN
def: "Museum of the Biological Laboratory, Scientific Society of China, Nanking, China." [COLLECTION:curator]
synonym: "Museum of the Biological Laboratory, Scientific Society of China, Nanking, China." EXACT []
is_a: COLLECTION:0000000 ! fish_collection_abbreviation

[Term]
id: COLLECTION:0000361
name: SU
def: "Stanford University. Specimens at CAS." [COLLECTION:curator]
synonym: "Stanford University. Specimens at CAS." EXACT []
is_a: COLLECTION:0000000 ! fish_collection_abbreviation

[Term]
id: COLLECTION:0000362
name: SUB
def: "Universite Bonn, Sammlung der Universite, Bonn, Germany." [COLLECTION:curator]
synonym: "Universite Bonn, Sammlung der Universite, Bonn, Germany." EXACT []
is_a: COLLECTION:0000000 ! fish_collection_abbreviation

[Term]
id: COLLECTION:0000363
name: SUF
def: "Shimonoseki University of Fisheries, Shimonoseki, Japan." [COLLECTION:curator]
synonym: "Shimonoseki University of Fisheries, Shimonoseki, Japan." EXACT []
is_a: COLLECTION:0000000 ! fish_collection_abbreviation

[Term]
id: COLLECTION:0000364
name: TAU
def: "Tel-Aviv University, Tel-Aviv, Israel." [COLLECTION:curator]
synonym: "Tel-Aviv University, Tel-Aviv, Israel." EXACT []
is_a: COLLECTION:0000000 ! fish_collection_abbreviation

[Term]
id: COLLECTION:0000365
name: TCWC
def: "Texas A&M University, Texas Cooperative Wildlife Collection, College Station, Texas, U.S.A." [COLLECTION:curator]
synonym: "Texas A&M University, Texas Cooperative Wildlife Collection, College Station, Texas, U.S.A." EXACT []
xref: urn\:lsid\:biocol.org\:col:35200
is_a: COLLECTION:0000000 ! fish_collection_abbreviation

[Term]
id: COLLECTION:0000366
name: TFMC
def: "Museo de Ciencias Naturales de Santa Cruz de Tenerife, Canary Islands." [COLLECTION:curator]
synonym: "Museo de Ciencias Naturales de Santa Cruz de Tenerife, Canary Islands." EXACT []
is_a: COLLECTION:0000000 ! fish_collection_abbreviation

[Term]
id: COLLECTION:0000367
name: TFRI
def: "Taiwan Fisheries Research Institute, Chilung, Taiwan." [COLLECTION:curator]
synonym: "Taiwan Fisheries Research Institute, Chilung, Taiwan." EXACT []
is_a: COLLECTION:0000000 ! fish_collection_abbreviation

[Term]
id: COLLECTION:0000368
name: THUP
def: "Tunghai University, Department of Zoology, Taichung, Taiwan." [COLLECTION:curator]
synonym: "Tunghai University, Department of Zoology, Taichung, Taiwan." EXACT []
is_a: COLLECTION:0000000 ! fish_collection_abbreviation

[Term]
id: COLLECTION:0000369
name: TISTR
def: "Thailand Institute for Scientific and Technological Research, Bangkok, Thailand." [COLLECTION:curator]
synonym: "Thailand Institute for Scientific and Technological Research, Bangkok, Thailand." EXACT []
is_a: COLLECTION:0000000 ! fish_collection_abbreviation

[Term]
id: COLLECTION:0000370
name: TIU
def: "Tokyo Imperial University, Science College Museum, Tokyo, Japan. Now ZMUT." [COLLECTION:curator]
synonym: "Tokyo Imperial University, Science College Museum, Tokyo, Japan. Now ZMUT." EXACT []
is_a: COLLECTION:0000000 ! fish_collection_abbreviation

[Term]
id: COLLECTION:0000371
name: TMBS
def: "Tatsuo Tanaka Memorial Biological Laboratory, Miyake-jima, Izu Islands, Japan." [COLLECTION:curator]
synonym: "Tatsuo Tanaka Memorial Biological Laboratory, Miyake-jima, Izu Islands, Japan." EXACT []
is_a: COLLECTION:0000000 ! fish_collection_abbreviation

[Term]
id: COLLECTION:0000372
name: TMFE
def: "Elasmobranchii Collection of the Department of Fisheries, Faculty of Marine Science and Technology, Tokai University." [COLLECTION:curator]
synonym: "Elasmobranchii Collection of the Department of Fisheries, Faculty of Marine Science and Technology, Tokai University." EXACT []
is_a: COLLECTION:0000000 ! fish_collection_abbreviation

[Term]
id: COLLECTION:0000373
name: TMH
def: "Tasmanian Museum and Art Gallery, Hobart, Tasmania, Australia." [COLLECTION:curator]
synonym: "Tasmanian Museum and Art Gallery, Hobart, Tasmania, Australia." EXACT []
is_a: COLLECTION:0000000 ! fish_collection_abbreviation

[Term]
id: COLLECTION:0000374
name: TMP
def: "Transvaal Museum, Pretoria, Transvaal, South Africa. Types at AMG." [COLLECTION:curator]
synonym: "Transvaal Museum, Pretoria, Transvaal, South Africa. Types at AMG." EXACT []
is_a: COLLECTION:0000000 ! fish_collection_abbreviation

[Term]
id: COLLECTION:0000375
name: TNHC
def: "Texas Memorial Museum, Texas Natural History Collection, Austin, Texas, U.S.A." [COLLECTION:curator]
synonym: "Texas Memorial Museum, Texas Natural History Collection, Austin, Texas, U.S.A." EXACT []
xref: urn\:lsid\:biocol.org\:col:35201
is_a: COLLECTION:0000000 ! fish_collection_abbreviation

[Term]
id: COLLECTION:0000376
name: TU
def: "Tulane University, Department of Zoology, New Orleans, Louisiana; Tulane University, Riverside Research Laboratories, Belle Chasse, Louisiana." [COLLECTION:curator]
synonym: "Tulane University, Department of Zoology, New Orleans, Louisiana; Tulane University, Riverside Research Laboratories, Belle Chasse, Louisiana." EXACT []
xref: urn\:lsid\:biocol.org\:col:35079
is_a: COLLECTION:0000000 ! fish_collection_abbreviation

[Term]
id: COLLECTION:0000377
name: TUFIL
def: "Tokyo University of Fisheries, Ichthyological Laboratory, Tokyo, Japan. Formerly IFI; now FAKU." [COLLECTION:curator]
synonym: "Tokyo University of Fisheries, Ichthyological Laboratory, Tokyo, Japan. Formerly IFI; now FAKU." EXACT []
is_a: COLLECTION:0000000 ! fish_collection_abbreviation

[Term]
id: COLLECTION:0000378
name: UAB
def: "Universidad Autonoma de Barcelona, Departamento de Biologia, Barcelona, Spain." [COLLECTION:curator]
synonym: "Universidad Autonoma de Barcelona, Departamento de Biologia, Barcelona, Spain." EXACT []
is_a: COLLECTION:0000000 ! fish_collection_abbreviation

[Term]
id: COLLECTION:0000379
name: UABCE
def: "Universidad de Autonoma de Baja California, Ensenada, Mexico." [COLLECTION:curator]
synonym: "Universidad de Autonoma de Baja California, Ensenada, Mexico." EXACT []
is_a: COLLECTION:0000000 ! fish_collection_abbreviation

[Term]
id: COLLECTION:0000380
name: UNCI
def: "Universite Nationale de Cote d'Ivoire, Abidjan, Ivory Coast." [COLLECTION:curator]
synonym: "Universite Nationale de Cote d'Ivoire, Abidjan, Ivory Coast." EXACT []
is_a: COLLECTION:0000000 ! fish_collection_abbreviation

[Term]
id: COLLECTION:0000381
name: UAM
def: "University of Alaska, Fairbanks, Alaska, U.S.A." [COLLECTION:curator]
synonym: "University of Alaska, Fairbanks, Alaska, U.S.A." EXACT []
xref: urn\:lsid\:biocol.org\:col:35075
is_a: COLLECTION:0000000 ! fish_collection_abbreviation

[Term]
id: COLLECTION:0000382
name: UAMZ
def: "University of Alberta Museum of Zoology, Alberta, Canada." [COLLECTION:curator]
synonym: "University of Alberta Museum of Zoology, Alberta, Canada." EXACT []
is_a: COLLECTION:0000000 ! fish_collection_abbreviation

[Term]
id: COLLECTION:0000383
name: UANL
def: "Universidad Autonoma de Nuevo Leon, Monterrey, Nuevo Leon, Mexico." [COLLECTION:curator]
synonym: "Universidad Autonoma de Nuevo Leon, Monterrey, Nuevo Leon, Mexico." EXACT []
is_a: COLLECTION:0000000 ! fish_collection_abbreviation

[Term]
id: COLLECTION:0000384
name: UAZ
def: "University of Arizona, Department of Ecology and Evolutionary Biology, Tucson, Arizona, U.S.A." [COLLECTION:curator]
synonym: "University of Arizona, Department of Ecology and Evolutionary Biology, Tucson, Arizona, U.S.A." EXACT []
is_a: COLLECTION:0000000 ! fish_collection_abbreviation

[Term]
id: COLLECTION:0000385
name: UBC
def: "University of British Columbia, Cowan Vertebrate Museum, Vancouver, British Columbia, Canada." [COLLECTION:curator]
synonym: "University of British Columbia, Cowan Vertebrate Museum, Vancouver, British Columbia, Canada." EXACT []
is_a: COLLECTION:0000000 ! fish_collection_abbreviation

[Term]
id: COLLECTION:0000386
name: UBJTL
def: "Universidad Bogota Jorge Tadeo Lozano, Colombia." [COLLECTION:curator]
synonym: "Universidad Bogota Jorge Tadeo Lozano, Colombia." EXACT []
is_a: COLLECTION:0000000 ! fish_collection_abbreviation

[Term]
id: COLLECTION:0000387
name: UCD
def: "University of California, Davis, California, U.S.A." [COLLECTION:curator]
synonym: "University of California, Davis, California, U.S.A." EXACT []
is_a: COLLECTION:0000000 ! fish_collection_abbreviation

[Term]
id: COLLECTION:0000388
name: UCLA
def: "University of California at Los Angeles, Department of Biology, Los Angeles, California. Much of collection now at LACM." [COLLECTION:curator]
synonym: "University of California at Los Angeles, Department of Biology, Los Angeles, California. Much of collection now at LACM." EXACT []
xref: urn\:lsid\:biocol.org\:col:35202
is_a: COLLECTION:0000000 ! fish_collection_abbreviation

[Term]
id: COLLECTION:0000389
name: UCR
def: "Universidad de Costa Rica, Museo de Zoologia, Depto. de Biologia, San Jose, Costa Rica." [COLLECTION:curator]
synonym: "Universidad de Costa Rica, Museo de Zoologia, Depto. de Biologia, San Jose, Costa Rica." EXACT []
xref: urn\:lsid\:biocol.org\:col:35203
is_a: COLLECTION:0000000 ! fish_collection_abbreviation

[Term]
id: COLLECTION:0000390
name: UDONECI
def: "Universidad de Oriente, Centro de Invest. Cient. del Nucleo de Nueva Esparta, Isla Margarita, Venezuela." [COLLECTION:curator]
synonym: "Universidad de Oriente, Centro de Invest. Cient. del Nucleo de Nueva Esparta, Isla Margarita, Venezuela." EXACT []
is_a: COLLECTION:0000000 ! fish_collection_abbreviation

[Term]
id: COLLECTION:0000391
name: UF
def: "University of Florida, Florida State Museum, Gainesville, Florida, U.S.A." [COLLECTION:curator]
synonym: "University of Florida, Florida State Museum, Gainesville, Florida, U.S.A." EXACT []
xref: urn\:lsid\:biocol.org\:col:35081
is_a: COLLECTION:0000000 ! fish_collection_abbreviation

[Term]
id: COLLECTION:0000392
name: UF-FSU
def: "See FSU." [COLLECTION:curator]
synonym: "See FSU." EXACT []
is_a: COLLECTION:0000000 ! fish_collection_abbreviation

[Term]
id: COLLECTION:0000393
name: UFPB
def: "Universidade Federal da Paraiba, Joao Pessoa, Brazil." [COLLECTION:curator]
synonym: "Universidade Federal da Paraiba, Joao Pessoa, Brazil." EXACT []
is_a: COLLECTION:0000000 ! fish_collection_abbreviation

[Term]
id: COLLECTION:0000394
name: UFRGS
def: "Universidade Federal do Rio Grande do Sul, Departamento de Zoologia, Porto Alegre, Rio Grande do Sul, Brazil." [COLLECTION:curator]
synonym: "Universidade Federal do Rio Grande do Sul, Departamento de Zoologia, Porto Alegre, Rio Grande do Sul, Brazil." EXACT []
is_a: COLLECTION:0000000 ! fish_collection_abbreviation

[Term]
id: COLLECTION:0000395
name: UFRJ
def: "Universidade Federal do Rio de Janeiro, Brazil. (synonym of MNRJ)" [COLLECTION:curator]
synonym: "Universidade Federal do Rio de Janeiro, Brazil. (synonym of MNRJ)" EXACT []
xref: urn\:lsid\:biocol.org\:col:35178
is_a: COLLECTION:0000000 ! fish_collection_abbreviation

[Term]
id: COLLECTION:0000396
name: UGAMNH
def: "University of Georgia, Museum of Natural History, Athens, Georgia, U.S.A." [COLLECTION:curator]
synonym: "University of Georgia, Museum of Natural History, Athens, Georgia, U.S.A." EXACT []
is_a: COLLECTION:0000000 ! fish_collection_abbreviation

[Term]
id: COLLECTION:0000397
name: UGM
def: "University of Guam, Mangilao, Guam." [COLLECTION:curator]
synonym: "University of Guam, Mangilao, Guam." EXACT []
is_a: COLLECTION:0000000 ! fish_collection_abbreviation

[Term]
id: COLLECTION:0000398
name: UH
def: "University of Hawaii, Honolulu, Hawaii. Types transferred to BPBM and some to USNM." [COLLECTION:curator]
synonym: "University of Hawaii, Honolulu, Hawaii. Types transferred to BPBM and some to USNM." EXACT []
is_a: COLLECTION:0000000 ! fish_collection_abbreviation

[Term]
id: COLLECTION:0000399
name: UI
def: "University of Ibadan, Ibadan, Nigeria." [COLLECTION:curator]
synonym: "University of Ibadan, Ibadan, Nigeria." EXACT []
is_a: COLLECTION:0000000 ! fish_collection_abbreviation

[Term]
id: COLLECTION:0000400
name: UMB
def: "Ubersee Museum, Bremen, Germany." [COLLECTION:curator]
synonym: "Ubersee Museum, Bremen, Germany." EXACT []
is_a: COLLECTION:0000000 ! fish_collection_abbreviation

[Term]
id: COLLECTION:0000401
name: UMIM
def: "University of Miami Ichthyological Museum, Coral Gables, Florida, U.S.A. No longer in existence, specimens mostly to USNM and UMML." [COLLECTION:curator]
synonym: "University of Miami Ichthyological Museum, Coral Gables, Florida, U.S.A. No longer in existence, specimens mostly to USNM and UMML." EXACT []
is_a: COLLECTION:0000000 ! fish_collection_abbreviation

[Term]
id: COLLECTION:0000402
name: UMML
def: "University of Miami Marine Laboratory, Miami, Florida. Most of collection transferred to UF." [COLLECTION:curator]
synonym: "University of Miami Marine Laboratory, Miami, Florida. Most of collection transferred to UF." EXACT []
is_a: COLLECTION:0000000 ! fish_collection_abbreviation

[Term]
id: COLLECTION:0000403
name: UMMZ
def: "University of Michigan Museum of Zoology, Ann Arbor, Michigan, U.S.A." [COLLECTION:curator]
synonym: "University of Michigan Museum of Zoology, Ann Arbor, Michigan, U.S.A." EXACT []
xref: urn\:lsid\:biocol.org\:col:35204
is_a: COLLECTION:0000000 ! fish_collection_abbreviation

[Term]
id: COLLECTION:0000404
name: UMOC
def: "University of Missouri, Museum of Zoology, Columbia, Missouri, U.S.A." [COLLECTION:curator]
synonym: "University of Missouri, Museum of Zoology, Columbia, Missouri, U.S.A." EXACT []
is_a: COLLECTION:0000000 ! fish_collection_abbreviation

[Term]
id: COLLECTION:0000405
name: UMUTZ
def: "Department of Zoology, University Museum, University of Tokyo, Tokyo, Japan. This abbreviation sometimes used; same as ZMUT." [COLLECTION:curator]
synonym: "Department of Zoology, University Museum, University of Tokyo, Tokyo, Japan. This abbreviation sometimes used; same as ZMUT." EXACT []
is_a: COLLECTION:0000000 ! fish_collection_abbreviation

[Term]
id: COLLECTION:0000406
name: UNAM
def: "Universidad Nacional Autonoma de Mexico, Departmento de Zoologia, Instituto de Biologia, Mexico, DF, Mexico. Same as IBUNAM." [COLLECTION:curator]
synonym: "Universidad Nacional Autonoma de Mexico, Departmento de Zoologia, Instituto de Biologia, Mexico, DF, Mexico. Same as IBUNAM." EXACT []
is_a: COLLECTION:0000000 ! fish_collection_abbreviation

[Term]
id: COLLECTION:0000407
name: UNEFM
def: "Universidad Experimental Francisco de Miranda, Venezuela." [COLLECTION:curator]
synonym: "Universidad Experimental Francisco de Miranda, Venezuela." EXACT []
is_a: COLLECTION:0000000 ! fish_collection_abbreviation

[Term]
id: COLLECTION:0000408
name: UNOAL
def: "University of Northern Alabama, Tuscalusa, Alabama, U.S.A." [COLLECTION:curator]
synonym: "University of Northern Alabama, Tuscalusa, Alabama, U.S.A." EXACT []
is_a: COLLECTION:0000000 ! fish_collection_abbreviation

[Term]
id: COLLECTION:0000409
name: UNOVC
def: "University of New Orleans, Department of Biological Sciences, New Orleans, Lousiania, U.S.A." [COLLECTION:curator]
synonym: "University of New Orleans, Department of Biological Sciences, New Orleans, Lousiania, U.S.A." EXACT []
is_a: COLLECTION:0000000 ! fish_collection_abbreviation

[Term]
id: COLLECTION:0000410
name: UNR
def: "University of Nevada, Museum of Biology, Reno, Nevada, U.S.A." [COLLECTION:curator]
synonym: "University of Nevada, Museum of Biology, Reno, Nevada, U.S.A." EXACT []
is_a: COLLECTION:0000000 ! fish_collection_abbreviation

[Term]
id: COLLECTION:0000411
name: UOMZ
def: "University of Oklahoma, Stovall Museum of Zoology, Norman, Oklahoma, U.S.A." [COLLECTION:curator]
synonym: "University of Oklahoma, Stovall Museum of Zoology, Norman, Oklahoma, U.S.A." EXACT []
is_a: COLLECTION:0000000 ! fish_collection_abbreviation

[Term]
id: COLLECTION:0000412
name: URB
def: "Ryukyu University Department of Zoology, Nakagusuku, Okinawa, Japan." [COLLECTION:curator]
synonym: "Ryukyu University Department of Zoology, Nakagusuku, Okinawa, Japan." EXACT []
is_a: COLLECTION:0000000 ! fish_collection_abbreviation

[Term]
id: COLLECTION:0000413
name: URM
def: "University of the Ryukyus, Nishihara, Okinawa, Japan." [COLLECTION:curator]
synonym: "University of the Ryukyus, Nishihara, Okinawa, Japan." EXACT []
is_a: COLLECTION:0000000 ! fish_collection_abbreviation

[Term]
id: COLLECTION:0000414
name: USA
def: "University of South Alabama, Mobile, Alabama, U.S.A." [COLLECTION:curator]
synonym: "University of South Alabama, Mobile, Alabama, U.S.A." EXACT []
is_a: COLLECTION:0000000 ! fish_collection_abbreviation

[Term]
id: COLLECTION:0000415
name: USBCF
def: "U. S. Bureau of Commercial Fisheries. Original collection with this abbreviation mostly now at USNM." [COLLECTION:curator]
synonym: "U. S. Bureau of Commercial Fisheries. Original collection with this abbreviation mostly now at USNM." EXACT []
is_a: COLLECTION:0000000 ! fish_collection_abbreviation

[Term]
id: COLLECTION:0000416
name: USFC
def: "U. S. Fish Commission. Original collection using this abbreviation mostly now at USNM." [COLLECTION:curator]
synonym: "U. S. Fish Commission. Original collection using this abbreviation mostly now at USNM." EXACT []
is_a: COLLECTION:0000000 ! fish_collection_abbreviation

[Term]
id: COLLECTION:0000417
name: USNM
def: "National Museum of Natural History, Washington D.C., U.S.A. Formerly United States National Museum; USNM acronym continues." [COLLECTION:curator]
synonym: "National Museum of Natural History, Washington D.C., U.S.A. Formerly United States National Museum; USNM acronym continues." EXACT []
xref: urn\:lsid\:biocol.org\:col:1002
is_a: COLLECTION:0000000 ! fish_collection_abbreviation

[Term]
id: COLLECTION:0000418
name: USP
def: "University of the South Pacific, Institute of Marine Resources, Suva, Fiji." [COLLECTION:curator]
synonym: "University of the South Pacific, Institute of Marine Resources, Suva, Fiji." EXACT []
is_a: COLLECTION:0000000 ! fish_collection_abbreviation

[Term]
id: COLLECTION:0000419
name: UT
def: "University of Tennessee, Department of Zoology, Knoxville, Tennessee, U.S.A." [COLLECTION:curator]
synonym: "University of Tennessee, Department of Zoology, Knoxville, Tennessee, U.S.A." EXACT []
is_a: COLLECTION:0000000 ! fish_collection_abbreviation

[Term]
id: COLLECTION:0000420
name: UTEP
def: "University of Texas at El Paso, Laboratory for Environmental Biology, El Paso, Texas, U.S.A." [COLLECTION:curator]
synonym: "University of Texas at El Paso, Laboratory for Environmental Biology, El Paso, Texas, U.S.A." EXACT []
is_a: COLLECTION:0000000 ! fish_collection_abbreviation

[Term]
id: COLLECTION:0000421
name: UUZM
def: "Uppsala University, Zoological Museum, Uppsala, Sweden." [COLLECTION:curator]
synonym: "Uppsala University, Zoological Museum, Uppsala, Sweden." EXACT []
is_a: COLLECTION:0000000 ! fish_collection_abbreviation

[Term]
id: COLLECTION:0000422
name: UW
def: "University of Washington, College of Fisheries, Seattle, Washington, U.S.A." [COLLECTION:curator]
synonym: "University of Washington, College of Fisheries, Seattle, Washington, U.S.A." EXACT []
xref: urn\:lsid\:biocol.org\:col:35205
is_a: COLLECTION:0000000 ! fish_collection_abbreviation

[Term]
id: COLLECTION:0000423
name: UZA
def: "Universidad Zoologia Aplicada, Departamento de Ecologia, Comunidad de Madrid, Madrid, Spain." [COLLECTION:curator]
synonym: "Universidad Zoologia Aplicada, Departamento de Ecologia, Comunidad de Madrid, Madrid, Spain." EXACT []
is_a: COLLECTION:0000000 ! fish_collection_abbreviation

[Term]
id: COLLECTION:0000424
name: VBCM
def: "Universidad Complutense de Madrid, Catedra de Vertebrados, Faculdad de Biologicas, Madrid, Spain." [COLLECTION:curator]
synonym: "Universidad Complutense de Madrid, Catedra de Vertebrados, Faculdad de Biologicas, Madrid, Spain." EXACT []
is_a: COLLECTION:0000000 ! fish_collection_abbreviation

[Term]
id: COLLECTION:0000425
name: VIMS
def: "Virginia Institute of Marine Science, Gloucester Point, Virginia, U.S.A." [COLLECTION:curator]
synonym: "Virginia Institute of Marine Science, Gloucester Point, Virginia, U.S.A." EXACT []
is_a: COLLECTION:0000000 ! fish_collection_abbreviation

[Term]
id: COLLECTION:0000426
name: VMM
def: "Vanderbilt Marine Museum, Centerport, New York, U.S.A. Most type specimens are now housed at the AMNH." [COLLECTION:curator]
synonym: "Vanderbilt Marine Museum, Centerport, New York, U.S.A. Most type specimens are now housed at the AMNH." EXACT []
is_a: COLLECTION:0000000 ! fish_collection_abbreviation

[Term]
id: COLLECTION:0000427
name: VSM
def: "Det Kgl. Norske Videnskabers Selskab Museet, Trondheim, Norway." [COLLECTION:curator]
synonym: "Det Kgl. Norske Videnskabers Selskab Museet, Trondheim, Norway." EXACT []
is_a: COLLECTION:0000000 ! fish_collection_abbreviation

[Term]
id: COLLECTION:0000428
name: VUW
def: "Victoria University, Wellington, New Zealand." [COLLECTION:curator]
synonym: "Victoria University, Wellington, New Zealand." EXACT []
is_a: COLLECTION:0000000 ! fish_collection_abbreviation

[Term]
id: COLLECTION:0000429
name: WAM
def: "Western Australian Museum, Perth, Western Australia, Australia." [COLLECTION:curator]
synonym: "Western Australian Museum, Perth, Western Australia, Australia." EXACT []
xref: urn\:lsid\:biocol.org\:col:1006
is_a: COLLECTION:0000000 ! fish_collection_abbreviation

[Term]
id: COLLECTION:0000430
name: WHOI
def: "Woods Hole Oceanographic Institution, Woods Hole, Massachusetts, U.S.A. Collection transferred to MCZ." [COLLECTION:curator]
synonym: "Woods Hole Oceanographic Institution, Woods Hole, Massachusetts, U.S.A. Collection transferred to MCZ." EXACT []
is_a: COLLECTION:0000000 ! fish_collection_abbreviation

[Term]
id: COLLECTION:0000431
name: WIAP
def: "Wistar Institute of Anatomy, Philadelphia, Pennsylvania, U.S.A. Now at ANSP." [COLLECTION:curator]
synonym: "Wistar Institute of Anatomy, Philadelphia, Pennsylvania, U.S.A. Now at ANSP." EXACT []
is_a: COLLECTION:0000000 ! fish_collection_abbreviation

[Term]
id: COLLECTION:0000432
name: WLMH
def: "West Lake Museum, Hangchow, Chekiang, China." [COLLECTION:curator]
synonym: "West Lake Museum, Hangchow, Chekiang, China." EXACT []
is_a: COLLECTION:0000000 ! fish_collection_abbreviation

[Term]
id: COLLECTION:0000433
name: XFCFC
def: "Xiamen Fisheries College, Fujian, China." [COLLECTION:curator]
synonym: "Xiamen Fisheries College, Fujian, China." EXACT []
is_a: COLLECTION:0000000 ! fish_collection_abbreviation

[Term]
id: COLLECTION:0000434
name: YCM
def: "Yokosuka City Museum, Yokosuka, Kanagawa, Japan." [COLLECTION:curator]
synonym: "Yokosuka City Museum, Yokosuka, Kanagawa, Japan." EXACT []
is_a: COLLECTION:0000000 ! fish_collection_abbreviation

[Term]
id: COLLECTION:0000435
name: YPM
def: "Yale University, Peabody Museum, New Haven, Connecticut, U.S.A." [COLLECTION:curator]
synonym: "Yale University, Peabody Museum, New Haven, Connecticut, U.S.A." EXACT []
xref: urn\:lsid\:biocol.org\:col:35206
is_a: COLLECTION:0000000 ! fish_collection_abbreviation

[Term]
id: COLLECTION:0000436
name: YU
def: "Yunnan University, Kunming, Yunnan, China." [COLLECTION:curator]
synonym: "Yunnan University, Kunming, Yunnan, China." EXACT []
is_a: COLLECTION:0000000 ! fish_collection_abbreviation

[Term]
id: COLLECTION:0000437
name: ZFMK
def: "Zoologisches Forschunginstitut und Museum Alexander Koenig, Bonn, Germany." [COLLECTION:curator]
synonym: "Zoologisches Forschunginstitut und Museum Alexander Koenig, Bonn, Germany." EXACT []
is_a: COLLECTION:0000000 ! fish_collection_abbreviation

[Term]
id: COLLECTION:0000438
name: ZIAN
def: "Zoological Institute, Academy of Sciences, Leningrad. Same as ZISP." [COLLECTION:curator]
synonym: "Zoological Institute, Academy of Sciences, Leningrad. Same as ZISP." EXACT []
is_a: COLLECTION:0000000 ! fish_collection_abbreviation

[Term]
id: COLLECTION:0000439
name: ZICUP
def: "Zoological Institute Charles University, Prague, Czechoslovakia." [COLLECTION:curator]
synonym: "Zoological Institute Charles University, Prague, Czechoslovakia." EXACT []
is_a: COLLECTION:0000000 ! fish_collection_abbreviation

[Term]
id: COLLECTION:0000440
name: ZIHU
def: "Hiroshima University, Zoological Institute, Hiroshima, Japan." [COLLECTION:curator]
synonym: "Hiroshima University, Zoological Institute, Hiroshima, Japan." EXACT []
is_a: COLLECTION:0000000 ! fish_collection_abbreviation

[Term]
id: COLLECTION:0000441
name: ZIK
def: "Ukrainian Academy of Sciences, Zoological Insitute, Kiev, Ukraine." [COLLECTION:curator]
synonym: "Ukrainian Academy of Sciences, Zoological Insitute, Kiev, Ukraine." EXACT []
is_a: COLLECTION:0000000 ! fish_collection_abbreviation

[Term]
id: COLLECTION:0000442
name: ZIKU
def: "Zoological Institute, Kochi University, Kochi, Japan." [COLLECTION:curator]
synonym: "Zoological Institute, Kochi University, Kochi, Japan." EXACT []
is_a: COLLECTION:0000000 ! fish_collection_abbreviation

[Term]
id: COLLECTION:0000443
name: ZIL
def: "Now ZISP." [COLLECTION:curator]
synonym: "Now ZISP." EXACT []
is_a: COLLECTION:0000000 ! fish_collection_abbreviation

[Term]
id: COLLECTION:0000444
name: ZIN
def: "Zoological Institute, Academy of Sciences, St. Petersburg, Russia [preferred acronym]. Also seen as ZIL and ZISP." [COLLECTION:curator]
synonym: "Zoological Institute, Academy of Sciences, St. Petersburg, Russia [preferred acronym]. Also seen as ZIL and ZISP." EXACT []
is_a: COLLECTION:0000000 ! fish_collection_abbreviation

[Term]
id: COLLECTION:0000445
name: ZISP
def: "See ZIN." [COLLECTION:curator]
synonym: "See ZIN." EXACT []
is_a: COLLECTION:0000000 ! fish_collection_abbreviation

[Term]
id: COLLECTION:0000446
name: ZIUT
def: "Zoological Institute of the University of Tokyo. Same as ZUMT." [COLLECTION:curator]
synonym: "Zoological Institute of the University of Tokyo. Same as ZUMT." EXACT []
is_a: COLLECTION:0000000 ! fish_collection_abbreviation

[Term]
id: COLLECTION:0000447
name: ZLSYU
def: "Zoological Laboratory, Sun Yatsen University, China." [COLLECTION:curator]
synonym: "Zoological Laboratory, Sun Yatsen University, China." EXACT []
is_a: COLLECTION:0000000 ! fish_collection_abbreviation

[Term]
id: COLLECTION:0000448
name: ZMA
def: "Universiteit van Amsterdam, Zoologisch Museum, Amsterdam, The Netherlands. Usually cited with a period representing a comma, as ZAM 110,456, which we have deleted." [COLLECTION:curator]
synonym: "Universiteit van Amsterdam, Zoologisch Museum, Amsterdam, The Netherlands. Usually cited with a period representing a comma, as ZAM 110,456, which we have deleted." EXACT []
xref: urn\:lsid\:biocol.org\:col:35207
is_a: COLLECTION:0000000 ! fish_collection_abbreviation

[Term]
id: COLLECTION:0000449
name: ZMAU
def: "Zoological Museum Andhra University, India." [COLLECTION:curator]
synonym: "Zoological Museum Andhra University, India." EXACT []
is_a: COLLECTION:0000000 ! fish_collection_abbreviation

[Term]
id: COLLECTION:0000450
name: ZMB
def: "Humboldt Universite, Museum fur Naturkunde, Berlin, Germany." [COLLECTION:curator]
synonym: "Humboldt Universite, Museum fur Naturkunde, Berlin, Germany." EXACT []
xref: urn\:lsid\:biocol.org\:col:35208
is_a: COLLECTION:0000000 ! fish_collection_abbreviation

[Term]
id: COLLECTION:0000451
name: ZMC
def: "Department of Biology, Zunyi Medical College, Guizhou, China." [COLLECTION:curator]
synonym: "Department of Biology, Zunyi Medical College, Guizhou, China." EXACT []
is_a: COLLECTION:0000000 ! fish_collection_abbreviation

[Term]
id: COLLECTION:0000452
name: ZMFMIB
def: "Zoological Museum Fan Memorial Institute of Biology, Tsing Hua University, Peiping, China." [COLLECTION:curator]
synonym: "Zoological Museum Fan Memorial Institute of Biology, Tsing Hua University, Peiping, China." EXACT []
is_a: COLLECTION:0000000 ! fish_collection_abbreviation

[Term]
id: COLLECTION:0000453
name: ZMH
def: "Universite Hamburg, Zoologisches Institut und Museum, Hamburg, Germany." [COLLECTION:curator]
synonym: "Universite Hamburg, Zoologisches Institut und Museum, Hamburg, Germany." EXACT []
xref: urn\:lsid\:biocol.org\:col:35209
is_a: COLLECTION:0000000 ! fish_collection_abbreviation

[Term]
id: COLLECTION:0000454
name: ZMMGU
def: "Zoological Museum, Moscow State University, Moscow, Russia. Also seen as ZMMU." [COLLECTION:curator]
synonym: "Zoological Museum, Moscow State University, Moscow, Russia. Also seen as ZMMU." EXACT []
is_a: COLLECTION:0000000 ! fish_collection_abbreviation

[Term]
id: COLLECTION:0000455
name: ZMMGY
def: "See ZMMU." [COLLECTION:curator]
synonym: "See ZMMU." EXACT []
is_a: COLLECTION:0000000 ! fish_collection_abbreviation

[Term]
id: COLLECTION:0000456
name: ZMMSU
def: "See ZMMU." [COLLECTION:curator]
synonym: "See ZMMU." EXACT []
is_a: COLLECTION:0000000 ! fish_collection_abbreviation

[Term]
id: COLLECTION:0000457
name: ZMMU
def: "Zoological Museum, Moscow University, Russia. Sometimes seen in literature as MMSU, ZMMSU, ZMMGY, ZMMGU." [COLLECTION:curator]
synonym: "Zoological Museum, Moscow University, Russia. Sometimes seen in literature as MMSU, ZMMSU, ZMMGY, ZMMGU." EXACT []
is_a: COLLECTION:0000000 ! fish_collection_abbreviation

[Term]
id: COLLECTION:0000458
name: ZMT
def: "Georgian State Museum, Zoological Section, Tbilisi, (Asiatic) Georgia." [COLLECTION:curator]
synonym: "Georgian State Museum, Zoological Section, Tbilisi, (Asiatic) Georgia." EXACT []
is_a: COLLECTION:0000000 ! fish_collection_abbreviation

[Term]
id: COLLECTION:0000459
name: ZMUA
def: "Zoological Museum, University of Amoy, China." [COLLECTION:curator]
synonym: "Zoological Museum, University of Amoy, China." EXACT []
is_a: COLLECTION:0000000 ! fish_collection_abbreviation

[Term]
id: COLLECTION:0000460
name: ZMUAS
def: "Zoological Museum, Ukrainian Academy of Sciences." [COLLECTION:curator]
synonym: "Zoological Museum, Ukrainian Academy of Sciences." EXACT []
is_a: COLLECTION:0000000 ! fish_collection_abbreviation

[Term]
id: COLLECTION:0000461
name: ZMUB
def: "Universitetet i Bergen, Zoologisk Museum, Bergen, Norway." [COLLECTION:curator]
synonym: "Universitetet i Bergen, Zoologisk Museum, Bergen, Norway." EXACT []
is_a: COLLECTION:0000000 ! fish_collection_abbreviation

[Term]
id: COLLECTION:0000462
name: ZMUC
def: "Kobenhavns Universitet Zoologisk Museum (Zoological Museum, University of Copenhagen), Copenhagen, Denmark." [COLLECTION:curator]
synonym: "Kobenhavns Universitet Zoologisk Museum (Zoological Museum, University of Copenhagen), Copenhagen, Denmark." EXACT []
xref: urn\:lsid\:biocol.org\:col:35210
is_a: COLLECTION:0000000 ! fish_collection_abbreviation

[Term]
id: COLLECTION:0000463
name: ZMUH
def: "Zoological Museum, University of Hanoi, Hanoi, Viet Nam." [COLLECTION:curator]
synonym: "Zoological Museum, University of Hanoi, Hanoi, Viet Nam." EXACT []
is_a: COLLECTION:0000000 ! fish_collection_abbreviation

[Term]
id: COLLECTION:0000464
name: ZMUI
def: "Zoological Museum, University of Istanbul, Turkey." [COLLECTION:curator]
synonym: "Zoological Museum, University of Istanbul, Turkey." EXACT []
is_a: COLLECTION:0000000 ! fish_collection_abbreviation

[Term]
id: COLLECTION:0000465
name: ZMUL
def: "Universitetets Lund, Zoologiska Museet, Lund, Sweden." [COLLECTION:curator]
synonym: "Universitetets Lund, Zoologiska Museet, Lund, Sweden." EXACT []
is_a: COLLECTION:0000000 ! fish_collection_abbreviation

[Term]
id: COLLECTION:0000466
name: ZMUO
def: "Universitetets I Oslo, Zoologisk Museum, Oslo, Norway." [COLLECTION:curator]
synonym: "Universitetets I Oslo, Zoologisk Museum, Oslo, Norway." EXACT []
is_a: COLLECTION:0000000 ! fish_collection_abbreviation

[Term]
id: COLLECTION:0000467
name: ZMUT
def: "University of Tokyo, Department of Zoology, University Museum, Tokyo, Japan. Same as ZUMT." [COLLECTION:curator]
synonym: "University of Tokyo, Department of Zoology, University Museum, Tokyo, Japan. Same as ZUMT." EXACT []
is_a: COLLECTION:0000000 ! fish_collection_abbreviation

[Term]
id: COLLECTION:0000468
name: ZMUU
def: "Uppsala Universitet, Zoologiska Museet, Uppsala, Sweden." [COLLECTION:curator]
synonym: "Uppsala Universitet, Zoologiska Museet, Uppsala, Sweden." EXACT []
is_a: COLLECTION:0000000 ! fish_collection_abbreviation

[Term]
id: COLLECTION:0000469
name: ZRC
def: "Zoological Reference Collection, National University of Singapore, Singapore." [COLLECTION:curator]
synonym: "Zoological Reference Collection, National University of Singapore, Singapore." EXACT []
xref: urn\:lsid\:biocol.org\:col:35211
is_a: COLLECTION:0000000 ! fish_collection_abbreviation

[Term]
id: COLLECTION:0000470
name: ZSI
def: "F" [COLLECTION:curator]
synonym: "F" EXACT []
synonym: "Zoological Survey of India, Calcutta, India." EXACT []
xref: urn\:lsid\:biocol.org\:col:35212
is_a: COLLECTION:0000000 ! fish_collection_abbreviation

[Term]
id: COLLECTION:0000471
name: ZSM
def: "Zoologische Museum Staatssammlung, Munchen, Germany." [COLLECTION:curator]
synonym: "Zoologische Museum Staatssammlung, Munchen, Germany." EXACT []
xref: urn\:lsid\:biocol.org\:col:35213
is_a: COLLECTION:0000000 ! fish_collection_abbreviation

[Term]
id: COLLECTION:0000472
name: ZSM/CMK
def: "Zoologische Museum Staatssammlung, Munchen/Collection of Maurice Kottelat." [COLLECTION:curator]
synonym: "Zoologische Museum Staatssammlung, Munchen/Collection of Maurice Kottelat." EXACT []
is_a: COLLECTION:0000000 ! fish_collection_abbreviation

[Term]
id: COLLECTION:0000473
name: ZSM/LIPI
def: "Zoologische Museum Staatssammlung, Munchen/specimens eventually to be transferred to Indonesian institution." [COLLECTION:curator]
synonym: "Zoologische Museum Staatssammlung, Munchen/specimens eventually to be transferred to Indonesian institution." EXACT []
is_a: COLLECTION:0000000 ! fish_collection_abbreviation

[Term]
id: COLLECTION:0000474
name: ZSP
def: "Zoological Survey of Pakistan, Karachi, Pakistan." [COLLECTION:curator]
synonym: "Zoological Survey of Pakistan, Karachi, Pakistan." EXACT []
is_a: COLLECTION:0000000 ! fish_collection_abbreviation

[Term]
id: COLLECTION:0000475
name: ZUEC
def: "Universidade Estadual de Campinas, Departmento do Zoologia, Sao Paulo, Sao Paulo, Brazil." [COLLECTION:curator]
synonym: "Universidade Estadual de Campinas, Departmento do Zoologia, Sao Paulo, Sao Paulo, Brazil." EXACT []
is_a: COLLECTION:0000000 ! fish_collection_abbreviation

[Term]
id: COLLECTION:0000476
name: ZUFES
def: "Universidad Federal do Espirito Santo, Brazil." [COLLECTION:curator]
synonym: "Universidad Federal do Espirito Santo, Brazil." EXACT []
is_a: COLLECTION:0000000 ! fish_collection_abbreviation

[Term]
id: COLLECTION:0000477
name: ZUMT
def: "Department of Zoology, University Museum, University of Tokyo, Tokyo, Japan. Also seen as ZMUT." [COLLECTION:curator]
synonym: "Department of Zoology, University Museum, University of Tokyo, Tokyo, Japan. Also seen as ZMUT." EXACT []
is_a: COLLECTION:0000000 ! fish_collection_abbreviation

[Term]
id: COLLECTION:0000478
name: ZVC
def: "Depto. de Zoologia Vertebrados de la Facultad de Humanidades y Ciencias, Montevideo, Uruguay." [COLLECTION:curator]
synonym: "Depto. de Zoologia Vertebrados de la Facultad de Humanidades y Ciencias, Montevideo, Uruguay." EXACT []
is_a: COLLECTION:0000000 ! fish_collection_abbreviation

[Term]
id: COLLECTION:0000479
name: ZZSZ
def: "Zoology Department, Faculty of Natural Sciences, University of Zagreb (Zoologijski Zavod, Priodoslovno-matematicki fakultet, Sveucilista u Zagrebu), Zagreb, Croatia." [COLLECTION:curator]
synonym: "Zoology Department, Faculty of Natural Sciences, University of Zagreb (Zoologijski Zavod, Priodoslovno-matematicki fakultet, Sveucilista u Zagrebu), Zagreb, Croatia." EXACT []
is_a: COLLECTION:0000000 ! fish_collection_abbreviation

[Term]
id: COLLECTION:0000480
name: UMMP
def: "University of Michigan Museum of Paleontology" [COLLECTION:curator]
synonym: "University of Michigan Museum of Paleontology" EXACT []
xref: urn\:lsid\:biocol.org\:col:35214
is_a: COLLECTION:0000000 ! fish_collection_abbreviation

[Term]
id: COLLECTION:0000481
name: UAIC
def: "University of Alabama Ichthyological Collection" [COLLECTION:curator]
synonym: "University of Alabama Ichthyological Collection" EXACT []
xref: urn\:lsid\:biocol.org\:col:35215
is_a: COLLECTION:0000000 ! fish_collection_abbreviation

[Term]
id: COLLECTION:0000482
name: LU
def: "Loyola University Chicago, Department of Biology, Chicago, Illinois, USA" [COLLECTION:curator]
synonym: "Loyola University Chicago, Department of Biology, Chicago, Illinois, USA" EXACT []
xref: urn\:lsid\:biocol.org\:col:35216
is_a: COLLECTION:0000000 ! fish_collection_abbreviation

[Term]
id: COLLECTION:0000483
name: DBAV.UERJ
def: "Departamento de Biologia Animal e Vegetal da Universidade do Estado do Rio de Janeiro, Rio de Janeiro, Brazil" [COLLECTION:curator]
synonym: "Departamento de Biologia Animal e Vegetal da Universidade do Estado do Rio de Janeiro, Rio de Janeiro, Brazil" EXACT []
xref: urn\:lsid\:biocol.org\:col:35217
is_a: COLLECTION:0000000 ! fish_collection_abbreviation

[Term]
id: COLLECTION:0000484
name: WMM
def: "Witte Memorial Museum, San Antonio, Texas, U.S.A." [COLLECTION:curator]
synonym: "Witte Memorial Museum, San Antonio, Texas, U.S.A." EXACT []
xref: urn\:lsid\:biocol.org\:col:35218
is_a: COLLECTION:0000000 ! fish_collection_abbreviation

[Term]
id: COLLECTION:0000485
name: SCNU
def: "South China Normal University, Guangzhou, P.C. China" [COLLECTION:curator]
synonym: "South China Normal University, Guangzhou, P.C. China" EXACT []
xref: urn\:lsid\:biocol.org\:col:35219
is_a: COLLECTION:0000000 ! fish_collection_abbreviation

[Term]
id: COLLECTION:0000486
name: LIRP
def: "Laboratorio de Ictiologia de Ribeirao Preto, Faculdade de Filosofia, Ciencias e Letras de Ribeirao Preto, Sao Paulo, Brazil" [COLLECTION:curator]
synonym: "Laboratorio de Ictiologia de Ribeirao Preto, Faculdade de Filosofia, Ciencias e Letras de Ribeirao Preto, Sao Paulo, Brazil" EXACT []
xref: urn\:lsid\:biocol.org\:col:35220
is_a: COLLECTION:0000000 ! fish_collection_abbreviation

[Term]
id: COLLECTION:0000487
name: FAK
def: "Department of Fisheries, Faculty of Agriculture, Kinki University." [COLLECTION:curator]
synonym: "Department of Fisheries, Faculty of Agriculture, Kinki University." EXACT []
xref: urn\:lsid\:biocol.org\:col:35221
is_a: COLLECTION:0000000 ! fish_collection_abbreviation

[Term]
id: COLLECTION:0000488
name: KPM-NI
def: "Kanagawa Prefectural Museum of Natural History, Kanagawa, Japan." [COLLECTION:curator]
synonym: "Kanagawa Prefectural Museum of Natural History, Kanagawa, Japan." EXACT []
xref: urn\:lsid\:biocol.org\:col:35223
is_a: COLLECTION:0000000 ! fish_collection_abbreviation

[Term]
id: COLLECTION:0000489
name: QVM
def: " Queen Victoria Museum & Art Gallery, Launceston, Tasmania, Australia. Several numbering systems, preferred style 1972:5:44 not 72/5/44." [COLLECTION:curator]
synonym: " Queen Victoria Museum & Art Gallery, Launceston, Tasmania, Australia. Several numbering systems, preferred style 1972:5:44 not 72/5/44." EXACT []
xref: urn\:lsid\:biocol.org\:col:35222
is_a: COLLECTION:0000000 ! fish_collection_abbreviation

[Term]
id: COLLECTION:0000490
name: UWM
def: "University of Warmia, Poland" [COLLECTION:curator]
synonym: "University of Warmia, Poland" EXACT []
xref: urn\:lsid\:biocol.org\:col:35224
is_a: COLLECTION:0000000 ! fish_collection_abbreviation

[Term]
id: COLLECTION:0000491
name: SIUE
def: "Southern Illinois University (Edwardsville), Edwardsville, Illinois, U.S.A." [COLLECTION:curator]
synonym: "Southern Illinois University (Edwardsville), Edwardsville, Illinois, U.S.A." EXACT []
is_a: COLLECTION:0000000 ! fish_collection_abbreviation

[Term]
id: COLLECTION:0000492
name: CNPICT
def: "Centro Nacional Patagonico-Ictiologia, Argentina" [COLLECTION:curator]
synonym: "Centro Nacional Patagonico-Ictiologia, Argentina" EXACT []
is_a: COLLECTION:0000000 ! fish_collection_abbreviation

[Term]
id: COLLECTION:0000493
name: DZSJRP
def: "Departamento de Zoologia, Universidade Estadual Paulista, Sao Jose do Rio Preto, Brazil." [COLLECTION:curator]
synonym: "Departamento de Zoologia, Universidade Estadual Paulista, Sao Jose do Rio Preto, Brazil." EXACT []
is_a: COLLECTION:0000000 ! fish_collection_abbreviation

[Term]
id: COLLECTION:0000494
name: SLUM
def: "Saint Louis University Museum, Saint Louis, Missouri, U.S.A." [COLLECTION:curator]
synonym: "Saint Louis University Museum, Saint Louis, Missouri, U.S.A." EXACT []
is_a: COLLECTION:0000000 ! fish_collection_abbreviation

[Term]
id: COLLECTION:0000495
name: FURG
def: "Fundacao Universidade do Rio Grande, Depart. de Oceanografia, Rio Grande, Rio Grande do Sul, Brazil" [COLLECTION:curator]
synonym: "Fundacao Universidade do Rio Grande, Depart. de Oceanografia, Rio Grande, Rio Grande do Sul, Brazil" EXACT []
xref: urn\:lsid\:biocol.org\:col:35225
is_a: COLLECTION:0000000 ! fish_collection_abbreviation

[Term]
id: COLLECTION:0000496
name: FAU
def: "Florida Atlantic University, Boca Raton, Florida, U. S. A." [COLLECTION:curator]
synonym: "Florida Atlantic University, Boca Raton, Florida, U. S. A." EXACT []
xref: urn\:lsid\:biocol.org\:col:35226
is_a: COLLECTION:0000000 ! fish_collection_abbreviation

[Term]
id: COLLECTION:0000497
name: LGP
def: "Laboratorio de Genetica de Peixes, Departamento de Biologia, Universidade de Sao Paulo, Brazil. " [COLLECTION:curator]
synonym: "Laboratorio de Genetica de Peixes, Departamento de Biologia, Universidade de Sao Paulo, Brazil. " EXACT []
xref: urn\:lsid\:biocol.org\:col:35227
is_a: COLLECTION:0000000 ! fish_collection_abbreviation

[Term]
id: COLLECTION:0000498
name: KUVP
def: "Vertebrate Paleotology, Museum of Natural History, The University of Kansas, Lawrence, U.S.A" [COLLECTION:curator]
synonym: "Vertebrate Paleotology, Museum of Natural History, The University of Kansas, Lawrence, U.S.A" EXACT []
xref: urn\:lsid\:biocol.org\:col:35052
is_a: COLLECTION:0000000 ! fish_collection_abbreviation

[Term]
id: COLLECTION:0000499
name: ADR
def: "D. Armando Diaz Romeral's private collection, Cuence Spain " [COLLECTION:curator]
synonym: "D. Armando Diaz Romeral's private collection, Cuence Spain " EXACT []
xref: urn\:lsid\:biocol.org\:col:35228
is_a: COLLECTION:0000000 ! fish_collection_abbreviation

[Term]
id: COLLECTION:0000500
name: IPMC 
def: "Institut de Paleontologia 'Miquel Crusafont', Sadabell, Barcelona, Spain." [COLLECTION:curator]
synonym: "Institut de Paleontologia 'Miquel Crusafont', Sadabell, Barcelona, Spain." EXACT []
is_a: COLLECTION:0000000 ! fish_collection_abbreviation

[Term]
id: COLLECTION:0000501
name: NHM
def: " Natural History Museum, London, UK" [COLLECTION:curator]
synonym: " Natural History Museum, London, UK" EXACT []
xref: urn\:lsid\:biocol.org\:col:1004
is_a: COLLECTION:0000000 ! fish_collection_abbreviation

[Term]
id: COLLECTION:0000502
name: PC
def: "Private collection of G. Arratia" [COLLECTION:curator]
synonym: "Private collection of G. Arratia" EXACT []
xref: urn\:lsid\:biocol.org\:col:35229
is_a: COLLECTION:0000000 ! fish_collection_abbreviation

[Term]
id: COLLECTION:0000503
name: PF
def: "Field Museum of Natural History, Chicago" [COLLECTION:curator]
synonym: "Field Museum of Natural History, Chicago" EXACT []
is_a: COLLECTION:0000000 ! fish_collection_abbreviation

[Term]
id: COLLECTION:0000504
name: SDSM
def: "South Dakota School of Mines and Technology" [COLLECTION:curator]
synonym: "South Dakota School of Mines and Technology" EXACT []
is_a: COLLECTION:0000000 ! fish_collection_abbreviation

[Term]
id: COLLECTION:0000505
name: UC
def: "University of California, Berkeley" [COLLECTION:curator]
synonym: "University of California, Berkeley" EXACT []
is_a: COLLECTION:0000000 ! fish_collection_abbreviation

[Term]
id: COLLECTION:0000506
name: LH
def: "specimens from the Las Hoyas at the UAM provisionally housed collection" [COLLECTION:curator]
synonym: "specimens from the Las Hoyas at the UAM provisionally housed collection" EXACT []
is_a: COLLECTION:0000000 ! fish_collection_abbreviation

[Term]
id: COLLECTION:0000507
name: IEI
def: "Institut d'Estudis llerdencs, Lerida, Spain" [COLLECTION:curator]
synonym: "Institut d'Estudis llerdencs, Lerida, Spain" EXACT []
is_a: COLLECTION:0000000 ! fish_collection_abbreviation

[Term]
id: COLLECTION:0000508
name: LP
def: "specimens from the La Pedrera, Montsec, at the IEI collection" [COLLECTION:curator]
synonym: "specimens from the La Pedrera, Montsec, at the IEI collection" EXACT []
is_a: COLLECTION:0000000 ! fish_collection_abbreviation

[Term]
id: COLLECTION:0000509
name: MGB
def: "Museu de Geologia, Barcelona, Spain" [COLLECTION:curator]
synonym: "Museu de Geologia, Barcelona, Spain" EXACT []
xref: urn\:lsid\:biocol.org\:col:35230
is_a: COLLECTION:0000000 ! fish_collection_abbreviation

[Term]
id: COLLECTION:0000510
name: LBUCH
def: "Laboratorio de Biologia, Universidad de Chile, Santiago-Sur, Chile" [COLLECTION:curator]
synonym: "Laboratorio de Biologia, Universidad de Chile, Santiago-Sur, Chile" EXACT []
xref: urn\:lsid\:biocol.org\:col:35231
is_a: COLLECTION:0000000 ! fish_collection_abbreviation

[Term]
id: COLLECTION:0000511
name: NWAFC
def: "Northwest S. Alaska Fisheries Center, Seattle, WA, USA" [COLLECTION:curator]
synonym: "Northwest S. Alaska Fisheries Center, Seattle, WA, USA" EXACT []
xref: urn\:lsid\:biocol.org\:col:35232
is_a: COLLECTION:0000000 ! fish_collection_abbreviation

