format-version: 1.2
date: 01:04:2011 12:15
saved-by: Paul
auto-generated-by: OBO-Edit 2.000-beta53
default-namespace: mouse_pathology.ontology
namespace-id-rule: * MPATH:$sequence(3,0,999)$
remark: The Pathbase mouse pathology ontology provides a description of mutant and transgenic mouse pathology phenotypes and incorporates 643 known mouse pathologies hierarchically organised as "instances of" pathological processes. Questions, comments and suggestions for amendment should be sent to the Co-ordinator, Dr. Paul Schofield, Dept. of Anatomy, University of Cambridge (PS@mole.bio.cam.ac.uk).The ontology was developed by the Pathbase consortium (http://www.pathbase.net) funded under the European Commission's Fifth Framework programme, Contract number QLRI-CT-1999-00320.
autogenerated-by: Pathbase version 2.2

[Term]
id: MPATH:0
name: pathology_ontology
def: "pathology_ontology" [Pathbase: Curation]

[Term]
id: MPATH:1
name: cell and tissue damage
def: "The sum of morphological and functional disturbances induced by cell and tissue damage, either from intrinsic gene dysfunction or as a result of external factors." [Pathbase: Pathology Committee]
is_a: MPATH:603 ! pathological anatomical entity

[Term]
id: MPATH:10
name: gangrene
def: "Extensive necrosis from whatever cause, often following chronic ischemia." [ISBN:0781727286]
synonym: "Mortification" RELATED [Pathbase: Curation]
is_a: MPATH:4 ! necrosis

[Term]
id: MPATH:100
name: placental abnormality
def: "Defect in placental growth, differentiation of circulation; maternal or embryonic component." [Pathbase: Pathology Committee]
is_a: MPATH:86 ! organ specific developmental defect

[Term]
id: MPATH:101
name: glycogen cell defect
def: "Lack of, displacement of, or abnormality in function or growth of the glycogen cells." [Pathbase: Curation]
is_a: MPATH:100 ! placental abnormality

[Term]
id: MPATH:102
name: labyrinth zone defect
def: "Defect in size, cellular composition, function or organisation of the labyrinthine zone of the placenta." [Pathbase: Pathology Committee]
is_a: MPATH:100 ! placental abnormality

[Term]
id: MPATH:103
name: placental vascular defect
def: "Any defect in the maternal or embryonic placental circulation." [Pathbase: Curation]
is_a: MPATH:100 ! placental abnormality

[Term]
id: MPATH:104
name: spongiotrophoblast defect
def: "Defect in size, cellular composition, function or organisation of the spongiotrophoblast zone of the placenta." [Pathbase: Curation]
is_a: MPATH:100 ! placental abnormality

[Term]
id: MPATH:105
name: circulatory disorder
def: "Lesions leading to or consequent on failure of, or atypical movement of, blood throughout the body." [Pathbase: Pathology Committee]
is_a: MPATH:603 ! pathological anatomical entity

[Term]
id: MPATH:106
name: fluid accumulation
def: "Abnormal accumulation of fluid; blood or lymph." [Pathbase: Curation]
is_a: MPATH:105 ! circulatory disorder

[Term]
id: MPATH:107
name: congestion
def: "Presence of an abnormal amount of fluid (but especially of blood) in the vessels or passages of a part or organ." [Pathbase: Pathology Committee]
is_a: MPATH:106 ! fluid accumulation

[Term]
id: MPATH:108
name: disseminated intravascular coagulation
def: "A syndrome consequent to uncontrolled activation of blood clotting factors leading to disseminated platelet lysis, and fibrin deposition, ultimately leading to bleeding and necrosis as a consequence of inhibition of fibrin polymerisation by degradation products." [ISBN:0781727286]
comment: Diagnosed by microthrombi in many organs.
synonym: "DIC" RELATED [Pathbase: Curation]
is_a: MPATH:105 ! circulatory disorder

[Term]
id: MPATH:109
name: edema
def: "An accumulation of an excessive amount of watery fluid in cells or intercellular tissues." [Pathbase: Curation]
is_a: MPATH:106 ! fluid accumulation

[Term]
id: MPATH:11
name: hemorrhagic necrosis
def: "Necrosis associated with local hemorrhage." [ISBN:0781727286]
is_a: MPATH:4 ! necrosis

[Term]
id: MPATH:110
name: embolus
def: "A plug formed from a variety of materials occluding a vessel or tube." [Pathbase: Pathology Committee]
is_a: MPATH:105 ! circulatory disorder

[Term]
id: MPATH:111
name: air embolism
def: "An bubble of air occluding flow through a blood or lymphatic vessel." [Pathbase: Curation]
is_a: MPATH:110 ! embolus

[Term]
id: MPATH:112
name: amniotic fluid embolism
def: "Occlusion of vessels caused by entry of amniotic fluid, cell and debris into the maternal circulation." [Pathbase: Curation]
is_a: MPATH:110 ! embolus

[Term]
id: MPATH:113
name: atrial embolism
def: "Occlusion of the outflow tract of the right atrium by a thrombus." [Pathbase: Curation]
is_a: MPATH:110 ! embolus

[Term]
id: MPATH:114
name: bone marrow embolism
def: "Occlusion of vessels caused by entry of bone marrow, often fatty debris into the circulation. Usually following trauma." [Pathbase: Pathology Committee]
is_a: MPATH:110 ! embolus

[Term]
id: MPATH:115
name: fat embolism
def: "Occlusion of vessels caused by entry of lipid or fatty cells into the circulation. Usually following trauma." [Pathbase: Curation]
is_a: MPATH:110 ! embolus

[Term]
id: MPATH:116
name: pulmonary embolism
def: "Occlusion of pulmonary vessels by an embolus." [Pathbase: Curation]
is_a: MPATH:110 ! embolus

[Term]
id: MPATH:117
name: skin embolism
def: "Occlusion of vessels, usually small arterioles in the dermis by various emboli." [Pathbase: Curation]
is_a: MPATH:110 ! embolus

[Term]
id: MPATH:118
name: systemic embolism
def: "Production of systemic vessel occlusion by emboli released from the left side of the heart, or the aorta." [Pathbase: Pathology Committee]
is_a: MPATH:110 ! embolus

[Term]
id: MPATH:119
name: hemorrhage and non-specified extravasation
def: "Abnormal release of whole blood or the cellular component from the circulation." [Pathbase: Curation]
is_a: MPATH:105 ! circulatory disorder

[Term]
id: MPATH:12
name: liquefactive necrosis
def: "Soft or fluid tissue remains of a circumscribed area of necrosis digested by proteolytic enzymes." [ISBN:0781727286]
is_a: MPATH:4 ! necrosis

[Term]
id: MPATH:120
name: ecchymosis
def: "A red/purple patch caused by extravasation of blood into the skin. Larger than petechiae." [ISBN:0781727286]
comment: May also be used for any organ, although more generally used with respect to the skin.
is_a: MPATH:119 ! hemorrhage and non-specified extravasation

[Term]
id: MPATH:121
name: hematoma
def: "A localised deposition of clotted or partially clotted extravasated blood." [ISBN:0781727286]
synonym: "Bruise" RELATED [Pathbase: Curation]
is_a: MPATH:119 ! hemorrhage and non-specified extravasation

[Term]
id: MPATH:122
name: petechia
def: "Small hemorrhagic spots in the skin caused by blood vessel breakdown." [ISBN:0781727286]
comment: Usually used with reference to the skin but can be used in the context of other organs.
is_a: MPATH:119 ! hemorrhage and non-specified extravasation

[Term]
id: MPATH:123
name: purpura
def: "Purple and variously colored lesions caused by extensive haemorrhage into the skin through ecchymoses/petechia." [ISBN:0781727286]
is_a: MPATH:119 ! hemorrhage and non-specified extravasation

[Term]
id: MPATH:124
name: infarct
def: "An area of necrosis resulting from a sudden cessation of arterial or venous blood supply." [Pathbase: Pathology Committee]
is_a: MPATH:105 ! circulatory disorder

[Term]
id: MPATH:125
name: thrombosis
def: "Presence of an occluding or mural thrombus in a blood vessel." [Pathbase: Curation]
is_a: MPATH:105 ! circulatory disorder

[Term]
id: MPATH:126
name: growth and differentiation defect
def: "Defects in growth (changes in proliferation or mass) and differentiation of cells tissues or organs." [Pathbase: Pathology Committee]
is_a: MPATH:603 ! pathological anatomical entity

[Term]
id: MPATH:127
name: atrophy
def: "A reduction in size of organs or tissues as a result of cell death, loss of cellularity of whatever cause, reduced cellular proliferation or decreased cellular volume." [Pathbase: Pathology Committee]
is_a: MPATH:604 ! defective growth and differentiation process

[Term]
id: MPATH:128
name: intra-epithelial neoplasia
def: "Non-invasive changes characterized by alteration in the size, shape and organization of the cellular components of an epithelial tissue. Do not confuse with developmental dysplasia MPATH:64." [Journal: Ward; J.M. ( 2002) J Toxicol. Pathol. 15; 123-128]
comment: This term has been previously used as a synonym for pre-malignant dysplasia or carcinoma in situ and is now to be preferred.
synonym: "intra-epithelial lesion" RELATED [Pathbase: Curation]
is_a: MPATH:556 ! potentially cancerous lesions

[Term]
id: MPATH:129
name: epithelial dysplasia
def: "epithelial dysplasia" [Pathbase: Pathology Committee]
comment: obsolete due to renaming of preneoplastic dysplasias and Intraepithelial neoplasias Use MPATH:128.
is_obsolete: true

[Term]
id: MPATH:13
name: piecemeal necrosis
def: "Sensu; hepaticobiliary system. Loss and degeneration of hepatocytes at the portal-lobular interface producing a moth-eaten irregular appearance. Piecemeal necrosis is associated with a lymphocytic infiltrate." [ISBN:0781727286]
is_a: MPATH:4 ! necrosis

[Term]
id: MPATH:130
name: mild intra-epithelial neoplasia
def: "Mild non-invasive changes in cell morphology and tissue architecture confined to the epithelium alone." [Journal: Ward; J.M. ( 2002) J Toxicol. Pathol. 15; 123-128]
synonym: "IENI" RELATED [Pathbase: Curation]
synonym: "low grade intraepithelial lesion" RELATED [Pathbase: Curation]
synonym: "mild epithelial dysplasia." RELATED [Pathbase: Curation]
is_a: MPATH:128 ! intra-epithelial neoplasia
created_by: George Gkoutos

[Term]
id: MPATH:131
name: moderate intra-epithelial epithelial neoplasia
def: "Moderate non-invasive changes in cell morphology and tissue architecture confined to the epithelium alone." [Journal: Ward; J.M. ( 2002) J Toxicol. Pathol. 15; 123-128]
synonym: "high grade intraepithelial lesion" RELATED [Pathbase: Curation]
synonym: "IENII" RELATED [Pathbase: Curation]
synonym: "moderate epithelial dysplasia" RELATED [Pathbase: Curation]
is_a: MPATH:128 ! intra-epithelial neoplasia
created_by: George Gkoutos

[Term]
id: MPATH:132
name: severe intra-epithelial neoplasia
def: "Severe non-invasive malignancy associated changes in cell morphology and tissue architecture confined to the epithelium alone." [Journal: Ward; J.M. ( 2002) J Toxicol. Pathol. 15; 123-128]
comment: Carcinoma in situ may be used in some systems as a synonym.
synonym: "carcinoma in situ" RELATED [Pathbase: Curation]
synonym: "high grade intra-epithelial lesion" RELATED [Pathbase: Curation]
synonym: "IENIII" RELATED [Pathbase: Curation]
synonym: "severe epithelial dysplasia" RELATED [Pathbase: Curation]
is_a: MPATH:128 ! intra-epithelial neoplasia
created_by: George Gkoutos

[Term]
id: MPATH:133
name: hypoplasia
def: "Small organ or structure; failure to develop to normal size." [Pathbase: Pathology Committee]
synonym: "Developmental hypoplasia" RELATED [Pathbase: Curation]
is_a: MPATH:604 ! defective growth and differentiation process
created_by: George Gkoutos

[Term]
id: MPATH:134
name: hyperplasia
def: "An increase in cell numbers in comparison to normal as a consequence of increased cell proliferation. Non -neoplastic process." [Pathbase: Pathology Committee]
is_a: MPATH:604 ! defective growth and differentiation process
created_by: George Gkoutos

[Term]
id: MPATH:135
name: epithelial and stromal hyperplasia
def: "Abnormal proliferation of epithelial and stromal cells." [Pathbase: Pathology Committee]
is_a: MPATH:602 ! hyperplastic tissue
created_by: George Gkoutos

[Term]
id: MPATH:136
name: fibroepithelial polyp
def: "A polypoid outgrowth of both epidermis and dermal fibrovascular tissue." [ISBN:0781727286]
synonym: "skin tag" RELATED [Pathbase: Curation]
is_a: MPATH:138 ! epithelial hyperplasia
created_by: George Gkoutos

[Term]
id: MPATH:137
name: fibroglandular hyperplasia
def: "Benign proliferation of glandular epithelium accompanied by proliferation of fibroblastic stroma." [Pathbase: Curation]
is_a: MPATH:135 ! epithelial and stromal hyperplasia
created_by: George Gkoutos

[Term]
id: MPATH:138
name: epithelial hyperplasia
def: "Abnormal proliferation of epithelial cells and epithelial components." [Pathbase: Pathology Committee]
is_a: MPATH:602 ! hyperplastic tissue
created_by: George Gkoutos

[Term]
id: MPATH:139
name: goblet cell hyperplasia
def: "Benign proliferation of goblet cells." [Pathbase: Curation]
is_a: MPATH:138 ! epithelial hyperplasia
created_by: George Gkoutos

[Term]
id: MPATH:14
name: process of degenerative change
def: "A pathological process of loss or degradation of function, or structural integrity, of a tissue, organ or cell." [Pathbase: Pathology Committee]
is_a: MPATH:597 ! cell and tissue damage process
created_by: George Gkoutos

[Term]
id: MPATH:140
name: hyperplastic polyp
def: "A benign polyp, usually in the colon, showing hyperplasia." [ISBN:0781727286]
is_a: MPATH:491 ! polyp
created_by: George Gkoutos

[Term]
id: MPATH:141
name: inflammatory polyp
def: "A projecting mass of granulation tissue which may become covered by regenerating epithelium." [ISBN:0781727286]
synonym: "pseudopolyp" RELATED [Pathbase: Curation]
is_a: MPATH:491 ! polyp
created_by: George Gkoutos

[Term]
id: MPATH:142
name: intraductal hyperplasia
def: "Benign hyperplasia of the ducts of the mammary gland. Ducts exhibit more than the usual two layer epithelium (inner cuboidal to columnar cells; outer layer of myoepithelium) without cytological atypia." [PMID:10713680]
is_a: MPATH:138 ! epithelial hyperplasia
created_by: George Gkoutos

[Term]
id: MPATH:143
name: microglandular hyperplasia
def: "Benign proliferation of glandular epithelia, eg. Endocervical glands. Consists of tightly packed glandular or tubular units, which vary in size, lined by a flattened-to-cuboidal epithelium." [ISBN:0781727286]
synonym: "microglandular adenosis" RELATED [Pathbase: Curation]
is_a: MPATH:138 ! epithelial hyperplasia
created_by: George Gkoutos

[Term]
id: MPATH:144
name: myoepithelial hyperplasia
def: "Benign proliferation of glandular myoepithelial cells." [Pathbase: Curation]
is_a: MPATH:138 ! epithelial hyperplasia
created_by: George Gkoutos

[Term]
id: MPATH:145
name: fat cell hyperplasia
def: "Benign proliferation of adipose tissue." [Pathbase: Pathology Committee]
is_a: MPATH:602 ! hyperplastic tissue
created_by: George Gkoutos

[Term]
id: MPATH:146
name: histiocytosis
def: "Benign proliferation of histiocytes." [Pathbase: Pathology Committee]
is_a: MPATH:602 ! hyperplastic tissue
created_by: George Gkoutos

[Term]
id: MPATH:147
name: lymphoid hyperplasia
def: "Benign enlargement of lymphoid tissues." [Pathbase: Pathology Committee]
synonym: "lymphoid hypertrophy" RELATED [Pathbase: Curation]
is_a: MPATH:602 ! hyperplastic tissue
created_by: George Gkoutos

[Term]
id: MPATH:148
name: mesothelial hyperplasia
def: "Benign proliferation of mesothelial cells lining body cavities presenting as small solid cell clusters or multiple layers with columnar morphology and delicate eosinophilic cytoplasm." [Pathbase: Mohr]
synonym: "mesothelioma" RELATED [Pathbase: Curation]
is_a: MPATH:602 ! hyperplastic tissue
created_by: George Gkoutos

[Term]
id: MPATH:149
name: squamous hyperplasia
def: "Benign proliferation of epidermal cells with hyperkeratosis. Variable growth pattern, regular to papillary (exophytic squamous cell hyperplasia)." [Pathbase: Pathology Committee]
synonym: "epidermal hyperplasia." RELATED [Pathbase: Curation]
synonym: "squamous cell hyperplasia" RELATED [Pathbase: Curation]
is_a: MPATH:602 ! hyperplastic tissue
created_by: George Gkoutos

[Term]
id: MPATH:15
name: general degenerative process
def: "Change of tissue to a lower state of integrity or less functional form, as in heart failure." [Pathbase: Pathology Committee]
is_a: MPATH:14 ! process of degenerative change
created_by: George Gkoutos

[Term]
id: MPATH:150
name: acanthosis
def: "Hyperplasia of the Malpighian layer (prickle cell) of the epidermis." [ISBN:0781727286]
is_a: MPATH:149 ! squamous hyperplasia
created_by: George Gkoutos

[Term]
id: MPATH:151
name: actinic keratosis
def: "Discrete, flat or elevated, verrucous, keratotic lesions. Epidermal changes are characterized by acanthosis, parakeratosis, and dyskeratoses. Dysplastic change is present and the keratinocytes vary in size and shape. Associated with UV exposure in humans. Not defined in mice to date." [Pathbase: Pathology Committee]
is_a: MPATH:149 ! squamous hyperplasia
is_a: MPATH:556 ! potentially cancerous lesions
created_by: George Gkoutos

[Term]
id: MPATH:152
name: basal cell hyperplasia
def: "Benign proliferation of the basal layer cells of the skin." [Pathbase: Curation]
is_a: MPATH:149 ! squamous hyperplasia
created_by: George Gkoutos

[Term]
id: MPATH:153
name: hypergranulosis
def: "Increased thickness of the granular layer of a stratified squamous epithelium, associated with hyperorthokeratosis." [Pathbase: Pathology Committee]
is_a: MPATH:149 ! squamous hyperplasia
created_by: George Gkoutos

[Term]
id: MPATH:154
name: hyperkeratosis
def: "Thickening of the surface layers (stratum corneum) in the skin or other stratified squamous epithelium. Cf. ortho- and para-keratosis." [Pathbase: Pathology Committee]
synonym: "cornification" RELATED [Pathbase: Curation]
synonym: "hyperorthokeratosis" RELATED [Pathbase: Curation]
synonym: "hyperparakeratosis" RELATED [Pathbase: Curation]
is_a: MPATH:149 ! squamous hyperplasia
created_by: George Gkoutos

[Term]
id: MPATH:155
name: orthokeratosis
def: "Thickening of the anuclear cell layer limited to the stratum corneum, as in a stratified squamous epithelium." [Pathbase: Pathology Committee]
is_a: MPATH:154 ! hyperkeratosis
created_by: George Gkoutos

[Term]
id: MPATH:156
name: parakeratosis
def: "Thickening of the surface cell layer of a stratified squamous epithelium with retention of nuclei in the cells of the stratum corneum." [Pathbase: Pathology Committee]
is_a: MPATH:154 ! hyperkeratosis
created_by: George Gkoutos

[Term]
id: MPATH:157
name: pseudoepithelioma/pseudocarcinoma
def: "Benign hyperplasia and down-growth of epidermal cells. Microscopically resembling well-differentiated squamous cell carcinoma." [ISBN:0781727286]
synonym: "pseudocarcinoma" RELATED [Pathbase: Curation]
synonym: "pseudocarcinomatous hyperplasia" RELATED [Pathbase: Curation]
synonym: "pseudoepitheliomatous hyperplasia" RELATED [Pathbase: Curation]
is_a: MPATH:149 ! squamous hyperplasia
created_by: George Gkoutos

[Term]
id: MPATH:158
name: seborrheic keratosis
def: "Superficial, benign, verrucous, often pigmented, greasy lesions consisting of proliferating epidermal cells, resembling basal cells, enclosing cornifying cysts." [ISBN:0781727286]
synonym: "Basal cell papilloma" RELATED [Pathbase: Curation]
synonym: "seborrheic verruca" RELATED [Pathbase: Curation]
is_a: MPATH:149 ! squamous hyperplasia
created_by: George Gkoutos

[Term]
id: MPATH:159
name: hypertrophy
def: "Increase in size or mass of a cell, tissue or organ without increase in cell proliferation. Cf. Hyperplasia MPATH: 133." [Pathbase: Pathology Committee]
is_a: MPATH:604 ! defective growth and differentiation process
created_by: George Gkoutos

[Term]
id: MPATH:16
name: myxoid/myxomatous degeneration
def: "A conversion of the connective tissues into a gelatinous or mucous substance." [ISBN:0781727286]
synonym: "Mucoid degeneration" RELATED [Pathbase: Curation]
synonym: "myxomatosis" RELATED [Pathbase: Curation]
is_a: MPATH:15 ! general degenerative process
created_by: George Gkoutos

[Term]
id: MPATH:160
name: metaplasia
def: "Abnormal transformation of an fully differentiated adult cell or tissue of one kind into a differentiated tissue of another kind. An adult instance of developmental transdifferentiation MPATH:85 Traditionally defined as a form of abnormal regeneration in which a type of cell different from that found normally in a given location is produced." [Pathbase: Pathology Committee]
is_a: MPATH:604 ! defective growth and differentiation process
created_by: George Gkoutos

[Term]
id: MPATH:161
name: cartilaginous metaplasia
def: "Metaplasia resulting in heterotopic formation of cartilage." [ISBN:0781727286]
is_a: MPATH:605 ! metaplastic tissue
created_by: George Gkoutos

[Term]
id: MPATH:162
name: epithelial metaplasia
def: "Metaplasia occurring within epithelia." [ISBN:0781727286]
is_a: MPATH:605 ! metaplastic tissue
created_by: George Gkoutos

[Term]
id: MPATH:163
name: apocrine metaplasia
def: "Alteration of acinar epithelium of, for example, mammary tissue to resemble apocrine glands." [ISBN:0781727286]
is_a: MPATH:162 ! epithelial metaplasia
created_by: George Gkoutos

[Term]
id: MPATH:164
name: gastric metaplasia
def: "Appearance of heterotopic gastric epithelium." [ISBN:0781727286]
is_a: MPATH:162 ! epithelial metaplasia
created_by: George Gkoutos

[Term]
id: MPATH:165
name: glandular metaplasia
def: "Development of heterotopic glandular epithelia." [ISBN:0781727286]
is_a: MPATH:162 ! epithelial metaplasia
created_by: George Gkoutos

[Term]
id: MPATH:166
name: goblet cell metaplasia
def: "Metaplasia resulting in formation of mucus secreting goblet cells." [ISBN:0781727286]
is_a: MPATH:162 ! epithelial metaplasia
created_by: George Gkoutos

[Term]
id: MPATH:167
name: intestinal metaplasia
def: "Appearance of heterotopic intestinal epithelium." [ISBN:0781727286]
is_a: MPATH:162 ! epithelial metaplasia
created_by: George Gkoutos

[Term]
id: MPATH:168
name: lipomatous metaplasia
def: "Metaplasia resulting in formation of fat cells." [ISBN:0781727286]
is_a: MPATH:605 ! metaplastic tissue
created_by: George Gkoutos

[Term]
id: MPATH:169
name: nephrogenic metaplasia
def: ".A rare benign neoplasm of the mucosa of the urinary bladder or the urethra, consisting of tubular structures resembling those of the nephron." [ISBN:0781727286]
synonym: "nephrogenic adenoma" RELATED [Pathbase: Curation]
is_a: MPATH:162 ! epithelial metaplasia
created_by: George Gkoutos

[Term]
id: MPATH:17
name: subcellular defect
def: "Defect of a subcellular structure or organelle." [Pathbase: Pathology Committee]
is_a: MPATH:1 ! cell and tissue damage
created_by: George Gkoutos

[Term]
id: MPATH:170
name: oncocytic metaplasia
def: "Appearance of oncocytic cells in for example an epithelium or tumor." [ISBN:0781727286]
comment: An oncocyte is an acidophilic cell containing numerous mitochondria - an oxophil cell.
is_a: MPATH:162 ! epithelial metaplasia
created_by: George Gkoutos

[Term]
id: MPATH:171
name: squamous metaplasia
def: "Change of a glandular or mucosal epithelium into squamous epithelium." [ISBN:0781727286]
is_a: MPATH:162 ! epithelial metaplasia
created_by: George Gkoutos

[Term]
id: MPATH:172
name: transitional cell metaplasia
def: "Metaplastic response of the transitional epithelium, for example in the bladder to give squamous metaplasia and glandular metaplasia for example." [ISBN:0781727286]
is_a: MPATH:162 ! epithelial metaplasia
created_by: George Gkoutos

[Term]
id: MPATH:173
name: myeloid metaplasia
def: "A progressive disease of the bone marrow where neoplastic bone marrow stem cells lodge and grow at sites outside the bone marrow." [ISBN:0781727286]
is_a: MPATH:512 ! myeloproliferative disease
created_by: George Gkoutos

[Term]
id: MPATH:174
name: osseous metaplasia
def: "Metaplasia resulting in formation of bone." [ISBN:0781727286]
synonym: "ectopic bone" BROAD []
is_a: MPATH:605 ! metaplastic tissue
created_by: George Gkoutos

[Term]
id: MPATH:175
name: healing and repair process
def: "The process, normal or abnormal, of damage repair or wound closure." [Pathbase: Pathology Committee]
is_a: MPATH:596 ! pathological process
created_by: George Gkoutos

[Term]
id: MPATH:176
name: connective tissue replacement
def: "Replacement of connective tissue by fibro-fatty deposits and scar tissue." [Pathbase: Curation]
is_a: MPATH:175 ! healing and repair process
created_by: George Gkoutos

[Term]
id: MPATH:177
name: angiogenesis
def: "Aberrant process of blood vessel formation and the subsequent remodeling process; does not refer to the initial establishment of the vascular network by vasculogenesis." [Pathbase: Curation]
is_a: MPATH:176 ! connective tissue replacement
created_by: George Gkoutos

[Term]
id: MPATH:178
name: extracellular matrix deposition
def: "Abnormal deposition of extracellular matrix proteins or other components." [Pathbase: Curation]
is_a: MPATH:176 ! connective tissue replacement
created_by: George Gkoutos

[Term]
id: MPATH:179
name: fibrin deposition
def: "Deposition of fibrin." [Pathbase: Curation]
is_a: MPATH:176 ! connective tissue replacement
created_by: George Gkoutos

[Term]
id: MPATH:18
name: cytoskeletal defect
def: "Defect in the structure or function of the cytoskeleton." [Pathbase: Pathology Committee]
is_a: MPATH:17 ! subcellular defect
created_by: George Gkoutos

[Term]
id: MPATH:180
name: fibroblast proliferation
def: "Abnormal or reactive proliferation of fibroblasts." [Pathbase: Curation]
is_a: MPATH:176 ! connective tissue replacement
created_by: George Gkoutos

[Term]
id: MPATH:181
name: fibrosis
def: "Reactive formation of fibrous tissue." [Pathbase: Curation]
is_a: MPATH:176 ! connective tissue replacement
created_by: George Gkoutos

[Term]
id: MPATH:182
name: gliosis
def: "Proliferation of astrocytes in an area of damage in the brain or spinal cord." [Pathbase: Curation]
is_a: MPATH:176 ! connective tissue replacement
created_by: George Gkoutos

[Term]
id: MPATH:183
name: granulation tissue
def: "Newly formed connective (vascular or fibrous)tissue caused by inflammation or healing (repair) processes. Microscopically consists of capillaries fibroblastic cells and inflammatory cells." [Pathbase: Pathology Committee]
is_a: MPATH:607 ! healing and repair structure
created_by: George Gkoutos

[Term]
id: MPATH:184
name: sclerosis
def: "Any pathological thickening or hardening of a tissue." [Pathbase: Curation]
synonym: "Induration" RELATED [Pathbase: Curation]
is_a: MPATH:176 ! connective tissue replacement
created_by: George Gkoutos

[Term]
id: MPATH:185
name: parenchymal regeneration
def: "Post-injury regeneration of the functional tissue parenchyma. Eg. Liver." [Pathbase: Curation]
is_a: MPATH:175 ! healing and repair process
created_by: George Gkoutos

[Term]
id: MPATH:186
name: complete parenchymal regeneration
def: "Complete healing through parenchymal regeneration - no fibrosis." [Pathbase: Curation]
is_a: MPATH:185 ! parenchymal regeneration
created_by: George Gkoutos

[Term]
id: MPATH:187
name: incomplete parenchymal regeneration
def: "Incomplete healing usually accompanied by fibrosis." [Pathbase: Pathology Committee]
is_a: MPATH:185 ! parenchymal regeneration
created_by: George Gkoutos

[Term]
id: MPATH:188
name: immunopathology
def: "Conditions resulting from inappropriate activation or suppression of the immune or inflammatory response." [Pathbase: Pathology Committee]
is_a: MPATH:596 ! pathological process
created_by: George Gkoutos

[Term]
id: MPATH:189
name: hypersensitivity disease
def: "Immune response resulting in tissue injury." [Pathbase: Curation]
is_a: MPATH:188 ! immunopathology
created_by: George Gkoutos

[Term]
id: MPATH:19
name: endoplasmic reticulum defect
def: "Defect in the structure or function of the endoplasmic reticulum." [Pathbase: Pathology Committee]
is_a: MPATH:17 ! subcellular defect
created_by: George Gkoutos

[Term]
id: MPATH:190
name: type I hypersensitivity
def: "This is manifested by localized or generalized reaction that occurs immediately (minutes) after exposure to an antigen to which the person/animal was previously sensitized. It is IgE-mediated, and mast cell activation and degranulation are hallmarks." [ISBN:0781727286]
is_a: MPATH:189 ! hypersensitivity disease
created_by: George Gkoutos

[Term]
id: MPATH:191
name: type II hypersensitivity
def: "Caused by an antibody/antigen reaction: antibodies are directly or indirectly cytotoxic to antigens on cell surfaces or in connective tissues." [ISBN:0781727286]
comment: Most often involves IgG and IgM. Complement activation is usually involved.
is_a: MPATH:189 ! hypersensitivity disease
created_by: George Gkoutos

[Term]
id: MPATH:192
name: type III hypersensitivity
def: "Tissue injury mediated by immune complexes. Generally involves immune complexes formed in the blood via antibodies encountering circulating antigens. Immune complexes then deposit in tissues (especially blood vessels and glomeruli), induce complement activation, and result in tissue injury." [ISBN:0781727286]
is_a: MPATH:189 ! hypersensitivity disease
created_by: George Gkoutos

[Term]
id: MPATH:193
name: type IV hypersensitivity
def: "An antigen-elicited cellular immune reaction that results in tissue damage, but does not require Ab participation. The response is seen at the area of contact." [ISBN:0781727286]
is_a: MPATH:189 ! hypersensitivity disease
created_by: George Gkoutos

[Term]
id: MPATH:194
name: immune mediated disease
def: "Tissue response to inappropriate immune/inflammatory process." [Pathbase: Curation]
is_a: MPATH:188 ! immunopathology
created_by: George Gkoutos

[Term]
id: MPATH:195
name: arthritis
def: "Inflammation of a joint." [Pathbase: Curation]
is_a: MPATH:212 ! inflammation
created_by: George Gkoutos

[Term]
id: MPATH:196
name: dermatitis
def: "Inflammation of the skin." [Pathbase: Curation]
is_a: MPATH:212 ! inflammation
created_by: George Gkoutos

[Term]
id: MPATH:197
name: glomerulonephritis
def: "Renal disease characterised by diffuse inflammatory changes in glomeruli not in response to an infectious agent or treatment." [Pathbase: Curation]
is_a: MPATH:212 ! inflammation
created_by: George Gkoutos

[Term]
id: MPATH:198
name: immune mediated hemolytic anaemia
def: "An anemic/erythrocytopenic condition resulting from an increased rate of immune mediated erythrocyte destruction." [ISBN:0781727286]
is_a: MPATH:212 ! inflammation
created_by: George Gkoutos

[Term]
id: MPATH:199
name: immune mediated thrombocytopenia
def: "A condition resulting from an increased rate of immune mediated platelet destruction." [ISBN:0781727286]
is_a: MPATH:212 ! inflammation
created_by: George Gkoutos

[Term]
id: MPATH:2
name: cell death
def: "Complete and irreversible cessation of metabolic activity." [Pathbase: Pathology Committee]
is_a: MPATH:597 ! cell and tissue damage process
created_by: George Gkoutos

[Term]
id: MPATH:20
name: golgi defect
def: "Defect in the structure or function of the golgi apparatus." [Pathbase: Pathology Committee]
is_a: MPATH:17 ! subcellular defect
created_by: George Gkoutos

[Term]
id: MPATH:200
name: myositis
def: "Inflammation of a muscle." [Pathbase: Curation]
synonym: "Initis" RELATED [Pathbase: Curation]
is_a: MPATH:212 ! inflammation
created_by: George Gkoutos

[Term]
id: MPATH:201
name: vasculitis
def: "Inflammation of a blood vessel." [Pathbase: Pathology Committee]
synonym: "angiitis" RELATED [Pathbase: Curation]
synonym: "arteritis" RELATED [Pathbase: Curation]
synonym: "lymphangiitis" RELATED [Pathbase: Curation]
synonym: "phlebitis" RELATED [Pathbase: Curation]
is_a: MPATH:212 ! inflammation
created_by: George Gkoutos

[Term]
id: MPATH:202
name: immunodeficiency disease
def: "Defective immune response; can be primary due to defect in immune system or secondary/acquired due to disease." [Pathbase: Curation]
is_a: MPATH:188 ! immunopathology
created_by: George Gkoutos

[Term]
id: MPATH:203
name: general immunodeficiency disease
def: "general immunodeficiency disease" [Pathbase: Curation]
comment: obsolete. Subsumed into MPATH:202
is_obsolete: true

[Term]
id: MPATH:204
name: chronic/recurrent inflammatory disease
def: "chronic/recurrent inflammatory disease" [Pathbase: Curation]
comment: obsolete. Subsumed into MPATH: 214.
is_obsolete: true

[Term]
id: MPATH:205
name: immunodeficiency associated infection
def: "Infection with bacteria, viruses or fungi subsequent to immunodeficiency." [Pathbase: Pathology Committee]
is_obsolete: true

[Term]
id: MPATH:206
name: primary immunodeficiency disease
def: "Disease due to primary molecular or cellular defect in the immune system or its development." [Pathbase: Curation]
is_a: MPATH:202 ! immunodeficiency disease
created_by: George Gkoutos

[Term]
id: MPATH:207
name: immunodeficiency - lymphoid defect
def: "Primary defect in the lymphoid arm of the immune system." [Pathbase: Curation]
is_a: MPATH:206 ! primary immunodeficiency disease
created_by: George Gkoutos

[Term]
id: MPATH:208
name: immunodeficiency - myeloid/phagocytic defect
def: "Primary defect in the myeloid arm of the immune system." [Pathbase: Curation]
is_a: MPATH:206 ! primary immunodeficiency disease
created_by: George Gkoutos

[Term]
id: MPATH:209
name: secondary immunodeficiency disease
def: "Defect in the immune system subsequent to external injury, infection, ablation or deficiency." [Pathbase: Curation]
is_a: MPATH:202 ! immunodeficiency disease
created_by: George Gkoutos

[Term]
id: MPATH:21
name: lysosomal defect
def: "Defect in the structure or function of the lysosomes." [Pathbase: Curation]
is_a: MPATH:17 ! subcellular defect
created_by: George Gkoutos

[Term]
id: MPATH:210
name: acquired immunodeficiency
def: "Defect in the immune system subsequent to external injury, infection or ablation." [Pathbase: Curation]
is_a: MPATH:209 ! secondary immunodeficiency disease
created_by: George Gkoutos

[Term]
id: MPATH:211
name: failed transfer of maternal immunoglobulin
def: "Defect in the immune system subsequent to failure to attain passive immunity from maternal transfer of immunoglobulins." [Pathbase: Pathology Committee]
is_a: MPATH:209 ! secondary immunodeficiency disease
created_by: George Gkoutos

[Term]
id: MPATH:212
name: inflammation
def: "A tissue reaction to an internal or external injury." [Pathbase: Pathology Committee]
is_a: MPATH:194 ! immune mediated disease
created_by: George Gkoutos

[Term]
id: MPATH:213
name: acute inflammation
def: "Inflammation with a recent onset, characterised histologically by primarily granulocyte infiltration, edema and hyperemia." [Pathbase: Pathology Committee]
comment: The five classical signs of inflammation: Rubor, tumor, calor, dolor, functio laesa (Galen 300BC).
is_a: MPATH:212 ! inflammation
created_by: George Gkoutos

[Term]
id: MPATH:214
name: chronic inflammation
def: "Chronic inflammatory condition characterised by infiltration of primarily lymphocytes." [Pathbase: Pathology Committee]
is_a: MPATH:212 ! inflammation
created_by: George Gkoutos

[Term]
id: MPATH:215
name: granulomatous inflammation
def: "Nodular inflammatory reaction, containing compactly grouped epithelioid cells, giant cells, and other macrophages. The basic inflammatory unit is termed a granuloma." [ISBN:0781727286]
is_a: MPATH:212 ! inflammation
created_by: George Gkoutos

[Term]
id: MPATH:216
name: necrotic inflammation
def: "Acute inflammatory reaction in which the predominant histological change is rapid diffuse necrosis throughout the affected tissue." [ISBN:0781727286]
is_a: MPATH:212 ! inflammation
created_by: George Gkoutos

[Term]
id: MPATH:217
name: ulcerative inflammation
def: "Combination of inflammation, often suppurative or granulomatous, with ulceration." [ISBN:0781727286]
comment: Ulcers may be a component or inflammation. Use MPATH: Ulcer
is_obsolete: true

[Term]
id: MPATH:218
name: neoplasm
def: "A tumor resulting from abnormal and uncontrolled autonomous new cell growth (proliferation)that may be benign or malignant." [Pathbase: Pathology Committee]
is_a: MPATH:603 ! pathological anatomical entity
created_by: George Gkoutos

[Term]
id: MPATH:219
name: adnexal and skin appendage tumor
def: "Tumors of the skin, its constituent structures and glands including the mammary gland, apocrine and eccrine glands, hair follicles and associated structures." [Pathbase: Curation]
is_a: MPATH:218 ! neoplasm
created_by: George Gkoutos

[Term]
id: MPATH:22
name: mitochondrial defect
def: "Defect in the structure or function of the mitochondria." [Pathbase: Curation]
is_a: MPATH:17 ! subcellular defect
created_by: George Gkoutos

[Term]
id: MPATH:220
name: apocrine adenocarcinoma
def: "Carcinoma of the glandular epithelium of apocrine glands (M-8401/3)." [Pathbase: Pathology Committee]
is_a: MPATH:219 ! adnexal and skin appendage tumor
is_a: MPATH:268 ! adenocarcinoma
created_by: George Gkoutos

[Term]
id: MPATH:221
name: apocrine adenoma
def: "Benign neoplasm of the epithelium of apocrine glands (M-8401/0)." [Pathbase: Curation]
is_a: MPATH:219 ! adnexal and skin appendage tumor
is_a: MPATH:270 ! adenoma
created_by: George Gkoutos

[Term]
id: MPATH:222
name: ceruminous adenocarcinoma
def: "Malignant carcinoma of the ceruminous gland (M-8420/3)." [Pathbase: Curation]
is_a: MPATH:219 ! adnexal and skin appendage tumor
is_a: MPATH:268 ! adenocarcinoma
created_by: George Gkoutos

[Term]
id: MPATH:223
name: ceruminous adenoma
def: "Benign adenomatous neoplasia of the ceruminous glands of the external auditory meatus (M-8420/0)." [Pathbase: Curation]
is_a: MPATH:219 ! adnexal and skin appendage tumor
is_a: MPATH:270 ! adenoma

[Term]
id: MPATH:224
name: clear cell hidradenoma
def: "Tumor derived from eccrine sweat glands composed of clear glycogen rich cells. ( M-84020 )." [Pathbase: Curation]
synonym: "Eccrine acrospiroma" RELATED [Pathbase: Curation]
synonym: "nodular hidradenoma" RELATED [Pathbase: Curation]
is_a: MPATH:219 ! adnexal and skin appendage tumor
is_a: MPATH:270 ! adenoma

[Term]
id: MPATH:225
name: eccrine gland adenocarcinoma
def: "Malignant neoplasm of the eccrine gland (M-8413/3)." [Pathbase: Curation]
is_a: MPATH:219 ! adnexal and skin appendage tumor
is_a: MPATH:268 ! adenocarcinoma

[Term]
id: MPATH:226
name: eccrine gland adenoma
def: "Benign neoplasm of the eccrine gland (M-8408/0)." [:Papillary adenoma]
is_a: MPATH:219 ! adnexal and skin appendage tumor
is_a: MPATH:270 ! adenoma

[Term]
id: MPATH:227
name: eccrine papillary adenoma
def: "Papillary form of eccrine sweat gland adenoma. (M -8408/0)." [Pathbase: Pathology Committee]
synonym: "benign neoplasm of the eccrine gland, papillary form" RELATED [Pathbase: Curation]
synonym: "Papillary adenoma" RELATED [Pathbase: Curation]
is_a: MPATH:219 ! adnexal and skin appendage tumor
is_a: MPATH:270 ! adenoma

[Term]
id: MPATH:228
name: papillary hidradenoma
def: "Benign apocrine sweat gland tumor (8405/0)." [Pathbase: Curation]
synonym: "Hidradenoma papilliferum" RELATED [Pathbase: Curation]
is_a: MPATH:219 ! adnexal and skin appendage tumor
is_a: MPATH:270 ! adenoma

[Term]
id: MPATH:229
name: sebaceous adenocarcinoma
def: "Malignant neoplasm of the sebaceous cells - rare areas of differentiation, severe nuclear atypia (M-8410/3)." [Pathbase: Curation]
synonym: "sebaceous carcinoma" RELATED [Pathbase: Curation]
is_a: MPATH:219 ! adnexal and skin appendage tumor
is_a: MPATH:268 ! adenocarcinoma

[Term]
id: MPATH:23
name: peroxysomal defect
def: "Defect in the structure or function of the peroxysomes." [Pathbase: Curation]
is_a: MPATH:17 ! subcellular defect

[Term]
id: MPATH:230
name: sebaceous adenoma
def: "Adenoma of sebaceous cells; regular architecture of gland not mantained. Large numbers of immature germinative cells present. Mitoses. (M-8410/0)." [Pathbase: Curation]
synonym: "Epithelioma" RELATED [Pathbase: Curation]
is_a: MPATH:219 ! adnexal and skin appendage tumor
is_a: MPATH:270 ! adenoma

[Term]
id: MPATH:231
name: syringoma
def: "A benign, often multiple, sometimes eruptive neoplasm of the sweat gland ducts composed of very small round cysts. (M-8407/0)." [Pathbase: Curation]
is_a: MPATH:219 ! adnexal and skin appendage tumor

[Term]
id: MPATH:232
name: trichoepithelioma
def: "Multiple small benign nodules derived from basal cells of hair follicles enclosing small cornified cell containing cysts. (M-8100/0)." [URL:http\://emice.nci.nih.gov/emice/mouse_models/organ_models/skin_models]
synonym: "benign" RELATED [Pathbase: Curation]
synonym: "Epithelioma adenoides cysticum" RELATED [Pathbase: Curation]
synonym: "hair follicle tumor" RELATED [Pathbase: Curation]
is_a: MPATH:575 ! basaloid follicular neoplasms

[Term]
id: MPATH:233
name: basal cell tumor
def: "Well circumscribed tumor of the basal cells of the epidermis. Rare mitotic figures, benign. (M8147/0)." [Pathbase: Pathology Committee]
synonym: "basal cell adenoma" RELATED [Pathbase: Curation]
synonym: "Benign basal cell tumor" RELATED [Pathbase: Curation]
is_a: MPATH:219 ! adnexal and skin appendage tumor
is_a: MPATH:270 ! adenoma

[Term]
id: MPATH:234
name: basal cell carcinoma
def: "Malignant neoplasm of the basal cells of the epidermis with local invasion. (M-8090/3)." [URL:http\://emice.nci.nih.gov/emice/mouse_models/organ_models/skin_models]
is_a: MPATH:549 ! carcinoma
is_a: MPATH:575 ! basaloid follicular neoplasms

[Term]
id: MPATH:235
name: blood vessel tumor
def: "Tumor of venous or arterial vessels or capillaries." [Pathbase: Pathology Committee]
is_a: MPATH:218 ! neoplasm

[Term]
id: MPATH:236
name: angiofibroma
def: ".A benign neoplasm of fibrous tissue in which there are multiple large and small dilated vascular channels ( M9160/0)." [Pathbase: Curation]
synonym: "Telangiectatic fibroma" RELATED [Pathbase: Curation]
is_a: MPATH:235 ! blood vessel tumor

[Term]
id: MPATH:237
name: angiokeratoma
def: "An intradermal capillary telangiectasis with hyperkeratosis and acanthosis (M-9141/0)." [Pathbase: Curation]
synonym: "keratoangioma" RELATED [Pathbase: Curation]
synonym: "telangiectasia verrucosa" RELATED [Pathbase: Curation]
synonym: "telangiectatic wart" RELATED [Pathbase: Curation]
is_a: MPATH:235 ! blood vessel tumor

[Term]
id: MPATH:238
name: hemangioblastoma
def: "A benign neoplasm frequently arising in the cerebellum composed of capillary vessel forming endothelial cells and stromal cells. (M-9161/1)." [Pathbase: Pathology Committee]
synonym: "Angioblastoma" RELATED [Pathbase: Curation]
is_a: MPATH:235 ! blood vessel tumor

[Term]
id: MPATH:239
name: hemangioendothelioma
def: "hemangioendothelioma" [Pathbase: Curation]
comment: obsolete Use Hemangioma MPATH: 240
is_obsolete: true

[Term]
id: MPATH:24
name: plasma membrane defect
def: "Defect in the structure or function of the plasma membrane." [Pathbase: Curation]
is_a: MPATH:17 ! subcellular defect

[Term]
id: MPATH:240
name: hemangioma
def: "Neoplasm derived from endothelial cells. May be of capillary or cavernous type with large vascular channels. (M-9130/0 + M-9120/0 respectively)." [PMID:8569146]
synonym: "Angioendothelioma." RELATED [Pathbase: Curation]
synonym: "Hemangioendothelioma, benign" RELATED [Pathbase: Curation]
is_a: MPATH:235 ! blood vessel tumor

[Term]
id: MPATH:241
name: hemangiopericytoma
def: "A vascular, usually benign, neoplasm composed of round and spindle cells derived from the pericytes and surround endothelium-lined vessels. (M-9150/0/1/3)." [Pathbase: Pathology Committee]
synonym: "Pericytoma" RELATED [Pathbase: Curation]
is_a: MPATH:235 ! blood vessel tumor

[Term]
id: MPATH:242
name: hemangiosarcoma
def: "Malignant neoplasm derived from pluripotential mesenchymal stem cells or endothelial cells of blood vessels. (M-9120/3)." [PMID:8569146]
synonym: "hemangioendothelioma malignant, angiosarcoma" RELATED [Pathbase: Curation]
synonym: "hemangioendothelioma malignant." RELATED [Pathbase: Curation]
synonym: "Hemangioma malignant" RELATED [Pathbase: Curation]
is_a: MPATH:235 ! blood vessel tumor
is_a: MPATH:551 ! sarcoma

[Term]
id: MPATH:243
name: central nervous system tumor
def: "Neoplasm of the neurones, glia or meninges of the CNS." [Pathbase: Curation]
is_a: MPATH:218 ! neoplasm

[Term]
id: MPATH:244
name: astrocytoma
def: "Glioma derived from astrocytes, both benign and malignant forms (M-9400/3)." [ISBN-13:9783794515530]
comment: Also see comments in Weiss, W.W, Israel, M. Cobbs, C., et al. (2002) Oncogene 21, 7453-7463.
synonym: "Astrocytic glioma" RELATED [Pathbase: Curation]
synonym: "astroglioma" RELATED [Pathbase: Curation]
is_a: MPATH:249 ! glioma

[Term]
id: MPATH:245
name: choroid plexus carcinoma
def: "Malignant neoplasm derived from the epithelial cells of the choroid plexus. (M-9390/3)." [ISBN-13:9783794515530]
is_a: MPATH:549 ! carcinoma
is_a: MPATH:565 ! tumors of neurepithelial tissue

[Term]
id: MPATH:246
name: choroid plexus papilloma
def: "Benign neoplasm derived from the epithelial cells of the choroid plexus. (M-9390/0)." [ISBN-13:9783794515530]
is_a: MPATH:264 ! fibroepithelial tumor
is_a: MPATH:565 ! tumors of neurepithelial tissue

[Term]
id: MPATH:247
name: ependymoma
def: "Neoplasm derived from the ependymal cells lining the ventricles and aqueduct of the brain and the central canal of the spinal cord. Malignant or benign. (M-9391/3)." [ISBN-13:9783794515530]
comment: Also see general scheme in Weiss, W.W, Israel, M. Cobbs, C., et al. (2002) Oncogene 21, 7453-7463.
is_a: MPATH:249 ! glioma

[Term]
id: MPATH:248
name: ependymoma malignant
def: "ependymoma malignant" [Pathbase: Curation]
comment: obsolete -subsumed into MPATH:247
is_obsolete: true

[Term]
id: MPATH:249
name: glioma
def: "Neoplasm derived from astrocytes and oligodendrocytes. (M-9380/3, M-9440/3)." [ISBN-13:9783794515530]
comment: Also see comments in: Weiss, W.W, Israel, M. Cobbs, C., et al. (2002) Oncogene 21, 7453-7463.
is_a: MPATH:565 ! tumors of neurepithelial tissue

[Term]
id: MPATH:25
name: tissue specific degenerative process
def: "Degenerative process characteristic of a particular tissue." [Pathbase: Curation]
is_a: MPATH:14 ! process of degenerative change

[Term]
id: MPATH:250
name: medulloblastoma
def: "Neoplasm derived from the primitive neurectodermal cells of the cerebellum. (M-9470/3). May be considered by some authorities a synonym of PNET in the CNS." [ISBN-13:9783794515530]
comment: Also see Weiss, W.W, Israel, M. Cobbs, C., et al. (2002) Oncogene 21, 7453-7463.
is_a: MPATH:373 ! CNS progenitor tumor

[Term]
id: MPATH:251
name: meningioma
def: "meningioma" [ISBN-13:9783794515530]
comment: Benign or malignant neoplasm derived from the meninges. (M-9530/0).
synonym: "Sarcoma, meningeal ( sensu malignant tumor)" RELATED [Pathbase: Curation]
is_a: MPATH:566 ! tumors of the meninges

[Term]
id: MPATH:252
name: oligodendroglioma
def: "Benign or malignant neoplasm derived form oligodendrocytes (M-9450/3)." [ISBN-13:9783794515530]
comment: Also see Weiss, W.W, Israel, M. Cobbs, C., et al. (2002) Oncogene 21, 7453-7463.
synonym: "glioma oligodendritic, malignant" RELATED [Pathbase: Curation]
synonym: "Glioma, oligodendritic, benign" RELATED [Pathbase: Curation]
is_a: MPATH:249 ! glioma

[Term]
id: MPATH:253
name: sub-ependymoma
def: "Neoplasm derived from sub-ependymal astrocytes (M-9383/1)." [ISBN-13:9783794515530]
comment: Also see general scheme in Weiss, W.W, Israel, M. Cobbs, C., et al. (2002) Oncogene 21, 7453-7463.
is_a: MPATH:249 ! glioma

[Term]
id: MPATH:254
name: complex tumor
def: "Tumors showing mutiple histological componants/differentiation." [Pathbase: Pathology Committee]
is_a: MPATH:218 ! neoplasm

[Term]
id: MPATH:255
name: adenoacanthoma
def: "Mixed tumor of glandular epithelia with squamous and glandular diffferentiation. (M-8570/3)." [Pathbase: Curation]
synonym: "adenoid squamous cell carcinoma" RELATED [Pathbase: Curation]
is_a: MPATH:254 ! complex tumor

[Term]
id: MPATH:256
name: carcinosarcoma
def: "Possible origin from smooth muscle cells or pluripotential embryonic mesenchymal cells. May show up to three cellular componants including carcinoma and sarcoma type appearances. (M-8980/3)." [Pathbase: Curation]
is_a: MPATH:254 ! complex tumor
is_a: MPATH:549 ! carcinoma
is_a: MPATH:551 ! sarcoma

[Term]
id: MPATH:257
name: craniopharyngioma
def: "A benign or malignant neoplasm, which may be cystic, developing from the epithelium of Rathke`s pouch and occuring with or close to the pituitary gland. (M-9350/1)." [Pathbase: Pathology Committee]
synonym: "Erdheim tumor" RELATED [Pathbase: Curation]
synonym: "Pituitary adamantinoma" RELATED [Pathbase: Curation]
synonym: "pituitary ameloblastoma" RELATED [Pathbase: Curation]
synonym: "Rathke pouch tumor" RELATED [Pathbase: Curation]
synonym: "suprasellar cyst" RELATED [Pathbase: Curation]
is_a: MPATH:254 ! complex tumor

[Term]
id: MPATH:258
name: mesodermal mixed tumor
def: "Neoplasm showing multiple phases, derived from mesoderm (M-8951/3)." [Pathbase: Curation]
is_a: MPATH:254 ! complex tumor

[Term]
id: MPATH:259
name: mucoepidermoid carcinoma
def: "Most commonly a salivary gland carcinoma of low grade malignancy composed of mucous, epidermoid, and intermediate cells. (M-8430/3)." [Pathbase: Curation]
is_a: MPATH:254 ! complex tumor

[Term]
id: MPATH:26
name: alopecia
def: "Absence of hair or loss of hair." [ISBN:0781727286]
is_a: MPATH:25 ! tissue specific degenerative process

[Term]
id: MPATH:260
name: mullerian mixed tumor
def: "Neoplasm usually of the uterus or adnexae containing carcinomatous and sarcomatous elements, sometimes with third or fourth components. (M-8950/3)." [Pathbase: Pathology Committee]
is_a: MPATH:254 ! complex tumor

[Term]
id: MPATH:261
name: nephroblastoma
def: "Embryonal tumor thought to be derived from metanephric blastema. Mono, bi or triphasic, sometimes with heterotypic differentiation. (M-8960/3)." [Pathbase: Pathology Committee]
synonym: "nephroma" RELATED [Pathbase: Curation]
is_a: MPATH:254 ! complex tumor

[Term]
id: MPATH:262
name: pulmonary blastoma
def: "A biphasic tumor containing a primitive epithelial component, that may resemble well-differentiated fetal adenocarcinoma and a primitive mesenchymal stroma, which occasionally has foci of osteosarcoma, chondrosarcoma or rhadomyosarcoma. (M-8972/3)." [Pathbase: Pathology Committee]
is_a: MPATH:254 ! complex tumor

[Term]
id: MPATH:263
name: rhabdoid sarcoma
def: "Sarcomatous tumors, presenting a wide histological, ultrastructural, and immunocytochemical spectrum. M-8963/3." [Pathbase: Curation]
synonym: "Malignant rhabdoid tumor" RELATED [Pathbase: Curation]
is_a: MPATH:254 ! complex tumor
is_a: MPATH:551 ! sarcoma

[Term]
id: MPATH:264
name: fibroepithelial tumor
def: "Tumors with epithelial invaginations/linings and a fibrillary and fibrocytic stroma. (M-9000 - M-9030)." [Pathbase: Curation]
is_a: MPATH:218 ! neoplasm

[Term]
id: MPATH:265
name: adenofibroma
def: "A benign neoplasm composed of glandular and fibrous tissues, predominantly glandular. (M-9013/0)." [Pathbase: Curation]
synonym: "Cystadenofibroma" RELATED [Pathbase: Curation]
synonym: "papillary adenofibroma" RELATED [Pathbase: Curation]
is_a: MPATH:264 ! fibroepithelial tumor

[Term]
id: MPATH:266
name: fibroadenoma
def: "A benign neoplasm derived from glandular epithelium, in which there is a abundant stroma of proliferating fibroblasts and connective tissue. (M-9010/0)." [Pathbase: Curation]
is_a: MPATH:264 ! fibroepithelial tumor

[Term]
id: MPATH:267
name: glandular tumor
def: "Neoplasms derived from glandular epithelial cells." [Pathbase: Curation]
is_a: MPATH:218 ! neoplasm

[Term]
id: MPATH:268
name: adenocarcinoma
def: "Malignant neoplasm of epithelial cells in glandular or glandlike pattern. (M-8140/3)." [Pathbase: Curation]
is_a: MPATH:267 ! glandular tumor
is_a: MPATH:549 ! carcinoma

[Term]
id: MPATH:269
name: adenocarcinoma in situ
def: "A noninvasive abnormal proliferation of glands believed to precede the appearance of invasive adenocarcinoma. (M-8140/2)." [Pathbase: Pathology Committee]
is_a: MPATH:268 ! adenocarcinoma
is_a: MPATH:556 ! potentially cancerous lesions

[Term]
id: MPATH:27
name: arthrosis
def: "Changes characterized by erosion of articular cartilage, either primary or secondary to trauma or other conditions. Not primarily an inflammatory process." [ISBN:0781727286]
synonym: "Degenerative joint disease" RELATED [Pathbase: Curation]
synonym: "osteoarthrosis" RELATED [Pathbase: Curation]
is_a: MPATH:25 ! tissue specific degenerative process

[Term]
id: MPATH:270
name: adenoma
def: "A benign epithelial neoplasm in which the tumor cells may form glands or glandlike structures. In different instances this may remain a benign tumor or progress to malignancy." [Pathbase: Pathology Committee]
is_a: MPATH:267 ! glandular tumor
is_a: MPATH:556 ! potentially cancerous lesions

[Term]
id: MPATH:271
name: adenomatous polyposis coli
def: "Spontaneous intestinal adenoma formation. Polyps increase in number, causing symptoms of chronic colitis and potentially transform into adenocarcinoma. (M-8220/0)." [Pathbase: Curation]
is_a: MPATH:267 ! glandular tumor
is_a: MPATH:556 ! potentially cancerous lesions

[Term]
id: MPATH:272
name: bronchioloalveolar adenoma
def: "Benign epithelial neoplasm of the lung. (M-8140/1) 1.2.1.2 in MMHCC classification." [PMID:15059877]
synonym: "Bronchial adenoma" RELATED [Pathbase: Curation]
synonym: "Bronchial adenoma, BA adenoma" RELATED [Pathbase: Curation]
xref: URL: http\://emice.nci.nih.gov/mouse_models/organ_models/lung_models/murinecancer/tumorclass
is_a: MPATH:270 ! adenoma

[Term]
id: MPATH:273
name: bronchioloalveolar carcinoma
def: "Malignant epithelial neoplasm of the lung. (M-8250/3) 1.2.3.2, 1.2.3.5 of MMHCC classification." [PMID:15059877]
synonym: "Bronchioloalveolar adenocarcinoma" RELATED [Pathbase: Curation]
synonym: "Bronchioloalveolar adenocarcinoma, bronchioalveolar carcinoma" RELATED [Pathbase: Curation]
xref: URL: http\://emice.nci.nih.gov/mouse_models/organ_models/lung_models/murinecancer/tumorclass
is_a: MPATH:268 ! adenocarcinoma
is_a: MPATH:549 ! carcinoma

[Term]
id: MPATH:274
name: clear cell adenocarcinoma
def: "An adenocarcinoma characterised by the presence of varying combinations of clear and hobnail-shaped tumor cells. (M-8310/3)." [Pathbase: Curation]
is_a: MPATH:268 ! adenocarcinoma

[Term]
id: MPATH:275
name: comedocarcinoma
def: "Form of carcinoma of the breast or other organ in which plugs of necrotic malignant cells are present in the ducts. (M -8501/3)." [Pathbase: Pathology Committee]
is_a: MPATH:267 ! glandular tumor
is_a: MPATH:549 ! carcinoma

[Term]
id: MPATH:276
name: cystadenocarcinoma
def: "Malignant neoplasm derived from glandular epithelium, in which cystic accumulations of retained secretions are formed. (M-8440/3)." [Pathbase: Curation]
is_a: MPATH:268 ! adenocarcinoma

[Term]
id: MPATH:277
name: cystadenoma
def: "A benign neoplasm derived from glandular epithelium, in which cystic accumulations of retained secretions are formed. (M-8440/0)." [Pathbase: Pathology Committee]
is_a: MPATH:270 ! adenoma

[Term]
id: MPATH:278
name: follicular adenocarcinoma
def: "Originates in the follicular cells of thyroid follicles. Papillary, solid and follicular forms. (M- 8330/3)." [Pathbase: Curation]
synonym: "Follicular carcinoma" RELATED [Pathbase: Curation]
is_a: MPATH:268 ! adenocarcinoma

[Term]
id: MPATH:279
name: follicular adenoma
def: "Adenoma derived from the follicular cells of the thyroid follicles. Follicular, paipillary and solid forms. M- 8330/0." [Pathbase: Curation]
is_a: MPATH:270 ! adenoma

[Term]
id: MPATH:28
name: atherosclerosis
def: "Characterised by irregular lipid deposits in the wall of arteries, causing narrowing of their lumens and proceeding eventually to fibrosis and calcification." [Pathbase: Pathology Committee]
comment: Note that in mouse and rats the initial lesions are mostly in the medial layer while in human they occur in the intima.
is_a: MPATH:25 ! tissue specific degenerative process

[Term]
id: MPATH:280
name: Harderian gland adenoma
def: "Adenoma derived from acinar epithelium of the harderian gland. Papillary, cystic, cystic-papillary and acinar forms." [Pathbase: Pathology Committee]
is_a: MPATH:270 ! adenoma

[Term]
id: MPATH:281
name: Harderian gland carcinoma
def: "Malignant tumor derived form acinar epithelium of the Harderian gland." [Pathbase: Pathology Committee]
is_a: MPATH:267 ! glandular tumor
is_a: MPATH:549 ! carcinoma

[Term]
id: MPATH:282
name: infiltrating duct carcinoma
def: "Derived from the mammary ductal epithelium and penetrating the stroma (M-8500/3)." [Pathbase: Pathology Committee]
synonym: "duct adenocarcinoma" RELATED [Pathbase: Curation]
synonym: "ductal carcinoma" RELATED [Pathbase: Curation]
synonym: "Infiltrating ductal adenocarcinoma" RELATED [Pathbase: Curation]
is_a: MPATH:268 ! adenocarcinoma
is_a: MPATH:549 ! carcinoma

[Term]
id: MPATH:283
name: intraductal carcinoma
def: "In situ carcinoma of the mammary ductal epithelium. (M- 8500/2)." [Pathbase: Curation]
comment: Made obsolete by inclusion in MPATH: 486 Ductal intra-epithelial neoplasia
synonym: "Ductal carcinoma in situ" RELATED [Pathbase: Curation]
synonym: "intraductal adenocarcinoma, non-infiltrating" RELATED [Pathbase: Curation]
is_obsolete: true

[Term]
id: MPATH:284
name: intraductal papillary carcinoma
def: "Infiltrating tumor with papillary morphology derived from the breast epithelium (M-8503/3)." [Pathbase: Curation]
synonym: "Intraductal papillary adenocarcinoma" RELATED [Pathbase: Curation]
is_a: MPATH:267 ! glandular tumor
is_a: MPATH:549 ! carcinoma

[Term]
id: MPATH:285
name: intraductal papilloma
def: "Benign papilloma arising from ductal epithelium (M- 8503/0 )." [Pathbase: Curation]
synonym: "Duct adenoma" RELATED [Pathbase: Curation]
synonym: "ductal papilloma" RELATED [Pathbase: Curation]
is_a: MPATH:267 ! glandular tumor
is_a: MPATH:445 ! papilloma
relationship: part_of MPATH:286 ! intraductal papillomatosis

[Term]
id: MPATH:286
name: intraductal papillomatosis
def: "Diffuse multiple adenomatous papillomas derived from the ductal epithelium of the breast. (M- 8505/0)." [Pathbase: Curation]
synonym: "Diffuse intraductal papillomatosis" RELATED [Pathbase: Curation]
is_a: MPATH:267 ! glandular tumor

[Term]
id: MPATH:287
name: islet cell adenoma
def: "Usually pancreatic B cell derived tumors mostly producing insulin. (M- 8150/0)." [Pathbase: Curation]
synonym: "Adenoma, endocrine pancreas" RELATED [Pathbase: Curation]
synonym: "adenomatosis" RELATED [Pathbase: Curation]
synonym: "islet (pancreatic) cell tumor benign" RELATED [Pathbase: Curation]
is_a: MPATH:270 ! adenoma

[Term]
id: MPATH:288
name: islet cell carcinoma
def: "Rare tumor of the islets of Langerhans, most of which produce insulin. (M- 8150/3)." [Pathbase: Pathology Committee]
synonym: "Adenocarcinoma, endocrine pancreas" RELATED [Pathbase: Curation]
synonym: "islet cell tumor, malignant" RELATED [Pathbase: Curation]
is_a: MPATH:267 ! glandular tumor
is_a: MPATH:549 ! carcinoma

[Term]
id: MPATH:289
name: lobular carcinoma
def: "A form of breast adenocarcinoma derived from lobular cells. (M-8520/3)." [Pathbase: Curation]
synonym: "Lobular adenocarcinoma" RELATED [Pathbase: Curation]
synonym: "lobular infiltrating carcinoma" RELATED [Pathbase: Curation]
is_a: MPATH:267 ! glandular tumor
is_a: MPATH:549 ! carcinoma

[Term]
id: MPATH:29
name: cataract
def: "Opacity of the lens." [PMID:9309781]
is_a: MPATH:1 ! cell and tissue damage

[Term]
id: MPATH:290
name: lobular carcinoma in situ
def: "Non-infiltrating form of lobular adenocarcinoma derived from the ductal epithelium. (M-8520/2)." [ISBN:0781727286]
synonym: "mammary intra-epithelial neoplasia" RELATED [Pathbase: Curation]
is_a: MPATH:267 ! glandular tumor
is_a: MPATH:556 ! potentially cancerous lesions

[Term]
id: MPATH:291
name: medullary carcinoma
def: "Derived from calcitonin-producing cells (thyroid). In humans a type of carcinoma composed of epithelial elements with considerable lymphoid stroma (breast). Not yet reported in mice. (M-8510/3)." [Pathbase: Pathology Committee]
synonym: "Medullary adenocarcinoma" RELATED [Pathbase: Curation]
is_a: MPATH:267 ! glandular tumor
is_a: MPATH:549 ! carcinoma

[Term]
id: MPATH:292
name: mucinous cystadenocarcinoma
def: "Malignant neoplasm derived from a glandular epithelium, eg. Ovary. Consisting of a solid to cystic mass lined with cuboidal pleomorphic epithelial cells producing a mucinous material. (M- 8470/3)." [Pathbase: Pathology Committee]
is_a: MPATH:276 ! cystadenocarcinoma

[Term]
id: MPATH:293
name: mucinous cystadenoma
def: "A benign neoplasm derived from glandular epithelium, in which cystic accumulations of mucinous retained secretions are formed. (M-8470/0)." [Pathbase: Pathology Committee]
is_a: MPATH:270 ! adenoma

[Term]
id: MPATH:294
name: myoepithelioma
def: "Tumor originating in myoepithelial cells of exocrine glandular structures; for example mammary gland, salivary gland and preputial/clitoral glands. (M-8982/0)." [Pathbase: Pathology Committee]
synonym: "myoepithelial adenoma" RELATED [Pathbase: Curation]
is_a: MPATH:219 ! adnexal and skin appendage tumor
is_a: MPATH:270 ! adenoma

[Term]
id: MPATH:295
name: papillary adenocarcinoma
def: "A malignant neoplasm derived from a glandular epithelium, in which solid tumors show papillary structures projecting onto fibrovascular stroma. (M-8260/3)." [Pathbase: Pathology Committee]
is_a: MPATH:268 ! adenocarcinoma

[Term]
id: MPATH:296
name: papillary adenoma
def: "A benign neoplasm derived from a glandular epithelium, in which solid tumors show papillary structures projecting onto fibrovascular stroma. (M-8260/0)." [Pathbase: Pathology Committee]
is_a: MPATH:270 ! adenoma

[Term]
id: MPATH:297
name: papillary cystadenocarcinoma
def: "A malignant neoplasm derived from glandular epithelium, in which cysts contain folds or papillary projections into the lumen. (M-8450/3)." [Pathbase: Pathology Committee]
is_a: MPATH:276 ! cystadenocarcinoma

[Term]
id: MPATH:298
name: papillary cystadenoma
def: "A benign neoplasm derived from glandular epithelium, in which cysts contain folds or papillary projections into the lumen. (M-8450/0)." [Pathbase: Pathology Committee]
is_a: MPATH:270 ! adenoma

[Term]
id: MPATH:299
name: pinealoma
def: "Originating from differentiated cells of the pineal parenchyma. Not to be confused with human pinealoma (syn: germinoma) non-gonadal germ cell tumors found in the pineal believed to be atypical teratomas. May be benign or malignant. If ectopic teratomas/teratocarcinomas use MP322 or MP321. (M-9360/1)." [Pathbase: Pathology Committee]
is_a: MPATH:267 ! glandular tumor

[Term]
id: MPATH:3
name: apoptosis
def: "Energy dependent cell death induced by intrinsic genetic or developmental programme, or external stimuli such as addition or withdrawal of cytokines or trophic factors, radiation, chemotherapeutic agents etc. Characterised by cell shrinkage, increases in membrane permeability, endonucleolyis and nuclear fragmentation resulting in the formation of rapidly endocytosed apoptotic bodies." [Pathbase: Pathology Committee]
synonym: "programmed cell death" RELATED [Pathbase: Curation]
is_a: MPATH:2 ! cell death

[Term]
id: MPATH:30
name: cystic medial necrosis
def: "Loss of muscle fibers and elastin in the media of the aorta, with accumulation of mucopolysaccharide." [ISBN:0781727286]
synonym: "Erdheim disease" RELATED [Pathbase: Curation]
synonym: "media necrosis aortae idiopathica cystica" RELATED [Pathbase: Curation]
synonym: "media necrosis of the aorta" RELATED [Pathbase: Curation]
synonym: "Mucoid medial degeneration" RELATED [Pathbase: Curation]
is_a: MPATH:4 ! necrosis

[Term]
id: MPATH:300
name: pineoblastoma
def: "Malignant neoplasms which arise from pineoblasts, the primitive pineal stem cells. (M-9362/3)." [Pathbase: Pathology Committee]
synonym: "Mixed pineal tumor" RELATED [Pathbase: Curation]
synonym: "pineal parenchymal tumor of intermediate differentiation" RELATED [Pathbase: Curation]
synonym: "transitional pineal tumor" RELATED [Pathbase: Curation]
is_a: MPATH:267 ! glandular tumor

[Term]
id: MPATH:301
name: pineocytoma
def: "A tumor arising in the pineal gland that resembles normal pineal parenchyma. (M-9361/1)." [Pathbase: Curation]
is_a: MPATH:267 ! glandular tumor

[Term]
id: MPATH:302
name: pituicytoma
def: "Benign tumor derived from the pituicytes ( glial cells of neurohypophysis) (M-8272/0)." [Pathbase: Curation]
synonym: "pituitary adenoma" RELATED [Pathbase: Curation]
is_a: MPATH:270 ! adenoma

[Term]
id: MPATH:303
name: pseudomyxoma peritonei
def: "Tumor characterized by extensive spread of a mucin-secreting neoplasm along the peritoneal surfaces (M-8480/6)." [Pathbase: Curation]
is_a: MPATH:267 ! glandular tumor

[Term]
id: MPATH:304
name: serous adenocarcinoma
def: "Adenocarcinoma from a serous gland producing and containing serous proteinaceous secretions (M-8441/3)." [Pathbase: Pathology Committee]
is_a: MPATH:268 ! adenocarcinoma

[Term]
id: MPATH:305
name: serous cystadenoma
def: "Ovarian cystadenoma composed of cells similar to tubal epithelium (M-8441/0)." [Pathbase: Curation]
is_a: MPATH:270 ! adenoma

[Term]
id: MPATH:306
name: signet ring cell carcinoma
def: "Adenocarcinoma of signet ring type arising from exocrine cells of the gastric mucosa or enterocytes of intestinal mucosa. (M-8490/3)." [PMID:12612914]
synonym: "Signet ring cell adenocarcinoma" RELATED [Pathbase: Curation]
synonym: "signet ring cell carcinoma" RELATED [Pathbase: Curation]
is_a: MPATH:268 ! adenocarcinoma

[Term]
id: MPATH:307
name: thyroid C-cell adenoma
def: "Benign neoplasm derived from the calcitonin producing C-cells of the thyroid gland." [Pathbase: Curation]
synonym: "Adenoma, parafollicular cell" RELATED [Pathbase: Curation]
synonym: "tumor c-cell benign" RELATED [Pathbase: Curation]
is_a: MPATH:270 ! adenoma

[Term]
id: MPATH:308
name: thyroid C-cell carcinoma
def: "Malignant neoplasm derived from the calcitonin producing C-cells of the thyroid gland. (M-8510/3, M-8345/3)." [Pathbase: Curation]
synonym: "Medullary carcinoma, parafollicular cell" RELATED [Pathbase: Curation]
synonym: "tumor c-cell malignant" RELATED [Pathbase: Curation]
is_a: MPATH:267 ! glandular tumor
is_a: MPATH:549 ! carcinoma

[Term]
id: MPATH:309
name: gonadal tumor
def: "Germ cell and non-germ cell tumors of the testis and ovary." [Pathbase: Pathology Committee]
is_a: MPATH:218 ! neoplasm

[Term]
id: MPATH:31
name: emphysema
def: "Abnormal accumulation of air in the interstitial connective tissue of a structure. Sensu Lung: Pulmonary emphysema; characterised by abnormal increase in the size of air (alveolar) spaces distal to the terminal bronchiole with degenerative changes in their walls and reduction in their number." [ISBN:0781727286]
is_a: MPATH:25 ! tissue specific degenerative process

[Term]
id: MPATH:310
name: germ cell tumor
def: "Neoplasms derived from germ cells. May be gonadal or extragonadal and are derived from primordial germ cells." [Pathbase: Pathology Committee]
is_a: MPATH:309 ! gonadal tumor

[Term]
id: MPATH:311
name: dermoid cyst
def: "Cystic ovarian teratomas with different mature cell types (M-9084/3)." [Pathbase: Curation]
is_a: MPATH:254 ! complex tumor
is_a: MPATH:310 ! germ cell tumor
is_a: MPATH:549 ! carcinoma

[Term]
id: MPATH:312
name: dysgerminoma
def: "Undifferentiated germ cell tumor of the ovary composed of solid sheets of large polygonal cells with rim of clear cytoplasm (M-9060/3)." [Pathbase: Curation]
synonym: "Seminoma (sensu male)" RELATED [Pathbase: Curation]
is_a: MPATH:310 ! germ cell tumor

[Term]
id: MPATH:313
name: embryonal carcinoma
def: "Germ cell derived malignant neoplasm of the testis or ovary, composed of anaplastic cells with indistinct cellular borders and large ovoid, round, or bean-shaped nuclei that may have large nucleoli. (M-9070/3 )." [Pathbase: Curation]
is_a: MPATH:310 ! germ cell tumor
is_a: MPATH:549 ! carcinoma

[Term]
id: MPATH:314
name: endodermal sinus tumor
def: "Germ cell derived tumors resembling parietal or visceral yolk sac endoderm derivatives. Abundant eosinophilic matrix surrounding nests and cords of neoplastic cells. (M-9071-3)." [Pathbase: Pathology Committee]
synonym: "Yolk sac carcinoma" RELATED [Pathbase: Curation]
is_a: MPATH:310 ! germ cell tumor
is_a: MPATH:549 ! carcinoma

[Term]
id: MPATH:315
name: gonadoblastoma
def: "Gonadal neoplasms that consist of aggregates of germ cells and sex cord elements (M-9073/1)." [Pathbase: Curation]
synonym: "Gonocytoma" RELATED [Pathbase: Curation]
is_a: MPATH:310 ! germ cell tumor

[Term]
id: MPATH:316
name: mixed germ cell tumor
def: "Malignant neoplasm of the testis/ovary including various elements of germ cell tumors (M-9085/3)." [Pathbase: Curation]
synonym: "Mixed teratoma and seminoma" RELATED [Pathbase: Curation]
is_a: MPATH:254 ! complex tumor
is_a: MPATH:310 ! germ cell tumor

[Term]
id: MPATH:317
name: seminoma
def: "Tumor derived from spermatogenic cells resembling spermatogenia or spermatocytes. NOS ( M9061/3)." [Pathbase: Curation]
synonym: "dysgerminoma" RELATED [Pathbase: Curation]
synonym: "Germinoma, malignant" RELATED [Pathbase: Curation]
synonym: "spermatoblastoma" RELATED [Pathbase: Curation]
synonym: "spermatocytoma, malignant." RELATED [Pathbase: Curation]
is_a: MPATH:310 ! germ cell tumor

[Term]
id: MPATH:318
name: classical seminoma
def: "As MPATH:317, but not spermatocytic (M-9061/3)." [Pathbase: Curation]
is_a: MPATH:317 ! seminoma

[Term]
id: MPATH:319
name: spermatocytic seminoma
def: "Neoplasm of the testis usually found within the tubule. Some debate as to whether it is of germ cell origin in contrast to classical seminoma. Three types of cells are identified in spermatocytic seminomas: those with small, intermediate, and large nuclei in humans. (M-9063/3)." [:Walt; H.; Oosterhuis; J.W. and Stevens; L.C. (1993)  Int J Androl; 16; 267-271]
synonym: "Spermatoma" RELATED [Pathbase: Curation]
is_a: MPATH:317 ! seminoma

[Term]
id: MPATH:32
name: glaucoma
def: "Increase in the intraocular pressure." [Pathbase: Curation]
is_a: MPATH:25 ! tissue specific degenerative process

[Term]
id: MPATH:320
name: struma ovarii
def: "Rare ovarian tumor, regarded as monodermal teratoma, in which thyroid tissue has surpassed the other elements; occasionally associated with hyperthyroidism (M-9090/0)." [Pathbase: Curation]
is_a: MPATH:310 ! germ cell tumor
is_a: MPATH:549 ! carcinoma

[Term]
id: MPATH:321
name: teratocarcinoma
def: "Mixed germ cell neoplasm contaning elements of embryonal carcinoma and teratoma (M-9081/3)." [Pathbase: Curation]
is_a: MPATH:254 ! complex tumor
is_a: MPATH:310 ! germ cell tumor
is_a: MPATH:549 ! carcinoma

[Term]
id: MPATH:322
name: teratoma
def: "Generally benign germ cell derived tumors of male or female containing derivatives from all three germ layers with differentiation in the malignant form being poor. Malignant tumors are highly metatstatic. (M-9080/1)." [Pathbase: Pathology Committee]
is_a: MPATH:254 ! complex tumor
is_a: MPATH:310 ! germ cell tumor

[Term]
id: MPATH:323
name: gonadal somatic cell tumor
def: "Neoplasms derived from the non-germ cell derived tissues of the testis and ovary." [Pathbase: Curation]
is_a: MPATH:309 ! gonadal tumor

[Term]
id: MPATH:324
name: androblastoma
def: "obsolete use Sertoli cell tumor MPATH: 331." [Pathbase: Curation]
is_obsolete: true

[Term]
id: MPATH:325
name: fibrothecoma
def: "obsolete use thecoma MPATH:334." [Pathbase: Curation]
is_obsolete: true

[Term]
id: MPATH:326
name: granulosa cell tumor
def: ". Derived from sex cord stromal cells. In male thought to be Sertoli cells. (M- 8620/1)." [PMID:9789961]
synonym: "gynoblastoma (sensu malignant form in ovary)" RELATED [Pathbase: Curation]
synonym: "Tumor, sex cord stromal, benign, granulosa cell type" RELATED [Pathbase: Curation]
is_a: MPATH:323 ! gonadal somatic cell tumor

[Term]
id: MPATH:327
name: gynandroblastoma
def: "gynandroblastoma" [Pathbase: Curation]
comment: obsolete Use sertoli-leydig cell tumor MPATH 332
is_obsolete: true

[Term]
id: MPATH:328
name: leydig cell tumor
def: "Tumor derived from Leydig cells (M-8650/1)." [Mahler M; Sundberg JP ( 1997) Spontaneous Leydig cell tumors in inbred laboratory mice Lab Animal Science 47:148-52]
synonym: "Interstitial cell tumor, benign" RELATED [Pathbase: Curation]
synonym: "Leydig cell adenoma" RELATED [Pathbase: Curation]
is_a: MPATH:323 ! gonadal somatic cell tumor

[Term]
id: MPATH:329
name: luteal cell tumor
def: "Tumor derived from sex cords composed of highly luteinised cells with extensive pale granular cytoplasm. (M- 8610/0)." [Pathbase: Curation]
synonym: "luteinised granulosa cell tumor, benign. Gonadal sex cord stromal tumor, benign, luteoma type" RELATED [Pathbase: Curation]
synonym: "Luteoma" RELATED [Pathbase: Curation]
is_a: MPATH:323 ! gonadal somatic cell tumor

[Term]
id: MPATH:33
name: intracellular and extracellular accumulation
def: "Accumulation of substances within, on the surface of or between cells." [Pathbase: Pathology Committee]
is_a: MPATH:1 ! cell and tissue damage

[Term]
id: MPATH:330
name: ovarian stromal tumor
def: "Tumor consists of a mixture of granulosa, luteal thecal, Sertoli and stromal cells. (M-8590/1)." [Pathbase: Curation]
is_a: MPATH:254 ! complex tumor
is_a: MPATH:323 ! gonadal somatic cell tumor

[Term]
id: MPATH:331
name: sertoli cell tumor
def: "Tumor derived from sex cord/stromal cells; Sertoli cells and can occur in both testis and ovary. (M-8640/1)." [Pathbase: Pathology Committee]
synonym: "Androblastoma" RELATED [Pathbase: Curation]
synonym: "arrhenoblastoma" RELATED [Pathbase: Curation]
synonym: "gonadal stromal tumor" RELATED [Pathbase: Curation]
synonym: "sex cord stromal tumor" RELATED [Pathbase: Curation]
synonym: "sustentacluar tumor" RELATED [Pathbase: Curation]
is_a: MPATH:323 ! gonadal somatic cell tumor

[Term]
id: MPATH:332
name: sertoli-leydig cell tumor
def: "Tumor of the ovary or testis containing granulosa or theca cell elements with a tubular componant of Sertoli cell type and producing simultaneous androgenic and estrogenic effects. (M-8631/0)." [Pathbase: Pathology Committee]
synonym: "Gynandroblastoma" RELATED [Pathbase: Curation]
is_a: MPATH:323 ! gonadal somatic cell tumor

[Term]
id: MPATH:333
name: sex cord tumor
def: "sex cord tumor" [Pathbase: Curation]
comment: obsolete: Use more specific terms: MPATH: 334, 331, 329, 326
is_obsolete: true

[Term]
id: MPATH:334
name: thecoma
def: "Derived from sex cord stromal cells, spindle shaped cells arranged in whorls or interlacing bundles. (M- 8600/0)." [Pathbase: Curation]
synonym: "Fibrothecoma" RELATED [Pathbase: Curation]
synonym: "theca cell tumor" RELATED [Pathbase: Curation]
is_a: MPATH:323 ! gonadal somatic cell tumor

[Term]
id: MPATH:335
name: hematopoietic/lymphoid malignancies/disorder
def: "Proliferative disorders and malignancies of the lymphoid and non lymphoid haematopoietic lineages." [URL:http\://www.bloodjournal.org/cgi/content/full/100/1/238/DC1/2]
is_a: MPATH:218 ! neoplasm

[Term]
id: MPATH:336
name: leukaemia
def: "leukaemia" [Pathbase: Curation]
comment: obsolete folowing reclassification.
is_obsolete: true

[Term]
id: MPATH:337
name: erythroid leukaemia
def: "Leukaemia with at least 50% of nucleated erythroid cells infiltrating haematopoietic tissue." [PMID:12070033]
xref: URL:http\://www.bloodjournal.org/cgi/content/full/100/1/238/DC1/2
is_a: MPATH:496 ! Non-Lymphoid leukaemias

[Term]
id: MPATH:338
name: granulocytic leukaemia
def: "granulocytic leukaemia" [Pathbase: Curation]
comment: obsolete following reclassification see: MPATH505
is_obsolete: true

[Term]
id: MPATH:339
name: lymphatic leukaemia
def: "lymphatic leukaemia" [Pathbase: Curation]
is_obsolete: true

[Term]
id: MPATH:34
name: amyloid deposition
def: "Extracellular deposition of amyloid protein." [ISBN:0781727286]
comment: Any group of chemically diverse proteins that appears microscopically homogeneous, but is composed of linear non-branching aggregated fibrils aranged in sheets when see under the electron microscope.
synonym: "Amyloidosis" RELATED [Pathbase: Curation]
is_a: MPATH:33 ! intracellular and extracellular accumulation

[Term]
id: MPATH:340
name: megakaryocytic leukaemia
def: "Leukaemia with at least 50% of megakaryocytic cells infiltrating haematopoietic tissue." [PMID:12070033]
xref: URL:http\://www.bloodjournal.org/cgi/content/full/100/1/238/DC1/2
is_a: MPATH:496 ! Non-Lymphoid leukaemias

[Term]
id: MPATH:341
name: myelodysplastic disorder
def: "Haematopoietic proliferation with evidence of trilineage dysplasia. Less than 20% should be blasts." [PMID:12070033]
xref: URL:http\://www.bloodjournal.org/cgi/content/full/100/1/238/DC1/2
is_a: MPATH:508 ! myeloid dysplasias

[Term]
id: MPATH:342
name: myeloid leukaemia
def: "Leukaemias of the myeloid lineage." [PMID:12070033]
synonym: "granulocytic leukaemia" RELATED [Pathbase: Curation]
xref: URL:http\://www.bloodjournal.org/cgi/content/full/100/1/238/DC1/2
is_a: MPATH:496 ! Non-Lymphoid leukaemias

[Term]
id: MPATH:343
name: lymphoma
def: "lymphoma" [Pathbase: Curation]
comment: obsolete; divided between subtypes of MPATH516, MPATH535
is_obsolete: true

[Term]
id: MPATH:344
name: follicle center cell lymphoma
def: "follicle center cell lymphoma" [Pathbase: Curation]
comment: obsolete; see MPATH 522
is_obsolete: true

[Term]
id: MPATH:345
name: immunoblastic lymphoma
def: "immunoblastic lymphoma" [Pathbase: Curation]
comment: obsolete; see MPATH525
is_obsolete: true

[Term]
id: MPATH:346
name: autoimmune mediated disease
is_a: MPATH:194 ! immune mediated disease
created_by: George Gkoutos
creation_date: 2011-03-22T01:12:01Z

[Term]
id: MPATH:347
name: small lymphocytic lymphoma
def: "small lymphocytic lymphoma" [Pathbase: Curation]
comment: obsolete; see MPATH520
is_obsolete: true

[Term]
id: MPATH:348
name: thymic lymphoma
def: "thymic lymphoma" [Pathbase: Curation]
comment: obsolete
is_obsolete: true

[Term]
id: MPATH:349
name: mast cell tumor
def: "mast cell tumor" [Pathbase: Curation]
comment: obsolete; see MPATH507
is_obsolete: true

[Term]
id: MPATH:35
name: bile deposition
def: "Intra- or extracellular deposition of bile pigments and their metabolites." [Pathbase: Pathology Committee]
is_a: MPATH:613 ! pigmentation

[Term]
id: MPATH:350
name: mastocytoma
def: "mastocytoma" [Pathbase: Curation]
comment: obsolete. See MPATH507
is_obsolete: true

[Term]
id: MPATH:351
name: thymoma
def: "A neoplasm in the anterior mediastinum, originating from thymic tissue, usually benign, and frequently encapsulated; occasionally invasive, but metastases are rare; histologically, consists of any type of thymic epithelial cell as well as lymphocytes that are usually abundant. (M-8580/1)." [ISBN:0781727286]
is_a: MPATH:218 ! neoplasm

[Term]
id: MPATH:352
name: hepatic tumor
def: "Tumors of the liver and biliary apparatus." [Pathbase: Curation]
is_a: MPATH:218 ! neoplasm

[Term]
id: MPATH:353
name: hepatocellular adenoma
def: "Benign neoplasm derived from hepatocytes. (M- 8170/0)." [Pathbase: Curation]
synonym: "hepatic adenoma, benign, liver cell tumor, benign" RELATED [Pathbase: Curation]
synonym: "hepatoma, benign" RELATED [Pathbase: Curation]
synonym: "nodule type A" RELATED [Pathbase: Curation]
is_a: MPATH:270 ! adenoma
is_a: MPATH:352 ! hepatic tumor

[Term]
id: MPATH:354
name: cholangiocarcinoma
def: "Malignant tumor derived from the bile duct epithelium. (M8160/3)." [Pathbase: Pathology Committee]
is_a: MPATH:352 ! hepatic tumor
is_a: MPATH:549 ! carcinoma

[Term]
id: MPATH:355
name: cholangiofibroma
def: "Develops from cholangiofibrosis, fibrosis of the biliary ducts and is only potentially malignant." [Pathbase: Curation]
is_a: MPATH:352 ! hepatic tumor

[Term]
id: MPATH:356
name: hepatoblastoma
def: "Malignant neoplasm of the liver of unknown origin . Liver blastemal cells, neoplastic hepatocytes, oval cells and biliary epithelial cells have been proposed. (M- 8970/3)." [Pathbase: Curation]
synonym: "embryonal hepatoma" RELATED [Pathbase: Curation]
synonym: "tumor, mixed, poorly differentiated" RELATED [Pathbase: Curation]
is_a: MPATH:352 ! hepatic tumor

[Term]
id: MPATH:357
name: hepatocellular carcinoma
def: "Malignant tumor derived from hepatocytes. (M- 8170/3)." [Book: Bannasche; P and Zerban; H. Preneoplastic and neoplastic lesions of the rat iver. In; Pathology of neoplasia and preneoplasia in rodents; P. Bannasch and W. Goessner; Editors. 1997. Schattauer; Stuttgart. p. 18-63]
synonym: "carcinoma, trabecular" RELATED [Pathbase: Curation]
synonym: "carcinoma, trabecular (liver)" RELATED [Pathbase: Curation]
synonym: "hepatoma, malignant" RELATED [Pathbase: Curation]
synonym: "nodule type B" RELATED [Pathbase: Curation]
is_a: MPATH:352 ! hepatic tumor
is_a: MPATH:549 ! carcinoma

[Term]
id: MPATH:358
name: melanocytic tumor
def: "Tumors derived from melanocytes." [Pathbase: Pathology Committee]
is_a: MPATH:219 ! adnexal and skin appendage tumor

[Term]
id: MPATH:359
name: melanoma
def: "Tumor of neurectodermal origin, usually melanocytes, showing dense deposition of melanin granules, although amelanotic melanomas have been reported. (M-8720/3)." [Book: Klein-Szanto; A.J.; Neoplastic and preneoplastic lesions of the mouse skin; in Pathology of neoplasia and preneoplasia in rodents; P. Bannasch and W. Goessner; Editors. 1997. Schattauer; Stuttgart. p. 1-18]
synonym: "melanosarcoma" RELATED [Pathbase: Curation]
synonym: "melanosarcoma, malignant melanoma" RELATED [Pathbase: Curation]
xref: URL: http\://emice.nci.nih.gov/emice/mouse_models/organ_models/skin_models/malignant_melanoma#melanoma_table
is_a: MPATH:358 ! melanocytic tumor

[Term]
id: MPATH:36
name: calcium deposition
def: "Intra or extracellular deposition of calcium usually as calcium phosphate." [Pathbase: Curation]
is_a: MPATH:555 ! mineralisation

[Term]
id: MPATH:360
name: melanoma in situ
def: "A potentially malignant lesion, melanoma in situ is the first phase of growth of melanoma, in which it is still confined to the epithelial domain (epidermis and adnexa) and has not passed through the basement membrane. (M-8720/2)." [Pathbase: Pathology Committee]
synonym: "level I melanoma" RELATED [Pathbase: Curation]
is_a: MPATH:358 ! melanocytic tumor
is_a: MPATH:556 ! potentially cancerous lesions

[Term]
id: MPATH:361
name: naevus
def: "Local lesion of the skin, often colored by hyperpigmentation or increased vascularity. May be predominantly epidermal, adnexal, melanocytic, vascular, or mesodermal, or a compound overgrowth of these tissues. Not necessarily pre-malignant. (M-8720/0)." [Pathbase: Pathology Committee]
synonym: "mole (sensu melanocytic nevus)" RELATED [Pathbase: Curation]
is_a: MPATH:358 ! melanocytic tumor

[Term]
id: MPATH:362
name: mesonephroma
def: "Benign or malignant neoplasm of the ovary and corpus uteri, thought to originate in mesonephric structures. (M-9110/3)." [Pathbase: Pathology Committee]
synonym: "mesonephric adenocarcinoma, wolffian duct carcinoma, mesonephroid tumor" RELATED [Pathbase: Curation]
is_a: MPATH:268 ! adenocarcinoma

[Term]
id: MPATH:363
name: mesonephric tumor
def: "Tumor beleived to be derived from mesonephric remnants. (M-8310/3)." [Pathbase: Curation]
synonym: "mesonephroid clear cell adenocarcinoma" RELATED [Pathbase: Curation]
is_a: MPATH:362 ! mesonephroma

[Term]
id: MPATH:364
name: mesothelial tumor
def: "mesothelial tumor" [Pathbase: Curation]
comment: obsolete; subsumed into MPATH365
is_obsolete: true

[Term]
id: MPATH:365
name: mesothelioma
def: "Benign or malignant neoplasm derived from the lining cells of the pleura and peritoneum, composed of spindle cells or fibrous tissue which may enclose glandlike spaces lined by cuboidal cells. Epithelioid, fibrous, cystis, papillary, and sarcomatoid variants. (M- 9050/3)." [Pathbase: Curation]
is_a: MPATH:218 ! neoplasm

[Term]
id: MPATH:366
name: neuroendocrine tumor
def: "Neoplasms derived from the neuroendocrine system." [Pathbase: Curation]
is_a: MPATH:218 ! neoplasm

[Term]
id: MPATH:367
name: carcinoid tumor
def: "Carcinoid tumors are of neuroendocrine origin and derived from primitive stem cells. Found predominantly in the lung and gut they are capable of secreting a large range of substances and have a number of histological subtypes. May resemble but are distinct from small cell lung carcinoma in the lung. (M-8240/3)." [Pathbase: Pathology Committee]
is_a: MPATH:366 ! neuroendocrine tumor

[Term]
id: MPATH:368
name: endocrine adenocarcinoma
def: "obsolete." [Pathbase: Curation]
is_obsolete: true

[Term]
id: MPATH:369
name: endocrine adenoma
def: "endocrine adenoma" [Pathbase: Curation]
is_obsolete: true

[Term]
id: MPATH:37
name: ceroid deposition
def: "Intracellular deposition of golden or yellow-brown pigment, acid fast and insoluble in lipid solvents. Believed to be a type of lipofuscin." [Pathbase: Pathology Committee]
is_a: MPATH:613 ! pigmentation

[Term]
id: MPATH:370
name: primitive neurectodermal tumor
def: "Primitive neuroectodermal tumors (PNET) are neoplasms derived from primitive neural stem cells either in the CNS or the periphery . These are small-cell, malignant embryonal tumors showing divergent differentiation of variable degree along neuronal, glial, or rarely mesenchymal lines. (M-9473/3, M-9364/3)." [ISBN-13:9783794515530]
synonym: "PNET" RELATED [Pathbase: Curation]
is_a: MPATH:373 ! CNS progenitor tumor
is_a: MPATH:570 ! peripheral nervous system tumors

[Term]
id: MPATH:371
name: small cell carcinoma
def: "Neuroendocrine cell derived anaplastic carcinoma composed of small cells, usually of the lung producing a variety of peptide hormones. (M-8041/3). 1.2.3.4 of MMHCC classification." [PMID:15059877]
comment: see: Meuwissen, R., Linn, S.C., Linnoila, R.I. et al. (2003) Induction of small cell lung cancer by somatic inactivation of both Trp53 and Rb1 in a conditional mouse model. Cancer cell, 4: 181-189. AND Calbo, J., Meuwissen, R., van Montfort, E. et al. (2005) Genotype-phenotype relationships in a mouse model for human small-cell lung cancer. Cold Spring Harbor symposia on quantitative biology, 70: 225-232. AND Meuwissen, R. and Berns, A. (2005) Mouse models for human lung cancer. Genes & development, 19: 643-664.
synonym: "oat cell carcinoma" RELATED [Pathbase: Curation]
xref: URL: http\://emice.nci.nih.gov/mouse_models/organ_models/lung_models/murinecancer/tumorclass
is_a: MPATH:366 ! neuroendocrine tumor
is_a: MPATH:549 ! carcinoma

[Term]
id: MPATH:372
name: tumorlet
def: "Small disseminated foci of atypical bronchiolar epithelial hyperplasia. Benign. (M- 8040/1)." [Pathbase: Pathology Committee]
is_a: MPATH:366 ! neuroendocrine tumor

[Term]
id: MPATH:373
name: CNS progenitor tumor
def: "Neoplasms derived from neuroepithelial precursors." [Pathbase: Pathology Committee]
comment: Renamed from neuroepitheliomatous tumor, to reflect primitive origins of this class of tumor.
is_a: MPATH:565 ! tumors of neurepithelial tissue

[Term]
id: MPATH:374
name: esthesioneuroblastoma
def: "A neoplasm of immature, poorly differentiated neuronal cells believed to arise from neuroepithelial precursors in the olfactory epithelium. (M- 9522/3)." [Pathbase: Curation]
synonym: "neuroblastoma, olfactory" RELATED [Pathbase: Curation]
synonym: "neuroepithelial carcinoma" RELATED [Pathbase: Curation]
synonym: "neuroepithelioma, olfactory" RELATED [Pathbase: Curation]
is_a: MPATH:373 ! CNS progenitor tumor

[Term]
id: MPATH:375
name: ganglioneuroma
def: "A benign neoplasm composed of mature ganglionic neurons scattered singly or in clumps within a relatively abundant and dense stroma of neurofibrils and collagenous fibers. (M-9490/0)." [Pathbase: Pathology Committee]
is_a: MPATH:570 ! peripheral nervous system tumors

[Term]
id: MPATH:376
name: neuroblastoma
def: "A malignant neoplasm characterized by immature, poorly differentiated nerve cells of embryonic type. (M-9500/3)." [ISBN-13:9783794515530]
is_a: MPATH:373 ! CNS progenitor tumor

[Term]
id: MPATH:377
name: pheochromocytoma
def: "A catecholamine-secreting tumor arising from the chromaffin cells of the sympathetic nervous system or adrenal medulla. May be benign or malignant. [See MPATH 398]. (M- 8510/3)." [Pathbase: Pathology Committee]
is_a: MPATH:366 ! neuroendocrine tumor

[Term]
id: MPATH:378
name: retinoblastoma
def: "Malignant juvenile neoplasm of the eye derived from primitive retinal precursor cells. (M- 9510/3)." [Pathbase: Curation]
is_a: MPATH:373 ! CNS progenitor tumor

[Term]
id: MPATH:379
name: odontogenic tumor
def: "Neoplasm arising from the tissues of the odontogenic apparatus. These tumors are derived from ectodermal tissue (epithelial tumors) or from mesodermal tissue (connective tissue tumors) or are composed of both components (mixed or composite odontogenic tumors) ." [Pathbase: Pathology Committee]
is_a: MPATH:218 ! neoplasm

[Term]
id: MPATH:38
name: copper deposition
def: "Intra and extracellular deposition of copper and copper containing proteins." [Pathbase: Curation]
is_a: MPATH:45 ! protein deposition
is_a: MPATH:555 ! mineralisation

[Term]
id: MPATH:380
name: ameloblastic fibroma
def: "A tumor consisting of proliferating strands and clumps of odontogenic epithelium in a highly cellular fibroblastic stroma resembling the dental papilla of developing teeth. The epithelial component are composed of peripheral cuboidal or cylindrical cells enclosing scant stellate cells. (M-9330/0)." [Pathbase: Pathology Committee]
is_a: MPATH:379 ! odontogenic tumor

[Term]
id: MPATH:381
name: ameloblastoma
def: "Benign odontogenic epithelial neoplasm that histologically mimics the embryonic enamel organ but does not differentiate to the point of forming dental hard tissue. Histologically dominated by epithelial cells in a scant fibroblastic stroma. (M-9310/0)." [Pathbase: Pathology Committee]
is_a: MPATH:379 ! odontogenic tumor

[Term]
id: MPATH:382
name: cementifying fibroma
def: "Benign neoplasm derived from pluripotential mesenchymal cells or cementoblasts. Well demarcated tumor occurring exclusively in the jaw containing spindle cells which undergo transformation to cuboidal cementoblasts forming multiple cementicle like bodies. ( M-9274/0)." [Pathbase: Curation]
synonym: "ossifying fibroma, cemento-ossifying fibroma" RELATED [Pathbase: Curation]
is_a: MPATH:379 ! odontogenic tumor

[Term]
id: MPATH:383
name: cementoblastoma
def: "A neoplasm arising from the periodontal ligament (M-9273/0)." [Pathbase: Curation]
synonym: "True cementoma" RELATED [Pathbase: Curation]
is_a: MPATH:379 ! odontogenic tumor

[Term]
id: MPATH:384
name: cementoma
def: "Reactive fibro-osseous lesion derived from odotongenic cells in the periodontal ligament (M-9272/0)." [Pathbase: Curation]
is_a: MPATH:379 ! odontogenic tumor

[Term]
id: MPATH:385
name: dentinoma
def: "Similar lesion to ameloblastic fibroma (MPATH380) , but also showing inductive changes that lead to the formation of dentine (M-9271/0)." [Pathbase: Curation]
synonym: "ameloblastic fibrodentinoma" RELATED [Pathbase: Curation]
is_a: MPATH:379 ! odontogenic tumor

[Term]
id: MPATH:386
name: odontogenic tumor
def: "odontogenic tumor" [Pathbase: Curation]
comment: redundant
is_obsolete: true

[Term]
id: MPATH:387
name: odontoma
def: "Hamartomatous malformation of odontogenic tissue. It may vary from nondescript masses of dental tissue (complex odontoma) to multiple well-formed teeth (compound odontoma). Cf ameloblastic fibro-odontoma. (M-9280/0)." [ISBN:0781727286]
is_a: MPATH:254 ! complex tumor
is_a: MPATH:379 ! odontogenic tumor
is_a: MPATH:74 ! hamartoma

[Term]
id: MPATH:388
name: osseous and chondromatous tumor
def: "Neoplasms of bone and cartilage." [Pathbase: Curation]
is_a: MPATH:218 ! neoplasm

[Term]
id: MPATH:389
name: chondroblastoma
def: "A benign or malignant neoplasm occuring in the epiphyses of long bones, consisting of highly cellular tissue resembling embryonic cartilage. (M-9230/0, /3)." [Pathbase: Pathology Committee]
is_a: MPATH:388 ! osseous and chondromatous tumor

[Term]
id: MPATH:39
name: glycogen deposition
def: "Intracellular deposition of glycogen." [Pathbase: Curation]
is_a: MPATH:33 ! intracellular and extracellular accumulation

[Term]
id: MPATH:390
name: chondroblastoma, malignant
def: "chondroblastoma, malignant" [Pathbase: Curation]
comment: Subsumed into MPATH:389
is_obsolete: true

[Term]
id: MPATH:391
name: chondroma
def: "A benign neoplasm derived from mesodermal cells that form cartilage composed of well differentiated hyaline cartilage (M-9220/0)." [Pathbase: Curation]
is_a: MPATH:388 ! osseous and chondromatous tumor

[Term]
id: MPATH:392
name: chondrosarcoma
def: "Malignant neoplasm derived form pluripotential mesenchymal cells, chondrocytes or chondroblasts. No production of osteoid. (M-9220/3)." [Pathbase: Pathology Committee]
is_a: MPATH:388 ! osseous and chondromatous tumor

[Term]
id: MPATH:393
name: osteoblastoma
def: "Generally benign osteogenic neoplasm of unknown aetiology. Aggressive form may be confused with osteosarcoma. NOT a syn for osteofibroma. (M-9200/0)." [Pathbase: Pathology Committee]
synonym: "giant osteoid osteoma, benign osteoblastoma" RELATED [Pathbase: Curation]
is_a: MPATH:388 ! osseous and chondromatous tumor

[Term]
id: MPATH:394
name: osteochondroma
def: "Benign bone tumor characterized by hyaline cartilage capped bony growths that project from the surface of the affected bone. (M-9210/0)." [Pathbase: Pathology Committee]
synonym: "cartilaginous exostosis" RELATED [Pathbase: Curation]
is_a: MPATH:388 ! osseous and chondromatous tumor

[Term]
id: MPATH:395
name: osteofibroma
def: "Benign neoplasm derived from pluripotential mesenchymal stem cells or osteoblasts composed of mature nbone trabelculae seperated by a stroma of spindle cells. (M- 9262/0)." [Pathbase: Curation]
is_a: MPATH:388 ! osseous and chondromatous tumor

[Term]
id: MPATH:396
name: osteoma
def: "Benign neoplasm derived from osteoblasts or osteocytes composed of very dense bone with predominantly woven structure. ( M-9180/0)." [Book: Luz; A and Gessner; W. ; Neoplastic bone lesions of the mouse; in Pathology of neoplasia and preneoplasia in rodents; P. Bannasch and W. Goessner; Editors. 1997. Schattauer; Stuttgart. p. 142-154]
synonym: "cancellous osteoma" RELATED [Pathbase: Curation]
synonym: "compact osteoma" RELATED [Pathbase: Curation]
synonym: "juxtacortical osteoma" RELATED [Pathbase: Curation]
synonym: "medullary osteoma" RELATED [Pathbase: Curation]
synonym: "osteoid osteoma" RELATED [Pathbase: Curation]
synonym: "spongious osteoma" RELATED [Pathbase: Curation]
synonym: "trabecular osteoma" RELATED [Pathbase: Curation]
is_a: MPATH:388 ! osseous and chondromatous tumor

[Term]
id: MPATH:397
name: osteosarcoma
def: "Malignant neoplasm derived form mesenchymal stem cells, osteoblasts or osteocytes. Highly invasive and destructive tumor rising in the skeleton with osteoid and immature woven bone. (M-9180/3)." [Pathbase: Curation]
synonym: "osteogenic sarcoma" RELATED [Pathbase: Curation]
is_a: MPATH:388 ! osseous and chondromatous tumor

[Term]
id: MPATH:398
name: paragangliomas and glomus tumor
def: "Generally benign neoplasms of CHIEF cells arising from neuroectodermal tissues, found in various parts of the body. Note that until recently, glomus tumors were believed to be derived from specialised vascular cells, which is incorrect. Paraganglioma is the preferred term.The nomenclature for pheochromocytoma and paraganglioma is inconsistent. The term paraganglioma is used to refer to any extra-adrenal tumor of the paraganglion system or nonfunctional tumor of the paraganglion system. Functional tumors are referred extra-adrenal pheochromocytoma." [Pathbase: Curation]
is_a: MPATH:366 ! neuroendocrine tumor

[Term]
id: MPATH:399
name: aortic body tumor
def: "Paraganglioma arising in the CHIEF cells of the aortic body (M-8691/1)." [Pathbase: Curation]
synonym: "aortic body paraganglioma" RELATED [Pathbase: Curation]
is_a: MPATH:398 ! paragangliomas and glomus tumor

[Term]
id: MPATH:4
name: necrosis
def: "Morpholological changes after intravital (Pathologic) death of one or more cells, or of a portion of tissue or organ, resulting from irreversible damage;characterised by mitochondrial swelling, nuclear pyknosis, karyolysis, swollen and abnormally pale basophilic staining; or karyorrhexis, rupture and fragmentation of the nucleus. Energy independent cf. Apoptosis MPATH 3." [ISBN:0781727286]
is_a: MPATH:2 ! cell death

[Term]
id: MPATH:40
name: hyalinosis
def: "Intracellular deposition of eosinophilic material." [PMID: 11794381]
synonym: "Hyaline degeneration, Eosinophilic cytoplasmic change" RELATED [Pathbase: Curation]
is_a: MPATH:33 ! intracellular and extracellular accumulation

[Term]
id: MPATH:400
name: carotid body tumor
def: "Paraganglioma arising in the CHIEF cells of the carotid body (M-8692/1)." [Pathbase: Pathology Committee]
synonym: "carotid body paraganglioma" RELATED [Pathbase: Curation]
is_a: MPATH:398 ! paragangliomas and glomus tumor

[Term]
id: MPATH:401
name: glomus jugulare tumor
def: "A glomus tumor arising from the chief cells of the paraganglia ( neurectodermal derivatives) , or glomus bodies, located within the wall (adventitia) of the jugular bulb. (8690/1)." [Pathbase: Curation]
is_a: MPATH:398 ! paragangliomas and glomus tumor

[Term]
id: MPATH:402
name: glomus tumor
def: "glomus tumor" [Pathbase: Curation]
comment: obsolete; use paraganglioma  M-8711/0) or specific example terms, MPATH399-401.
is_obsolete: true

[Term]
id: MPATH:403
name: paraganglioma
def: "A neoplasm composed of derivatives of CHIEF cells usually in single encapsulated nodular masses surrounded with sustentacular cells. ( M- 8711/0)." [Pathbase: Curation]
synonym: "chemodectomas" RELATED [Pathbase: Curation]
synonym: "glomus tumor" RELATED [Pathbase: Curation]
synonym: "non-chromaffin paragangliomas" RELATED [Pathbase: Curation]
is_a: MPATH:398 ! paragangliomas and glomus tumor

[Term]
id: MPATH:404
name: soft tissue tumor
def: "Neoplasms of the soft and connective tissues." [Pathbase: Curation]
is_a: MPATH:218 ! neoplasm

[Term]
id: MPATH:405
name: chordoma
def: "Believed to arise from primitive notochord remnants . Usually occurs along the axial skeleton and is characterised by the presence of bubble cells containing large unstained cytoplasmic vacuoles with central or eccentricc nuclei. Benign but locally invasive. (M-9370/3)." [Pathbase: Curation]
is_a: MPATH:404 ! soft tissue tumor

[Term]
id: MPATH:406
name: dermatofibrosarcoma
def: "Highly recurrent, infiltrative skin tumors of intermediate malignancy derived from fibroblasts/fibrocytes. Human condition dermatofibrosarcoma protruberans (M-8832/3)." [Pathbase: Curation]
is_a: MPATH:404 ! soft tissue tumor
is_a: MPATH:551 ! sarcoma

[Term]
id: MPATH:407
name: fibroma
def: "Benign neoplasm of fibroblasts/fibrocytes with poor/moderate cellularity. (M-8810/0)." [Pathbase: Pathology Committee]
comment: "Soft tissue" qualifier removed by Pathology Panel to increase scope of term.
is_a: MPATH:404 ! soft tissue tumor

[Term]
id: MPATH:408
name: soft tissue fibrosarcoma
def: "Malignant tumor derived from pluripotential mesenchymal stem cells; fibroblasts, fibrocytes (M-8810/3)." [Pathbase: Pathology Committee]
is_a: MPATH:404 ! soft tissue tumor
is_a: MPATH:551 ! sarcoma

[Term]
id: MPATH:409
name: fibrous histiocytoma
def: "Benign or maligant tumor derived from pluripotential mesenchymal stem cells showing fibrous and histiocytic differentiation (M-8830/0)." [Pathbase: Curation]
is_a: MPATH:404 ! soft tissue tumor

[Term]
id: MPATH:41
name: iron deposition
def: "Extra- or intra-cellular deposition of iron, iron containing proteins or hemosiderin." [Pathbase: Curation]
is_a: MPATH:45 ! protein deposition
is_a: MPATH:555 ! mineralisation

[Term]
id: MPATH:410
name: giant cell tumor of soft tissue
def: "Malignant or benign tumor of pluripotential mesenchymal stem cells giving rise to large multinucleated cells (M- 9251/1)." [Pathbase: Pathology Committee]
synonym: "giant cell fibrous histiocytoma" RELATED [Pathbase: Curation]
is_a: MPATH:404 ! soft tissue tumor

[Term]
id: MPATH:411
name: granular cell tumor/alveolar sarcoma
def: "granular cell tumor/alveolar sarcoma" [Pathbase: Curation]
comment: obsolete. Use specific terms MPATH: 412 or MPATH: 413
is_obsolete: true

[Term]
id: MPATH:412
name: alveolar soft part sarcoma
def: "Malignant tumor of unknown origin though probably myogenic due to expression of MyoD and other myogenic lineage markers. Consists of grouped polygonal tumor cells with granular eosinophilic cytoplasm arranged in an organ-like configuration separated by thin fibrovascular septa. Central areas within these nests of cells become necrotic, and the loss of architecture produces an alveolar appearance. (M-9581/3)." [Pathbase: Pathology Committee]
is_a: MPATH:404 ! soft tissue tumor
is_a: MPATH:551 ! sarcoma

[Term]
id: MPATH:413
name: granular cell tumor
def: "Large polygonal or round cell tumors with abundant acidophilic cytoplasm containing PAS positive granules. Found especially in the uterine cervix. Aetiology unknown. (M-9580/0)." [Pathbase: Pathology Committee]
synonym: "myoblastoma" RELATED [Pathbase: Curation]
is_a: MPATH:423 ! myomatous tumor

[Term]
id: MPATH:414
name: histiocytic sarcoma
def: "histiocytic sarcoma" [Pathbase: Curation]
comment: redundant use MPATH506
is_obsolete: true

[Term]
id: MPATH:415
name: lipomatous tumor
def: "Tumors derived from the lipogenic lineage or showing predominantly lipomatous differentiation." [Pathbase: Curation]
is_a: MPATH:404 ! soft tissue tumor

[Term]
id: MPATH:416
name: angiomyolipoma
def: "Benign renal neoplasm composed of fat, vascular, and smooth muscle elements. Associated with tuberous sclerosis in humans. Aetiology unknown, but the combination of elements may reflect a lesion specific pattern of metaplasia. (M-8860/0)." [Pathbase: Pathology Committee]
is_a: MPATH:254 ! complex tumor
is_a: MPATH:415 ! lipomatous tumor

[Term]
id: MPATH:417
name: lipoma
def: "Benign neoplasia derived from lipoblasts or lipocytes of white or brown fat. May be angiomatous or hibernomatous. (M- 8850/0)." [Pathbase: Pathology Committee]
is_a: MPATH:415 ! lipomatous tumor

[Term]
id: MPATH:418
name: liposarcoma
def: "Malignant neoplasms which probably originate in primitive mesenchymal stem cell populations differentiating down a lipomatous pathway. (M-8850/3)." [Pathbase: Pathology Committee]
is_a: MPATH:415 ! lipomatous tumor
is_a: MPATH:551 ! sarcoma

[Term]
id: MPATH:419
name: lymphatic vessel tumor
def: "Neoplasms of the lymphatic vessels." [Pathbase: Curation]
is_a: MPATH:404 ! soft tissue tumor

[Term]
id: MPATH:42
name: lipid deposition
def: "Extra or intracellular deposition of lipid." [Pathbase: Curation]
is_a: MPATH:33 ! intracellular and extracellular accumulation

[Term]
id: MPATH:420
name: lymphangioma
def: "Benign hamartomatous malformation of the lymphatic ducts. Usually found in the skin and may be superficial or deep. (M-9170/0)." [ISBN:0781727286]
synonym: "Cystic hygroma" RELATED [Pathbase: Curation]
is_a: MPATH:419 ! lymphatic vessel tumor
is_a: MPATH:74 ! hamartoma

[Term]
id: MPATH:421
name: lymphangiomyomatosis
def: "Characterized by benign peribronchial, perivascular, and perilymphatic proliferation of atypical smooth muscle resulting in vascular and airway obstruction, cyst formation, and a progressive decline in lung function. (M- 9174/1)." [Pathbase: Curation]
synonym: "Lymphangioleiomyomatosis." RELATED [Pathbase: Curation]
is_a: MPATH:419 ! lymphatic vessel tumor

[Term]
id: MPATH:422
name: lymphangiosarcoma
def: "A malignant neoplasm derived from vascular tissue in which the neoplastic cells originate from the endothelial cells of lymphatic vessels. (M-9170/3)." [Pathbase: Curation]
is_a: MPATH:419 ! lymphatic vessel tumor
is_a: MPATH:551 ! sarcoma

[Term]
id: MPATH:423
name: myomatous tumor
def: "Neoplasms derived from myogenic lineages or predominantly composed of cells showing myomatous differentiation." [Pathbase: Curation]
is_a: MPATH:404 ! soft tissue tumor

[Term]
id: MPATH:424
name: intravascular leiomyomatosis
def: "Benign leiomyoma that invades vascular spaces. (M-8890/1)." [Pathbase: Curation]
is_a: MPATH:423 ! myomatous tumor

[Term]
id: MPATH:425
name: leiomyoma
def: "Benign neoplasm derived from smooth muscle cells. (M-8890/0)." [Pathbase: Curation]
is_a: MPATH:423 ! myomatous tumor

[Term]
id: MPATH:426
name: leiomyosarcoma
def: "Malignant tumor derived form pluripotential mesenchymal stem cells or smooth muscle cells. (M- 8890/3)." [Pathbase: Curation]
is_a: MPATH:423 ! myomatous tumor
is_a: MPATH:551 ! sarcoma

[Term]
id: MPATH:427
name: myoblastoma
def: "myoblastoma" [Pathbase: Curation]
comment: obsolete. Syn of granular cell tumor. MPATH 413
is_obsolete: true

[Term]
id: MPATH:428
name: rhabdomyosarcoma
def: "Malignant tumor of striated muscle or pluripotential mesenchymal stem cells. (M-8900/3)." [Pathbase: Curation]
is_a: MPATH:423 ! myomatous tumor
is_a: MPATH:551 ! sarcoma

[Term]
id: MPATH:429
name: myxomatous tumor
def: "Neoplasms resembling primitive mesenchymal tissue with a soft mucous matrix." [Pathbase: Curation]
is_a: MPATH:404 ! soft tissue tumor

[Term]
id: MPATH:43
name: lipofuscin deposition
def: "Intracellular deposition of brown pigment granules probably representing lipid-containing residues of lysosomal digestion. Often age related." [Pathbase: Pathology Committee]
is_a: MPATH:613 ! pigmentation

[Term]
id: MPATH:430
name: angiomyxoma
def: "Angiomyxoma is a poorly circumscribed, slowly growing lesion composed of spindle-shaped and stellate cells evenly distributed in an abundant myxoid matrix. The lesion contains numerous vessels, often showing some hyalinization of their walls, and occasionally surrounded by a few smooth muscle cells. Immunohistochemically, tumor cells may express desmin and/ or smooth muscle actin (M-8841/1)." [Pathbase: Curation]
is_a: MPATH:429 ! myxomatous tumor

[Term]
id: MPATH:431
name: myxoma
def: "A benign neoplasm derived from pluripotential mesenchymal stem cells of connective tissue, consisting chiefly of polyhedral and stellate cells that are loosely embedded in a soft mucoid matrix. May show multiple differentiated components. (M-8840/0)." [Pathbase: Pathology Committee]
is_a: MPATH:429 ! myxomatous tumor

[Term]
id: MPATH:432
name: myxosarcoma
def: "A malignant neoplasm derived from pluripotential mesenchymal stem cells of connective tissue, consisting chiefly of polyhedral and stellate cells that are loosely embedded in a soft mucoid matrix. (M-8840/3)." [Pathbase: Curation]
is_a: MPATH:429 ! myxomatous tumor
is_a: MPATH:551 ! sarcoma

[Term]
id: MPATH:433
name: nerve sheath tumor
def: "Neoplasms of the nerve sheath." [Pathbase: Pathology Committee]
is_a: MPATH:404 ! soft tissue tumor
is_a: MPATH:570 ! peripheral nervous system tumors

[Term]
id: MPATH:434
name: neurilemmoma
def: "neurilemmoma" [Pathbase: Curation]
comment: obsolete. Use schwannoma MPATH438
is_obsolete: true

[Term]
id: MPATH:435
name: neurofibroma
def: "Peripheral nerve tumor consisting of chaotic arrays of wavy schwann cell bundles and fibroblasts interspersed within a matrix rich in collagen and mucopolysaccharide. (M9540/0)." [ISBN-13:9783794515530]
is_a: MPATH:433 ! nerve sheath tumor

[Term]
id: MPATH:436
name: neurofibromatosis
def: "Systemic manifestation of MPATH:435 ( M-9540/1)." [Pathbase: Curation]
is_a: MPATH:433 ! nerve sheath tumor

[Term]
id: MPATH:437
name: neurofibrosarcoma
def: "Malignant neoplasm derived from Schwann cells. (M-9540/3)." [ISBN-13:9783794515530]
synonym: "malignant peripheral nerve sheath tumor" RELATED [Pathbase: Curation]
is_a: MPATH:433 ! nerve sheath tumor
is_a: MPATH:551 ! sarcoma

[Term]
id: MPATH:438
name: schwannoma
def: "May be malignant or benign, Schwann cell derived tumor considered to be neurectodermal with some acquired mesenchymal features. (M-9560/0)." [ISBN-13:9783794515530]
synonym: "neurilemoma" RELATED [Pathbase: Curation]
synonym: "neurinoma, benign" RELATED [Pathbase: Curation]
is_a: MPATH:433 ! nerve sheath tumor

[Term]
id: MPATH:439
name: synovial-like tumor
def: "Neoplasms of synovial origin." [Pathbase: Curation]
is_a: MPATH:404 ! soft tissue tumor

[Term]
id: MPATH:44
name: melanin deposition
def: "Intra or extracellular deposition of melanin." [Pathbase: Pathology Committee]
is_a: MPATH:613 ! pigmentation

[Term]
id: MPATH:440
name: synovial sarcoma
def: "Malignant neoplasm occurring in close association with tendon sheaths and joint capsules. Biphasic in humans , showing a mixed spindle cell and epithelioid like morphology; this is not seen in rodents to date. (M-9040/3)." [Pathbase: Pathology Committee]
synonym: "Synovial cell sarcoma" RELATED [Pathbase: Curation]
is_a: MPATH:439 ! synovial-like tumor
is_a: MPATH:551 ! sarcoma

[Term]
id: MPATH:441
name: synovioma
def: "synovioma" [Pathbase: Curation]
comment: Obsolete. Use MPATH:440
is_obsolete: true

[Term]
id: MPATH:442
name: squamous cell tumor
def: "Neoplasms of stratified squamous epithelial cells." [Pathbase: Pathology Committee]
is_a: MPATH:218 ! neoplasm

[Term]
id: MPATH:443
name: inverted squamous papilloma
def: "A benign tumor consisting of villous or arborescent outgrowths of fibrovascular stroma covered by neoplastic epithelial cells in which proliferating epithelium is invaginated beneath the surface and is more smoothly rounded. (M-8053/0)." [Pathbase: Pathology Committee]
synonym: "endophytic papilloma" RELATED [Pathbase: Curation]
synonym: "invaginated papilloma" RELATED [Pathbase: Curation]
is_a: MPATH:219 ! adnexal and skin appendage tumor
is_a: MPATH:442 ! squamous cell tumor
is_a: MPATH:445 ! papilloma

[Term]
id: MPATH:444
name: keratoacanthoma
def: "Skin type is thought to arise from follicular epithelium of hair follicles; found in other epithelia. Composed of multiple cup shaped cavities filled with lamellated concentrically arranged or homogeneous cornified masses." [Pathbase: Pathology Committee]
synonym: "epithelioma, intracutaneous, cornifying" RELATED [Pathbase: Curation]
is_a: MPATH:219 ! adnexal and skin appendage tumor
is_a: MPATH:442 ! squamous cell tumor

[Term]
id: MPATH:445
name: papilloma
def: "A benign tumor consisting of villous or arborescent outgrowths of fibrovascular stroma covered by neoplastic epithelial cells (M-8050/0)." [Pathbase: Pathology Committee]
is_a: MPATH:264 ! fibroepithelial tumor
is_a: MPATH:556 ! potentially cancerous lesions

[Term]
id: MPATH:446
name: squamous cell carcinoma
def: "Malignant tumor derived from stratified squamous cells. (M-8070/3)." [Pathbase: Pathology Committee]
synonym: "carcinoma, epidermoid ( sensu epidermal derived tumors)" RELATED [Pathbase: Curation]
is_a: MPATH:219 ! adnexal and skin appendage tumor
is_a: MPATH:442 ! squamous cell tumor
is_a: MPATH:549 ! carcinoma

[Term]
id: MPATH:447
name: squamous cell carcinoma in situ
def: "Pre-neoplastic intraepithelial lesion of squamous cells (M-8070/2)." [Pathbase: Pathology Committee]
synonym: "IENIII" RELATED [Pathbase: Curation]
synonym: "severe intra-epithelial neoplasia" RELATED [Pathbase: Curation]
is_a: MPATH:219 ! adnexal and skin appendage tumor
is_a: MPATH:442 ! squamous cell tumor
is_a: MPATH:556 ! potentially cancerous lesions

[Term]
id: MPATH:448
name: squamous cell papilloma
def: "A benign tumor consisting of villous or arborescent outgrowths of fibrovascular stroma covered by neoplastic squamous epithelial cells." [Pathbase: Pathology Committee]
synonym: "Exophytic papilloma" RELATED [Pathbase: Curation]
is_a: MPATH:219 ! adnexal and skin appendage tumor
is_a: MPATH:442 ! squamous cell tumor
is_a: MPATH:445 ! papilloma

[Term]
id: MPATH:449
name: verrucous carcinoma
def: "A well-differentiated papillary squamous cell carcinoma. (M-8051/3)." [Pathbase: Curation]
is_a: MPATH:442 ! squamous cell tumor
is_a: MPATH:549 ! carcinoma

[Term]
id: MPATH:45
name: protein deposition
def: "Non-specified intra or extracellular deposition of protein." [Pathbase: Curation]
is_a: MPATH:33 ! intracellular and extracellular accumulation

[Term]
id: MPATH:450
name: transitional cell tumor
def: "Neoplasms of transitional epithelia, eg kidney, ureter , bladder , cervix." [Pathbase: Pathology Committee]
is_a: MPATH:218 ! neoplasm

[Term]
id: MPATH:451
name: transitional cell carcinoma
def: "Malignant neoplasm of transitional cells (M-8120/3)." [Pathbase: Curation]
is_a: MPATH:450 ! transitional cell tumor
is_a: MPATH:549 ! carcinoma

[Term]
id: MPATH:452
name: transitional cell carcinoma in situ
def: "Pre-malignant intra-epithelial neoplasm of transitional cells (M-8120/2)." [Pathbase: Pathology Committee]
synonym: "severe intra-epithelial neoplasia" RELATED [Pathbase: Curation]
is_a: MPATH:450 ! transitional cell tumor
is_a: MPATH:556 ! potentially cancerous lesions

[Term]
id: MPATH:453
name: transitional cell papilloma
def: "Pre-malignant lesion of transitional cells, papillomatous form ( M- 8120/1)." [Pathbase: Pathology Committee]
is_a: MPATH:450 ! transitional cell tumor

[Term]
id: MPATH:454
name: trophoblastic tumor
def: "Tumors derived directly from trophoblastic tissue or differentiated from germ cell tumor origins." [Pathbase: Curation]
is_a: MPATH:218 ! neoplasm

[Term]
id: MPATH:455
name: choriocarcinoma
def: "Tumor derived from malignant trophoblastic cells. May be found in the uterus, ovary and testis. May also be derived from teratomas and teratocarcinomas in males. (M-9100/3)." [Pathbase: Pathology Committee]
synonym: "Chorioepithelioma, malignant." RELATED [Pathbase: Curation]
is_a: MPATH:310 ! germ cell tumor
is_a: MPATH:454 ! trophoblastic tumor

[Term]
id: MPATH:456
name: hydatidiform mole
def: "Vesicular or cystic tumor with hydropic villi resulting from the proliferation of trophoblast in the absence ( complete) or the presence ( partial) of an embryo. Most complete moles are homozygous androgenetic XX 46.(M-9100/0)." [Pathbase: Curation]
synonym: "cystic mole" RELATED [Pathbase: Curation]
synonym: "gestational trophoblastic disease" RELATED [Pathbase: Curation]
is_a: MPATH:454 ! trophoblastic tumor

[Term]
id: MPATH:457
name: placental site trophoblastic tumor
def: "Neoplastic proliferation of intermediate trophoblasts that invades the myometrium at the placental site after a pregnancy. (M-9104/1)." [Pathbase: Pathology Committee]
is_a: MPATH:454 ! trophoblastic tumor

[Term]
id: MPATH:458
name: normal
def: "Normal." [Pathbase: Pathology Committee]
is_a: MPATH:0 ! pathology_ontology

[Term]
id: MPATH:459
name: obsolete
def: "obsolete" [Pathbase: Pathology Committee]
is_obsolete: true

[Term]
id: MPATH:46
name: uric acid deposition
def: "Extracellular deposition of uric acid crystals." [Pathbase: Curation]
is_a: MPATH:33 ! intracellular and extracellular accumulation

[Term]
id: MPATH:460
name: nuclear defect
def: "Defect in the structure or function of the nuclear membrane or matrix or other component." [Pathbase: Curation]
is_a: MPATH:17 ! subcellular defect

[Term]
id: MPATH:461
name: cataract; capsular-epithelial
def: "Proliferation of lens epithelium and capsule leading to fibrous metaplasia and anterior subcapsular cataract ( ASC) . Possible developmental origin." [ISBN:08493086 4X]
is_a: MPATH:29 ! cataract

[Term]
id: MPATH:462
name: cataract; nuclear and cortical
def: "Nuclear cataract of developmental origin with tendency to progress with age and involve the cortex and capsule." [ISBN:08493086 4X]
is_a: MPATH:29 ! cataract

[Term]
id: MPATH:463
name: cataract; cortical liquefactive
def: "Of developmental origins; nucleus and cortex become completely liquefied in post-natal life." [ISBN:08493086 4X]
is_a: MPATH:29 ! cataract

[Term]
id: MPATH:464
name: cataract; lens extrusion
def: "Involves capsular rupture usually of the posterior lens capsule, close to birth or in the first few weeks postpartum. Cortical material spills into the vitreous humor and may be disseminated through the eye." [ISBN:08493086 4X]
is_a: MPATH:29 ! cataract

[Term]
id: MPATH:465
name: glaucoma developmental
def: "Consequent on developmental abnormalities in the trabecular network and Schlemm`s canal in the angle." [ISBN:08493086 4X]
is_a: MPATH:32 ! glaucoma

[Term]
id: MPATH:466
name: glaucoma; open angle
def: "Failure of drainage of the eye for unknown reasons." [ISBN:08493086 4X]
is_a: MPATH:32 ! glaucoma

[Term]
id: MPATH:467
name: glaucoma; angle closure
def: "Develops when the angle caused by the iris and cornea closes. May occur because of anatomically narrow angles or adhesions." [ISBN:08493086 4X]
is_a: MPATH:32 ! glaucoma

[Term]
id: MPATH:468
name: pseudocyst
def: "Formation of extracellular (sensu pancreas) non-epithelial bounded spaces containing accumulated products or substances." [Pathbase: Pathology Committee]
is_a: MPATH:1 ! cell and tissue damage

[Term]
id: MPATH:469
name: symmetry defect
def: "Any aberration of the normal symmetrical organisation of the body pattern." [Pathbase: Curation]
is_a: MPATH:56 ! developmental and adult structural  defect

[Term]
id: MPATH:47
name: intracellular and extracellular depletion
def: "Loss of specific intra- and extracellular substances." [Pathbase: Pathology Committee]
is_a: MPATH:1 ! cell and tissue damage

[Term]
id: MPATH:470
name: left/right axis defect
def: "Left/Right (mediolateral) axis aberration of the normal symmetrical organisation of the body pattern." [Pathbase: Pathology Committee]
comment: For example as seen in the mutation <situs inversus>.
is_a: MPATH:469 ! symmetry defect

[Term]
id: MPATH:471
name: anterior/posterior axis defect
def: "Anteroposterior aberration of the normal symmetrical organisation of the body pattern." [Pathbase: Curation]
is_a: MPATH:469 ! symmetry defect

[Term]
id: MPATH:472
name: Dorsal/ventral axis defect
def: "Dorsoventral aberration of the normal symmetrical organisation of the body pattern." [Pathbase: Curation]
is_a: MPATH:469 ! symmetry defect

[Term]
id: MPATH:473
name: developmental cystic dysplasia
def: "Developmental dysplasia showing epithelial cell bounded cavities." [Pathbase: Pathology Committee]
is_a: MPATH:64 ! developmental dysplasia

[Term]
id: MPATH:474
name: ectasia
def: "Dilation of a tubular structure." [Pathbase: Pathology Committee]
comment: Often associated with an obstruction.
is_a: MPATH:66 ! dilatation

[Term]
id: MPATH:475
name: ductal ectasia
def: "Dilation of a ductal structure." [Pathbase: Curation]
is_a: MPATH:474 ! ectasia

[Term]
id: MPATH:476
name: telangiectasia
def: "A lesion formed by a dilated capillary or terminal artery." [Pathbase: Curation]
is_a: MPATH:474 ! ectasia

[Term]
id: MPATH:477
name: choristoma
def: "Similar to hamartoma, including the mass lesion requirement, but unlike hamartoma, includes heterotopic tissue of an adult or embryonic nature ( topographical and developmental anomaly)." [ISBN:0781727286]
synonym: "Choristoblastoma" RELATED [Pathbase: Curation]
is_a: MPATH:56 ! developmental and adult structural  defect

[Term]
id: MPATH:478
name: angiogenesis defect
def: "Abnormality in developmental angiogenesis." [Pathbase: Pathology Committee]
is_a: MPATH:599 ! developmental process abnormalities

[Term]
id: MPATH:479
name: vasculogenesis defect
def: "Defect in formation of blood vessels by vasculogenesis, proliferation or recruitment of endothelial cells." [Pathbase: Pathology Committee]
is_a: MPATH:599 ! developmental process abnormalities

[Term]
id: MPATH:48
name: decalcification
def: "Process of loss of calcium from normally calcified tissue, usually bone." [Pathbase: Curation]
is_a: MPATH:47 ! intracellular and extracellular depletion

[Term]
id: MPATH:480
name: decidual defect
def: "Any defect in the formation, architecture, cellular composition or function of the maternal decidua." [Pathbase: Curation]
is_a: MPATH:100 ! placental abnormality

[Term]
id: MPATH:481
name: pre-neoplastic lesions
def: "Lesions likely to result in progression to frank tumors, which may be classified as pre-neoplastic or pre-cancerous." [Journal: Ward; J.M. ( 2002) J Toxicol. Pathol. 15; 123-128]
comment: Obsolete; replaced by potentially pre-cancerous lesions (MPATH 556) as many are actually neoplastic but do not progress to cancer.
is_obsolete: true

[Term]
id: MPATH:482
name: focal hyperplasia
def: "Localised hyperplastic lesion. Polyclonal lesions are probably benign but clonal lesions may progress to malignancy." [Pathbase: Pathology Committee]
is_a: MPATH:602 ! hyperplastic tissue

[Term]
id: MPATH:483
name: atypical hyperplasia
def: "Presence of localised areas within for example adenomas showing characteristics of neoplastic (tumor) progression, eg focal carcinoma." [Pathbase: Pathology Committee]
comment: Considered to be too vague to be useful.
is_obsolete: true

[Term]
id: MPATH:484
name: hyperplastic nodule
def: "Expansion of small hyperplastic lesions to become macroscopically nodules, compressing adjacent cells." [Pathbase: Pathology Committee]
synonym: "hyperplastic nodules" RELATED [Pathbase: Curation]
is_a: MPATH:602 ! hyperplastic tissue

[Term]
id: MPATH:485
name: carcinoma in situ
def: "May be used in some systems in preference to its synonyms to indicate lesion specific aprearances. A lesion characterised by changes of the type associated with invasive carcinoma, but physically bounded by the lining epithelium and without local invasion." [Pathbase: Pathology Committee]
comment: Subsumed into MPATH: 132
synonym: "severe epithelial dysplasia" RELATED [Pathbase: Curation]
synonym: "severe intraepithelial neoplasia" RELATED [Pathbase: Curation]
is_obsolete: true

[Term]
id: MPATH:486
name: ductal intra-epithelial neoplasia
def: "Pre-malignant hyperplastic and/or dysplastic change in the mammary gland epithelium with the potential to give rise to malignant tumors." [PMID:10713680]
comment: This term covers the range of DIN (MIN) including severe intra-epithelial neoplasia (IENIII), alternatively termed in situ carcinoma of the mammary ductal epithelium. (M- 8500/2). See Tavassoli FA. (1998) Mod Pathol. 11:140-54. Ductal carcinoma in situ: introduction of the concept of ductal intraepithelial neoplasia for further definition.
synonym: "DIN" RELATED [Pathbase: Curation]
synonym: "Ductal carcinoma in situ" RELATED [Pathbase: Curation]
synonym: "intraductal adenocarcinoma, non-infiltrating" RELATED [Pathbase: Curation]
synonym: "mammary intra-epithelial neoplasia" RELATED [Pathbase: Curation]
synonym: "MIN" RELATED [Pathbase: Curation]
is_a: MPATH:267 ! glandular tumor
is_a: MPATH:556 ! potentially cancerous lesions

[Term]
id: MPATH:487
name: intestinal intra-epithelial neoplasia
def: "Histologically apparent areas of dysplasia that are not grossly visible (smaller than 0.5-1 mm). Lesions may involve single or multiple glands." [PMID:12612914]
synonym: "GIN" RELATED [Pathbase: Curation]
synonym: "IIN" RELATED [Pathbase: Curation]
synonym: "microadenoma" RELATED [Pathbase: Curation]
is_a: MPATH:128 ! intra-epithelial neoplasia

[Term]
id: MPATH:488
name: prostate intra-epithelial neoplasia
def: "See reference for definition." [ISBN:0-19-512338-7]
synonym: "PIN" RELATED [Pathbase: Curation]
xref: URL: http\://emice.nci.nih.gov/emice/mouse_models/organ_models/prostate_models/path_class_mouse
is_a: MPATH:128 ! intra-epithelial neoplasia

[Term]
id: MPATH:489
name: stomach, oesophagus and pancreatic intra-epithelial neoplasia
def: "stomach, oesophagus and pancreatic intra-epithelial neoplasia" [ISBN:0-19-512338-7]
synonym: "PANIN" RELATED [Pathbase: Curation]
is_a: MPATH:128 ! intra-epithelial neoplasia

[Term]
id: MPATH:49
name: demyelination
def: "Reduction of myelin content in neuronal sheath." [Pathbase: Curation]
is_a: MPATH:47 ! intracellular and extracellular depletion

[Term]
id: MPATH:490
name: adenomatous polyp
def: "Benign neoplastic growth containing areas of adenomatous structure (progression)." [Pathbase: Curation]
synonym: "polypoid adenoma, cellular polyp." RELATED [Pathbase: Curation]
is_a: MPATH:270 ! adenoma
relationship: part_of MPATH:271 ! adenomatous polyposis coli

[Term]
id: MPATH:491
name: polyp
def: "A mass of tissue which projects outward or upward from the normal surface level being macroscopically visible as a hemispheroidal, spheroidal, or irregular moundlike structure growing from a relatively broad base or a slender stalk." [ISBN:0781727286]
is_a: MPATH:138 ! epithelial hyperplasia

[Term]
id: MPATH:492
name: membraneous glomerulonephritis
def: "Glomerulonephritis characterized by diffuse thickening of glomerular capillary basement membranes, due in part to subepithelial deposits of immunoglobulins separated by spikes of basement membrane material,." [ISBN:0781727286]
is_a: MPATH:197 ! glomerulonephritis

[Term]
id: MPATH:493
name: membraneoproliferative glomerulonephritis
def: "A chronic glomerulonephritis characterized by mesangial cell proliferation, increased lobular separation of glomeruli, thickening of glomerular capillary walls and increased mesangial matrix,." [ISBN:0781727286]
is_a: MPATH:197 ! glomerulonephritis

[Term]
id: MPATH:494
name: autoimmune glomerulonephritis
def: "Glomerulonephritis caused by autoimmune attack on the glomerulus." [ISBN:0781727286]
comment: Needs multiple parentage with autoimmune mediated disease
is_a: MPATH:197 ! glomerulonephritis

[Term]
id: MPATH:495
name: glomangioma
def: "Tumor derived from the capillary glomus with arteriovenous capillary anastomoses. Often characterized by multiple tumors resembling cavernous hemangioma (M-8712/0)." [Pathbase: Curation]
is_a: MPATH:235 ! blood vessel tumor

[Term]
id: MPATH:496
name: Non-Lymphoid leukaemias
def: "Neoplasms of non-lymphoid haematopoietic lineage. Must have at least 20% blast cells to meet this definition." [PMID:12070033]
xref: URL:http\://www.bloodjournal.org/cgi/content/full/100/1/238/DC1/2
is_a: MPATH:515 ! Non-Lymphoid neoplasias

[Term]
id: MPATH:497
name: myeloid leukaemia without maturation
def: "Leukaemia in which neoplastic cells are poorly differentiated and not monocytic. At least 90% of the cells have to be blasts." [PMID:12070033]
synonym: "myeloblastic leukaemia without maturation" RELATED [Pathbase: Curation]
synonym: "myeloid leukaemia (myeloblastic type)" RELATED [Pathbase: Curation]
synonym: "poorly differentiated myeloid leukaemia" RELATED [Pathbase: Curation]
xref: URL:http\://www.bloodjournal.org/cgi/content/full/100/1/238/DC1/2
is_a: MPATH:342 ! myeloid leukaemia

[Term]
id: MPATH:498
name: myeloid leukaemia with maturation
def: "Leukaemia in which neoplastic cells are moderately differentiated with a neutrophilic but not monocytic component. At least 20% of the cells have to be blasts." [PMID:12070033]
synonym: "myeloblastic laeukaemia with maturation" RELATED [Pathbase: Curation]
synonym: "poorly differentiated myeloid leukaemia" RELATED [Pathbase: Curation]
xref: URL:http\://www.bloodjournal.org/cgi/content/full/100/1/238/DC1/2
is_a: MPATH:342 ! myeloid leukaemia

[Term]
id: MPATH:499
name: nesidioblastosis
def: "Abnormal proliferation of beta cells of developing islets often leading to marked diffuse or focal beta-cell hyperplasia. Considered to generate a potentially cancerous lesion." [PMCID: 1964945]
synonym: "Beta-cell nesidioblastosis" RELATED [Pathbase: Curation]
synonym: "congenital insulinomas" RELATED [Pathbase: Curation]
synonym: "diffused or generalised islet cell hyperplasia" RELATED [Pathbase: Curation]
synonym: "endocrine dysplasia" RELATED [Pathbase: Curation]
synonym: "focal adenomatosis" RELATED [Pathbase: Curation]
synonym: "microadenomatosis" RELATED [Pathbase: Curation]
synonym: "multifocal and focal ductulo-insular proliferation (nesidioblastosis)" RELATED [Pathbase: Curation]
synonym: "nesidioblastoma" RELATED [Pathbase: Curation]
synonym: "nesidiodysplasia" RELATED [Pathbase: Curation]
is_a: MPATH:64 ! developmental dysplasia

[Term]
id: MPATH:5
name: bridging necrosis
def: "Area of liver necrosis that bridges adjacent portal areas and central veins." [ISBN:0781727286]
is_a: MPATH:4 ! necrosis

[Term]
id: MPATH:50
name: glycogen depletion
def: "Reduction in intracellular glycogen content." [Pathbase: Curation]
is_a: MPATH:47 ! intracellular and extracellular depletion

[Term]
id: MPATH:500
name: myeloproliferative disease-like myeloid leukaemia
def: "Leukaemia in which neoplastic cells are well differentiated and in which there are fewer than 20% blasts." [PMID:12070033]
synonym: "myeloid leukaemia, chonic type" RELATED [Pathbase: Curation]
synonym: "well differentiated myeloid leukaemia" RELATED [Pathbase: Curation]
xref: URL:http\://www.bloodjournal.org/cgi/content/full/100/1/238/DC1/2
is_a: MPATH:342 ! myeloid leukaemia

[Term]
id: MPATH:501
name: myelomonocytic leukaemia
def: "Leukaemia in which neoplastic cells are moderately differentiated with a neutrophilic and a monocytic component. At least 20% of the cells have to be blasts." [PMID:12070033]
synonym: "myeloid leukaemia, myelomonocytic type" RELATED [Pathbase: Curation]
xref: URL:http\://www.bloodjournal.org/cgi/content/full/100/1/238/DC1/2
is_a: MPATH:342 ! myeloid leukaemia

[Term]
id: MPATH:502
name: monocytic leukaemia
def: "Leukaemia in which neoplastic cells are poorly or moderately differentiated with a monocytic but no neutrophilic component. At least 20% of the cells must be blasts." [PMID:12070033]
xref: URL:http\://www.bloodjournal.org/cgi/content/full/100/1/238/DC1/2
is_a: MPATH:342 ! myeloid leukaemia

[Term]
id: MPATH:503
name: biphenotypic leukaemia
def: "A leukaemia with at least 90% blasts and differentiation markers of the myeloid and lymphoid lineage." [PMID:12070033]
xref: URL:http\://www.bloodjournal.org/cgi/content/full/100/1/238/DC1/2
is_a: MPATH:496 ! Non-Lymphoid leukaemias

[Term]
id: MPATH:504
name: non-lymphoid hematopoietic sarcomas
def: "Solid tumor mass composed of non-lymphoid haematopoietic cells." [PMID:12070033]
xref: URL:http\://www.bloodjournal.org/cgi/content/full/100/1/238/DC1/2
is_a: MPATH:335 ! hematopoietic/lymphoid malignancies/disorder
is_a: MPATH:551 ! sarcoma

[Term]
id: MPATH:505
name: granulocytic sarcoma
def: "Solid tumor mass composed predominantly of granulocytic or relatively undifferentiated non-lymphoid haematopoietic cells." [PMID:12070033]
xref: URL:http\://www.bloodjournal.org/cgi/content/full/100/1/238/DC1/2
is_a: MPATH:504 ! non-lymphoid hematopoietic sarcomas

[Term]
id: MPATH:506
name: histiocytic sarcoma
def: "Solid tumor mass composed predominantly of histiocytic cells (M-9775/3)." [PMID:12070033]
synonym: "histiocytic lymphoma" RELATED [Pathbase: Curation]
synonym: "Kupffer cell sarcoma (sensu liver)" RELATED [Pathbase: Curation]
synonym: "malignant lymphoma, histiocytic type" RELATED [Pathbase: Curation]
synonym: "reticulum cell sarcoma, type A" RELATED [Pathbase: Curation]
synonym: "reticulum cell sarcoma, type A, reticulosarcoma" RELATED [Pathbase: Curation]
xref: URL:http\://www.bloodjournal.org/cgi/content/full/100/1/238/DC1/2
is_a: MPATH:504 ! non-lymphoid hematopoietic sarcomas

[Term]
id: MPATH:507
name: mast cell sarcoma
def: "Solid tumor mass composed of mast cells." [PMID:12070033]
synonym: "malignant mastocytoma" RELATED [Pathbase: Curation]
synonym: "mast cell tumor" RELATED [Pathbase: Curation]
synonym: "mastocytosis" RELATED [Pathbase: Curation]
xref: URL:http\://www.bloodjournal.org/cgi/content/full/100/1/238/DC1/2
is_a: MPATH:504 ! non-lymphoid hematopoietic sarcomas

[Term]
id: MPATH:508
name: myeloid dysplasias
def: "Haematopoietic proliferation with evidence of trilineage dysplasia." [PMID:12070033]
xref: URL:http\://www.bloodjournal.org/cgi/content/full/100/1/238/DC1/2
is_a: MPATH:515 ! Non-Lymphoid neoplasias

[Term]
id: MPATH:509
name: cytopenia with increased blasts
def: "Haematopoietic proliferation with evidence of trilineage dysplasia. More than 20% should be blasts." [PMID:12070033]
xref: URL:http\://www.bloodjournal.org/cgi/content/full/100/1/238/DC1/2
is_a: MPATH:508 ! myeloid dysplasias

[Term]
id: MPATH:51
name: hypocalcification
def: "Intrinsic abnormally low level of calcification in a tissue cf. MPATH: 48." [Pathbase: Curation]
is_a: MPATH:47 ! intracellular and extracellular depletion

[Term]
id: MPATH:510
name: myeloid proliferations (non-reactive)
def: "Non-reactive persistent accumulation of non-lymphoid haematopoietic cells. Genetically determined." [PMID:12070033]
xref: URL:http\://www.bloodjournal.org/cgi/content/full/100/1/238/DC1/2
is_a: MPATH:515 ! Non-Lymphoid neoplasias

[Term]
id: MPATH:511
name: Myeloproliferation (genetic)
def: "Non-reactive persistent accumulation of non-lymphoid haematopoietic cells in the blood which do not infiltrate the spleen and the bone marrow. Genetically determined." [PMID:12070033]
xref: URL:http\://www.bloodjournal.org/cgi/content/full/100/1/238/DC1/2
is_a: MPATH:510 ! myeloid proliferations (non-reactive)

[Term]
id: MPATH:512
name: myeloproliferative disease
def: "Non-reactive persistent accumulation of non-lymphoid haematopoietic cells in the blood which infiltrate the spleen and the bone marrow." [PMID:12070033]
xref: URL:http\://www.bloodjournal.org/cgi/content/full/100/1/238/DC1/2
is_a: MPATH:510 ! myeloid proliferations (non-reactive)

[Term]
id: MPATH:513
name: Lymphoid neoplasms
def: "Neoplasms of the B or T cell lineage." [PMID:12070034]
is_a: MPATH:335 ! hematopoietic/lymphoid malignancies/disorder

[Term]
id: MPATH:514
name: B cell neoplasms
def: "B cell neoplasms" [Pathbase: Pathology Committee]
is_obsolete: true

[Term]
id: MPATH:515
name: Non-Lymphoid neoplasias
def: "Hematological neoplasias of non-lymphoid origin." [PMID:12070033]
xref: URL:http\://www.bloodjournal.org/cgi/content/full/100/1/238/DC1/2
is_a: MPATH:335 ! hematopoietic/lymphoid malignancies/disorder

[Term]
id: MPATH:516
name: B-cell neoplasms
def: "Neoplasm of the B cell lymphoid lineage." [Pathbase: Curation]
is_a: MPATH:513 ! Lymphoid neoplasms

[Term]
id: MPATH:517
name: precursor B cell neoplasms
def: "Lymphoma originating from precursor B-cells." [PMID:12070034]
is_a: MPATH:516 ! B-cell neoplasms

[Term]
id: MPATH:518
name: precursor B -cell lymphoblastic lymphoma/leukaemia
def: "Lymphoma originating in a precursor B-cell." [PMID:12070034]
synonym: "lymphoblastic leukaemia" RELATED [Pathbase: Curation]
synonym: "lymphoblastic lymphoma" RELATED [Pathbase: Curation]
is_a: MPATH:517 ! precursor B cell neoplasms

[Term]
id: MPATH:519
name: Mature B-cell neoplasms
def: "Lymphomas originating in peripheral B cells." [PMID:12070034]
is_a: MPATH:516 ! B-cell neoplasms

[Term]
id: MPATH:52
name: lipid depletion
def: "Reduction in cellular or plasma lipid content." [Pathbase: Curation]
is_a: MPATH:47 ! intracellular and extracellular depletion

[Term]
id: MPATH:520
name: small B-cell lymphoma
def: "Diffuse accumulation of small mature B-cells." [Book: Morse; et al. (2002) Blood 100; 246-258]
synonym: "small lymphocytic lymphoma" RELATED [Pathbase: Curation]
synonym: "well differentiated lymphocytic lymphoma" RELATED [Pathbase: Curation]
is_a: MPATH:519 ! Mature B-cell neoplasms

[Term]
id: MPATH:521
name: splenic marginal zone lymphoma
def: "A lymphoid proliferation of cells of the marginal zone of the white pulp of the spleen." [PMID:12070034]
synonym: "SMZL" RELATED [Pathbase: Curation]
is_a: MPATH:519 ! Mature B-cell neoplasms

[Term]
id: MPATH:522
name: follicular B cell lymphoma
def: "A lymphoid proliferation composed of a mixture of centroblasts and centrocytes that may or may not have a nodular(follicular)pattern. The follicular dendritic cell network is not present, unlike in the human. The equivalent typical translocation (Chr. 14:18 )seen in humans has not been reported in the mouse." [PMID:12070034]
synonym: "centroblastic/centrocytic lymphoma" RELATED [Pathbase: Curation]
synonym: "follicular center cell lymphoma, small cell or mixed" RELATED [Pathbase: Curation]
synonym: "follicular lymphoma" RELATED [Pathbase: Curation]
is_a: MPATH:519 ! Mature B-cell neoplasms

[Term]
id: MPATH:523
name: Diffuse large B-cell lymphoma
def: "Diffuse proliferation of large B lymphoid cells." [PMID:12070034]
synonym: "DLBCL" RELATED [Pathbase: Curation]
is_a: MPATH:519 ! Mature B-cell neoplasms

[Term]
id: MPATH:524
name: diffuse large B-cell lymphoma, centroblastic type
def: "Diffuse follicular centre cell lymphoma mainly composed of centroblasts." [PMID:12070034]
synonym: "centroblastic lymphoma" RELATED [Pathbase: Curation]
is_a: MPATH:523 ! Diffuse large B-cell lymphoma

[Term]
id: MPATH:525
name: diffuse large B-cell lymphoma, immunoblastic type
def: "Diffuse large B cell lymphoma with increased number of immunoblasts." [PMID:12070034]
synonym: "Immunoblastic lymphoma" RELATED [Pathbase: Curation]
is_a: MPATH:523 ! Diffuse large B-cell lymphoma

[Term]
id: MPATH:526
name: diffuse large B-cell lymphoma, histiocyte associated
def: "Diffuse large B-cell lymphoma with more than 50% histiocytes." [PMID:12070034]
synonym: "DLCL (HS)" RELATED [Pathbase: Curation]
is_a: MPATH:523 ! Diffuse large B-cell lymphoma

[Term]
id: MPATH:527
name: primary mediastinal (thymic) diffuse large B cell lymphoma
def: "Primary B-cell lymphoma of the thymus. Reported in C57BL/6 mice infected with replication defective MuLV. Not clear that this is the equivalent of the human disease." [PMID:12070034]
is_a: MPATH:523 ! Diffuse large B-cell lymphoma

[Term]
id: MPATH:528
name: classic Burkitt lymphoma
def: "Highly proliferative B-cell lymphoma characteristically seen in c-Myc transgenic mice, derived from mature B cells." [PMID:12070034]
is_a: MPATH:519 ! Mature B-cell neoplasms

[Term]
id: MPATH:529
name: Burkitt-like lymphoma
def: "Highly proliferative mature B-cell lymphoma, poorly defined." [PMID:12070034]
is_a: MPATH:519 ! Mature B-cell neoplasms

[Term]
id: MPATH:53
name: osteopenia
def: "Reduced bone mass due to inadequate synthesis of osteoid, resulting in decreased calcification." [ISBN:0781727286]
is_a: MPATH:47 ! intracellular and extracellular depletion

[Term]
id: MPATH:530
name: Plasma cell neoplasms
def: "Diffuse proliferation of mature plasma cells. Clonal by definition. Includes the equivalent of human myeloma (ICD-O 9732/3)." [PMID:12070034]
synonym: "Myeloma ( human )" RELATED [Pathbase: Curation]
xref: URL: http\://emice.nci.nih.gov/emice/mouse_models/organ_models/hema_models/hema_mouse_class
is_a: MPATH:516 ! B-cell neoplasms

[Term]
id: MPATH:531
name: B-natural killer cell lymphoma
def: "Unusual lymphoma type described in thymectomised (SL/Kh x AKR/Ms) F1 mice. No equivalent found in human to date. See reference for detailed phenotype." [Lu; L-M.; et al (1999) Jpn J. Cancer Res. 90: 1218-1223]
is_a: MPATH:516 ! B-cell neoplasms

[Term]
id: MPATH:532
name: plasmacytoma
def: "Diffuse proliferation of mature plasma cells. Clonal by definition." [PMID:12070034]
xref: URL: http\://emice.nci.nih.gov/emice/mouse_models/organ_models/hema_models/hema_mouse_class
is_a: MPATH:530 ! Plasma cell neoplasms

[Term]
id: MPATH:533
name: extraosseous plasmacytoma
def: "Diffuse proliferation of mature plasma cells. Clonal by definition. Frequently found in IL6 transgenic mice. Characteristically involves spleen and nodes rather than peritoneum." [PMID:12070034]
is_a: MPATH:530 ! Plasma cell neoplasms

[Term]
id: MPATH:534
name: anaplastic plasmacytoma
def: "Diffuse proliferation of immature plasma cells or plasma blasts." [PMID:12070034]
is_a: MPATH:530 ! Plasma cell neoplasms

[Term]
id: MPATH:535
name: T-cell neoplasms
def: "Neoplasms derived from cells of the T lymphocyte lineage." [PMID:12070034]
is_a: MPATH:513 ! Lymphoid neoplasms

[Term]
id: MPATH:536
name: precursor T-cell neoplasms
def: "Neoplasms of precursor T cells." [PMID:12070034]
is_a: MPATH:535 ! T-cell neoplasms

[Term]
id: MPATH:537
name: precursor T-cell lymphoblastic lymphoma/leukaemia
def: "Precursor T cell derived neoplasia. Most commonly found in the thymus." [PMID:12070034]
synonym: "thymic lymphoma" RELATED [Pathbase: Curation]
is_a: MPATH:536 ! precursor T-cell neoplasms

[Term]
id: MPATH:538
name: mature T-cell neoplasms
def: "Non-thymic neoplasms of mature T cell origin." [PMID:12070034]
is_a: MPATH:535 ! T-cell neoplasms

[Term]
id: MPATH:539
name: small T-cell lymphoma
def: "Accumulation of small mature T cells. No human counterpart known to date." [PMID:12070034]
is_a: MPATH:538 ! mature T-cell neoplasms

[Term]
id: MPATH:54
name: osteoporosis
def: "Reduction in the quantity of bone or atrophy of skeletal tissue. More severe than MPATH: 53 with gross changes to bone matrix." [ISBN:0781727286]
is_a: MPATH:47 ! intracellular and extracellular depletion

[Term]
id: MPATH:540
name: T cell neoplasms character undetermined
def: "T cell neoplasms which cannot currently be classified into known subtypes." [PMID:12070034]
is_a: MPATH:535 ! T-cell neoplasms

[Term]
id: MPATH:541
name: T large cell anaplastic lymphoma
def: "Diffuse large pleiomorphic T cell lymphoma. This entity does not correspond to human anaplastic large cell lymphoma." [PMID:12070034]
is_a: MPATH:540 ! T cell neoplasms character undetermined

[Term]
id: MPATH:542
name: T natural killer cell lymphoma
def: "Neoplasm of large granular T cells of CD8 phenotype." [PMID:12070034]
is_a: MPATH:535 ! T-cell neoplasms

[Term]
id: MPATH:543
name: cholangioma
def: "Benign neoplasm of the biliary duct. Occurs in solid and cystic forms. (M-8160/0)." [Pathbase: Pathology Committee]
is_a: MPATH:352 ! hepatic tumor

[Term]
id: MPATH:544
name: hepatocholangiocellular adenoma
def: "Benign tumor of unknown origin showing features of hepatocelluar adenoma and cholangioma." [Pathbase: Pathology Committee]
is_a: MPATH:254 ! complex tumor
is_a: MPATH:270 ! adenoma
is_a: MPATH:352 ! hepatic tumor

[Term]
id: MPATH:545
name: hepatocholangiocellular carcinoma
def: "Malignant tumor of unknown origin showing features of hepatocelluar carcinoma and cholangiocarcinoma. (M-8180/3)." [Pathbase: Pathology Committee]
is_a: MPATH:254 ! complex tumor
is_a: MPATH:352 ! hepatic tumor
is_a: MPATH:549 ! carcinoma

[Term]
id: MPATH:546
name: blepharitis
is_a: MPATH:212 ! inflammation
created_by: George Gkoutos
creation_date: 2011-03-22T03:07:49Z

[Term]
id: MPATH:547
name: mucous secretions
def: "Extracellular accumulation of mucous secretions." [Pathbase: Pathology Committee]
comment: Mucus is the clear viscous secretion of the mucous membranes. Consisting of mucin, epithelial cells, leukocytes and various inorganic salts dissolved in water.
is_a: MPATH:33 ! intracellular and extracellular accumulation

[Term]
id: MPATH:548
name: papillary transitional cell carcinoma
def: "A generally malignant neoplasm consisting of villous or arborescent outgrowths of fibrovascular stroma covered by atypical neoplastic epithelial or urothelial cells cells." [Book: Kunze; E. (1994) Preneoplastic and neoplastic lesions of the Rat urinary bladder. In; Pathology of Neoplasia and Preneoplasia in Rodents. Eds. Bannach; P.;  and Goessner; W.;  Vol 1 p 114. Schattauer; Stuttgart New York]
is_a: MPATH:264 ! fibroepithelial tumor
is_a: MPATH:450 ! transitional cell tumor

[Term]
id: MPATH:549
name: carcinoma
def: "Any of various types of malignant neoplasm derived from epithelial cells, chiefly glandular (adenocarcinoma) or squamous (squamous cell carcinoma)." [Pathbase: Curation]
is_a: MPATH:218 ! neoplasm

[Term]
id: MPATH:55
name: developmental and structural abnormality
def: "Developmental and structural abnormalities occurring during embryonic development or during adult life." [Pathbase: Pathology Committee]
is_a: MPATH:603 ! pathological anatomical entity

[Term]
id: MPATH:550
name: sarcoma
def: "A connective tissue neoplasm, usually highly malignant, formed by proliferation of mesodermal cells." [Pathbase: Pathology Committee]
is_obsolete: true

[Term]
id: MPATH:551
name: sarcoma
def: "A connective tissue neoplasm, usually highly malignant, formed by proliferation of mesodermal cells." [Pathbase: Curation]
is_a: MPATH:218 ! neoplasm

[Term]
id: MPATH:552
name: Clara cell adenoma
def: "Benign tumor of the Clara cells of the bronchioalveolar epithelium." [Book: Hahn; F.F. and Boorman; GA. neoplasia and pre-neoplasia in the lung. In Pathology of Neoplasia and Preneoplasia in Rodents. Vol.2. p 39. (1997) Schattauer ( Stuttgart and New York)]
comment: Merged with MPATH:272 following recommendations of MMHC 2003.
xref: URL: http\://emice.nci.nih.gov/mouse_models/organ_models/lung_models/murinecancer/tumorclass
is_obsolete: true

[Term]
id: MPATH:553
name: neuritis
def: "Inflammation of a nerve." [ISBN:0781727286]
is_a: MPATH:212 ! inflammation

[Term]
id: MPATH:554
name: dystrophy
def: "Regressive changes which may increase in severity, and which may result from defective nutrition or support of a tissue or organ." [Pathbase: Pathology Committee]
comment: Most often used for diseases in which a structure does not develop properly (not necessarily in an embryonic context) and undergoes degradation.
is_a: MPATH:14 ! process of degenerative change

[Term]
id: MPATH:555
name: mineralisation
def: "Deposition of any homogeneous inorganic material." [ISBN:0781727286]
is_a: MPATH:33 ! intracellular and extracellular accumulation

[Term]
id: MPATH:556
name: potentially cancerous lesions
def: "Lesions which in some cases have the potential to become progressively growing malignant tumors." [Pathbase: Pathology Committee]
is_a: MPATH:218 ! neoplasm

[Term]
id: MPATH:557
name: aberrant crypt foci
def: "Sensu gastrointsestinal tract. visible microscopically in whole mount colonic tissue. One or more crypts larger than most, have a thickened layer of epithelial cells that stain more intensely with methylene blue. Some have a slit shaped luminal opening, and increased pericryptal space and are elevated from the focal plane of the microscope. ACF is not a histologic diagnosis." [PMID:12612914]
comment: Use IEN1 MPATH:130 instead. Suppressed as not strictly a histological diagnosis.
synonym: "ACF" RELATED [Pathbase: Curation]
is_obsolete: true

[Term]
id: MPATH:558
name: adenomyoepithelioma
def: "Adenocarcinoma type tumor with both glandular and squamous differentiation. (M-8983/0)." [PMID:10713680]
is_a: MPATH:254 ! complex tumor

[Term]
id: MPATH:559
name: Acinar adenocarcinoma
def: "Tumor composed of small glandular clusters with small lumens." [PMID:10713680]
is_a: MPATH:268 ! adenocarcinoma

[Term]
id: MPATH:56
name: developmental and adult structural  defect
def: "Structural, physical or other general defect of prenatal development of the embryo, the placenta or the adult." [Pathbase: Pathology Committee]
is_a: MPATH:55 ! developmental and structural abnormality

[Term]
id: MPATH:560
name: cribriform adenocarcinoma
def: "Tumor composed of sheets or nests of cells forming lumens with round, punched out spaces." [PMID:10713680]
is_a: MPATH:268 ! adenocarcinoma

[Term]
id: MPATH:561
name: adenosquamous carcinoma
def: "Mixed adeno- and squamous cell carcinoma. Not yet reported in mice. M-8560/3." [PMID:12612914]
is_a: MPATH:268 ! adenocarcinoma
is_a: MPATH:442 ! squamous cell tumor

[Term]
id: MPATH:562
name: torsion
def: "The twisting of a bodily organ or part on its own axis." [Pathbase: Pathology Committee]
is_a: MPATH:56 ! developmental and adult structural  defect

[Term]
id: MPATH:563
name: mucinous carcinoma
def: "carcinoma derived from gastrointestinal epithelium with a high mucinous content. (M-8480/3)." [PMID:12612914]
synonym: "mucinous adenocarcinoma" RELATED [Pathbase: Curation]
is_a: MPATH:268 ! adenocarcinoma

[Term]
id: MPATH:564
name: glioblastoma
def: "Develop primarily through increasing anaplasia of well differentiated gliomas, mainly astrocytomas or oligodendrogliomas. Typically large and contain cells of different sizes with irrregular nuclei and atypical mitotic figures. (M-9440/3)." [ISBN-13:9783794515530]
comment: Also see Weiss, W.W, Israel, M. Cobbs, C., et al. (2002) Oncogene 21, 7453-7463.
synonym: "glioblastoma multiforme" RELATED [Pathbase: Curation]
synonym: "monstrocytoma" RELATED [Pathbase: Curation]
is_a: MPATH:249 ! glioma

[Term]
id: MPATH:565
name: tumors of neurepithelial tissue
def: "Tumors of neuronal and non-neuronal cells derived from embryonic neurepithelium." [Pathbase: Pathology Committee]
is_a: MPATH:243 ! central nervous system tumor

[Term]
id: MPATH:566
name: tumors of the meninges
def: "tumors of the meninges" [Pathbase: Curation]
is_a: MPATH:243 ! central nervous system tumor

[Term]
id: MPATH:567
name: pilocytic astrocytoma
def: "Glial cell derived tumor composed of bipolar cells with long `hairlike` GFAP-positive processes. (M9421/1)." [Nervous System. Radovsky A and Mahler; J.S. In: Maronpot; R. Pathology of the Mouse. (1999) Cache River Press. Vienna IL]
comment: Often cystic in children and generally considered benign.
synonym: "cystic cerebellar astrocytoma" RELATED [Pathbase: Curation]
is_a: MPATH:244 ! astrocytoma

[Term]
id: MPATH:568
name: mixed glioma
def: "Mixed tumor containing astrocytes within an oligodendroglioma or vice versa. In some cases both components may be neoplastic. (M-9382/3)." [ISBN-13:9783794515530]
comment: Also see Weiss, W.W, Israel, M. Cobbs, C., et al. (2002) Oncogene 21, 7453-7463.
is_a: MPATH:249 ! glioma
is_a: MPATH:254 ! complex tumor

[Term]
id: MPATH:569
name: granular cell tumor
def: "granular cell tumor" [ISBN-13:9783794515530]
comment: Subsumed into MP:413 as incidence in meninges, whilst a characteristic lesion, is the same type of tumor as that originally classified under myomatous tumors. Describe meningeal granular cell tumor using MP:413 and the anatomical descriptor.
is_obsolete: true

[Term]
id: MPATH:57
name: agenesis
def: "Failure of a tissue or organ to develop." [Pathbase: Pathology Committee]
synonym: "Agenesia" RELATED [Pathbase: Curation]
is_a: MPATH:599 ! developmental process abnormalities

[Term]
id: MPATH:570
name: peripheral nervous system tumors
def: "Tumors of the peripheral nervous system." [Pathbase: Pathology Committee]
is_a: MPATH:218 ! neoplasm

[Term]
id: MPATH:571
name: pilomatricoma
def: "Tumor composed of the epithelial components of the most proximal (trichogenic) portion of the hair follicle associated with an aberrent hair cortex type of cornification (ghost cells or shadow cells). The most primitive cellular component consists of basophilic cells having scanty cytoplasm and nuclei that occasionally overlap to some extent. In humans mineralisation is common." [See: Gat; U.; DasGupta; R.; Degenstein; L. and Fuchs; E. (1998) De Novo hair follicle morphogenesis and hair tumors in mice expressing a truncated beta-catenin in skin Cell; 95; 605-614.]
is_a: MPATH:575 ! basaloid follicular neoplasms

[Term]
id: MPATH:572
name: ossifying fibroma
def: "Ossifying fibromas are benign tumors derived from pluripotential mesenchymal stem cells or osteoblasts. Occur spontaneously or in response to radiation. Preferentially located in mandible, maxilla and caudal spine. Composed of a characteristically regular trabecular bone pattern embedded in a fibrous stroma. Proliferating component consists of spindle cells which give rise to cuboidal osteoblasts to form rounded bodies or trabeculae. Bone trabeculae resemble the alphabet soup shapes characteristic of fibrous dysplasia in humans. In contrast to fibrous dysplasia the bone trabeculae of ossifying fibroma are mostly lamellar and ringed by active osteoblasts." [Book: Luz A; Goessner; W.;and Murray AB.(1991) Ossifying fibroma; mouse. In; Jones TC; Mohr U; Hunt RD (eds) Monographs on pathology of laboratory animals. Cardiovascular and musculoskeletal systems. Springer; Berlin Heidelberg New York Tokyo; pp 228-232]
is_a: MPATH:388 ! osseous and chondromatous tumor

[Term]
id: MPATH:573
name: inverted transitional cell papilloma
def: "Pre-malignant lesion of transitional cells, papillomatous form, in which proliferating epithelium is invaginated beneath the surface." [Pathbase: Curation]
is_a: MPATH:453 ! transitional cell papilloma

[Term]
id: MPATH:574
name: nephroblastomatosis
def: "Persistence of metanephrogenic blastema or its presence in the wrong place or at the wrong time. Associated with hyperplastic nephrogenic rests." [PMID:8383276]
is_a: MPATH:64 ! developmental dysplasia

[Term]
id: MPATH:575
name: basaloid follicular neoplasms
def: "This is a new diagnostic term that the MMHC pathology panel felt best described a diagnostically challenging set of tumors that share the feature of being compose of basaloid cells showing follicular differentiation to some extent. These tumors are common in GEM involving the hedgehog signaling pathway and frequently have more than one of the histologic patterns listed below. The designation of benign and malignant has been excluded from the primary diagnosis purposely, as this is frequently difficult to determine in these characteristically well circumscribed tumors. The presence of a disorganized (non-palisaded) sheet-like growth pattern, tumor necrosis, or numerous mitoses are felt to represent malignant transformation." [URL:http\://emice.nci.nih.gov/emice/mouse_models/organ_models/skin_models]
is_a: MPATH:219 ! adnexal and skin appendage tumor

[Term]
id: MPATH:576
name: trichofolliculoma
def: "Basaloid neoplasm with numerous mature hair follicles and hair formation." [URL:http\://emice.nci.nih.gov/emice/mouse_models/organ_models/skin_models]
relationship: part_of MPATH:575 ! basaloid follicular neoplasms

[Term]
id: MPATH:577
name: spiradenoma
def: "Cellular neoplasm with well formed palisades of basaloid cells adjacent to less basophilic smaller cells with occasional central deposition of amorphous eosinophilic material. These tumors share some features with cylindroma type tumors but have a less well developed jigsaw puzzle-like architecture and tend to be more cellular." [URL:http\://emice.nci.nih.gov/emice/mouse_models/organ_models/skin_models/hierarchical_classification]
is_a: MPATH:575 ! basaloid follicular neoplasms

[Term]
id: MPATH:578
name: trichoblastoma
def: "Basaloid neoplasm with frequent primitive hair follicles." [URL:http\://emice.nci.nih.gov/emice/mouse_models/organ_models/skin_models/hierarchical_classification]
is_a: MPATH:575 ! basaloid follicular neoplasms

[Term]
id: MPATH:579
name: ulcer
def: "Loss of epithelium and the basement membrane (full thickness). Cf Erosion." [Pathbase: Pathology Committee]
is_a: MPATH:1 ! cell and tissue damage

[Term]
id: MPATH:58
name: aplasia
def: "Absence of an organ or tissue coupled with persistence of the organ/tissue primordium, which fails to develop completely." [ISBN:0781727286]
is_a: MPATH:599 ! developmental process abnormalities

[Term]
id: MPATH:580
name: Erosion
def: "Partial epithelial denudation not penetrating to the basement membrane." [Pathbase: Pathology Committee]
is_a: MPATH:15 ! general degenerative process

[Term]
id: MPATH:581
name: desmoplasia
def: "Connective tissue proliferative reaction induced by a neoplastic process." [Pathbase: Pathology Committee]
synonym: "scirrhous" RELATED [Pathbase: Curation]
synonym: "sclerosis" RELATED [Pathbase: Curation]
is_a: MPATH:604 ! defective growth and differentiation process

[Term]
id: MPATH:582
name: Cicatricial alopecia
def: "Scarring of the hair follicle without affecting the adjacent dermis. Pigment may be associated with fibrous tract in pigmented individuals." [Pathbase: Curation]
is_a: MPATH:26 ! alopecia

[Term]
id: MPATH:583
name: scarring alopecia
def: "Loss of hair follicles in a diffuse dermal scar." [Pathbase: Pathology Committee]
is_a: MPATH:26 ! alopecia

[Term]
id: MPATH:584
name: myelofibrosis
def: "In mice the term refers to accumulation of fibrous connective tissue in the medullary cavity of bones; usually in old mice. In humans the term is synonymous with myeloid metaplasia." [Pathbase: Pathology Committee]
is_a: MPATH:25 ! tissue specific degenerative process

[Term]
id: MPATH:585
name: acidophilic macrophage pneumonia
def: "A mixed inflammatory infiltrate in the pulmonary airways with predominant intra-alveolar macrophage component with intra- and extracellular, elongated, bright eosinophilic/acidophilic crystals." [:Murray AB; Luz A ( 1990 ) Acidophilic macrophage pneumonia in laboratory mice. Vet Pathol.  27; 274-81]
comment: Crystals and acidophilic material have been reported as various materials including Ym1 and Ym2 proteins and blood pigment derivatives and Eotaxin.
is_a: MPATH:33 ! intracellular and extracellular accumulation

[Term]
id: MPATH:586
name: polycystic disease
def: "A group of degenerative disorders resulting in multiple cysts in tissues." [Pathbase: Pathology Committee]
synonym: "polycystic kidney disease" RELATED [Pathbase: Curation]
synonym: "polycystic liver disease" RELATED [Pathbase: Curation]
synonym: "polycystic ovary" RELATED [Pathbase: Curation]
is_a: MPATH:25 ! tissue specific degenerative process

[Term]
id: MPATH:587
name: Cribriform epididymal hyperplasia
def: "The lesion is characterized microscopically by epithelial cells with atypical hyperchromatic nuclei, vacuolization, intratubular lumina formation, infrequent apoptosis, and rare mitotic figures. In contrast to germ cells, the cells of CEH do not express alpha-fetoprotein, carcinoembryonic antigen, or S-100. Ultrastructurally, the cells are pleomorphic with stereocilia at their apical borders and within intratubular lumina, and are supported by a basement membrane. CEH does not appear to be a preneoplastic change." [Journal: La Perle KM; Blomme EA; Sagartz JE; Capen CC (2002) Epididymal cribriform hyperplasia with nuclear atypia in p53 homozygous knockout. Comp Med.  2002 52\:568-71.]
comment: Cribriform epididymal hyperplasia was initially described as an incidental finding in human orchidectomy specimens. Recently, this condition was also described in mice, homozygous for a targeted mutation in p53.
is_a: MPATH:602 ! hyperplastic tissue

[Term]
id: MPATH:588
name: Dysplasia
def: "Dysplasia" [Pathbase: Pathology Committee]
is_obsolete: true

[Term]
id: MPATH:589
name: dysplasia
def: "Distortion or deficiency of the tissue or cellular architecture." [Pathbase: Pathology Committee]
comment: Note that with respect to developmental processes the term dysplasia is often used with greater specificity to describe aberrant developmental processes of proliferation and differentation, in which case MPATH: 64 Developmental dysplasia should be used.
is_a: MPATH:604 ! defective growth and differentiation process

[Term]
id: MPATH:59
name: defective branching morphogenesis
def: "Defect in the process determining number, angle, pattern or rate of branching of tubular branched structures eg. Glandular ducts." [Pathbase: Pathology Committee]
is_a: MPATH:599 ! developmental process abnormalities

[Term]
id: MPATH:590
name: fibro-osseous lesion
def: "Lesion of bone showing accelerated osteoclastic bone resorption coupled with fibroplasia. Later stages show proliferation of osteoblasts." [Book: Albassam MA; Courtney CL (1996) Nonneoplastic and neoplastic lesions of the bone. In; Mohr U; Dungworth DL; Capen CC; Carlton WW; Sundberg JP; Ward JM (eds) Pathobiology of the aging mouse. Vol 2. Musculoskeletal system. ILSI Press; Washington D.C.; pp 425-437]
comment: The benign fibro-osseous lesions (BFOL) represent a clinically diverse group of disorders of bone that share similar histopathologic features. As a group, they are relatively common in the craniofacial complex, especially the jaws. Common in some inbred strains notably B6C3F1 females. Note that many of the synonyms have been used historically and may not be accurate. See:  Albassam MA, Courtney CL (1996) Nonneoplastic and neoplastic lesions of the bone. In: Mohr U, Dungworth DL, Capen CC, Carlton WW, Sundberg JP, Ward JM (eds) Pathobiology of the aging mouse. Vol 2. Musculoskeletal system. ILSI Press, Washington D.C., pp 425-437. AND  Albassam MA, Wojcinski ZW, Barsoum NJ, Smith, GS (1991) Spontaneous fibro-osseous proliferative lesions in the sternums and femurs of B6C3F1 mice. Vet Path 28: 381-388.
synonym: "fibrous dysplasia" RELATED [Pathbase: Curation]
synonym: "fibrous osteodystrophy" RELATED [Pathbase: Curation]
synonym: "osteodysplasia" RELATED [Pathbase: Curation]
synonym: "osteodystrophy" RELATED [Pathbase: Curation]
synonym: "osteofibrosis" RELATED [Pathbase: Curation]
is_a: MPATH:589 ! dysplasia

[Term]
id: MPATH:591
name: fatty infiltration
def: "Accumulation of mature adipose tissue in a healing wound site or otherwise in response to tissue damage." [Pathbase: Pathology Committee]
is_a: MPATH:607 ! healing and repair structure

[Term]
id: MPATH:592
name: osteopetrosis
def: "Excessive formation of dense trabecular bone and mineralized cartilage, especially in long bones, leading to obliteration of marrow spaces and to anemia with myeloid metaplasia and hepatosplenomegaly beginning in infancy, to bone fragility, and to progressive deafness and blindness." [PMID:15625335]
synonym: "Albers-Schoenberg disease" RELATED [Pathbase: Curation]
synonym: "marble bone disease" RELATED [Pathbase: Curation]
synonym: "marble bones" RELATED [Pathbase: Curation]
is_a: MPATH:589 ! dysplasia

[Term]
id: MPATH:593
name: Myeloma
def: "Plasma cell myeloma - (ICD-O 9732/3)." [Pathbase: Pathology Committee]
is_obsolete: true

[Term]
id: MPATH:594
name: cystic hyperplasia
def: "Formation of multiple retention cysts from obstruction of ducts or glands by hyperplasia of the lining epithelium." [Pathbase: Pathology Committee]
is_a: MPATH:135 ! epithelial and stromal hyperplasia

[Term]
id: MPATH:595
name: extramedullary hemopoiesis
def: "The formation of and development of blood cells outside the red pulp of the spleen. Composed of varying numbers of megakaryocytes as well as myeloid and erythroid precursors." [:Ward; J.M.; Mann; P.C.; Mrishima; H.; and Frith; C.H. Thymus; Spleen and Lymph nodes. Ch 13.  p342. In Maronpot; R. Pathology of the Mouse. (1999) Cache River Press. Vienna IL]
is_a: MPATH:515 ! Non-Lymphoid neoplasias

[Term]
id: MPATH:596
name: pathological process
def: "The organic response of tissues to external insult, injury or underlying genetic or epigenetic lesion." [Pathbase: Pathology Committee]
is_a: MPATH:0 ! pathology_ontology

[Term]
id: MPATH:597
name: cell and tissue damage process
def: "Processes occurring during cell and tissue damage of either intrinsic or extrinsic etiology." [Pathbase: Pathology Committee]
is_a: MPATH:596 ! pathological process

[Term]
id: MPATH:598
name: degenerative entity
def: "degenerative entity" [Pathbase: Pathology Committee]
is_obsolete: true

[Term]
id: MPATH:599
name: developmental process abnormalities
def: "developmental process abnormalities" [Pathbase: Pathology Committee]
is_a: MPATH:596 ! pathological process

[Term]
id: MPATH:6
name: caseous necrosis
def: "Necrosis characteristic of some inflammatory conditions which represents necrosis with loss of structure of the various cellular and tissue elements; affected tissue manifests a friable, crumbly consistency." [ISBN:0781727286]
is_a: MPATH:4 ! necrosis

[Term]
id: MPATH:60
name: communication defect
def: "Failure of two cavities, voids or lumens to connect." [Pathbase: Curation]
is_a: MPATH:56 ! developmental and adult structural  defect

[Term]
id: MPATH:600
name: branching defect
def: "Aberrant branch or branching pattern of a branched structure such as the bronchus." [Pathbase: Curation]
is_a: MPATH:56 ! developmental and adult structural  defect

[Term]
id: MPATH:601
name: developmental hypertrophy
def: "Increase of the size or cellularity of an organ or tissue as a consequence of loss of normal regulation of cell proliferation." [Pathbase: Pathology Committee]
is_a: MPATH:599 ! developmental process abnormalities

[Term]
id: MPATH:602
name: hyperplastic tissue
def: "An organ or a tissue with an abnormal increase in the number of cells as a consequence of cell proliferation." [Pathbase: Pathology Committee]
is_a: MPATH:126 ! growth and differentiation defect

[Term]
id: MPATH:603
name: pathological anatomical entity
def: "Anatomically located instance of pathological response or entity." [Pathbase: Pathology Committee]
is_a: MPATH:0 ! pathology_ontology

[Term]
id: MPATH:604
name: defective growth and differentiation process
def: "Abnormal increase or decrease in the rate of cell growth or cell division including associated changes in the differentiation state of adult cells." [Pathbase: Pathology Committee]
comment: Excludes abnormalities of developmental proliferation and differentiation.
is_a: MPATH:596 ! pathological process

[Term]
id: MPATH:605
name: metaplastic tissue
def: "A tissue or group of cells in which there has been abnormal transformation of an fully differentiated adult cell or tissue of one kind into a differentiated tissue of another kind." [Pathbase: Pathology Committee]
comment: Nearly exclusively used in an adult context.
is_a: MPATH:126 ! growth and differentiation defect

[Term]
id: MPATH:606
name: neoplasia
def: "The pathological process that results in the formation and growth of a neoplasm." [Pathbase: Pathology Committee]
comment: Literally: new growth of cells. Neoplasia refers to the unscheduled or abnormal growth of cells, potentially resulting in a benign or malignant tumour. Neoplasms include potentially cancerous lesions as well as full malignancies but not all neoplasms are potentially cancerous.
synonym: "neoplastic process" RELATED [Pathbase: Curation]
is_a: MPATH:596 ! pathological process

[Term]
id: MPATH:607
name: healing and repair structure
def: "Physical entity or structure associated with normal or abnormal tissue healing or repair following extrinsic or intrinsic damage." [Pathbase: Pathology Committee]
is_a: MPATH:603 ! pathological anatomical entity

[Term]
id: MPATH:608
name: abscess
def: "A circumscribed collection of purulent exudate frequently associated with swelling and other signs of inflammation." [ISBN:0781727286]
comment: Generally occur following damage or infection with subsequent inflammatory response. Result of the body`s defensive reaction to foreign material.
is_a: MPATH:607 ! healing and repair structure

[Term]
id: MPATH:609
name: empyema
def: "Pus in a body cavity; when used without qualification, refers specifically to pyothorax." [ISBN:0781727286]
is_a: MPATH:607 ! healing and repair structure

[Term]
id: MPATH:61
name: curvature defect
def: "Inappropriate curvature of a structure." [Pathbase: Curation]
is_a: MPATH:56 ! developmental and adult structural  defect

[Term]
id: MPATH:610
name: angiectasia
def: "Dilatation of a blood vessel or valve." [ISBN:0781727286]
is_a: MPATH:474 ! ectasia

[Term]
id: MPATH:611
name: glossitis
def: "Acute or chronic inflammation of the tongue." [Pathbase: Pathology Committee]
is_a: MPATH:212 ! inflammation

[Term]
id: MPATH:612
name: Abscess
def: "A circumscribed collection of purulent exudate frequently associated with swelling and other signs of inflammation." [ISBN:0781727286]
comment: Alternately a cavity formed by liquefactive necrosis within solid tissue.    Obsoleted by MPATH 608
is_obsolete: true

[Term]
id: MPATH:613
name: pigmentation
def: "Coloration, either normal or pathologic, of the skin or tissues resulting from a deposit of pigment." [ISBN:0781727286]
is_a: MPATH:33 ! intracellular and extracellular accumulation

[Term]
id: MPATH:614
name: concretion
def: "Solid material formed by aggregation of discrete units or particles." [ISBN:0781727286]
is_a: MPATH:33 ! intracellular and extracellular accumulation

[Term]
id: MPATH:615
name: cardiomyopathy
def: "A disease of the heart muscle or myocardium proper." [:NCI Thesaurus / A7567983]
comment: Cardiomyopathies may be classified as either primary or secondary, on the basis of etiology, or on the pathophysiology of the lesion: hypertrophic, dilated, or restrictive.
is_a: MPATH:25 ! tissue specific degenerative process

[Term]
id: MPATH:616
name: hyperostosis
def: "Hypertrophy of bone characterised by an abnormal increase in non-neoplastic skeletal bone mass. These may be proliferative or non-proliferative lesions." [Long; P.H.; and Leininger; J.R ( 1999) Bones Joints and synovia; p663. in: Pathology of the Mouse. Ed Maronpot; R. Cache River Press]
synonym: "osteosclerosis" RELATED [Pathbase: Curation]
is_a: MPATH:159 ! hypertrophy

[Term]
id: MPATH:617
name: focus of cellular alteration
def: "Focal lesions of hepatocytes characterised primarily by altered cytoplasmic tinctorial properties. Classified as basophilic, eosinophilic, clear cell or mixed type." [Pathbase: Mohr]
comment: More recently amphophilic cell foci, diffusely basophilic cell foci and vacuolated cell foci have been described.
synonym: "Areas of cellular alteration" RELATED [Pathbase: Curation]
synonym: "Enzyme altered focus" RELATED [Pathbase: Curation]
synonym: "Focus of altered hepatocytes (fah)" RELATED [Pathbase: Curation]
synonym: "Hyperplastic focus" RELATED [Pathbase: Curation]
synonym: "Phenotypically altered focus" RELATED [Pathbase: Curation]
synonym: "Preneoplastic focus" RELATED [Pathbase: Curation]
is_a: MPATH:556 ! potentially cancerous lesions

[Term]
id: MPATH:618
name: myeloid hyperplasia
def: "Hyperplasia of myeloid lineage, usually in the spleen." [Pathbase: Pathology Committee]
comment: Myeloid hyperplasia ia a common diagnosis in mouse spleen. In the normal mouse spleen, a low degree of production of myeloid cells occurs (neutrophils, erythroid cells and megakaryocytes). Commonly in aging mice, due to tumors and inflammatory lesions, the mouse myeloid system in bone marrow and spleen react and become hyperplastic. In the spleen it is diagnosed as  "myeloid hyperplasia" (MH), in the past it was often extramedullary hematopoiesis, which is still used by some but it is normal to a low degree in normal mouse  spleen.
is_a: MPATH:515 ! Non-Lymphoid neoplasias

[Term]
id: MPATH:619
name: truncoconal septal defect
def: "Septal defect lying between the aorta and pulmonary trunks caused by failure of the spiral septum to separate the truncus arteriosus." [Pathbase: Pathology Committee]
is_a: MPATH:93 ! cardiac septation defect

[Term]
id: MPATH:62
name: cyst
def: "Formation of an epithelium bounded cavity not associated with neoplasia." [Pathbase: Pathology Committee]
is_a: MPATH:56 ! developmental and adult structural  defect

[Term]
id: MPATH:620
name: inter-atrial septal defect
def: "Incomplete closure of the inter-atrial septum due to failure of the primary or secondary septum." [Pathbase: Curation]
is_a: MPATH:93 ! cardiac septation defect

[Term]
id: MPATH:621
name: inter-ventricular septal defect
def: "Failure of the inter-ventricular septum to completely close between the left and right ventricles." [Pathbase: Curation]
is_a: MPATH:93 ! cardiac septation defect

[Term]
id: MPATH:622
name: steatosis
def: "Abnormal retention of lipids within a cell. Physically apparent as lipid within liposomes of parenchymal cells." [Pathbase: Curation]
comment: Most commonly associated with degenerative change in the liver.
synonym: "adipose degeneration" RELATED [Pathbase: Curation]
synonym: "fatty change" RELATED [Pathbase: Curation]
synonym: "fatty degeneration" RELATED [Pathbase: Curation]
is_a: MPATH:33 ! intracellular and extracellular accumulation

[Term]
id: MPATH:623
name: synechia
def: "An adhesion, usually between the iris and the cornea or the lens capsule." [Millodot; Michel and Daniel Laby. Dictionary of Ophthalmology. London: Butterworth Heinemann; 2002]
comment: May also be seen in the uterus ( in humans Asherman`s syndrome).
is_a: MPATH:56 ! developmental and adult structural  defect

[Term]
id: MPATH:624
name: involution
def: "Turning in of the edges of a structure." [ISBN:0781727286]
comment: Not return of an enlarged organ to its normal size.
is_a: MPATH:56 ! developmental and adult structural  defect

[Term]
id: MPATH:625
name: avulsion
def: "Tearing away or separation of two structures or parts." [ISBN:0781727286]
is_a: MPATH:56 ! developmental and adult structural  defect

[Term]
id: MPATH:626
name: prolapse
def: "To sink down, said of an organ or other part. A sinking of an organ or other part, especially its appearance at a natural or artificial orifice." [ISBN:0781727286]
is_a: MPATH:56 ! developmental and adult structural  defect

[Term]
id: MPATH:627
name: pyogranulomatous inflammation
def: "An inflammatory process in which there is infiltration of polymorphonuclear cells into a more chronic area of inflammation characterized by mononuclear cells, macrophages, lymphocytes and possibly plasma cells." [Pathbase: Pathology Committee]
is_a: MPATH:215 ! granulomatous inflammation

[Term]
id: MPATH:628
name: pyogenic granuloma
def: "A small rounded mass of inflamed, highly vascular granulation tissue on the skin, frequently having an ulcerated surface. More likely a true neoplasm rather than a reactive lesion." [Mills; S.E.; Cooper; P.H. & Fechner; R.E. (1980). Lobular capillary hemangioma: the underlying lesion of pyogenic granuloma. A study of 73 cases from the oral and nasal mucous membranes. Am J Surg Pathol; 4; 470-9.]
synonym: "lobular capillary hemangioma" RELATED [Pathbase: Curation]
is_a: MPATH:240 ! hemangioma

[Term]
id: MPATH:629
name: cavernous hemangioma
def: "Deep cutaneous hemangioma with large dilated vascular spaces that manifests spontaneous involution." [ISBN:0781727286]
is_a: MPATH:240 ! hemangioma

[Term]
id: MPATH:63
name: depletion
def: "The removal of accumulated fluids or solids." [Pathbase: Pathology Committee]
is_a: MPATH:599 ! developmental process abnormalities

[Term]
id: MPATH:630
name: karyomegaly
def: "Abnormally increased nuclear size." [Pathbase: Pathology Committee]
is_a: MPATH:460 ! nuclear defect

[Term]
id: MPATH:631
name: hypertrophic tissue
def: "Tissue or cells undergoing hypertrophy, MPATH: 159." [Pathbase: Pathology Committee]
is_a: MPATH:126 ! growth and differentiation defect

[Term]
id: MPATH:632
name: Hepatocytomegaly
def: "Increase in size of hepatocytes characterised by organelle hyperplasia and enlarged cellular volume." [Journal: Ward; J.M.; Anver; M.R.; Haines; D.C. & Benveniste; R.E. (1994). Chronic active hepatitis in mice caused by Helicobacter hepaticus. Am J Pathol; 145; 959-68.]
comment: Hepatocytomegaly is an enlargement of the hepatocytes and is generally classified into three types: hepatocellular hypertrophy, megalocytosis, and hepatocellular vacuolation. Hepatocellular hypertrophy is an enlargement of cellular diameter without accompanying nuclear changes, leading to a net gain in the dry mass of the liver. Megalocytosis is characterized by enlargement of both the cell and the nucleus, and hepatocellular vacuolation is characterized by vacuolation, or formation of pockets of fluid within the hepatocytes.
xref: PMID:7943185
is_a: MPATH:631 ! hypertrophic tissue

[Term]
id: MPATH:633
name: cholelithiasis
def: "Presence of concretions in the gallbladder or bile ducts." [ISBN:0781727286]
is_a: MPATH:614 ! concretion

[Term]
id: MPATH:634
name: furunculosis
def: "Focal suppurative inflammation of the skin and subcutaneous tissues, enclosing a central slough or `core`." [ISBN:9780702027888]
synonym: "Boil" RELATED [Pathbase: Curation]
is_a: MPATH:212 ! inflammation

[Term]
id: MPATH:635
name: hydronephrosis
def: "Swelling of the kidneys when urine flow is obstructed in any of part of the urinary tract." [ISBN:9780702027888]
is_a: MPATH:33 ! intracellular and extracellular accumulation

[Term]
id: MPATH:636
name: steatitis
def: "Inflammation of fatty tissue." [Pathbase: Pathology Committee]
is_a: MPATH:212 ! inflammation

[Term]
id: MPATH:637
name: bursal cyst
def: "A retention cyst, resulting from an obstruction to the duct of a gland, within a bursa." [Pathbase: Pathology Committee]
is_a: MPATH:62 ! cyst

[Term]
id: MPATH:638
name: cellulitis
def: "An acute, diffuse, spreading, edematous, suppurative inflammation of the deep subcutaneous tissues and sometimes muscle, which may be associated with abscess formation." [URL:http\://cancerweb.ncl.ac.uk/cgi-bin/omd?action=Search+OMD&query=cellulitis]
comment: It is usually caused by infection of an operative or traumatic wound, burn or other cutaneous lesion by various bacteria, but group A streptococci and Staphylococcus aureus are the most common aetiological agents.
is_a: MPATH:212 ! inflammation

[Term]
id: MPATH:639
name: hydrocephalus
def: "Accumulation of water in the ventricles of the brain." [Pathbase: Pathology Committee]
is_a: MPATH:33 ! intracellular and extracellular accumulation

[Term]
id: MPATH:64
name: developmental dysplasia
def: "Abnormal development (of organs or tissues) or an abnormal structure resulting from such growth." [Pathbase: Pathology Committee]
comment: The word dysplasia as commonly used refers to a precursor state to neoplasia. This is not the context used for this MPATH term.
is_a: MPATH:599 ! developmental process abnormalities

[Term]
id: MPATH:640
name: osteoid deposition
def: "Deposition of organic bone matrix." [Pathbase: Pathology  Committee]
is_a: MPATH:178 ! extracellular matrix deposition

[Term]
id: MPATH:641
name: epidermal inclusion cyst
def: "Intradermal or subcutaneous cyst, the wall of which is stratified epithelium containing keratohyalin granules, surrounding a core of debris." [Pathbase: Curation]
is_a: MPATH:62 ! cyst

[Term]
id: MPATH:642
name: cholesterol deposition
def: "Intra or extracellular deposition of cholesterol." [Pathbase: Curation]
comment: Often diagnosed morphologically by the presence of cholesterol clefts - bare regions of a section where accumulated cholesterol has been removed by histological processing.
is_a: MPATH:33 ! intracellular and extracellular accumulation

[Term]
id: MPATH:643
name: serous exudate
def: "Non-cellular fluid that filters from the circulatory system and accumulates in lesions or areas of inflammation." [Pathbase: Pathology  Committee]
is_a: MPATH:106 ! fluid accumulation

[Term]
id: MPATH:644
name: crystalloid formation
def: "Accumulation of chitinase-like protein." [Pathbase: Curation]
is_a: MPATH:33 ! intracellular and extracellular accumulation

[Term]
id: MPATH:645
name: epicarditis
is_a: MPATH:212 ! inflammation
created_by: George Gkoutos
creation_date: 2011-03-22T03:09:08Z

[Term]
id: MPATH:646
name: chondroarthritis
is_a: MPATH:212 ! inflammation
created_by: George Gkoutos
creation_date: 2011-03-22T03:12:07Z

[Term]
id: MPATH:647
name: interstitial nephritis
is_a: MPATH:212 ! inflammation
is_a: MPATH:676 ! nephritis
created_by: George Gkoutos
creation_date: 2011-03-22T03:14:35Z

[Term]
id: MPATH:648
name: interstitial pancreatitis
is_a: MPATH:212 ! inflammation
created_by: George Gkoutos
creation_date: 2011-03-22T03:16:02Z

[Term]
id: MPATH:649
name: otitis media
is_a: MPATH:212 ! inflammation
created_by: George Gkoutos
creation_date: 2011-03-22T03:16:36Z

[Term]
id: MPATH:65
name: developmental hypoplasia
def: "Underdevelopment of an organ due to a decrease in the number of cells through failure to proliferate leading to lack of development." [Pathbase: Pathology Committee]
is_obsolete: true

[Term]
id: MPATH:650
name: proliferative dermatitis
is_a: MPATH:212 ! inflammation
created_by: George Gkoutos
creation_date: 2011-03-22T03:17:25Z

[Term]
id: MPATH:651
name: ventral glossitis
is_a: MPATH:611 ! glossitis
created_by: George Gkoutos
creation_date: 2011-03-22T03:18:00Z

[Term]
id: MPATH:652
name: histiocytosis
is_a: MPATH:194 ! immune mediated disease
created_by: George Gkoutos
creation_date: 2011-03-22T03:19:47Z

[Term]
id: MPATH:653
name: langerhans cell histiocytosis
synonym: "histiocytosis X" EXACT []
is_a: MPATH:652 ! histiocytosis
created_by: George Gkoutos
creation_date: 2011-03-22T03:20:12Z

[Term]
id: MPATH:654
name: non-Langerhans cell histiocytosis
synonym: "hemophagocytic syndrome" EXACT []
is_a: MPATH:652 ! histiocytosis
created_by: George Gkoutos
creation_date: 2011-03-22T03:20:52Z

[Term]
id: MPATH:655
name: lingual adenitis
is_a: MPATH:212 ! inflammation
created_by: George Gkoutos
creation_date: 2011-03-22T03:36:05Z

[Term]
id: MPATH:656
name: hemolysis
def: "Rupture or disruption of erythrocytes with release of contents." [MPATH:Curation]
comment: May be immune-mediated, induced by infectious organisms, or intrinsic disturbance of cell physiology or membrane/cytoskeletal integrity.
is_a: MPATH:25 ! tissue specific degenerative process
created_by: Paul
creation_date: 2011-04-01T12:08:29Z

[Term]
id: MPATH:657
name: rhinitis
is_a: MPATH:212 ! inflammation
created_by: George Gkoutos
creation_date: 2011-03-22T03:45:17Z

[Term]
id: MPATH:658
name: foreign body rhinitis
is_a: MPATH:657 ! rhinitis
created_by: George Gkoutos
creation_date: 2011-03-22T03:45:36Z

[Term]
id: MPATH:659
name: foreign body dermatitis
is_a: MPATH:196 ! dermatitis
created_by: George Gkoutos
creation_date: 2011-03-22T03:46:02Z

[Term]
id: MPATH:66
name: dilatation
def: "Increase in the diameter of an orifice or tubular structure beyond its normal dimensions." [Pathbase: Pathology Committee]
is_a: MPATH:56 ! developmental and adult structural  defect

[Term]
id: MPATH:660
name: gastritis
is_a: MPATH:212 ! inflammation
created_by: George Gkoutos
creation_date: 2011-03-22T03:46:42Z

[Term]
id: MPATH:661
name: foreign body gastritis
is_a: MPATH:660 ! gastritis
created_by: George Gkoutos
creation_date: 2011-03-22T03:47:05Z

[Term]
id: MPATH:662
name: foreign body glossitis
is_a: MPATH:611 ! glossitis
created_by: George Gkoutos
creation_date: 2011-03-22T03:47:40Z

[Term]
id: MPATH:663
name: peritonitis
is_a: MPATH:212 ! inflammation
created_by: George Gkoutos
creation_date: 2011-03-22T03:48:33Z

[Term]
id: MPATH:664
name: granulomatous peritonitis
is_a: MPATH:215 ! granulomatous inflammation
is_a: MPATH:663 ! peritonitis
created_by: George Gkoutos
creation_date: 2011-03-22T03:48:51Z

[Term]
id: MPATH:665
name: foreign body granulomatous peritonitis
is_a: MPATH:215 ! granulomatous inflammation
is_a: MPATH:663 ! peritonitis
created_by: George Gkoutos
creation_date: 2011-03-22T03:49:26Z

[Term]
id: MPATH:666
name: periodontitis
is_a: MPATH:212 ! inflammation
created_by: George Gkoutos
creation_date: 2011-03-22T03:50:05Z

[Term]
id: MPATH:667
name: foreign body periodontitis
is_a: MPATH:666 ! periodontitis
created_by: George Gkoutos
creation_date: 2011-03-22T03:50:24Z

[Term]
id: MPATH:668
name: tracheitis
is_a: MPATH:212 ! inflammation
created_by: George Gkoutos
creation_date: 2011-03-22T03:51:20Z

[Term]
id: MPATH:669
name: foreign body tracheitis
is_a: MPATH:668 ! tracheitis
created_by: George Gkoutos
creation_date: 2011-03-22T03:52:00Z

[Term]
id: MPATH:67
name: displacement and deformity
def: "Abnormal location, orientation, number, loss or non-specified deformity of a structure or tissue." [Pathbase: Pathology Committee]
is_a: MPATH:599 ! developmental process abnormalities

[Term]
id: MPATH:670
name: granulomatous epicarditis
is_a: MPATH:215 ! granulomatous inflammation
is_a: MPATH:645 ! epicarditis
created_by: George Gkoutos
creation_date: 2011-03-22T03:52:48Z

[Term]
id: MPATH:671
name: mastitis
is_a: MPATH:212 ! inflammation
created_by: George Gkoutos
creation_date: 2011-02-19T04:01:58Z

[Term]
id: MPATH:672
name: mastocytosis
synonym: "Urticaria pigmentosa" EXACT []
is_a: MPATH:212 ! inflammation
created_by: George Gkoutos
creation_date: 2011-02-19T04:05:08Z

[Term]
id: MPATH:673
name: metritis
is_a: MPATH:212 ! inflammation
created_by: George Gkoutos
creation_date: 2011-02-19T04:06:30Z

[Term]
id: MPATH:674
name: osteomyelitis
is_a: MPATH:212 ! inflammation
created_by: George Gkoutos
creation_date: 2011-02-19T04:08:00Z

[Term]
id: MPATH:675
name: psoriasiform dermatitis
is_a: MPATH:196 ! dermatitis
created_by: George Gkoutos
creation_date: 2011-02-19T04:09:12Z

[Term]
id: MPATH:676
name: nephritis
is_a: MPATH:212 ! inflammation
created_by: George Gkoutos
creation_date: 2011-02-19T04:10:14Z

[Term]
id: MPATH:677
name: pyelonephritis
is_a: MPATH:676 ! nephritis
created_by: George Gkoutos
creation_date: 2011-02-19T04:10:51Z

[Term]
id: MPATH:678
name: septic nephritis
is_a: MPATH:676 ! nephritis
created_by: George Gkoutos
creation_date: 2011-02-19T04:12:09Z

[Term]
id: MPATH:679
name: urocystitis
is_a: MPATH:212 ! inflammation
created_by: George Gkoutos
creation_date: 2011-02-19T04:12:43Z

[Term]
id: MPATH:68
name: diverticulum
def: "A blind ended outpouching through the wall of a tubular organ or bounded cavity." [Pathbase: Curation]
is_a: MPATH:56 ! developmental and adult structural  defect

[Term]
id: MPATH:680
name: septic urocystitis
is_a: MPATH:679 ! urocystitis
created_by: George Gkoutos
creation_date: 2011-02-19T04:13:07Z

[Term]
id: MPATH:681
name: septicemia
is_a: MPATH:212 ! inflammation
created_by: George Gkoutos
creation_date: 2011-02-19T04:13:38Z

[Term]
id: MPATH:682
name: arteritis
is_a: MPATH:201 ! vasculitis
created_by: George Gkoutos
creation_date: 2011-02-19T04:15:16Z

[Term]
id: MPATH:683
name: degenerative arthritis
is_a: MPATH:195 ! arthritis
is_a: MPATH:25 ! tissue specific degenerative process
is_a: MPATH:684 ! arthropathy
created_by: George Gkoutos
creation_date: 2011-02-19T04:16:05Z

[Term]
id: MPATH:684
name: arthropathy
is_a: MPATH:25 ! tissue specific degenerative process
is_a: MPATH:655 ! lingual adenitis
created_by: George Gkoutos
creation_date: 2011-02-19T04:17:26Z

[Term]
id: MPATH:685
name: accessory organ
is_a: MPATH:84 ! supernumerary structure
created_by: George Gkoutos
creation_date: 2011-02-19T04:26:34Z

[Term]
id: MPATH:686
name: amputation
is_a: MPATH:67 ! displacement and deformity
created_by: George Gkoutos
creation_date: 2011-02-19T04:30:20Z

[Term]
id: MPATH:687
name: autoamputation
is_a: MPATH:686 ! amputation
created_by: George Gkoutos
creation_date: 2011-02-19T04:30:41Z

[Term]
id: MPATH:688
name: aortitis
is_a: MPATH:201 ! vasculitis
created_by: George Gkoutos
creation_date: 2011-02-19T04:34:31Z

[Term]
id: MPATH:689
name: lymphangitis
is_a: MPATH:201 ! vasculitis
created_by: George Gkoutos
creation_date: 2011-02-19T04:35:13Z

[Term]
id: MPATH:69
name: ectopia
def: "ectopia" [Pathbase: Curation]
comment: obsolete - Subsumed into heterotopia MPATH:76
is_obsolete: true

[Term]
id: MPATH:690
name: phlebitis
is_a: MPATH:201 ! vasculitis
created_by: George Gkoutos
creation_date: 2011-02-19T04:36:16Z

[Term]
id: MPATH:691
name: pustule
synonym: "cutaneous abscess" EXACT []
is_a: MPATH:608 ! abscess
created_by: George Gkoutos
creation_date: 2011-02-19T04:45:08Z

[Term]
id: MPATH:692
name: ulcerative blepharitis
is_a: MPATH:546 ! blepharitis
created_by: George Gkoutos
creation_date: 2011-02-19T04:56:39Z

[Term]
id: MPATH:693
name: pyometra
is_a: MPATH:673 ! metritis
created_by: George Gkoutos
creation_date: 2011-02-19T05:02:23Z

[Term]
id: MPATH:694
name: acidophilic anterior pituitary gland adenoma
is_a: MPATH:270 ! adenoma
created_by: George Gkoutos
creation_date: 2011-02-19T05:05:05Z

[Term]
id: MPATH:695
name: spindle cell sarcoma
is_a: MPATH:551 ! sarcoma
created_by: George Gkoutos
creation_date: 2011-02-19T05:12:17Z

[Term]
id: MPATH:696
name: spindle cell hyperplasia
is_a: MPATH:602 ! hyperplastic tissue
created_by: George Gkoutos
creation_date: 2011-02-19T05:13:13Z

[Term]
id: MPATH:697
name: alopecia areata
is_a: MPATH:26 ! alopecia
created_by: George Gkoutos
creation_date: 2011-02-19T05:17:30Z

[Term]
id: MPATH:698
name: exostosis
is_a: MPATH:126 ! growth and differentiation defect
created_by: George Gkoutos
creation_date: 2011-02-19T05:23:34Z

[Term]
id: MPATH:699
name: ankylosing exostosis
is_a: MPATH:698 ! exostosis
created_by: George Gkoutos
creation_date: 2011-02-19T05:24:05Z

[Term]
id: MPATH:7
name: coagulation necrosis
def: "A type of necrosis in which the affected cells or tissue are reduced to homogeneous eosinophilic mass without nuclear staining, as a result of the protein coagulation, eg. Infarct. Tissue architecture persists." [ISBN:0781727286]
is_a: MPATH:4 ! necrosis

[Term]
id: MPATH:70
name: fistula
def: "An abnormal passage between two internal organs or leading from a cavity to the body surface." [Pathbase: Curation]
is_a: MPATH:56 ! developmental and adult structural  defect

[Term]
id: MPATH:700
name: ascites
is_a: MPATH:33 ! intracellular and extracellular accumulation
created_by: George Gkoutos
creation_date: 2011-02-19T05:24:55Z

[Term]
id: MPATH:701
name: developmental aspermia
is_a: MPATH:599 ! developmental process abnormalities
created_by: George Gkoutos
creation_date: 2011-02-19T05:29:50Z

[Term]
id: MPATH:702
name: acquired aspermia
is_a: MPATH:604 ! defective growth and differentiation process
created_by: George Gkoutos
creation_date: 2011-02-19T05:30:40Z

[Term]
id: MPATH:703
name: developmental hypoplasia
is_a: MPATH:599 ! developmental process abnormalities
created_by: George Gkoutos
creation_date: 2011-02-19T05:31:21Z

[Term]
id: MPATH:704
name: thyroiditis
is_a: MPATH:212 ! inflammation
created_by: George Gkoutos
creation_date: 2011-02-19T08:28:41Z

[Term]
id: MPATH:705
name: acinar atrophy
is_a: MPATH:127 ! atrophy
created_by: George Gkoutos
creation_date: 2011-02-19T10:33:51Z

[Term]
id: MPATH:706
name: cryptorchidism
is_a: MPATH:86 ! organ specific developmental defect
created_by: George Gkoutos
creation_date: 2011-02-19T10:37:34Z

[Term]
id: MPATH:707
name: angiolipoma
is_a: MPATH:415 ! lipomatous tumor
created_by: George Gkoutos
creation_date: 2011-02-20T08:44:41Z

[Term]
id: MPATH:71
name: fusion defect
def: "Failure of two or more structures ( not voids or lumens) to join together." [ISBN:0781727286]
is_a: MPATH:599 ! developmental process abnormalities

[Term]
id: MPATH:711
name: situs ambiguus
is_a: MPATH:470 ! left/right axis defect
created_by: George Gkoutos
creation_date: 2011-02-20T12:06:02Z

[Term]
id: MPATH:712
name: heterotaxy
is_a: MPATH:470 ! left/right axis defect
created_by: George Gkoutos
creation_date: 2011-02-20T12:06:38Z

[Term]
id: MPATH:713
name: situs ambiguus totalis
synonym: "situs inversus with dextrocardia" RELATED []
xref: XX:<new dbxref>
is_a: MPATH:720 ! situs inversus
created_by: George Gkoutos
creation_date: 2011-02-20T12:07:15Z

[Term]
id: MPATH:714
name: situs inversus with levocardia
is_a: MPATH:720 ! situs inversus
created_by: George Gkoutos
creation_date: 2011-02-20T12:08:14Z

[Term]
id: MPATH:715
name: sinusitis
is_a: MPATH:212 ! inflammation
created_by: George Gkoutos
creation_date: 2011-02-20T12:10:00Z

[Term]
id: MPATH:716
name: ciliary motility defect
synonym: "primary ciliary dyskinesis" RELATED []
is_a: MPATH:17 ! subcellular defect
created_by: George Gkoutos
creation_date: 2011-02-20T12:14:20Z

[Term]
id: MPATH:717
name: sequestrum
comment: Most often used in the context of bone.
is_a: MPATH:1 ! cell and tissue damage
created_by: George Gkoutos
creation_date: 2011-02-20T02:28:51Z

[Term]
id: MPATH:719
name: bronchiectasia
is_a: MPATH:474 ! ectasia
created_by: George Gkoutos
creation_date: 2011-02-20T12:04:36Z

[Term]
id: MPATH:72
name: growth acceleration
def: "Increase in the rate of growth of an organism, organ or tissue as a consequence of increased proliferation, reduced cell death, or a combination. Not due to an increase in cell size; see Hypertrophy MPATH: 159." [Pathbase: Pathology Committee]
is_a: MPATH:599 ! developmental process abnormalities

[Term]
id: MPATH:720
name: situs inversus
is_a: MPATH:470 ! left/right axis defect
created_by: George Gkoutos
creation_date: 2011-02-20T12:05:38Z

[Term]
id: MPATH:73
name: growth arrest
def: "The cessation of fetal or embryonic growth beyond a particular stage." [Pathbase: Pathology Committee]
is_a: MPATH:599 ! developmental process abnormalities

[Term]
id: MPATH:74
name: hamartoma
def: "A focal malformation resembling a neoplasm which results from faulty development of an organ; composed of an abnormal mixture of tissue elements, or an abnormal proportion of a single element. Growth and location are usually normal for that tissue cf. Heterotopia/Choristoma MPATH:76/MPATH:477." [ISBN:0781727286]
is_a: MPATH:56 ! developmental and adult structural  defect

[Term]
id: MPATH:75
name: hernia
def: "Protrusion of a loop or wall of an organ through an abnormal opening." [Pathbase: Curation]
is_a: MPATH:56 ! developmental and adult structural  defect

[Term]
id: MPATH:76
name: heterotopia
def: "Congenital appearance of a body part or tissue or cell type in a region where it is not normally found ( topographical anomaly)." [Pathbase: Pathology Committee]
synonym: "Ectopia" RELATED [Pathbase: Curation]
is_a: MPATH:67 ! displacement and deformity

[Term]
id: MPATH:77
name: homoeotic change
def: "Stricto sensu: replacement of one body part or tissue by an homologous structure or tissue, but commonly used incorrectly to describe non-homologous transformations better described as heterotopias or ectopias." [Pathbase: Pathology Committee]
is_a: MPATH:599 ! developmental process abnormalities

[Term]
id: MPATH:78
name: incomplete closure
def: "Incomplete closure of a void or lumen due to failure of growth or fusion of bounding walls." [Pathbase: Pathology Committee]
is_a: MPATH:599 ! developmental process abnormalities

[Term]
id: MPATH:79
name: malposition
def: "Abnormal position or orientation of a structure insufficient to be called a heterotopia." [Pathbase: Curation]
synonym: "Misplacement" RELATED [Pathbase: Curation]
is_a: MPATH:76 ! heterotopia

[Term]
id: MPATH:8
name: fat necrosis
def: "Dead and dying adipose tissue, characterized by the formation of small gray or white foci of soapy (saponified) cellular debris." [ISBN:0781727286]
is_a: MPATH:4 ! necrosis

[Term]
id: MPATH:80
name: obstruction and stenosis
def: "Occlusion ( partial or complete) of a lumen or space, internally by a space occupying mass or, in the case of stenosis, by local reduction in the diameter of a vessel, duct or the intestine." [Pathbase: Pathology Committee]
is_a: MPATH:56 ! developmental and adult structural  defect

[Term]
id: MPATH:81
name: perforation
def: "Presence of a hole/channel through a normally imperforate structure often a membrane or septum." [Pathbase: Pathology Committee]
is_a: MPATH:56 ! developmental and adult structural  defect

[Term]
id: MPATH:82
name: persistent embryonic structure
def: "Persistence of an embryonic structure or tissue into the post-natal period in its normal location; (Chronological/temporal anomaly)." [Pathbase: Pathology Committee]
synonym: "Embryonic rest." RELATED [Pathbase: Curation]
is_a: MPATH:56 ! developmental and adult structural  defect

[Term]
id: MPATH:83
name: septation defect
def: "Any defect in the formation of septae not describable as perforation." [Pathbase: Curation]
is_a: MPATH:56 ! developmental and adult structural  defect

[Term]
id: MPATH:84
name: supernumerary structure
def: "Additional structure whether normally located or not." [Pathbase: Curation]
is_a: MPATH:56 ! developmental and adult structural  defect

[Term]
id: MPATH:85
name: transdifferentiation
def: "Alteration in the differentiation of a cell or tissue already showing a different, recognisable, differentiated state." [Pathbase: Pathology Committee]
comment: This term is generally used in the context of embryonic cells or stem cells.
is_a: MPATH:599 ! developmental process abnormalities

[Term]
id: MPATH:86
name: organ specific developmental defect
def: "Developmental defect characteristic of a particular organ or organ system which may be a recognised syndrome or a complex defect showing multiple manifestations." [Pathbase: Curation]
is_a: MPATH:55 ! developmental and structural abnormality

[Term]
id: MPATH:87
name: germ cell defect
def: "Abnormal morphology, differentiation or location of primordial germ cells or their descendents. Not neoplastic." [Pathbase: Curation]
is_a: MPATH:86 ! organ specific developmental defect

[Term]
id: MPATH:88
name: nephroblastomatosis
def: "nephroblastomatosis" [Pathbase: Curation]
comment: Obsolete - subsumed into MPATH:82
is_obsolete: true

[Term]
id: MPATH:89
name: cardiovascular developmental defect
def: "Abnormal development of the heart or vascular tissue resulting in morphological abnormality." [Pathbase: Curation]
is_a: MPATH:86 ! organ specific developmental defect

[Term]
id: MPATH:9
name: fibrinoid necrosis
def: "Necrosis in which the necrotic tissue shows deeply eosinophilic staining similar to that of fibrin." [ISBN:0781727286]
comment: Frequently occurs in the walls of blood vessels and in connective tissue in diseases such as disseminated Lupus erythrematosis and polyarteritis nodosa, scleroderma, dermatomyositis and rheumatic fever.
is_a: MPATH:4 ! necrosis

[Term]
id: MPATH:90
name: aneurysm
def: "Localised dilation of an artery or heart chamber usually due to an acquired or congenital weakness of the wall of the artery or chamber." [Pathbase: Pathology Committee]
is_a: MPATH:56 ! developmental and adult structural  defect

[Term]
id: MPATH:91
name: arteriovenous anastomosis
def: "Formation of vessels between arterioles and venules bypassing capillary circulation." [Pathbase: Curation]
synonym: "Anastomosis arteriolovenularis" RELATED [Pathbase: Curation]
synonym: "anastomosis arteriovenosa" RELATED [Pathbase: Curation]
synonym: "arteriolovenular anastomosis" RELATED [Pathbase: Curation]
is_a: MPATH:89 ! cardiovascular developmental defect

[Term]
id: MPATH:92
name: cardiac defect
def: "Structural, organisational or growth related defects in cardiac development." [Pathbase: Curation]
synonym: "heart abnormalities" RELATED [Pathbase: Curation]
is_a: MPATH:89 ! cardiovascular developmental defect

[Term]
id: MPATH:93
name: cardiac septation defect
def: "Abnormality in the wall between the atria or ventricles, or defects in the truncoconal septum, of the heart; usually incomplete closure." [Pathbase: Curation]
is_a: MPATH:92 ! cardiac defect

[Term]
id: MPATH:94
name: valve defect
def: "Malformation of the membranous folds of the heart that prevent reflux of fluid." [Pathbase: Curation]
is_a: MPATH:92 ! cardiac defect

[Term]
id: MPATH:95
name: hypertrophic ventricle
def: "Thickening of the wall of one or both of the heart ventricles." [Pathbase: Pathology Committee]
is_a: MPATH:92 ! cardiac defect

[Term]
id: MPATH:96
name: hypoplastic ventricle
def: "Reduction in cell number of one or both of the two lower chambers of the heart." [Pathbase: Pathology Committee]
is_a: MPATH:92 ! cardiac defect

[Term]
id: MPATH:97
name: dissecting aneurysm
def: "Follows the presence of a hematoma in the wall of an artery Splitting of the media occurs, blood enters the split through a tear in the intima." [ISBN:0781727286]
is_a: MPATH:90 ! aneurysm

[Term]
id: MPATH:98
name: lymphangiectasis
def: "A stretching and widening of the lymphatic vessels." [Pathbase: Pathology Committee]
synonym: "Lymphectasia" RELATED [Pathbase: Curation]
synonym: "telangiectasia lymphatica" RELATED [Pathbase: Curation]
is_a: MPATH:474 ! ectasia
is_a: MPATH:89 ! cardiovascular developmental defect

[Term]
id: MPATH:99
name: varices
def: "An enlarged and often tortuous vein." [Pathbase: Pathology Committee]
is_a: MPATH:56 ! developmental and adult structural  defect

[Typedef]
id: is_a
name: is a

[Typedef]
id: part_of
name: part of
is_transitive: true

